<?xml version="1.0"?>


<!DOCTYPE rdf:RDF [
    <!ENTITY rda-fields "http://bibframe.org/rda/" >
    <!ENTITY marc-fields "http://bibframe.org/marc/" >
    <!ENTITY dcterms "http://purl.org/dc/terms/" >
    <!ENTITY prov "http://www.w3.org/ns/prov#" >
    <!ENTITY vocab "http://bibframe.org/vocab/" >
    <!ENTITY owl "http://www.w3.org/2002/07/owl#" >
    <!ENTITY bfmain "http://bibframe.org/vocab/main" >
    <!ENTITY bframe "http://bibframe.org/vocab/frame" >
    <!ENTITY dc "http://purl.org/dc/elements/1.1/" >
    <!ENTITY xsd "http://www.w3.org/2001/XMLSchema#" >
    <!ENTITY bf-abstract "http://bibframe.org/model-abstract/" >
    <!ENTITY skos "http://www.w3.org/2004/02/skos/core#" >
    <!ENTITY rdfs "http://www.w3.org/2000/01/rdf-schema#" >
    <!ENTITY rdf "http://www.w3.org/1999/02/22-rdf-syntax-ns#" >
]>


<rdf:RDF xmlns="http://bibframe.org/vocab/"
     xml:base="http://bibframe.org/vocab/"
     xmlns:dc="http://purl.org/dc/elements/1.1/"
     xmlns:prov="http://www.w3.org/ns/prov#"
     xmlns:bf-abstract="http://bibframe.org/model-abstract/"
     xmlns:bfmain="&vocab;main"
     xmlns:dcterms="http://purl.org/dc/terms/"
     xmlns:rdfs="http://www.w3.org/2000/01/rdf-schema#"
     xmlns:rda-fields="http://bibframe.org/rda/"
     xmlns:marc-fields="http://bibframe.org/marc/"
     xmlns:xsd="http://www.w3.org/2001/XMLSchema#"
     xmlns:owl="http://www.w3.org/2002/07/owl#"
     xmlns:rdf="http://www.w3.org/1999/02/22-rdf-syntax-ns#"
     xmlns:vocab="http://bibframe.org/vocab/"
     xmlns:skos="http://www.w3.org/2004/02/skos/core#"
     xmlns:bframe="&vocab;frame">
    <owl:Ontology rdf:about="http://bibframe.org/vocab/">
        <owl:versionInfo rdf:datatype="&xsd;string">Initially automatically generated.</owl:versionInfo>
        <dcterms:modified>2014-12-10T20:23:05.638677Z</dcterms:modified>
    </owl:Ontology>
    


    <!-- 
    ///////////////////////////////////////////////////////////////////////////////////////
    //
    // Annotation properties
    //
    ///////////////////////////////////////////////////////////////////////////////////////
     -->

    


    <!-- http://bibframe.org/vocab/abbreviatedTitle -->

    <owl:AnnotationProperty rdf:about="&vocab;abbreviatedTitle">
        <rdfs:label>Abbreviated title</rdfs:label>
        <rdfs:comment>Title as abbreviated for indexing or identification.</rdfs:comment>
    </owl:AnnotationProperty>
    


    <!-- http://bibframe.org/vocab/absorbed -->

    <owl:AnnotationProperty rdf:about="&vocab;absorbed">
        <rdfs:label>Absorbed</rdfs:label>
        <rdfs:comment>Work that has been incorporated into another Work</rdfs:comment>
        <dcterms:modified>2014-04-10 (Updated subproperty)</dcterms:modified>
        <rdfs:subPropertyOf rdf:resource="&vocab;precededBy"/>
    </owl:AnnotationProperty>
    


    <!-- http://bibframe.org/vocab/absorbedBy -->

    <owl:AnnotationProperty rdf:about="&vocab;absorbedBy">
        <rdfs:label>Absorbed by</rdfs:label>
        <dcterms:modified>2014-04-10 (Updated subproperty)</dcterms:modified>
        <rdfs:comment>Work that incorporates another work.</rdfs:comment>
        <rdfs:subPropertyOf rdf:resource="&vocab;succeededBy"/>
    </owl:AnnotationProperty>
    


    <!-- http://bibframe.org/vocab/absorbedInPart -->

    <owl:AnnotationProperty rdf:about="&vocab;absorbedInPart">
        <rdfs:label>Absorbed in part</rdfs:label>
        <rdfs:comment>Work that has been partially incorporated into another work.</rdfs:comment>
        <dcterms:modified>2014-04-10 (Updated subproperty)</dcterms:modified>
        <rdfs:subPropertyOf rdf:resource="&vocab;precededBy"/>
    </owl:AnnotationProperty>
    


    <!-- http://bibframe.org/vocab/absorbedInPartBy -->

    <owl:AnnotationProperty rdf:about="&vocab;absorbedInPartBy">
        <rdfs:label>Absorbed in part by</rdfs:label>
        <dcterms:modified>2014-04-10 (Updated subproperty)</dcterms:modified>
        <rdfs:comment>Work that incorporates part of the content of another work.</rdfs:comment>
        <rdfs:subPropertyOf rdf:resource="&vocab;succeededBy"/>
    </owl:AnnotationProperty>
    


    <!-- http://bibframe.org/vocab/accessCondition -->

    <owl:AnnotationProperty rdf:about="&vocab;accessCondition">
        <rdfs:label>Access condition</rdfs:label>
        <rdfs:comment>Allowances and restrictions on access.</rdfs:comment>
        <rdfs:domain rdf:resource="&vocab;HeldMaterial"/>
    </owl:AnnotationProperty>
    


    <!-- http://bibframe.org/vocab/accompaniedBy -->

    <owl:AnnotationProperty rdf:about="&vocab;accompaniedBy">
        <rdfs:label>Accompanied by</rdfs:label>
        <dcterms:modified>2014-04-10 (Range updated)</dcterms:modified>
        <rdfs:comment>Resource that has an accompanying resource which adds to it</rdfs:comment>
        <rdfs:subPropertyOf rdf:resource="&vocab;relatedTo"/>
    </owl:AnnotationProperty>
    


    <!-- http://bibframe.org/vocab/accompanies -->

    <owl:AnnotationProperty rdf:about="&vocab;accompanies">
        <rdfs:label>Accompanies</rdfs:label>
        <rdfs:comment>Resource that adds to or is issued with the described resource</rdfs:comment>
        <dcterms:modified>2014-04-10 (Range updated)</dcterms:modified>
        <rdfs:subPropertyOf rdf:resource="&vocab;relatedTo"/>
    </owl:AnnotationProperty>
    


    <!-- http://bibframe.org/vocab/annotates -->

    <owl:AnnotationProperty rdf:about="&vocab;annotates">
        <rdfs:label>Target of Annotation</rdfs:label>
        <rdfs:comment>Resource to which the annotation relates.</rdfs:comment>
    </owl:AnnotationProperty>
    


    <!-- http://bibframe.org/vocab/annotationAssertedBy -->

    <owl:AnnotationProperty rdf:about="&vocab;annotationAssertedBy">
        <rdfs:label>Annotation asserted by</rdfs:label>
        <rdfs:comment>Annotation was asserted by the given entity.</rdfs:comment>
    </owl:AnnotationProperty>
    


    <!-- http://bibframe.org/vocab/annotationBody -->

    <owl:AnnotationProperty rdf:about="&vocab;annotationBody">
        <rdfs:label>Annotation Body</rdfs:label>
        <rdfs:comment>Content of the annotation about the resource.</rdfs:comment>
    </owl:AnnotationProperty>
    


    <!-- http://bibframe.org/vocab/annotationSource -->

    <owl:AnnotationProperty rdf:about="&vocab;annotationSource">
        <rdfs:label>Annotation Source</rdfs:label>
        <rdfs:comment>Source of the annotation.</rdfs:comment>
    </owl:AnnotationProperty>
    


    <!-- http://bibframe.org/vocab/ansi -->

    <owl:AnnotationProperty rdf:about="&vocab;ansi">
        <rdfs:label>ANSI number</rdfs:label>
        <rdfs:comment>American National Standards Institute identifier.</rdfs:comment>
    </owl:AnnotationProperty>
    


    <!-- http://bibframe.org/vocab/arrangement -->

    <owl:AnnotationProperty rdf:about="&vocab;arrangement">
        <rdfs:label>Organization and Arrangement</rdfs:label>
        <rdfs:comment>Information about the organization and arrangement of a collection of resources.</rdfs:comment>
    </owl:AnnotationProperty>
    


    <!-- http://bibframe.org/vocab/aspectRatio -->

    <owl:AnnotationProperty rdf:about="&vocab;aspectRatio">
        <rdfs:label>Aspect ratio</rdfs:label>
        <rdfs:comment>Proportional relationship between an image&apos;s width and its height.</rdfs:comment>
        <rdfs:domain rdf:resource="&vocab;Instance"/>
    </owl:AnnotationProperty>
    


    <!-- http://bibframe.org/vocab/assertionDate -->

    <owl:AnnotationProperty rdf:about="&vocab;assertionDate">
        <rdfs:label>Annotation Assertion Date</rdfs:label>
        <rdfs:comment>Date when annotation was asserted.</rdfs:comment>
        <rdfs:domain rdf:resource="&vocab;Annotation"/>
    </owl:AnnotationProperty>
    


    <!-- http://bibframe.org/vocab/audience -->

    <owl:AnnotationProperty rdf:about="&vocab;audience">
        <rdfs:label>Audience</rdfs:label>
        <rdfs:comment>Information that identifies the specific audience or intellectual level for which the content of the resource is considered appropriate.</rdfs:comment>
        <rdfs:domain rdf:resource="&vocab;IntendedAudience"/>
    </owl:AnnotationProperty>
    


    <!-- http://bibframe.org/vocab/audienceAssigner -->

    <owl:AnnotationProperty rdf:about="&vocab;audienceAssigner">
        <rdfs:label>Audience assigner</rdfs:label>
        <rdfs:comment>Entity that assigned the intended audience information.</rdfs:comment>
        <rdfs:domain rdf:resource="&vocab;IntendedAudience"/>
    </owl:AnnotationProperty>
    


    <!-- http://bibframe.org/vocab/authorityAssigner -->

    <owl:AnnotationProperty rdf:about="&vocab;authorityAssigner">
        <rdfs:label>Authority assigner</rdfs:label>
        <rdfs:comment>Entity that assigned the information.</rdfs:comment>
    </owl:AnnotationProperty>
    


    <!-- http://bibframe.org/vocab/authoritySource -->

    <owl:AnnotationProperty rdf:about="&vocab;authoritySource">
        <rdfs:label>Authority source</rdfs:label>
        <rdfs:comment>Authority list from which a value is taken.</rdfs:comment>
        <rdfs:domain rdf:resource="&vocab;Authority"/>
    </owl:AnnotationProperty>
    


    <!-- http://bibframe.org/vocab/authorizedAccessPoint -->

    <owl:AnnotationProperty rdf:about="&vocab;authorizedAccessPoint">
        <rdfs:label>Authorized access point</rdfs:label>
        <rdfs:comment>Controlled string form of a resource label intended to help uniquely identify it, such as a unique title or a unique name plus title.</rdfs:comment>
        <rdfs:domain rdf:resource="&vocab;Resource"/>
    </owl:AnnotationProperty>
    


    <!-- http://bibframe.org/vocab/awardNote -->

    <owl:AnnotationProperty rdf:about="&vocab;awardNote">
        <rdfs:label>Award note</rdfs:label>
        <rdfs:comment>Information on awards associated with the described resource.</rdfs:comment>
        <rdfs:domain rdf:resource="&vocab;Instance"/>
    </owl:AnnotationProperty>
    


    <!-- http://bibframe.org/vocab/barcode -->

    <owl:AnnotationProperty rdf:about="&vocab;barcode">
        <rdfs:label>Barcode</rdfs:label>
        <rdfs:comment>Identification number of the physical item.</rdfs:comment>
        <rdfs:domain rdf:resource="&vocab;HeldItem"/>
    </owl:AnnotationProperty>
    


    <!-- http://bibframe.org/vocab/carrierCategory -->

    <owl:AnnotationProperty rdf:about="&vocab;carrierCategory">
        <rdfs:label>Carrier type</rdfs:label>
        <rdfs:comment>Categorization reflecting the format of the storage medium and housing of a carrier.</rdfs:comment>
    </owl:AnnotationProperty>
    


    <!-- http://bibframe.org/vocab/cartographicAscensionAndDeclination -->

    <owl:AnnotationProperty rdf:about="&vocab;cartographicAscensionAndDeclination">
        <rdfs:label>Cartographic ascension and declination</rdfs:label>
        <rdfs:comment>System for identifying the location of a celestial object in the sky covered by the cartographic content of a resource using the angles of right ascension and declination.</rdfs:comment>
        <rdfs:domain rdf:resource="&vocab;Cartography"/>
    </owl:AnnotationProperty>
    


    <!-- http://bibframe.org/vocab/cartographicCoordinates -->

    <owl:AnnotationProperty rdf:about="&vocab;cartographicCoordinates">
        <rdfs:label>Cartographic coordinates</rdfs:label>
        <rdfs:comment>Mathematical system for identifying the area covered by the cartographic content of a resource, Expressed either by means of longitude and latitude on the surface of planets or by the angles of right ascension and declination for celestial cartographic content.</rdfs:comment>
        <rdfs:domain rdf:resource="&vocab;Cartography"/>
    </owl:AnnotationProperty>
    


    <!-- http://bibframe.org/vocab/cartographicEquinox -->

    <owl:AnnotationProperty rdf:about="&vocab;cartographicEquinox">
        <rdfs:label>Cartographic equinox</rdfs:label>
        <rdfs:comment>One of two points of intersection of the ecliptic and the celestial equator, occupied by the sun when its declination is 0 degrees.</rdfs:comment>
        <rdfs:domain rdf:resource="&vocab;Cartography"/>
    </owl:AnnotationProperty>
    


    <!-- http://bibframe.org/vocab/cartographicExclusionGRing -->

    <owl:AnnotationProperty rdf:about="&vocab;cartographicExclusionGRing">
        <rdfs:label>Cartographic G ring area excluded</rdfs:label>
        <rdfs:comment>Coordinate pairs that identify the closed non-intersecting boundary of the area contained within the G-polygon outer ring that is excluded.</rdfs:comment>
        <rdfs:domain rdf:resource="&vocab;Cartography"/>
    </owl:AnnotationProperty>
    


    <!-- http://bibframe.org/vocab/cartographicOuterGRing -->

    <owl:AnnotationProperty rdf:about="&vocab;cartographicOuterGRing">
        <rdfs:label>Cartographic outer G ring area covered</rdfs:label>
        <rdfs:comment>Coordinate pairs that identify the closed non-intersecting boundary of the area covered.</rdfs:comment>
        <rdfs:domain rdf:resource="&vocab;Cartography"/>
    </owl:AnnotationProperty>
    


    <!-- http://bibframe.org/vocab/cartographicProjection -->

    <owl:AnnotationProperty rdf:about="&vocab;cartographicProjection">
        <rdfs:label>Cartographic projection</rdfs:label>
        <rdfs:comment>Method or system used to represent the surface of the Earth or of a celestial sphere on a plane.</rdfs:comment>
        <rdfs:domain rdf:resource="&vocab;Cartography"/>
    </owl:AnnotationProperty>
    


    <!-- http://bibframe.org/vocab/cartographicScale -->

    <owl:AnnotationProperty rdf:about="&vocab;cartographicScale">
        <rdfs:label>Cartographic scale</rdfs:label>
        <rdfs:comment>Ratio of the dimensions of a form contained or embodied in a resource to the dimensions of the entity it represents.</rdfs:comment>
        <rdfs:domain rdf:resource="&vocab;Cartography"/>
    </owl:AnnotationProperty>
    


    <!-- http://bibframe.org/vocab/categorySource -->

    <owl:AnnotationProperty rdf:about="&vocab;categorySource">
        <rdfs:label>Category source</rdfs:label>
        <rdfs:comment>Category list from which value is taken.</rdfs:comment>
        <rdfs:domain rdf:resource="&vocab;Category"/>
    </owl:AnnotationProperty>
    


    <!-- http://bibframe.org/vocab/categoryType -->

    <owl:AnnotationProperty rdf:about="&vocab;categoryType">
        <rdfs:label>Type of category</rdfs:label>
        <rdfs:comment>Type of category recorded, e.g., content, genre, media, form, carrier.</rdfs:comment>
        <rdfs:domain rdf:resource="&vocab;Category"/>
    </owl:AnnotationProperty>
    


    <!-- http://bibframe.org/vocab/categoryValue -->

    <owl:AnnotationProperty rdf:about="&vocab;categoryValue">
        <rdfs:label>Category</rdfs:label>
        <rdfs:comment>Category code or text.</rdfs:comment>
        <rdfs:domain rdf:resource="&vocab;Category"/>
    </owl:AnnotationProperty>
    


    <!-- http://bibframe.org/vocab/circulationStatus -->

    <owl:AnnotationProperty rdf:about="&vocab;circulationStatus">
        <rdfs:label>Circulation status</rdfs:label>
        <rdfs:comment>Circulation status of an item.</rdfs:comment>
        <rdfs:domain rdf:resource="&vocab;HeldItem"/>
    </owl:AnnotationProperty>
    


    <!-- http://bibframe.org/vocab/classification -->

    <owl:AnnotationProperty rdf:about="&vocab;classification">
        <rdfs:label>Classification</rdfs:label>
        <rdfs:comment>Classification number in any scheme.</rdfs:comment>
    </owl:AnnotationProperty>
    


    <!-- http://bibframe.org/vocab/classificationAssigner -->

    <owl:AnnotationProperty rdf:about="&vocab;classificationAssigner">
        <rdfs:label>Institution assigning classification</rdfs:label>
        <rdfs:comment>Entity that assigned the classification number.</rdfs:comment>
        <rdfs:domain rdf:resource="&vocab;Classification"/>
    </owl:AnnotationProperty>
    


    <!-- http://bibframe.org/vocab/classificationDdc -->

    <owl:AnnotationProperty rdf:about="&vocab;classificationDdc">
        <rdfs:label>DDC Classification</rdfs:label>
        <rdfs:comment>Dewey Decimal Classification number used for subject access.</rdfs:comment>
    </owl:AnnotationProperty>
    


    <!-- http://bibframe.org/vocab/classificationDesignation -->

    <owl:AnnotationProperty rdf:about="&vocab;classificationDesignation">
        <rdfs:label>Classification designation</rdfs:label>
        <rdfs:comment>Designates whether the classification number contained in the field is from the standard or optional part of the schedules or tables.</rdfs:comment>
        <rdfs:domain rdf:resource="&vocab;Classification"/>
    </owl:AnnotationProperty>
    


    <!-- http://bibframe.org/vocab/classificationEdition -->

    <owl:AnnotationProperty rdf:about="&vocab;classificationEdition">
        <rdfs:label>Classification scheme edition</rdfs:label>
        <rdfs:comment>Edition of the classification scheme, such as full, abridged or a number, when a classification scheme designates editions.</rdfs:comment>
        <dcterms:modified>2014-10-09 (Updated)</dcterms:modified>
        <rdfs:domain rdf:resource="&vocab;Classification"/>
    </owl:AnnotationProperty>
    


    <!-- http://bibframe.org/vocab/classificationItem -->

    <owl:AnnotationProperty rdf:about="&vocab;classificationItem">
        <rdfs:label>Classification item number</rdfs:label>
        <rdfs:comment>Number attached to a classification number that indicates a particular item.</rdfs:comment>
        <rdfs:domain rdf:resource="&vocab;Classification"/>
    </owl:AnnotationProperty>
    


    <!-- http://bibframe.org/vocab/classificationLcc -->

    <owl:AnnotationProperty rdf:about="&vocab;classificationLcc">
        <rdfs:label>LCC Classification</rdfs:label>
        <rdfs:comment>Library of Congress Classification number used for subject access.</rdfs:comment>
    </owl:AnnotationProperty>
    


    <!-- http://bibframe.org/vocab/classificationNlm -->

    <owl:AnnotationProperty rdf:about="&vocab;classificationNlm">
        <rdfs:label>NLM classification</rdfs:label>
        <rdfs:comment>National Library of Medicine Classification number used for subject access</rdfs:comment>
    </owl:AnnotationProperty>
    


    <!-- http://bibframe.org/vocab/classificationNumber -->

    <owl:AnnotationProperty rdf:about="&vocab;classificationNumber">
        <rdfs:label>Classification number</rdfs:label>
        <rdfs:comment>Classification number (single class number or beginning number of a span) that indicates the subject by applying a formal system of coding and organizing resources.</rdfs:comment>
        <rdfs:domain rdf:resource="&vocab;Classification"/>
    </owl:AnnotationProperty>
    


    <!-- http://bibframe.org/vocab/classificationNumberUri -->

    <owl:AnnotationProperty rdf:about="&vocab;classificationNumberUri">
        <rdfs:label>Classification number URI</rdfs:label>
        <rdfs:comment>Classification number represented as a URI.</rdfs:comment>
    </owl:AnnotationProperty>
    


    <!-- http://bibframe.org/vocab/classificationScheme -->

    <owl:AnnotationProperty rdf:about="&vocab;classificationScheme">
        <rdfs:label>Classification scheme</rdfs:label>
        <rdfs:comment>Formal scheme from which a classification number is taken.</rdfs:comment>
        <rdfs:domain rdf:resource="&vocab;Classification"/>
    </owl:AnnotationProperty>
    


    <!-- http://bibframe.org/vocab/classificationSpanEnd -->

    <owl:AnnotationProperty rdf:about="&vocab;classificationSpanEnd">
        <rdfs:label>Classification number span end</rdfs:label>
        <rdfs:comment>Ending number of classification number span.</rdfs:comment>
        <rdfs:domain rdf:resource="&vocab;Classification"/>
    </owl:AnnotationProperty>
    


    <!-- http://bibframe.org/vocab/classificationStatus -->

    <owl:AnnotationProperty rdf:about="&vocab;classificationStatus">
        <rdfs:label>Classification status</rdfs:label>
        <rdfs:comment>Indicator that the classification number is canceled or invalid.</rdfs:comment>
        <rdfs:domain rdf:resource="&vocab;Classification"/>
    </owl:AnnotationProperty>
    


    <!-- http://bibframe.org/vocab/classificationTable -->

    <owl:AnnotationProperty rdf:about="&vocab;classificationTable">
        <rdfs:label>Classification table identification</rdfs:label>
        <rdfs:comment>DDC Table identification. Number of the table from which the classification number in a subdivision record is taken.</rdfs:comment>
        <rdfs:domain rdf:resource="&vocab;Classification"/>
    </owl:AnnotationProperty>
    


    <!-- http://bibframe.org/vocab/classificationTableSeq -->

    <owl:AnnotationProperty rdf:about="&vocab;classificationTableSeq">
        <rdfs:label>Classification table sequence number</rdfs:label>
        <rdfs:comment>Sequence number or other identifier for an internal classification subarrangement or add in a classification scheme.</rdfs:comment>
        <rdfs:domain rdf:resource="&vocab;Classification"/>
    </owl:AnnotationProperty>
    


    <!-- http://bibframe.org/vocab/classificationUdc -->

    <owl:AnnotationProperty rdf:about="&vocab;classificationUdc">
        <rdfs:label>UDC Classification</rdfs:label>
        <rdfs:comment>Universal Decimal Classification number used for subject access.</rdfs:comment>
    </owl:AnnotationProperty>
    


    <!-- http://bibframe.org/vocab/coden -->

    <owl:AnnotationProperty rdf:about="&vocab;coden">
        <rdfs:label>CODEN</rdfs:label>
        <rdfs:comment>Identifier for scientific and technical periodical titles assigned by the International CODEN Section of Chemical Abstracts Service.</rdfs:comment>
    </owl:AnnotationProperty>
    


    <!-- http://bibframe.org/vocab/colorContent -->

    <owl:AnnotationProperty rdf:about="&vocab;colorContent">
        <rdfs:label>Color content</rdfs:label>
        <rdfs:comment>Color characteristics, e.g. black and white, multicolored, etc.</rdfs:comment>
        <dcterms:modified>2014-10-14 (Updated)</dcterms:modified>
        <rdfs:domain rdf:resource="&vocab;Instance"/>
    </owl:AnnotationProperty>
    


    <!-- http://bibframe.org/vocab/componentOf -->

    <owl:AnnotationProperty rdf:about="&vocab;componentOf">
        <rdfs:label>Held item</rdfs:label>
        <rdfs:comment>Link to held material</rdfs:comment>
    </owl:AnnotationProperty>
    


    <!-- http://bibframe.org/vocab/contentAccessibility -->

    <owl:AnnotationProperty rdf:about="&vocab;contentAccessibility">
        <rdfs:label>Content accessibility note</rdfs:label>
        <rdfs:comment>Content that assists those with a sensory impairment for greater understanding of content, e.g., labels, captions.</rdfs:comment>
        <rdfs:domain rdf:resource="&vocab;Instance"/>
    </owl:AnnotationProperty>
    


    <!-- http://bibframe.org/vocab/contentCategory -->

    <owl:AnnotationProperty rdf:about="&vocab;contentCategory">
        <rdfs:label>Content type</rdfs:label>
        <rdfs:comment>Categorization reflecting the fundamental form of communication in which the content is expressed and the human sense through which it is intended to be perceived.</rdfs:comment>
    </owl:AnnotationProperty>
    


    <!-- http://bibframe.org/vocab/contentsNote -->

    <owl:AnnotationProperty rdf:about="&vocab;contentsNote">
        <rdfs:label>Contents</rdfs:label>
        <rdfs:comment>List of subunits of the resource.</rdfs:comment>
        <rdfs:domain rdf:resource="&vocab;Instance"/>
    </owl:AnnotationProperty>
    


    <!-- http://bibframe.org/vocab/continuedBy -->

    <owl:AnnotationProperty rdf:about="&vocab;continuedBy">
        <rdfs:label>Continued by</rdfs:label>
        <dcterms:modified>2014-04-10 (Updated subproperty)</dcterms:modified>
        <rdfs:comment>Work whose content continues an earlier work under a new title.</rdfs:comment>
        <rdfs:subPropertyOf rdf:resource="&vocab;succeededBy"/>
    </owl:AnnotationProperty>
    


    <!-- http://bibframe.org/vocab/continuedInPartBy -->

    <owl:AnnotationProperty rdf:about="&vocab;continuedInPartBy">
        <rdfs:label>Continued in part by</rdfs:label>
        <rdfs:comment>Work part of whose content separated from an earlier work to form a new work.</rdfs:comment>
        <dcterms:modified>2014-04-10 (Updated subproperty)</dcterms:modified>
        <rdfs:subPropertyOf rdf:resource="&vocab;succeededBy"/>
    </owl:AnnotationProperty>
    


    <!-- http://bibframe.org/vocab/continues -->

    <owl:AnnotationProperty rdf:about="&vocab;continues">
        <rdfs:label>Continues</rdfs:label>
        <rdfs:comment>Work that is continued by the content of a later work under a new title.</rdfs:comment>
        <dcterms:modified>2014-04-10 (Updated subproperty)</dcterms:modified>
        <rdfs:subPropertyOf rdf:resource="&vocab;precededBy"/>
    </owl:AnnotationProperty>
    


    <!-- http://bibframe.org/vocab/continuesInPart -->

    <owl:AnnotationProperty rdf:about="&vocab;continuesInPart">
        <rdfs:label>Continues in part</rdfs:label>
        <rdfs:comment>Work that split into two or more separate works with new titles.</rdfs:comment>
        <dcterms:modified>2014-04-10 (Updated subproperty)</dcterms:modified>
        <rdfs:subPropertyOf rdf:resource="&vocab;precededBy"/>
    </owl:AnnotationProperty>
    


    <!-- http://bibframe.org/vocab/copyNote -->

    <owl:AnnotationProperty rdf:about="&vocab;copyNote">
        <rdfs:label>Copy note</rdfs:label>
        <rdfs:comment>Information about this copy.</rdfs:comment>
        <rdfs:domain rdf:resource="&vocab;HeldItem"/>
    </owl:AnnotationProperty>
    


    <!-- http://bibframe.org/vocab/copyrightDate -->

    <owl:AnnotationProperty rdf:about="&vocab;copyrightDate">
        <rdfs:label>Copyright date</rdfs:label>
        <rdfs:comment>Date associated with a claim of protection under copyright or a similar regime.</rdfs:comment>
        <rdfs:domain rdf:resource="&vocab;Provider"/>
    </owl:AnnotationProperty>
    


    <!-- http://bibframe.org/vocab/coverArt -->

    <owl:AnnotationProperty rdf:about="&vocab;coverArt">
        <rdfs:label>Cover art</rdfs:label>
        <rdfs:comment>Cover art image.</rdfs:comment>
    </owl:AnnotationProperty>
    


    <!-- http://bibframe.org/vocab/coverArtFor -->

    <owl:AnnotationProperty rdf:about="&vocab;coverArtFor">
        <rdfs:label>Cover art of instance</rdfs:label>
        <rdfs:comment>Resource to which the cover art pertains.</rdfs:comment>
    </owl:AnnotationProperty>
    


    <!-- http://bibframe.org/vocab/coverArtThumb -->

    <owl:AnnotationProperty rdf:about="&vocab;coverArtThumb">
        <rdfs:label>Thumbnail of cover art</rdfs:label>
        <rdfs:comment>Thumbnail version of cover art image.</rdfs:comment>
    </owl:AnnotationProperty>
    


    <!-- http://bibframe.org/vocab/custodialHistory -->

    <owl:AnnotationProperty rdf:about="&vocab;custodialHistory">
        <rdfs:label>Custodial history</rdfs:label>
        <rdfs:comment>Information about the provenance, such as origin, ownership and custodial history (chain of custody), of a resource.</rdfs:comment>
        <rdfs:domain rdf:resource="&vocab;Instance"/>
    </owl:AnnotationProperty>
    


    <!-- http://bibframe.org/vocab/dataSource -->

    <owl:AnnotationProperty rdf:about="&vocab;dataSource">
        <rdfs:label>Has data source</rdfs:label>
        <rdfs:comment>Work that is a data source to which the described resource is related. It may contain information about other files, printed sources, or collection procedures.</rdfs:comment>
    </owl:AnnotationProperty>
    


    <!-- http://bibframe.org/vocab/derivativeOf -->

    <owl:AnnotationProperty rdf:about="&vocab;derivativeOf">
        <rdfs:label>Is derivative of</rdfs:label>
        <rdfs:comment>Work is a modification of a source work.</rdfs:comment>
        <dcterms:modified>2014-04-30 (New)</dcterms:modified>
        <rdfs:subPropertyOf rdf:resource="&vocab;relatedTo"/>
    </owl:AnnotationProperty>
    


    <!-- http://bibframe.org/vocab/descriptionOf -->

    <owl:AnnotationProperty rdf:about="&vocab;descriptionOf">
        <rdfs:label>Is description of</rdfs:label>
        <rdfs:comment>Related resource that is analyzed, commented upon, critiqued, evaluated, reviewed, or otherwise described by the resource.</rdfs:comment>
        <dcterms:modified>2014-04-30 (New)</dcterms:modified>
        <rdfs:subPropertyOf rdf:resource="&vocab;relatedTo"/>
    </owl:AnnotationProperty>
    


    <!-- http://bibframe.org/vocab/dimensions -->

    <owl:AnnotationProperty rdf:about="&vocab;dimensions">
        <rdfs:label>Dimensions</rdfs:label>
        <rdfs:comment>Measurements of the carrier or carriers and/or the container of a resource.</rdfs:comment>
        <rdfs:domain rdf:resource="&vocab;Instance"/>
    </owl:AnnotationProperty>
    


    <!-- http://bibframe.org/vocab/dissertationDegree -->

    <owl:AnnotationProperty rdf:about="&vocab;dissertationDegree">
        <rdfs:label>Degree</rdfs:label>
        <rdfs:comment>Degree for which author was a candidate.</rdfs:comment>
        <rdfs:domain rdf:resource="&vocab;Work"/>
    </owl:AnnotationProperty>
    


    <!-- http://bibframe.org/vocab/dissertationIdentifier -->

    <owl:AnnotationProperty rdf:about="&vocab;dissertationIdentifier">
        <rdfs:label>Dissertation identifier</rdfs:label>
        <rdfs:comment>Identifier assigned to a dissertation for identification purposes .</rdfs:comment>
    </owl:AnnotationProperty>
    


    <!-- http://bibframe.org/vocab/dissertationInstitution -->

    <owl:AnnotationProperty rdf:about="&vocab;dissertationInstitution">
        <rdfs:label>Degree issuing institution</rdfs:label>
        <rdfs:comment>Name of degree granting institution.</rdfs:comment>
    </owl:AnnotationProperty>
    


    <!-- http://bibframe.org/vocab/dissertationNote -->

    <owl:AnnotationProperty rdf:about="&vocab;dissertationNote">
        <rdfs:label>Dissertation note</rdfs:label>
        <rdfs:comment>Textual information about the dissertation.</rdfs:comment>
        <rdfs:domain rdf:resource="&vocab;Work"/>
    </owl:AnnotationProperty>
    


    <!-- http://bibframe.org/vocab/dissertationYear -->

    <owl:AnnotationProperty rdf:about="&vocab;dissertationYear">
        <rdfs:label>Year degree awarded</rdfs:label>
        <rdfs:comment>Year degree awarded.</rdfs:comment>
        <rdfs:domain rdf:resource="&vocab;Work"/>
    </owl:AnnotationProperty>
    


    <!-- http://bibframe.org/vocab/distribution -->

    <owl:AnnotationProperty rdf:about="&vocab;distribution">
        <rdfs:label>Distribution event</rdfs:label>
        <rdfs:comment>Information relating to distribution of an instance.</rdfs:comment>
    </owl:AnnotationProperty>
    


    <!-- http://bibframe.org/vocab/doi -->

    <owl:AnnotationProperty rdf:about="&vocab;doi">
        <rdfs:label>DOI</rdfs:label>
        <rdfs:comment>Digital Object Identifier.</rdfs:comment>
    </owl:AnnotationProperty>
    


    <!-- http://bibframe.org/vocab/duration -->

    <owl:AnnotationProperty rdf:about="&vocab;duration">
        <rdfs:label>Duration</rdfs:label>
        <rdfs:comment>Information about the playing time or duration in an unstructured form, e.g., &quot;2 hours&quot;.</rdfs:comment>
        <rdfs:domain rdf:resource="&vocab;Instance"/>
    </owl:AnnotationProperty>
    


    <!-- http://bibframe.org/vocab/ean -->

    <owl:AnnotationProperty rdf:about="&vocab;ean">
        <rdfs:label>EAN</rdfs:label>
        <rdfs:comment>International Article Identifier.</rdfs:comment>
    </owl:AnnotationProperty>
    


    <!-- http://bibframe.org/vocab/edition -->

    <owl:AnnotationProperty rdf:about="&vocab;edition">
        <rdfs:label>Edition statement</rdfs:label>
        <rdfs:comment>Information identifying the edition or version of the resource.</rdfs:comment>
        <rdfs:domain rdf:resource="&vocab;Instance"/>
    </owl:AnnotationProperty>
    


    <!-- http://bibframe.org/vocab/editionResponsibility -->

    <owl:AnnotationProperty rdf:about="&vocab;editionResponsibility">
        <rdfs:label>Edition responsibility</rdfs:label>
        <rdfs:comment>Statement relating to the identification of any persons, families, or corporate bodies responsible for the edition being described.</rdfs:comment>
        <rdfs:domain rdf:resource="&vocab;Instance"/>
    </owl:AnnotationProperty>
    


    <!-- http://bibframe.org/vocab/electronicLocator -->

    <owl:AnnotationProperty rdf:about="&vocab;electronicLocator">
        <rdfs:label>Electronic location</rdfs:label>
        <dcterms:modified>2014-04-28 (New)</dcterms:modified>
        <rdfs:comment>Electronic location from which the resource is available.</rdfs:comment>
    </owl:AnnotationProperty>
    


    <!-- http://bibframe.org/vocab/enumerationAndChronology -->

    <owl:AnnotationProperty rdf:about="&vocab;enumerationAndChronology">
        <rdfs:label>Enumeration and chronology</rdfs:label>
        <rdfs:comment>Numbering and dates of holding.</rdfs:comment>
        <rdfs:domain rdf:resource="&vocab;HeldMaterial"/>
    </owl:AnnotationProperty>
    


    <!-- http://bibframe.org/vocab/event -->

    <owl:AnnotationProperty rdf:about="&vocab;event">
        <rdfs:label>Event associated with content</rdfs:label>
        <rdfs:comment>Information about the geographic area/or time period covered by an event (e.g., a report).</rdfs:comment>
        <dcterms:modified>2014-05-16 (Updated)</dcterms:modified>
    </owl:AnnotationProperty>
    


    <!-- http://bibframe.org/vocab/eventAgent -->

    <owl:AnnotationProperty rdf:about="&vocab;eventAgent">
        <rdfs:label>Agent for event</rdfs:label>
        <dcterms:modified>2014-05-16 (Updated)</dcterms:modified>
        <rdfs:comment>Person or organization associated with event.</rdfs:comment>
    </owl:AnnotationProperty>
    


    <!-- http://bibframe.org/vocab/eventDate -->

    <owl:AnnotationProperty rdf:about="&vocab;eventDate">
        <rdfs:label>Date(s) of event</rdfs:label>
        <rdfs:comment>Date, time or period of event.</rdfs:comment>
        <dcterms:modified>2014-05-16 (Updated)</dcterms:modified>
        <rdfs:domain rdf:resource="&vocab;Event"/>
    </owl:AnnotationProperty>
    


    <!-- http://bibframe.org/vocab/eventPlace -->

    <owl:AnnotationProperty rdf:about="&vocab;eventPlace">
        <rdfs:label>Place of event</rdfs:label>
        <rdfs:comment>Geographic area associated with event.</rdfs:comment>
    </owl:AnnotationProperty>
    


    <!-- http://bibframe.org/vocab/expressionOf -->

    <owl:AnnotationProperty rdf:about="&vocab;expressionOf">
        <rdfs:label>Expression of</rdfs:label>
        <dcterms:modified>2014-04-10 (Updated subproperty)</dcterms:modified>
        <rdfs:comment>Expression has a related work. For use to connect Works under FRBR/RDA rules.</rdfs:comment>
    </owl:AnnotationProperty>
    


    <!-- http://bibframe.org/vocab/extent -->

    <owl:AnnotationProperty rdf:about="&vocab;extent">
        <rdfs:label>Extent</rdfs:label>
        <rdfs:comment>Number and type of units and/or subunits making up a resource.</rdfs:comment>
        <rdfs:domain rdf:resource="&vocab;Instance"/>
    </owl:AnnotationProperty>
    


    <!-- http://bibframe.org/vocab/findingAid -->

    <owl:AnnotationProperty rdf:about="&vocab;findingAid">
        <rdfs:label>Has finding aid</rdfs:label>
        <rdfs:comment>Relationship is to a finding aid or similar control materials for archival, visual, and manuscript resources.</rdfs:comment>
        <rdfs:subPropertyOf rdf:resource="&vocab;accompaniedBy"/>
    </owl:AnnotationProperty>
    


    <!-- http://bibframe.org/vocab/fingerprint -->

    <owl:AnnotationProperty rdf:about="&vocab;fingerprint">
        <rdfs:label>Fingerprint identifier</rdfs:label>
        <rdfs:comment>Identifier that is used to assist in the identification of antiquarian books by recording information comprising groups of characters taken from specified positions on specified pages of the book.</rdfs:comment>
    </owl:AnnotationProperty>
    


    <!-- http://bibframe.org/vocab/formDesignation -->

    <owl:AnnotationProperty rdf:about="&vocab;formDesignation">
        <rdfs:label>Form designation</rdfs:label>
        <rdfs:comment>Class or genre to which a Work or Instance belongs.</rdfs:comment>
        <dcterms:modified>2014-03-21 (Range updated)</dcterms:modified>
        <rdfs:domain rdf:resource="&vocab;Title"/>
    </owl:AnnotationProperty>
    


    <!-- http://bibframe.org/vocab/format -->

    <owl:AnnotationProperty rdf:about="&vocab;format">
        <rdfs:label>Format</rdfs:label>
        <dcterms:modified>2014-10-27 (Updated)</dcterms:modified>
        <rdfs:comment>File format or physical medium of an instance.</rdfs:comment>
        <rdfs:domain rdf:resource="&vocab;Instance"/>
    </owl:AnnotationProperty>
    


    <!-- http://bibframe.org/vocab/formatOfMusic -->

    <owl:AnnotationProperty rdf:about="&vocab;formatOfMusic">
        <rdfs:label>Format of music</rdfs:label>
        <rdfs:comment>Format of a musical composition, e.g. full score, condensed score, vocal score, etc.</rdfs:comment>
        <rdfs:domain rdf:resource="&vocab;Instance"/>
    </owl:AnnotationProperty>
    


    <!-- http://bibframe.org/vocab/frequency -->

    <owl:AnnotationProperty rdf:about="&vocab;frequency">
        <rdfs:label>Frequency</rdfs:label>
        <rdfs:comment>Intervals at which the issues or parts of a serial or the updates to an integrating resource are issued.</rdfs:comment>
        <rdfs:domain rdf:resource="&vocab;Instance"/>
    </owl:AnnotationProperty>
    


    <!-- http://bibframe.org/vocab/frequencyNote -->

    <owl:AnnotationProperty rdf:about="&vocab;frequencyNote">
        <rdfs:label>Frequency note</rdfs:label>
        <rdfs:comment>Current or former publication frequency of a resource.</rdfs:comment>
        <rdfs:domain rdf:resource="&vocab;Instance"/>
    </owl:AnnotationProperty>
    


    <!-- http://bibframe.org/vocab/geographicCoverageNote -->

    <owl:AnnotationProperty rdf:about="&vocab;geographicCoverageNote">
        <rdfs:label>Geographic coverage</rdfs:label>
        <rdfs:comment>Geographic entities covered by the resource.</rdfs:comment>
        <rdfs:domain rdf:resource="&vocab;Work"/>
    </owl:AnnotationProperty>
    


    <!-- http://bibframe.org/vocab/graphicScaleNote -->

    <owl:AnnotationProperty rdf:about="&vocab;graphicScaleNote">
        <rdfs:label>Graphic scale</rdfs:label>
        <rdfs:comment>Textual information about scale, including the scale of graphic material item such as architectural drawings or three-dimensional artifacts.</rdfs:comment>
        <rdfs:domain rdf:resource="&vocab;Instance"/>
    </owl:AnnotationProperty>
    


    <!-- http://bibframe.org/vocab/hasAccompaniment -->

    <owl:AnnotationProperty rdf:about="&vocab;hasAccompaniment"/>
    


    <!-- http://bibframe.org/vocab/hasAuthority -->

    <owl:AnnotationProperty rdf:about="&vocab;hasAuthority">
        <rdfs:label>Authority information</rdfs:label>
        <rdfs:comment>Link to controlled form of name or subject and other information about.</rdfs:comment>
        <dcterms:modified>2014-04-10 (Updated range)</dcterms:modified>
    </owl:AnnotationProperty>
    


    <!-- http://bibframe.org/vocab/hasDerivative -->

    <owl:AnnotationProperty rdf:about="&vocab;hasDerivative">
        <rdfs:label>Has derivative</rdfs:label>
        <rdfs:comment>Work has a modification for which it is the source.</rdfs:comment>
        <dcterms:modified>2014-04-10 (Range updated)</dcterms:modified>
        <rdfs:subPropertyOf rdf:resource="&vocab;relatedTo"/>
    </owl:AnnotationProperty>
    


    <!-- http://bibframe.org/vocab/hasDescription -->

    <owl:AnnotationProperty rdf:about="&vocab;hasDescription">
        <rdfs:label>Has description</rdfs:label>
        <rdfs:comment>Related resource that analyzes, comments on, critiques, evaluates, reviews, or otherwise describes the resource.</rdfs:comment>
        <dcterms:modified>2014-04-10 (Range updated)</dcterms:modified>
        <rdfs:subPropertyOf rdf:resource="&vocab;relatedTo"/>
    </owl:AnnotationProperty>
    


    <!-- http://bibframe.org/vocab/hasEquivalent -->

    <owl:AnnotationProperty rdf:about="&vocab;hasEquivalent">
        <rdfs:label>Equivalence</rdfs:label>
        <rdfs:comment>Instance embodies the same expression of a work as the resource being described.</rdfs:comment>
        <dcterms:modified>2014-04-10 (Range updated)</dcterms:modified>
        <rdfs:subPropertyOf rdf:resource="&vocab;relatedTo"/>
    </owl:AnnotationProperty>
    


    <!-- http://bibframe.org/vocab/hasExpression -->

    <owl:AnnotationProperty rdf:about="&vocab;hasExpression">
        <rdfs:label>Expressed as</rdfs:label>
        <rdfs:comment>Work has a related expression. For use to connect Works under FRBR/RDA rules.</rdfs:comment>
        <dcterms:modified>2014-04-10 (Updated subproperty)</dcterms:modified>
    </owl:AnnotationProperty>
    


    <!-- http://bibframe.org/vocab/hasInstance -->

    <owl:AnnotationProperty rdf:about="&vocab;hasInstance">
        <rdfs:label>Instance of Work</rdfs:label>
        <rdfs:comment>Work has a related Instance/manifestation. For use to connect Works to Instances in the BIBFRAME structure.</rdfs:comment>
        <dcterms:modified>2014--03-21 (Updated definition)</dcterms:modified>
    </owl:AnnotationProperty>
    


    <!-- http://bibframe.org/vocab/hasPart -->

    <owl:AnnotationProperty rdf:about="&vocab;hasPart">
        <rdfs:label>Has part</rdfs:label>
        <rdfs:comment>Resource that is included either physically or logically contained in the described resource</rdfs:comment>
        <dcterms:modified>2014-04-10 (Range updated)</dcterms:modified>
        <rdfs:subPropertyOf rdf:resource="&vocab;relatedTo"/>
    </owl:AnnotationProperty>
    


    <!-- http://bibframe.org/vocab/hdl -->

    <owl:AnnotationProperty rdf:about="&vocab;hdl">
        <rdfs:label>Handle</rdfs:label>
        <rdfs:comment>Unique and persistent identifier for digital objects developed by the Corporation for National Research Initiatives.</rdfs:comment>
    </owl:AnnotationProperty>
    


    <!-- http://bibframe.org/vocab/heldBy -->

    <owl:AnnotationProperty rdf:about="&vocab;heldBy">
        <rdfs:label>Held by</rdfs:label>
        <rdfs:comment>Entity holding the item or from which it is available</rdfs:comment>
    </owl:AnnotationProperty>
    


    <!-- http://bibframe.org/vocab/holdingFor -->

    <owl:AnnotationProperty rdf:about="&vocab;holdingFor">
        <rdfs:label>Holding for</rdfs:label>
        <rdfs:comment>Instance for which holding is reported</rdfs:comment>
    </owl:AnnotationProperty>
    


    <!-- http://bibframe.org/vocab/identifier -->

    <owl:AnnotationProperty rdf:about="&vocab;identifier">
        <rdfs:label>Identifier</rdfs:label>
        <rdfs:comment>Number or code that uniquely identifies an entity.</rdfs:comment>
    </owl:AnnotationProperty>
    


    <!-- http://bibframe.org/vocab/identifierAssigner -->

    <owl:AnnotationProperty rdf:about="&vocab;identifierAssigner">
        <rdfs:label>Identifier assigner</rdfs:label>
        <rdfs:comment>Entity that assigned the identifier.</rdfs:comment>
        <rdfs:domain rdf:resource="&vocab;Identifier"/>
    </owl:AnnotationProperty>
    


    <!-- http://bibframe.org/vocab/identifierQualifier -->

    <owl:AnnotationProperty rdf:about="&vocab;identifierQualifier">
        <rdfs:label>Identifier qualifier</rdfs:label>
        <rdfs:comment>Qualifying information associated with the identifier, e.g. specifying its applicability.</rdfs:comment>
        <rdfs:domain rdf:resource="&vocab;Identifier"/>
    </owl:AnnotationProperty>
    


    <!-- http://bibframe.org/vocab/identifierScheme -->

    <owl:AnnotationProperty rdf:about="&vocab;identifierScheme">
        <rdfs:label>Identifier scheme</rdfs:label>
        <rdfs:comment>Scheme within which the identifier is unique.</rdfs:comment>
        <dcterms:modified>2014-06-04 (Updated mapping)</dcterms:modified>
        <dcterms:modified>&apos;2014-06-04 (Updated range)</dcterms:modified>
    </owl:AnnotationProperty>
    


    <!-- http://bibframe.org/vocab/identifierStatus -->

    <owl:AnnotationProperty rdf:about="&vocab;identifierStatus">
        <rdfs:label>Identifier status</rdfs:label>
        <rdfs:comment>Indication of whether the identifier is canceled or invalid.</rdfs:comment>
        <rdfs:domain rdf:resource="&vocab;Identifier"/>
    </owl:AnnotationProperty>
    


    <!-- http://bibframe.org/vocab/identifierValue -->

    <owl:AnnotationProperty rdf:about="&vocab;identifierValue">
        <rdfs:label>Identifier value</rdfs:label>
        <rdfs:comment>Value of the identifier.</rdfs:comment>
        <rdfs:domain rdf:resource="&vocab;Identifier"/>
    </owl:AnnotationProperty>
    


    <!-- http://bibframe.org/vocab/illustrationNote -->

    <owl:AnnotationProperty rdf:about="&vocab;illustrationNote">
        <rdfs:label>Illustrative content note</rdfs:label>
        <rdfs:comment>Information about illustrative material in the resource.</rdfs:comment>
        <rdfs:domain rdf:resource="&vocab;Instance"/>
    </owl:AnnotationProperty>
    


    <!-- http://bibframe.org/vocab/index -->

    <owl:AnnotationProperty rdf:about="&vocab;index">
        <rdfs:label>Index</rdfs:label>
        <rdfs:comment>Work has an accompanying index</rdfs:comment>
        <rdfs:subPropertyOf rdf:resource="&vocab;accompaniedBy"/>
    </owl:AnnotationProperty>
    


    <!-- http://bibframe.org/vocab/instanceOf -->

    <owl:AnnotationProperty rdf:about="&vocab;instanceOf">
        <rdfs:label>Instance of</rdfs:label>
        <rdfs:comment>Work this resource instantiates or manifests. For use to connect Instances to Works in the BIBFRAME structure.</rdfs:comment>
        <dcterms:modified>2014--03-21 (Updated definition)</dcterms:modified>
    </owl:AnnotationProperty>
    


    <!-- http://bibframe.org/vocab/instanceTitle -->

    <owl:AnnotationProperty rdf:about="&vocab;instanceTitle">
        <rdfs:label>Instance title</rdfs:label>
        <rdfs:comment>Word, character, or group of words and/or characters that is the main name of an instance.</rdfs:comment>
    </owl:AnnotationProperty>
    


    <!-- http://bibframe.org/vocab/isan -->

    <owl:AnnotationProperty rdf:about="&vocab;isan">
        <rdfs:label>ISAN</rdfs:label>
        <rdfs:comment>International Standard Audiovisual Number.</rdfs:comment>
    </owl:AnnotationProperty>
    


    <!-- http://bibframe.org/vocab/isbn -->

    <owl:AnnotationProperty rdf:about="&vocab;isbn">
        <rdfs:label>ISBN</rdfs:label>
        <rdfs:comment>International Standard Book Number.</rdfs:comment>
    </owl:AnnotationProperty>
    


    <!-- http://bibframe.org/vocab/isbn10 -->

    <owl:AnnotationProperty rdf:about="&vocab;isbn10">
        <rdfs:label>ISBN-10</rdfs:label>
        <rdfs:comment>10 digit version of the International Standard Book Number.</rdfs:comment>
    </owl:AnnotationProperty>
    


    <!-- http://bibframe.org/vocab/isbn13 -->

    <owl:AnnotationProperty rdf:about="&vocab;isbn13">
        <rdfs:label>ISBN-13</rdfs:label>
        <rdfs:comment>13 digit version of the International Standard Book Number.</rdfs:comment>
    </owl:AnnotationProperty>
    


    <!-- http://bibframe.org/vocab/ismn -->

    <owl:AnnotationProperty rdf:about="&vocab;ismn">
        <rdfs:label>ISMN</rdfs:label>
        <rdfs:comment>International Standard Music Number.</rdfs:comment>
    </owl:AnnotationProperty>
    


    <!-- http://bibframe.org/vocab/iso -->

    <owl:AnnotationProperty rdf:about="&vocab;iso">
        <rdfs:label>ISO number</rdfs:label>
        <rdfs:comment>International Organization for Standardization standard number.</rdfs:comment>
    </owl:AnnotationProperty>
    


    <!-- http://bibframe.org/vocab/issn -->

    <owl:AnnotationProperty rdf:about="&vocab;issn">
        <rdfs:label>ISSN</rdfs:label>
        <rdfs:comment>International Standard Serial Number identifier.</rdfs:comment>
    </owl:AnnotationProperty>
    


    <!-- http://bibframe.org/vocab/issnL -->

    <owl:AnnotationProperty rdf:about="&vocab;issnL">
        <rdfs:label>ISSN-L</rdfs:label>
        <rdfs:comment>International Standard Serial Number that links together various media versions of a continuing resource.</rdfs:comment>
    </owl:AnnotationProperty>
    


    <!-- http://bibframe.org/vocab/issueNumber -->

    <owl:AnnotationProperty rdf:about="&vocab;issueNumber">
        <rdfs:label>Audio issue number</rdfs:label>
        <rdfs:comment>Number used to identify the issue designation, or serial identification, assigned by a publisher to a sound recording.</rdfs:comment>
    </owl:AnnotationProperty>
    


    <!-- http://bibframe.org/vocab/issuedWith -->

    <owl:AnnotationProperty rdf:about="&vocab;issuedWith">
        <rdfs:label>Issued with</rdfs:label>
        <rdfs:comment>Instance that is issued on the same carrier as the manifestation being described.</rdfs:comment>
        <rdfs:subPropertyOf rdf:resource="&vocab;hasAccompaniment"/>
    </owl:AnnotationProperty>
    


    <!-- http://bibframe.org/vocab/istc -->

    <owl:AnnotationProperty rdf:about="&vocab;istc">
        <rdfs:label>ISTC</rdfs:label>
        <rdfs:comment>International Standard Text code, a numbering system developed to enable the unique identification of textual works.</rdfs:comment>
        <dcterms:modified>a,z</dcterms:modified>
    </owl:AnnotationProperty>
    


    <!-- http://bibframe.org/vocab/iswc -->

    <owl:AnnotationProperty rdf:about="&vocab;iswc">
        <rdfs:label>ISWC</rdfs:label>
        <rdfs:comment>International Standard Musical Work Code, a unique, persistent reference number for the identification of musical works.</rdfs:comment>
    </owl:AnnotationProperty>
    


    <!-- http://bibframe.org/vocab/itemId -->

    <owl:AnnotationProperty rdf:about="&vocab;itemId">
        <rdfs:label>System item identifier</rdfs:label>
        <rdfs:comment>Identification number assigned to data about one item held.</rdfs:comment>
        <rdfs:domain rdf:resource="&vocab;HeldItem"/>
    </owl:AnnotationProperty>
    


    <!-- http://bibframe.org/vocab/keyTitle -->

    <owl:AnnotationProperty rdf:about="&vocab;keyTitle">
        <rdfs:label>Key title</rdfs:label>
        <rdfs:comment>Unique title for a continuing resource that is assigned by the ISSN International Center in conjunction with an ISSN.</rdfs:comment>
    </owl:AnnotationProperty>
    


    <!-- http://bibframe.org/vocab/label -->

    <owl:AnnotationProperty rdf:about="&vocab;label">
        <rdfs:label>Label</rdfs:label>
        <rdfs:comment>Text string expressing the property value.</rdfs:comment>
        <rdfs:domain rdf:resource="&vocab;Resource"/>
    </owl:AnnotationProperty>
    


    <!-- http://bibframe.org/vocab/languageNote -->

    <owl:AnnotationProperty rdf:about="&vocab;languageNote">
        <rdfs:label>Language note</rdfs:label>
        <rdfs:comment>Note concerning the language of the material or its parts.</rdfs:comment>
        <rdfs:domain rdf:resource="&vocab;Work"/>
    </owl:AnnotationProperty>
    


    <!-- http://bibframe.org/vocab/languageOfPart -->

    <owl:AnnotationProperty rdf:about="&vocab;languageOfPart">
        <rdfs:label>Language of part</rdfs:label>
        <rdfs:comment>Language or notation system used to convey the content of the resource (associated with part or all of a resource).</rdfs:comment>
        <rdfs:domain rdf:resource="&vocab;Language"/>
    </owl:AnnotationProperty>
    


    <!-- http://bibframe.org/vocab/languageOfPartUri -->

    <owl:AnnotationProperty rdf:about="&vocab;languageOfPartUri">
        <rdfs:label>Language of part URI</rdfs:label>
        <rdfs:comment>Language or notation system used to convey the content of the resource (associated with part or all of a resource).</rdfs:comment>
    </owl:AnnotationProperty>
    


    <!-- http://bibframe.org/vocab/languageSource -->

    <owl:AnnotationProperty rdf:about="&vocab;languageSource">
        <rdfs:label>Language source</rdfs:label>
        <rdfs:comment>Language code or name list from which value is taken.</rdfs:comment>
        <rdfs:domain rdf:resource="&vocab;Language"/>
    </owl:AnnotationProperty>
    


    <!-- http://bibframe.org/vocab/lcOverseasAcq -->

    <owl:AnnotationProperty rdf:about="&vocab;lcOverseasAcq">
        <rdfs:label>LC acquisition program</rdfs:label>
        <rdfs:comment>Identification number assigned by the Library of Congress to works acquired through one of its overseas acquisition programs.</rdfs:comment>
    </owl:AnnotationProperty>
    


    <!-- http://bibframe.org/vocab/lccn -->

    <owl:AnnotationProperty rdf:about="&vocab;lccn">
        <rdfs:label>LCCN</rdfs:label>
        <rdfs:comment>Library of Congress Control Number, which identifies the resource description.</rdfs:comment>
    </owl:AnnotationProperty>
    


    <!-- http://bibframe.org/vocab/legalDeposit -->

    <owl:AnnotationProperty rdf:about="&vocab;legalDeposit">
        <rdfs:label>Copyright number</rdfs:label>
        <rdfs:comment>Number assigned to a copyright or legal deposit, which Identifies a resource description.</rdfs:comment>
    </owl:AnnotationProperty>
    


    <!-- http://bibframe.org/vocab/lendingPolicy -->

    <owl:AnnotationProperty rdf:about="&vocab;lendingPolicy">
        <rdfs:label>Lending policy</rdfs:label>
        <rdfs:comment>Policy statement about whether and with what restrictions the holding may be lent</rdfs:comment>
        <rdfs:domain rdf:resource="&vocab;HeldMaterial"/>
    </owl:AnnotationProperty>
    


    <!-- http://bibframe.org/vocab/local -->

    <owl:AnnotationProperty rdf:about="&vocab;local">
        <rdfs:label>Local identifier</rdfs:label>
        <rdfs:comment>Identifier established locally and not a standard number.</rdfs:comment>
    </owl:AnnotationProperty>
    


    <!-- http://bibframe.org/vocab/manufacture -->

    <owl:AnnotationProperty rdf:about="&vocab;manufacture">
        <rdfs:label>Manufacture event</rdfs:label>
        <rdfs:comment>Information relating to manufacture of an instance.</rdfs:comment>
    </owl:AnnotationProperty>
    


    <!-- http://bibframe.org/vocab/materialArrangement -->

    <owl:AnnotationProperty rdf:about="&vocab;materialArrangement">
        <rdfs:label>Arrangement of material</rdfs:label>
        <rdfs:comment>Pattern of arrangement of materials within a unit.</rdfs:comment>
        <rdfs:domain rdf:resource="&vocab;Arrangement"/>
    </owl:AnnotationProperty>
    


    <!-- http://bibframe.org/vocab/materialHierarchicalLevel -->

    <owl:AnnotationProperty rdf:about="&vocab;materialHierarchicalLevel">
        <rdfs:label>Hierarchical level of material</rdfs:label>
        <rdfs:comment>Hierarchical position of the described materials relative to other material from the same source.</rdfs:comment>
        <rdfs:domain rdf:resource="&vocab;Arrangement"/>
    </owl:AnnotationProperty>
    


    <!-- http://bibframe.org/vocab/materialOrganization -->

    <owl:AnnotationProperty rdf:about="&vocab;materialOrganization">
        <rdfs:label>Organization of material</rdfs:label>
        <rdfs:comment>Manner in which resource is divided into smaller units.</rdfs:comment>
        <rdfs:domain rdf:resource="&vocab;Arrangement"/>
    </owl:AnnotationProperty>
    


    <!-- http://bibframe.org/vocab/materialPart -->

    <owl:AnnotationProperty rdf:about="&vocab;materialPart">
        <rdfs:label>Part of material</rdfs:label>
        <rdfs:comment>Part of the resource to which information applies.</rdfs:comment>
        <rdfs:domain rdf:resource="&vocab;Arrangement"/>
    </owl:AnnotationProperty>
    


    <!-- http://bibframe.org/vocab/matrixNumber -->

    <owl:AnnotationProperty rdf:about="&vocab;matrixNumber">
        <rdfs:label>Audio matrix number</rdfs:label>
        <rdfs:comment>Matrix number from the master from which a specific sound recording was pressed.</rdfs:comment>
    </owl:AnnotationProperty>
    


    <!-- http://bibframe.org/vocab/mediaCategory -->

    <owl:AnnotationProperty rdf:about="&vocab;mediaCategory">
        <rdfs:label>Media type</rdfs:label>
        <rdfs:comment>Categorization reflecting the general type of intermediation device required to view, play, run, etc., the content of a resource.</rdfs:comment>
    </owl:AnnotationProperty>
    


    <!-- http://bibframe.org/vocab/mergedToForm -->

    <owl:AnnotationProperty rdf:about="&vocab;mergedToForm">
        <rdfs:label>Merged to form</rdfs:label>
        <rdfs:comment>One of two or more works that come together to form a new work.</rdfs:comment>
        <dcterms:modified>2014-04-10 (Updated subproperty)</dcterms:modified>
        <rdfs:subPropertyOf rdf:resource="&vocab;succeededBy"/>
    </owl:AnnotationProperty>
    


    <!-- http://bibframe.org/vocab/modeOfIssuance -->

    <owl:AnnotationProperty rdf:about="&vocab;modeOfIssuance">
        <rdfs:label>Mode of issuance</rdfs:label>
        <rdfs:comment>Categorization reflecting whether a resource is issued in one or more parts, the way it is updated, and its intended termination.</rdfs:comment>
        <rdfs:domain rdf:resource="&vocab;Instance"/>
    </owl:AnnotationProperty>
    


    <!-- http://bibframe.org/vocab/musicPlate -->

    <owl:AnnotationProperty rdf:about="&vocab;musicPlate">
        <rdfs:label>Music plate number</rdfs:label>
        <rdfs:comment>Number assigned by a music publisher to a specific music publication.</rdfs:comment>
    </owl:AnnotationProperty>
    


    <!-- http://bibframe.org/vocab/musicPublisherNumber -->

    <owl:AnnotationProperty rdf:about="&vocab;musicPublisherNumber">
        <rdfs:label>Music publisher number</rdfs:label>
        <rdfs:comment>Number assigned to a music publication other than an issue, matrix, or plate number.</rdfs:comment>
    </owl:AnnotationProperty>
    


    <!-- http://bibframe.org/vocab/nban -->

    <owl:AnnotationProperty rdf:about="&vocab;nban">
        <rdfs:label>NBAN</rdfs:label>
        <rdfs:comment>National Bibliography Agency Number, which identifies the resource description.</rdfs:comment>
    </owl:AnnotationProperty>
    


    <!-- http://bibframe.org/vocab/nbn -->

    <owl:AnnotationProperty rdf:about="&vocab;nbn">
        <rdfs:label>NBN</rdfs:label>
        <rdfs:comment>National Bibliography Number, which identifies the resource description.</rdfs:comment>
    </owl:AnnotationProperty>
    


    <!-- http://bibframe.org/vocab/notation -->

    <owl:AnnotationProperty rdf:about="&vocab;notation">
        <rdfs:label>Notation system</rdfs:label>
        <rdfs:comment>Information on the alphabet, script, or symbol system used to convey the content of the resource, including specialized scripts, typefaces, tactile notation, and musical notation.</rdfs:comment>
        <rdfs:domain rdf:resource="&vocab;Instance"/>
    </owl:AnnotationProperty>
    


    <!-- http://bibframe.org/vocab/originDate -->

    <owl:AnnotationProperty rdf:about="&vocab;originDate">
        <rdfs:label>Associated title date</rdfs:label>
        <dcterms:modified>2014-07-23 (Example added)</dcterms:modified>
        <rdfs:comment>Date or date range associated with the creation of the work.</rdfs:comment>
        <rdfs:domain rdf:resource="&vocab;Work"/>
    </owl:AnnotationProperty>
    


    <!-- http://bibframe.org/vocab/originPlace -->

    <owl:AnnotationProperty rdf:about="&vocab;originPlace">
        <rdfs:label>Associated title place</rdfs:label>
        <rdfs:comment>Place from which the creation of the work originated.</rdfs:comment>
    </owl:AnnotationProperty>
    


    <!-- http://bibframe.org/vocab/originalVersion -->

    <owl:AnnotationProperty rdf:about="&vocab;originalVersion">
        <rdfs:label>Has original version</rdfs:label>
        <rdfs:comment>Instance is the original version of which this resource is a reproduction.</rdfs:comment>
        <rdfs:subPropertyOf rdf:resource="&vocab;derivativeOf"/>
    </owl:AnnotationProperty>
    


    <!-- http://bibframe.org/vocab/otherEdition -->

    <owl:AnnotationProperty rdf:about="&vocab;otherEdition">
        <rdfs:label>hasOtherEdition</rdfs:label>
        <rdfs:comment>Resource has other available editions, for example simultaneously published language editions or reprints.</rdfs:comment>
        <rdfs:subPropertyOf rdf:resource="&vocab;derivativeOf"/>
    </owl:AnnotationProperty>
    


    <!-- http://bibframe.org/vocab/otherPhysicalFormat -->

    <owl:AnnotationProperty rdf:about="&vocab;otherPhysicalFormat">
        <rdfs:label>Has other physical format</rdfs:label>
        <dcterms:modified>2014-10-14 (Updated)</dcterms:modified>
        <rdfs:comment>Resource that is manifested in another physical carrier.</rdfs:comment>
        <rdfs:subPropertyOf rdf:resource="&vocab;hasEquivalent"/>
    </owl:AnnotationProperty>
    


    <!-- http://bibframe.org/vocab/partNumber -->

    <owl:AnnotationProperty rdf:about="&vocab;partNumber">
        <rdfs:label>Part number</rdfs:label>
        <rdfs:comment>Part or section number of a title.</rdfs:comment>
        <rdfs:domain rdf:resource="&vocab;Title"/>
    </owl:AnnotationProperty>
    


    <!-- http://bibframe.org/vocab/partOf -->

    <owl:AnnotationProperty rdf:about="&vocab;partOf">
        <rdfs:label>Is part of</rdfs:label>
        <rdfs:comment>Resource in which the described resource is physically or logically contained.</rdfs:comment>
        <dcterms:modified>2014-04-30 (New)</dcterms:modified>
        <rdfs:subPropertyOf rdf:resource="&vocab;relatedTo"/>
    </owl:AnnotationProperty>
    


    <!-- http://bibframe.org/vocab/partTitle -->

    <owl:AnnotationProperty rdf:about="&vocab;partTitle">
        <rdfs:label>Part title</rdfs:label>
        <rdfs:comment>Part or section name of a title.</rdfs:comment>
        <rdfs:domain rdf:resource="&vocab;Title"/>
    </owl:AnnotationProperty>
    


    <!-- http://bibframe.org/vocab/postalRegistration -->

    <owl:AnnotationProperty rdf:about="&vocab;postalRegistration">
        <rdfs:label>Postal registration number</rdfs:label>
        <rdfs:comment>Number assigned to a publication for which the specified postal service permits the use of a special mailing class privilege.</rdfs:comment>
    </owl:AnnotationProperty>
    


    <!-- http://bibframe.org/vocab/precededBy -->

    <owl:AnnotationProperty rdf:about="&vocab;precededBy">
        <rdfs:label>Preceded By</rdfs:label>
        <dcterms:modified>2014-04-10 (Renamed)</dcterms:modified>
        <rdfs:comment>Resource that precedes the resource being described (e.g., is earlier in time or before in narrative).</rdfs:comment>
        <rdfs:subPropertyOf rdf:resource="&vocab;relatedTo"/>
    </owl:AnnotationProperty>
    


    <!-- http://bibframe.org/vocab/preferredCitation -->

    <owl:AnnotationProperty rdf:about="&vocab;preferredCitation">
        <rdfs:label>Preferred citation</rdfs:label>
        <rdfs:comment>Citation to the resource preferred by its custodian.</rdfs:comment>
        <rdfs:domain rdf:resource="&vocab;Instance"/>
    </owl:AnnotationProperty>
    


    <!-- http://bibframe.org/vocab/production -->

    <owl:AnnotationProperty rdf:about="&vocab;production">
        <rdfs:label>Production event</rdfs:label>
        <rdfs:comment>Information relating to production of an instance.</rdfs:comment>
    </owl:AnnotationProperty>
    


    <!-- http://bibframe.org/vocab/provider -->

    <owl:AnnotationProperty rdf:about="&vocab;provider">
        <rdfs:label>Provider</rdfs:label>
        <rdfs:comment>Place, name, and/or date information relating to the publication, printing, distribution, issue, release, or production instance.</rdfs:comment>
    </owl:AnnotationProperty>
    


    <!-- http://bibframe.org/vocab/providerDate -->

    <owl:AnnotationProperty rdf:about="&vocab;providerDate">
        <rdfs:label>Provider date</rdfs:label>
        <rdfs:comment>Date associated with the publication, printing, distribution, issue, release or production of the instance.</rdfs:comment>
        <rdfs:domain rdf:resource="&vocab;Provider"/>
    </owl:AnnotationProperty>
    


    <!-- http://bibframe.org/vocab/providerName -->

    <owl:AnnotationProperty rdf:about="&vocab;providerName">
        <rdfs:label>Provider name</rdfs:label>
        <rdfs:comment>Name of the entity responsible for the publication, printing, distribution, issue, release or production of the instance.</rdfs:comment>
    </owl:AnnotationProperty>
    


    <!-- http://bibframe.org/vocab/providerPlace -->

    <owl:AnnotationProperty rdf:about="&vocab;providerPlace">
        <rdfs:label>Provider place</rdfs:label>
        <rdfs:comment>Place associated with the publication, printing, distribution, issue, release or production of the instance.</rdfs:comment>
    </owl:AnnotationProperty>
    


    <!-- http://bibframe.org/vocab/providerRole -->

    <owl:AnnotationProperty rdf:about="&vocab;providerRole">
        <rdfs:label>Provider role</rdfs:label>
        <rdfs:comment>The type of role played by the provider of an instance, e.g. production, publication, manufacture, distribution.</rdfs:comment>
        <rdfs:domain rdf:resource="&vocab;Provider"/>
    </owl:AnnotationProperty>
    


    <!-- http://bibframe.org/vocab/providerStatement -->

    <owl:AnnotationProperty rdf:about="&vocab;providerStatement">
        <rdfs:label>Provider statement</rdfs:label>
        <rdfs:comment>Transcribed provider statement</rdfs:comment>
        <rdfs:domain rdf:resource="&vocab;Instance"/>
    </owl:AnnotationProperty>
    


    <!-- http://bibframe.org/vocab/publication -->

    <owl:AnnotationProperty rdf:about="&vocab;publication">
        <rdfs:label>Publication event</rdfs:label>
        <rdfs:comment>Information relating to publication of an instance.</rdfs:comment>
    </owl:AnnotationProperty>
    


    <!-- http://bibframe.org/vocab/publisherNumber -->

    <owl:AnnotationProperty rdf:about="&vocab;publisherNumber">
        <rdfs:label>Other publisher number</rdfs:label>
        <rdfs:comment>Number assigned by a publisher that is not one of the specific defined types.</rdfs:comment>
    </owl:AnnotationProperty>
    


    <!-- http://bibframe.org/vocab/referenceAuthority -->

    <owl:AnnotationProperty rdf:about="&vocab;referenceAuthority">
        <rdfs:label>Other authority information</rdfs:label>
        <rdfs:comment>Link to authority information</rdfs:comment>
        <dcterms:modified>2014-03-27 (Updated)</dcterms:modified>
    </owl:AnnotationProperty>
    


    <!-- http://bibframe.org/vocab/relatedInstance -->

    <owl:AnnotationProperty rdf:about="&vocab;relatedInstance">
        <rdfs:label>Related Instance</rdfs:label>
        <rdfs:comment>General instance to instance relationship.</rdfs:comment>
    </owl:AnnotationProperty>
    


    <!-- http://bibframe.org/vocab/relatedTo -->

    <owl:AnnotationProperty rdf:about="&vocab;relatedTo">
        <rdfs:label>Related resource</rdfs:label>
        <rdfs:comment>Any relationship between work or instance resources.</rdfs:comment>
        <dcterms:modified>2014-04-10 (Range updated)</dcterms:modified>
    </owl:AnnotationProperty>
    


    <!-- http://bibframe.org/vocab/relatedWork -->

    <owl:AnnotationProperty rdf:about="&vocab;relatedWork">
        <rdfs:label>Related Work</rdfs:label>
        <rdfs:comment>General work to work relationship.</rdfs:comment>
    </owl:AnnotationProperty>
    


    <!-- http://bibframe.org/vocab/relatorRole -->

    <owl:AnnotationProperty rdf:about="&vocab;relatorRole">
        <rdfs:label>Agent role</rdfs:label>
        <rdfs:comment>Specific role of agent.</rdfs:comment>
        <dcterms:modified>2014-04-30 (New)</dcterms:modified>
        <rdfs:domain rdf:resource="&vocab;Relator"/>
    </owl:AnnotationProperty>
    


    <!-- http://bibframe.org/vocab/reportNumber -->

    <owl:AnnotationProperty rdf:about="&vocab;reportNumber">
        <rdfs:label>Technical report number</rdfs:label>
        <rdfs:comment>Identification number of a report that is not a Standard Technical Report Number.</rdfs:comment>
    </owl:AnnotationProperty>
    


    <!-- http://bibframe.org/vocab/reproduction -->

    <owl:AnnotationProperty rdf:about="&vocab;reproduction">
        <rdfs:label>Has reproduction</rdfs:label>
        <rdfs:comment>Instance that reproduces another Instance embodying the same work.</rdfs:comment>
        <rdfs:subPropertyOf rdf:resource="&vocab;hasEquivalent"/>
    </owl:AnnotationProperty>
    


    <!-- http://bibframe.org/vocab/reproductionPolicy -->

    <owl:AnnotationProperty rdf:about="&vocab;reproductionPolicy">
        <rdfs:label>Reproduction policy</rdfs:label>
        <rdfs:comment>Policy statement about whether reproductions of the holding can be made</rdfs:comment>
        <dcterms:modified>2014-10-21 (Added)</dcterms:modified>
        <rdfs:domain rdf:resource="&vocab;HeldMaterial"/>
    </owl:AnnotationProperty>
    


    <!-- http://bibframe.org/vocab/resourcePart -->

    <owl:AnnotationProperty rdf:about="&vocab;resourcePart">
        <rdfs:label>Resource part</rdfs:label>
        <rdfs:comment>Part of a resource for which language is being indicated.</rdfs:comment>
        <rdfs:domain rdf:resource="&vocab;Language"/>
    </owl:AnnotationProperty>
    


    <!-- http://bibframe.org/vocab/responsibilityStatement -->

    <owl:AnnotationProperty rdf:about="&vocab;responsibilityStatement">
        <rdfs:label>Edition responsibility</rdfs:label>
        <rdfs:comment>Statement relating to the identification and/or function of any persons, families, or corporate bodies responsible for the creation of, or contributing to the content of a resource.</rdfs:comment>
        <rdfs:domain rdf:resource="&vocab;Instance"/>
    </owl:AnnotationProperty>
    


    <!-- http://bibframe.org/vocab/retentionPolicy -->

    <owl:AnnotationProperty rdf:about="&vocab;retentionPolicy">
        <rdfs:label>Retention policy</rdfs:label>
        <rdfs:comment>Policy statement about how many and/or how long the holdings are retained</rdfs:comment>
        <dcterms:modified>2014-10-21 (Added)</dcterms:modified>
        <rdfs:domain rdf:resource="&vocab;HeldMaterial"/>
    </owl:AnnotationProperty>
    


    <!-- http://bibframe.org/vocab/review -->

    <owl:AnnotationProperty rdf:about="&vocab;review">
        <rdfs:label>Review content</rdfs:label>
        <rdfs:comment>Review content.</rdfs:comment>
    </owl:AnnotationProperty>
    


    <!-- http://bibframe.org/vocab/reviewOf -->

    <owl:AnnotationProperty rdf:about="&vocab;reviewOf">
        <rdfs:label>Resource reviewed</rdfs:label>
        <rdfs:comment>Resource to which the review pertains.</rdfs:comment>
    </owl:AnnotationProperty>
    


    <!-- http://bibframe.org/vocab/separatedFrom -->

    <owl:AnnotationProperty rdf:about="&vocab;separatedFrom">
        <rdfs:label>Separated from</rdfs:label>
        <rdfs:comment>Work that spun off a part of its content to form a new work.</rdfs:comment>
        <dcterms:modified>2014-04-10 (Updated subproperty)</dcterms:modified>
        <rdfs:subPropertyOf rdf:resource="&vocab;precededBy"/>
    </owl:AnnotationProperty>
    


    <!-- http://bibframe.org/vocab/serialFirstIssue -->

    <owl:AnnotationProperty rdf:about="&vocab;serialFirstIssue">
        <rdfs:label>Serial first issue</rdfs:label>
        <rdfs:comment>Beginning date of an instance and/or the sequential designations.</rdfs:comment>
        <rdfs:domain rdf:resource="&vocab;Instance"/>
    </owl:AnnotationProperty>
    


    <!-- http://bibframe.org/vocab/serialLastIssue -->

    <owl:AnnotationProperty rdf:about="&vocab;serialLastIssue">
        <rdfs:label>Serial last issue</rdfs:label>
        <rdfs:comment>Ending date of an instance and/or the sequential designations.</rdfs:comment>
        <rdfs:domain rdf:resource="&vocab;Instance"/>
    </owl:AnnotationProperty>
    


    <!-- http://bibframe.org/vocab/series -->

    <owl:AnnotationProperty rdf:about="&vocab;series">
        <rdfs:label>Has series</rdfs:label>
        <rdfs:comment>Work in which the part has been issued; the title of the larger work appears on the part.</rdfs:comment>
        <dcterms:modified>2014-10-14 (Updated)</dcterms:modified>
        <rdfs:subPropertyOf rdf:resource="&vocab;partOf"/>
    </owl:AnnotationProperty>
    


    <!-- http://bibframe.org/vocab/shelfMark -->

    <owl:AnnotationProperty rdf:about="&vocab;shelfMark">
        <rdfs:label>Shelf Location</rdfs:label>
        <rdfs:comment>Physical location, such as a call number or a special shelf/location indicator.</rdfs:comment>
        <rdfs:domain rdf:resource="&vocab;HeldItem"/>
    </owl:AnnotationProperty>
    


    <!-- http://bibframe.org/vocab/shelfMarkDdc -->

    <owl:AnnotationProperty rdf:about="&vocab;shelfMarkDdc">
        <rdfs:label>DDC call number</rdfs:label>
        <rdfs:comment>Shelf mark based on Dewey Decimal Classification.</rdfs:comment>
        <rdfs:domain rdf:resource="&vocab;HeldItem"/>
    </owl:AnnotationProperty>
    


    <!-- http://bibframe.org/vocab/shelfMarkLcc -->

    <owl:AnnotationProperty rdf:about="&vocab;shelfMarkLcc">
        <rdfs:label>LCC call number</rdfs:label>
        <rdfs:comment>Shelf mark based on Library of Congress Classification.</rdfs:comment>
        <rdfs:domain rdf:resource="&vocab;HeldItem"/>
    </owl:AnnotationProperty>
    


    <!-- http://bibframe.org/vocab/shelfMarkNlm -->

    <owl:AnnotationProperty rdf:about="&vocab;shelfMarkNlm">
        <rdfs:label>NLM call number</rdfs:label>
        <rdfs:comment>Shelf mark based on National Library of Medicine Classification.</rdfs:comment>
        <rdfs:domain rdf:resource="&vocab;HeldItem"/>
    </owl:AnnotationProperty>
    


    <!-- http://bibframe.org/vocab/shelfMarkScheme -->

    <owl:AnnotationProperty rdf:about="&vocab;shelfMarkScheme">
        <rdfs:label>Shelf mark scheme</rdfs:label>
        <rdfs:comment>Scheme from which a shelf mark is taken.</rdfs:comment>
        <rdfs:domain rdf:resource="&vocab;HeldItem"/>
    </owl:AnnotationProperty>
    


    <!-- http://bibframe.org/vocab/shelfMarkUdc -->

    <owl:AnnotationProperty rdf:about="&vocab;shelfMarkUdc">
        <rdfs:label>UDC call number</rdfs:label>
        <rdfs:comment>Shelf mark based on Universal Decimal Classification.</rdfs:comment>
        <rdfs:domain rdf:resource="&vocab;HeldItem"/>
    </owl:AnnotationProperty>
    


    <!-- http://bibframe.org/vocab/sici -->

    <owl:AnnotationProperty rdf:about="&vocab;sici">
        <rdfs:label>SICI</rdfs:label>
        <rdfs:comment>Serial Item and Contribution Identifier.</rdfs:comment>
    </owl:AnnotationProperty>
    


    <!-- http://bibframe.org/vocab/soundContent -->

    <owl:AnnotationProperty rdf:about="&vocab;soundContent">
        <rdfs:label>Sound content</rdfs:label>
        <rdfs:comment>Indication of whether the production of sound is an integral part of the resource.</rdfs:comment>
        <rdfs:domain rdf:resource="&vocab;Instance"/>
    </owl:AnnotationProperty>
    


    <!-- http://bibframe.org/vocab/splitInto -->

    <owl:AnnotationProperty rdf:about="&vocab;splitInto">
        <rdfs:label>Split into</rdfs:label>
        <dcterms:modified>2014-04-10 (Updated subproperty)</dcterms:modified>
        <rdfs:comment>One of two or more works resulting from the division of an earlier work into separate works.</rdfs:comment>
        <rdfs:subPropertyOf rdf:resource="&vocab;succeededBy"/>
    </owl:AnnotationProperty>
    


    <!-- http://bibframe.org/vocab/startOfReview -->

    <owl:AnnotationProperty rdf:about="&vocab;startOfReview">
        <rdfs:label>Review beginning</rdfs:label>
        <rdfs:comment>First part of review.</rdfs:comment>
        <rdfs:domain rdf:resource="&vocab;Review"/>
    </owl:AnnotationProperty>
    


    <!-- http://bibframe.org/vocab/startOfSummary -->

    <owl:AnnotationProperty rdf:about="&vocab;startOfSummary">
        <rdfs:label>Summary beginning</rdfs:label>
        <rdfs:comment>First part of description.</rdfs:comment>
        <rdfs:domain rdf:resource="&vocab;Summary"/>
    </owl:AnnotationProperty>
    


    <!-- http://bibframe.org/vocab/stockNumber -->

    <owl:AnnotationProperty rdf:about="&vocab;stockNumber">
        <rdfs:label>Stock number</rdfs:label>
        <rdfs:comment>Identification number such as distributor, publisher, or vendor number.</rdfs:comment>
    </owl:AnnotationProperty>
    


    <!-- http://bibframe.org/vocab/strn -->

    <owl:AnnotationProperty rdf:about="&vocab;strn">
        <rdfs:label>STRN</rdfs:label>
        <rdfs:comment>Standard Technical Report Number.</rdfs:comment>
    </owl:AnnotationProperty>
    


    <!-- http://bibframe.org/vocab/studyNumber -->

    <owl:AnnotationProperty rdf:about="&vocab;studyNumber">
        <rdfs:label>Study number</rdfs:label>
        <rdfs:comment>Identification number for a computer data file.</rdfs:comment>
    </owl:AnnotationProperty>
    


    <!-- http://bibframe.org/vocab/subLocation -->

    <owl:AnnotationProperty rdf:about="&vocab;subLocation">
        <rdfs:label>Held in sublocation</rdfs:label>
        <dcterms:modified>2014-04-28 (Updated Mapping)</dcterms:modified>
        <rdfs:comment>Specific place within the holding entity where the item is located or made available</rdfs:comment>
        <rdfs:domain rdf:resource="&vocab;HeldMaterial"/>
    </owl:AnnotationProperty>
    


    <!-- http://bibframe.org/vocab/subject -->

    <owl:AnnotationProperty rdf:about="&vocab;subject">
        <rdfs:label>Subject</rdfs:label>
        <rdfs:comment>Subject term(s) describing a resource.</rdfs:comment>
    </owl:AnnotationProperty>
    


    <!-- http://bibframe.org/vocab/subseries -->

    <owl:AnnotationProperty rdf:about="&vocab;subseries">
        <rdfs:label>Has subseries</rdfs:label>
        <rdfs:comment>Work, which is part of another series, in which the part has been issued.</rdfs:comment>
        <dcterms:modified>2014-10-14 (Updated)</dcterms:modified>
        <rdfs:subPropertyOf rdf:resource="&vocab;hasPart"/>
    </owl:AnnotationProperty>
    


    <!-- http://bibframe.org/vocab/subseriesOf -->

    <owl:AnnotationProperty rdf:about="&vocab;subseriesOf">
        <rdfs:label>Subseries of</rdfs:label>
        <rdfs:comment>Work in which the part consistently appears; the title of the larger work appears on all issues or parts of the subseries).</rdfs:comment>
        <dcterms:modified>2014-10-14 (Updated)</dcterms:modified>
        <rdfs:subPropertyOf rdf:resource="&vocab;partOf"/>
    </owl:AnnotationProperty>
    


    <!-- http://bibframe.org/vocab/subtitle -->

    <owl:AnnotationProperty rdf:about="&vocab;subtitle">
        <rdfs:label>Subtitle</rdfs:label>
        <rdfs:comment>Word, character, or group of words and/or characters that contains the remainder of the title information after the main title.</rdfs:comment>
        <rdfs:domain rdf:resource="&vocab;Title"/>
    </owl:AnnotationProperty>
    


    <!-- http://bibframe.org/vocab/succeededBy -->

    <owl:AnnotationProperty rdf:about="&vocab;succeededBy">
        <rdfs:label>Succeeded By</rdfs:label>
        <dcterms:modified>2014-04-10 (Renamed)</dcterms:modified>
        <rdfs:comment>Resource that succeeds the resource being described (e.g., later in time or after in a narrative).</rdfs:comment>
        <rdfs:subPropertyOf rdf:resource="&vocab;relatedTo"/>
    </owl:AnnotationProperty>
    


    <!-- http://bibframe.org/vocab/summary -->

    <owl:AnnotationProperty rdf:about="&vocab;summary">
        <rdfs:label>Summary content</rdfs:label>
        <rdfs:comment>Summary or abstract of the target work or instance.</rdfs:comment>
    </owl:AnnotationProperty>
    


    <!-- http://bibframe.org/vocab/summaryOf -->

    <owl:AnnotationProperty rdf:about="&vocab;summaryOf">
        <rdfs:label>Resource summarized</rdfs:label>
        <rdfs:comment>Resource to which the description pertains.</rdfs:comment>
        <rdfs:domain rdf:resource="&vocab;Summary"/>
        <rdfs:subPropertyOf rdf:resource="&vocab;annotates"/>
    </owl:AnnotationProperty>
    


    <!-- http://bibframe.org/vocab/supersededBy -->

    <owl:AnnotationProperty rdf:about="&vocab;supersededBy">
        <rdfs:label>Superseded by</rdfs:label>
        <dcterms:modified>2014-04-10 (Updated subproperty)</dcterms:modified>
        <rdfs:comment>Later Work used in place of an earlier work, usually because the later work contains updated or new information.</rdfs:comment>
        <rdfs:subPropertyOf rdf:resource="&vocab;succeededBy"/>
    </owl:AnnotationProperty>
    


    <!-- http://bibframe.org/vocab/supersededInPartBy -->

    <owl:AnnotationProperty rdf:about="&vocab;supersededInPartBy">
        <rdfs:label>Superseded in part by</rdfs:label>
        <rdfs:comment>Later Work used in part in place of an earlier work, usually because the later work contains updated or new information.</rdfs:comment>
        <dcterms:modified>2014-04-10 (Updated subproperty)</dcterms:modified>
        <rdfs:subPropertyOf rdf:resource="&vocab;succeededBy"/>
    </owl:AnnotationProperty>
    


    <!-- http://bibframe.org/vocab/supersedes -->

    <owl:AnnotationProperty rdf:about="&vocab;supersedes">
        <rdfs:label>Supersedes</rdfs:label>
        <dcterms:modified>2014-04-10 (Updated subproperty)</dcterms:modified>
        <rdfs:comment>Earlier work whose content has been replaced by a later work, usually because the later work contains updated or new information.</rdfs:comment>
        <rdfs:subPropertyOf rdf:resource="&vocab;precededBy"/>
    </owl:AnnotationProperty>
    


    <!-- http://bibframe.org/vocab/supersedesInPart -->

    <owl:AnnotationProperty rdf:about="&vocab;supersedesInPart">
        <rdfs:label>Supersedes in part</rdfs:label>
        <dcterms:modified>2014-04-10 (Updated subproperty)</dcterms:modified>
        <rdfs:comment>Earlier work whose content has been partially replaced by a later work, usually because the later work contains updated or new information.</rdfs:comment>
        <rdfs:subPropertyOf rdf:resource="&vocab;precededBy"/>
    </owl:AnnotationProperty>
    


    <!-- http://bibframe.org/vocab/supplement -->

    <owl:AnnotationProperty rdf:about="&vocab;supplement">
        <rdfs:label>Has supplement</rdfs:label>
        <rdfs:comment>Work that updates or otherwise complements the predominant work.</rdfs:comment>
        <rdfs:subPropertyOf rdf:resource="&vocab;accompaniedBy"/>
    </owl:AnnotationProperty>
    


    <!-- http://bibframe.org/vocab/supplementTo -->

    <owl:AnnotationProperty rdf:about="&vocab;supplementTo">
        <rdfs:label>Supplement to</rdfs:label>
        <rdfs:comment>Work that is updated or otherwise complemented by the augmenting work.</rdfs:comment>
        <rdfs:subPropertyOf rdf:resource="&vocab;accompanies"/>
    </owl:AnnotationProperty>
    


    <!-- http://bibframe.org/vocab/supplementaryContentNote -->

    <owl:AnnotationProperty rdf:about="&vocab;supplementaryContentNote">
        <rdfs:label>Supplementary content note</rdfs:label>
        <rdfs:comment>Information on the presence of one or more bibliographies, discographies, filmographies, and/or other bibliographic references in a described resource or in accompanying material.</rdfs:comment>
        <rdfs:domain rdf:resource="&vocab;Instance"/>
    </owl:AnnotationProperty>
    


    <!-- http://bibframe.org/vocab/systemNumber -->

    <owl:AnnotationProperty rdf:about="&vocab;systemNumber">
        <rdfs:label>System control number</rdfs:label>
        <rdfs:comment>Control number of a system other than LCCN or NBAN, which Identifies a resource description.</rdfs:comment>
    </owl:AnnotationProperty>
    


    <!-- http://bibframe.org/vocab/tableOfContents -->

    <owl:AnnotationProperty rdf:about="&vocab;tableOfContents">
        <rdfs:label>Table of contents content</rdfs:label>
        <rdfs:comment>Table of contents of the target work or instance.</rdfs:comment>
    </owl:AnnotationProperty>
    


    <!-- http://bibframe.org/vocab/tableOfContentsFor -->

    <owl:AnnotationProperty rdf:about="&vocab;tableOfContentsFor">
        <rdfs:label>Table of contents of resource</rdfs:label>
        <rdfs:comment>Resource to which the table of contents pertains.</rdfs:comment>
    </owl:AnnotationProperty>
    


    <!-- http://bibframe.org/vocab/temporalCoverageNote -->

    <owl:AnnotationProperty rdf:about="&vocab;temporalCoverageNote">
        <rdfs:label>Temporal coverage</rdfs:label>
        <rdfs:comment>Time period covered by the resource.</rdfs:comment>
        <rdfs:domain rdf:resource="&vocab;Work"/>
    </owl:AnnotationProperty>
    


    <!-- http://bibframe.org/vocab/titleAttribute -->

    <owl:AnnotationProperty rdf:about="&vocab;titleAttribute">
        <rdfs:label>Other title attribute</rdfs:label>
        <rdfs:comment>Other distinguishing characteristic of a work, such as version, etc..</rdfs:comment>
        <rdfs:domain rdf:resource="&vocab;Title"/>
    </owl:AnnotationProperty>
    


    <!-- http://bibframe.org/vocab/titleQualifier -->

    <owl:AnnotationProperty rdf:about="&vocab;titleQualifier">
        <rdfs:label>Title qualifier</rdfs:label>
        <rdfs:comment>Qualifier of title information to make it unique.</rdfs:comment>
        <rdfs:domain rdf:resource="&vocab;Title"/>
    </owl:AnnotationProperty>
    


    <!-- http://bibframe.org/vocab/titleSource -->

    <owl:AnnotationProperty rdf:about="&vocab;titleSource">
        <rdfs:label>Title source</rdfs:label>
        <rdfs:comment>Title list from which title is taken, e.g., list of abbreviated titles.</rdfs:comment>
        <rdfs:domain rdf:resource="&vocab;Title"/>
    </owl:AnnotationProperty>
    


    <!-- http://bibframe.org/vocab/titleStatement -->

    <owl:AnnotationProperty rdf:about="&vocab;titleStatement">
        <rdfs:label>Transcribed title</rdfs:label>
        <rdfs:comment>Title transcribed from an instance.</rdfs:comment>
        <dcterms:modified>2014-09-03 (Updated)</dcterms:modified>
        <rdfs:domain rdf:resource="&vocab;Instance"/>
    </owl:AnnotationProperty>
    


    <!-- http://bibframe.org/vocab/titleType -->

    <owl:AnnotationProperty rdf:about="&vocab;titleType">
        <rdfs:label>Variant title type</rdfs:label>
        <dcterms:modified>2014-08-07 (Example added)</dcterms:modified>
        <rdfs:comment>Type of title variation, e.g., acronym, cover, spine. .</rdfs:comment>
        <rdfs:domain rdf:resource="&vocab;Title"/>
    </owl:AnnotationProperty>
    


    <!-- http://bibframe.org/vocab/titleValue -->

    <owl:AnnotationProperty rdf:about="&vocab;titleValue">
        <rdfs:label>Title</rdfs:label>
        <rdfs:comment>Title being addressed.</rdfs:comment>
        <rdfs:domain rdf:resource="&vocab;Title"/>
    </owl:AnnotationProperty>
    


    <!-- http://bibframe.org/vocab/titleVariationDate -->

    <owl:AnnotationProperty rdf:about="&vocab;titleVariationDate">
        <rdfs:label>Variant title date</rdfs:label>
        <rdfs:comment>Date or sequential designation of title variation.</rdfs:comment>
        <rdfs:domain rdf:resource="&vocab;Title"/>
    </owl:AnnotationProperty>
    


    <!-- http://bibframe.org/vocab/translation -->

    <owl:AnnotationProperty rdf:about="&vocab;translation">
        <rdfs:label>Has translation</rdfs:label>
        <rdfs:comment>Work that translates the text of the source entity into a language different from that of the original.</rdfs:comment>
        <rdfs:subPropertyOf rdf:resource="&vocab;derivativeOf"/>
    </owl:AnnotationProperty>
    


    <!-- http://bibframe.org/vocab/translationOf -->

    <owl:AnnotationProperty rdf:about="&vocab;translationOf">
        <rdfs:label>Translation of</rdfs:label>
        <rdfs:comment>Work that has been translated, i.e., the text expressed in a language different from that of the original work).</rdfs:comment>
        <rdfs:subPropertyOf rdf:resource="&vocab;hasDerivative"/>
    </owl:AnnotationProperty>
    


    <!-- http://bibframe.org/vocab/unionOf -->

    <owl:AnnotationProperty rdf:about="&vocab;unionOf">
        <rdfs:label>Union of</rdfs:label>
        <dcterms:modified>2014-04-10 (Updated subproperty)</dcterms:modified>
        <rdfs:comment>One of two or more works which came together to form a new work.</rdfs:comment>
        <rdfs:subPropertyOf rdf:resource="&vocab;precededBy"/>
    </owl:AnnotationProperty>
    


    <!-- http://bibframe.org/vocab/upc -->

    <owl:AnnotationProperty rdf:about="&vocab;upc">
        <rdfs:label>UPC</rdfs:label>
        <rdfs:comment>Universal Product Code.</rdfs:comment>
    </owl:AnnotationProperty>
    


    <!-- http://bibframe.org/vocab/uri -->

    <owl:AnnotationProperty rdf:about="&vocab;uri">
        <rdfs:label>URI</rdfs:label>
        <rdfs:comment>Uniform Resource Identifier.</rdfs:comment>
    </owl:AnnotationProperty>
    


    <!-- http://bibframe.org/vocab/urn -->

    <owl:AnnotationProperty rdf:about="&vocab;urn">
        <rdfs:label>URN</rdfs:label>
        <rdfs:comment>Uniform Resource Number.</rdfs:comment>
    </owl:AnnotationProperty>
    


    <!-- http://bibframe.org/vocab/videorecordingNumber -->

    <owl:AnnotationProperty rdf:about="&vocab;videorecordingNumber">
        <rdfs:label>Videorecording number</rdfs:label>
        <rdfs:comment>Number assigned by a publisher to a videorecording.</rdfs:comment>
    </owl:AnnotationProperty>
    


    <!-- http://bibframe.org/vocab/workTitle -->

    <owl:AnnotationProperty rdf:about="&vocab;workTitle">
        <rdfs:label>Work title</rdfs:label>
        <rdfs:comment>Title or form of title chosen to identify the work, such as a preferred title, preferred title with additions, uniform title, etc..</rdfs:comment>
    </owl:AnnotationProperty>
    


    <!-- http://purl.org/dc/elements/1.1/date -->

    <owl:AnnotationProperty rdf:about="&dc;date"/>
    


    <!-- http://purl.org/dc/elements/1.1/relation -->

    <owl:AnnotationProperty rdf:about="&dc;relation"/>
    


    <!-- http://purl.org/dc/terms/created -->

    <owl:AnnotationProperty rdf:about="&dcterms;created">
        <rdfs:label xml:lang="en">Date Created</rdfs:label>
        <dcterms:issued rdf:datatype="&xsd;date">2000-07-11</dcterms:issued>
        <dcterms:modified rdf:datatype="&xsd;date">2008-01-14</dcterms:modified>
        <rdfs:comment xml:lang="en">Date of creation of the resource.</rdfs:comment>
        <dcterms:hasVersion rdf:resource="http://dublincore.org/usage/terms/history/#created-003"/>
        <rdfs:subPropertyOf rdf:resource="&dc;date"/>
        <rdfs:isDefinedBy rdf:resource="http://purl.org/dc/terms/"/>
        <rdfs:subPropertyOf rdf:resource="&dcterms;date"/>
    </owl:AnnotationProperty>
    


    <!-- http://purl.org/dc/terms/date -->

    <owl:AnnotationProperty rdf:about="&dcterms;date"/>
    


    <!-- http://purl.org/dc/terms/description -->

    <owl:AnnotationProperty rdf:about="&dcterms;description"/>
    


    <!-- http://purl.org/dc/terms/hasPart -->

    <owl:AnnotationProperty rdf:about="&dcterms;hasPart">
        <rdfs:label xml:lang="en">Has Part</rdfs:label>
        <dcterms:issued rdf:datatype="&xsd;date">2000-07-11</dcterms:issued>
        <dcterms:modified rdf:datatype="&xsd;date">2008-01-14</dcterms:modified>
        <rdfs:comment xml:lang="en">A related resource that is included either physically or logically in the described resource.</rdfs:comment>
        <skos:note xml:lang="en">This term is intended to be used with non-literal values as defined in the DCMI Abstract Model (http://dublincore.org/documents/abstract-model/).  As of December 2007, the DCMI Usage Board is seeking a way to express this intention with a formal range declaration.</skos:note>
        <dcterms:hasVersion rdf:resource="http://dublincore.org/usage/terms/history/#hasPart-003"/>
        <rdfs:subPropertyOf rdf:resource="&dc;relation"/>
        <rdfs:isDefinedBy rdf:resource="http://purl.org/dc/terms/"/>
        <rdfs:subPropertyOf rdf:resource="&dcterms;relation"/>
    </owl:AnnotationProperty>
    


    <!-- http://purl.org/dc/terms/hasVersion -->

    <owl:AnnotationProperty rdf:about="&dcterms;hasVersion"/>
    


    <!-- http://purl.org/dc/terms/isPartOf -->

    <owl:AnnotationProperty rdf:about="&dcterms;isPartOf">
        <rdfs:label xml:lang="en">Is Part Of</rdfs:label>
        <dcterms:issued rdf:datatype="&xsd;date">2000-07-11</dcterms:issued>
        <dcterms:modified rdf:datatype="&xsd;date">2008-01-14</dcterms:modified>
        <rdfs:comment xml:lang="en">A related resource in which the described resource is physically or logically included.</rdfs:comment>
        <skos:note xml:lang="en">This term is intended to be used with non-literal values as defined in the DCMI Abstract Model (http://dublincore.org/documents/abstract-model/).  As of December 2007, the DCMI Usage Board is seeking a way to express this intention with a formal range declaration.</skos:note>
        <dcterms:hasVersion rdf:resource="http://dublincore.org/usage/terms/history/#isPartOf-003"/>
        <rdfs:subPropertyOf rdf:resource="&dc;relation"/>
        <rdfs:isDefinedBy rdf:resource="http://purl.org/dc/terms/"/>
        <rdfs:subPropertyOf rdf:resource="&dcterms;relation"/>
    </owl:AnnotationProperty>
    


    <!-- http://purl.org/dc/terms/issued -->

    <owl:AnnotationProperty rdf:about="&dcterms;issued"/>
    


    <!-- http://purl.org/dc/terms/modified -->

    <owl:AnnotationProperty rdf:about="&dcterms;modified"/>
    


    <!-- http://purl.org/dc/terms/relation -->

    <owl:AnnotationProperty rdf:about="&dcterms;relation">
        <rdfs:label xml:lang="en">Relation</rdfs:label>
        <dcterms:issued rdf:datatype="&xsd;date">2008-01-14</dcterms:issued>
        <dcterms:modified rdf:datatype="&xsd;date">2008-01-14</dcterms:modified>
        <rdfs:comment xml:lang="en">A related resource.</rdfs:comment>
        <dcterms:description xml:lang="en">Recommended best practice is to identify the related resource by means of a string conforming to a formal identification system. </dcterms:description>
        <skos:note xml:lang="en">This term is intended to be used with non-literal values as defined in the DCMI Abstract Model (http://dublincore.org/documents/abstract-model/).  As of December 2007, the DCMI Usage Board is seeking a way to express this intention with a formal range declaration.</skos:note>
        <dcterms:hasVersion rdf:resource="http://dublincore.org/usage/terms/history/#relationT-001"/>
        <rdfs:subPropertyOf rdf:resource="&dc;relation"/>
        <rdfs:isDefinedBy rdf:resource="http://purl.org/dc/terms/"/>
    </owl:AnnotationProperty>
    


    <!-- http://www.w3.org/2004/02/skos/core#note -->

    <owl:AnnotationProperty rdf:about="&skos;note"/>
    


    <!-- http://www.w3.org/ns/prov#category -->

    <owl:AnnotationProperty rdf:about="&prov;category"/>
    


    <!-- http://www.w3.org/ns/prov#component -->

    <owl:AnnotationProperty rdf:about="&prov;component"/>
    


    <!-- http://www.w3.org/ns/prov#editorialNote -->

    <owl:AnnotationProperty rdf:about="&prov;editorialNote"/>
    


    <!-- http://www.w3.org/ns/prov#inverse -->

    <owl:AnnotationProperty rdf:about="&prov;inverse"/>
    


    <!-- http://www.w3.org/ns/prov#qualifiedForm -->

    <owl:AnnotationProperty rdf:about="&prov;qualifiedForm"/>
    


    <!-- http://www.w3.org/ns/prov#sharesDefinitionWith -->

    <owl:AnnotationProperty rdf:about="&prov;sharesDefinitionWith"/>
    


    <!-- 
    ///////////////////////////////////////////////////////////////////////////////////////
    //
    // Datatypes
    //
    ///////////////////////////////////////////////////////////////////////////////////////
     -->

    


    <!-- http://www.w3.org/2001/XMLSchema#date -->

    <rdfs:Datatype rdf:about="&xsd;date"/>
    


    <!-- 
    ///////////////////////////////////////////////////////////////////////////////////////
    //
    // Object Properties
    //
    ///////////////////////////////////////////////////////////////////////////////////////
     -->

    


    <!-- http://bibframe.org/vocab/abbreviatedTitle -->

    <owl:ObjectProperty rdf:about="&vocab;abbreviatedTitle">
        <rdfs:label>Abbreviated title</rdfs:label>
        <rdfs:comment>Title as abbreviated for indexing or identification.</rdfs:comment>
        <rdfs:domain rdf:resource="&vocab;Instance"/>
        <rdfs:range rdf:resource="&vocab;Title"/>
        <rdfs:subPropertyOf rdf:resource="&vocab;instanceTitle"/>
    </owl:ObjectProperty>
    


    <!-- http://bibframe.org/vocab/absorbed -->

    <owl:ObjectProperty rdf:about="&vocab;absorbed">
        <rdfs:label>Absorbed</rdfs:label>
        <rdfs:comment>Work that has been incorporated into another Work</rdfs:comment>
        <dcterms:modified>2014-04-10 (Updated subproperty)</dcterms:modified>
        <rdfs:range rdf:resource="&vocab;Work"/>
        <rdfs:domain rdf:resource="&vocab;Work"/>
    </owl:ObjectProperty>
    


    <!-- http://bibframe.org/vocab/absorbedBy -->

    <owl:ObjectProperty rdf:about="&vocab;absorbedBy">
        <rdfs:label>Absorbed by</rdfs:label>
        <dcterms:modified>2014-04-10 (Updated subproperty)</dcterms:modified>
        <rdfs:comment>Work that incorporates another work.</rdfs:comment>
        <rdfs:range rdf:resource="&vocab;Work"/>
        <rdfs:domain rdf:resource="&vocab;Work"/>
    </owl:ObjectProperty>
    


    <!-- http://bibframe.org/vocab/absorbedInPart -->

    <owl:ObjectProperty rdf:about="&vocab;absorbedInPart">
        <rdfs:label>Absorbed in part</rdfs:label>
        <rdfs:comment>Work that has been partially incorporated into another work.</rdfs:comment>
        <dcterms:modified>2014-04-10 (Updated subproperty)</dcterms:modified>
        <rdfs:range rdf:resource="&vocab;Work"/>
        <rdfs:domain rdf:resource="&vocab;Work"/>
    </owl:ObjectProperty>
    


    <!-- http://bibframe.org/vocab/absorbedInPartBy -->

    <owl:ObjectProperty rdf:about="&vocab;absorbedInPartBy">
        <rdfs:label>Absorbed in part by</rdfs:label>
        <dcterms:modified>2014-04-10 (Updated subproperty)</dcterms:modified>
        <rdfs:comment>Work that incorporates part of the content of another work.</rdfs:comment>
        <rdfs:domain rdf:resource="&vocab;Work"/>
        <rdfs:range rdf:resource="&vocab;Work"/>
    </owl:ObjectProperty>
    


    <!-- http://bibframe.org/vocab/agent -->

    <owl:ObjectProperty rdf:about="&vocab;agent">
        <rdfs:label>Associated agent</rdfs:label>
        <rdfs:comment>Entity associated with a resource or element of description</rdfs:comment>
        <rdfs:range rdf:resource="&vocab;Authority"/>
    </owl:ObjectProperty>
    


    <!-- http://bibframe.org/vocab/annotates -->

    <owl:ObjectProperty rdf:about="&vocab;annotates">
        <rdfs:label>Target of Annotation</rdfs:label>
        <rdfs:comment>Resource to which the annotation relates.</rdfs:comment>
        <rdfs:domain rdf:resource="&vocab;Annotation"/>
        <rdfs:range rdf:resource="&rdfs;Resource"/>
    </owl:ObjectProperty>
    


    <!-- http://bibframe.org/vocab/annotationAssertedBy -->

    <owl:ObjectProperty rdf:about="&vocab;annotationAssertedBy">
        <rdfs:label>Annotation asserted by</rdfs:label>
        <rdfs:comment>Annotation was asserted by the given entity.</rdfs:comment>
        <rdfs:range rdf:resource="&vocab;Agent"/>
        <rdfs:domain rdf:resource="&vocab;Annotation"/>
    </owl:ObjectProperty>
    


    <!-- http://bibframe.org/vocab/annotationBody -->

    <owl:ObjectProperty rdf:about="&vocab;annotationBody">
        <rdfs:label>Annotation Body</rdfs:label>
        <rdfs:comment>Content of the annotation about the resource.</rdfs:comment>
        <rdfs:domain rdf:resource="&vocab;Annotation"/>
        <rdfs:range rdf:resource="&rdfs;Resource"/>
    </owl:ObjectProperty>
    


    <!-- http://bibframe.org/vocab/annotationSource -->

    <owl:ObjectProperty rdf:about="&vocab;annotationSource">
        <rdfs:label>Annotation Source</rdfs:label>
        <rdfs:comment>Source of the annotation.</rdfs:comment>
        <rdfs:range rdf:resource="&vocab;Agent"/>
        <rdfs:domain rdf:resource="&vocab;Annotation"/>
    </owl:ObjectProperty>
    


    <!-- http://bibframe.org/vocab/ansi -->

    <owl:ObjectProperty rdf:about="&vocab;ansi">
        <rdfs:label>ANSI number</rdfs:label>
        <rdfs:comment>American National Standards Institute identifier.</rdfs:comment>
        <rdfs:range rdf:resource="&vocab;Identifier"/>
        <rdfs:domain rdf:resource="&vocab;Instance"/>
        <rdfs:subPropertyOf rdf:resource="&vocab;identifier"/>
    </owl:ObjectProperty>
    


    <!-- http://bibframe.org/vocab/arrangement -->

    <owl:ObjectProperty rdf:about="&vocab;arrangement">
        <rdfs:label>Organization and Arrangement</rdfs:label>
        <rdfs:comment>Information about the organization and arrangement of a collection of resources.</rdfs:comment>
        <rdfs:range rdf:resource="&vocab;Arrangement"/>
        <rdfs:domain rdf:resource="&vocab;Instance"/>
    </owl:ObjectProperty>
    


    <!-- http://bibframe.org/vocab/authorityAssigner -->

    <owl:ObjectProperty rdf:about="&vocab;authorityAssigner">
        <rdfs:label>Authority assigner</rdfs:label>
        <rdfs:comment>Entity that assigned the information.</rdfs:comment>
        <rdfs:range rdf:resource="&vocab;Agent"/>
        <rdfs:domain rdf:resource="&vocab;Authority"/>
    </owl:ObjectProperty>
    


    <!-- http://bibframe.org/vocab/carrierCategory -->

    <owl:ObjectProperty rdf:about="&vocab;carrierCategory">
        <rdfs:label>Carrier type</rdfs:label>
        <rdfs:comment>Categorization reflecting the format of the storage medium and housing of a carrier.</rdfs:comment>
        <rdfs:range rdf:resource="&vocab;Category"/>
        <rdfs:domain rdf:resource="&vocab;Instance"/>
    </owl:ObjectProperty>
    


    <!-- http://bibframe.org/vocab/cartography -->

    <owl:ObjectProperty rdf:about="&vocab;cartography">
        <rdfs:label>Cartographic data</rdfs:label>
        <dcterms:modified>2014-03-27 (Updated)</dcterms:modified>
        <rdfs:comment>Cartographic data that identifies scale, coordinates, etc.</rdfs:comment>
        <rdfs:range rdf:resource="&vocab;Cartography"/>
    </owl:ObjectProperty>
    


    <!-- http://bibframe.org/vocab/classification -->

    <owl:ObjectProperty rdf:about="&vocab;classification">
        <rdfs:label>Classification</rdfs:label>
        <rdfs:comment>Classification number in any scheme.</rdfs:comment>
        <rdfs:range rdf:resource="&vocab;Classification"/>
        <rdfs:domain rdf:resource="&vocab;Work"/>
    </owl:ObjectProperty>
    


    <!-- http://bibframe.org/vocab/classificationDdc -->

    <owl:ObjectProperty rdf:about="&vocab;classificationDdc">
        <rdfs:label>DDC Classification</rdfs:label>
        <rdfs:comment>Dewey Decimal Classification number used for subject access.</rdfs:comment>
        <rdfs:range rdf:resource="&vocab;Classification"/>
        <rdfs:domain rdf:resource="&vocab;Work"/>
        <rdfs:subPropertyOf rdf:resource="&vocab;classification"/>
    </owl:ObjectProperty>
    


    <!-- http://bibframe.org/vocab/classificationLcc -->

    <owl:ObjectProperty rdf:about="&vocab;classificationLcc">
        <rdfs:label>LCC Classification</rdfs:label>
        <rdfs:comment>Library of Congress Classification number used for subject access.</rdfs:comment>
        <rdfs:range rdf:resource="&vocab;Classification"/>
        <rdfs:domain rdf:resource="&vocab;Work"/>
        <rdfs:subPropertyOf rdf:resource="&vocab;classification"/>
    </owl:ObjectProperty>
    


    <!-- http://bibframe.org/vocab/classificationNlm -->

    <owl:ObjectProperty rdf:about="&vocab;classificationNlm">
        <rdfs:label>NLM classification</rdfs:label>
        <rdfs:comment>National Library of Medicine Classification number used for subject access</rdfs:comment>
        <rdfs:range rdf:resource="&vocab;Classification"/>
        <rdfs:domain rdf:resource="&vocab;Work"/>
        <rdfs:subPropertyOf rdf:resource="&vocab;classification"/>
    </owl:ObjectProperty>
    


    <!-- http://bibframe.org/vocab/classificationNumberUri -->

    <owl:ObjectProperty rdf:about="&vocab;classificationNumberUri">
        <rdfs:label>Classification number URI</rdfs:label>
        <rdfs:comment>Classification number represented as a URI.</rdfs:comment>
        <rdfs:domain rdf:resource="&vocab;Classification"/>
        <rdfs:range rdf:resource="&rdfs;Resource"/>
    </owl:ObjectProperty>
    


    <!-- http://bibframe.org/vocab/classificationUdc -->

    <owl:ObjectProperty rdf:about="&vocab;classificationUdc">
        <rdfs:label>UDC Classification</rdfs:label>
        <rdfs:comment>Universal Decimal Classification number used for subject access.</rdfs:comment>
        <rdfs:range rdf:resource="&vocab;Classification"/>
        <rdfs:domain rdf:resource="&vocab;Work"/>
        <rdfs:subPropertyOf rdf:resource="&vocab;classification"/>
    </owl:ObjectProperty>
    


    <!-- http://bibframe.org/vocab/coden -->

    <owl:ObjectProperty rdf:about="&vocab;coden">
        <rdfs:label>CODEN</rdfs:label>
        <rdfs:comment>Identifier for scientific and technical periodical titles assigned by the International CODEN Section of Chemical Abstracts Service.</rdfs:comment>
        <rdfs:range rdf:resource="&vocab;Identifier"/>
        <rdfs:domain rdf:resource="&vocab;Instance"/>
        <rdfs:subPropertyOf rdf:resource="&vocab;identifier"/>
    </owl:ObjectProperty>
    


    <!-- http://bibframe.org/vocab/componentOf -->

    <owl:ObjectProperty rdf:about="&vocab;componentOf">
        <rdfs:label>Held item</rdfs:label>
        <rdfs:comment>Link to held material</rdfs:comment>
        <rdfs:domain rdf:resource="&vocab;HeldItem"/>
        <rdfs:range rdf:resource="&vocab;HeldMaterial"/>
    </owl:ObjectProperty>
    


    <!-- http://bibframe.org/vocab/contentCategory -->

    <owl:ObjectProperty rdf:about="&vocab;contentCategory">
        <rdfs:label>Content type</rdfs:label>
        <rdfs:comment>Categorization reflecting the fundamental form of communication in which the content is expressed and the human sense through which it is intended to be perceived.</rdfs:comment>
        <rdfs:range rdf:resource="&vocab;Category"/>
        <rdfs:domain rdf:resource="&vocab;Work"/>
    </owl:ObjectProperty>
    


    <!-- http://bibframe.org/vocab/continuedBy -->

    <owl:ObjectProperty rdf:about="&vocab;continuedBy">
        <rdfs:label>Continued by</rdfs:label>
        <dcterms:modified>2014-04-10 (Updated subproperty)</dcterms:modified>
        <rdfs:comment>Work whose content continues an earlier work under a new title.</rdfs:comment>
        <rdfs:domain rdf:resource="&vocab;Work"/>
        <rdfs:range rdf:resource="&vocab;Work"/>
    </owl:ObjectProperty>
    


    <!-- http://bibframe.org/vocab/continuedInPartBy -->

    <owl:ObjectProperty rdf:about="&vocab;continuedInPartBy">
        <rdfs:label>Continued in part by</rdfs:label>
        <rdfs:comment>Work part of whose content separated from an earlier work to form a new work.</rdfs:comment>
        <dcterms:modified>2014-04-10 (Updated subproperty)</dcterms:modified>
        <rdfs:domain rdf:resource="&vocab;Work"/>
        <rdfs:range rdf:resource="&vocab;Work"/>
    </owl:ObjectProperty>
    


    <!-- http://bibframe.org/vocab/continues -->

    <owl:ObjectProperty rdf:about="&vocab;continues">
        <rdfs:label>Continues</rdfs:label>
        <rdfs:comment>Work that is continued by the content of a later work under a new title.</rdfs:comment>
        <dcterms:modified>2014-04-10 (Updated subproperty)</dcterms:modified>
        <rdfs:domain rdf:resource="&vocab;Work"/>
        <rdfs:range rdf:resource="&vocab;Work"/>
    </owl:ObjectProperty>
    


    <!-- http://bibframe.org/vocab/continuesInPart -->

    <owl:ObjectProperty rdf:about="&vocab;continuesInPart">
        <rdfs:label>Continues in part</rdfs:label>
        <rdfs:comment>Work that split into two or more separate works with new titles.</rdfs:comment>
        <dcterms:modified>2014-04-10 (Updated subproperty)</dcterms:modified>
        <rdfs:domain rdf:resource="&vocab;Work"/>
        <rdfs:range rdf:resource="&vocab;Work"/>
    </owl:ObjectProperty>
    


    <!-- http://bibframe.org/vocab/contributor -->

    <owl:ObjectProperty rdf:about="&vocab;contributor">
        <rdfs:label>Contributor role</rdfs:label>
        <rdfs:comment>Generalized expressive responsibility role.</rdfs:comment>
        <rdfs:range rdf:resource="&vocab;Authority"/>
    </owl:ObjectProperty>
    


    <!-- http://bibframe.org/vocab/coverArt -->

    <owl:ObjectProperty rdf:about="&vocab;coverArt">
        <rdfs:label>Cover art</rdfs:label>
        <rdfs:comment>Cover art image.</rdfs:comment>
        <rdfs:domain rdf:resource="&vocab;CoverArt"/>
        <rdfs:subPropertyOf rdf:resource="&vocab;annotationBody"/>
        <rdfs:range rdf:resource="&rdfs;Resource"/>
    </owl:ObjectProperty>
    


    <!-- http://bibframe.org/vocab/coverArtFor -->

    <owl:ObjectProperty rdf:about="&vocab;coverArtFor">
        <rdfs:label>Cover art of instance</rdfs:label>
        <rdfs:comment>Resource to which the cover art pertains.</rdfs:comment>
        <rdfs:domain rdf:resource="&vocab;CoverArt"/>
        <rdfs:range rdf:resource="&vocab;Instance"/>
        <rdfs:subPropertyOf rdf:resource="&vocab;annotates"/>
    </owl:ObjectProperty>
    


    <!-- http://bibframe.org/vocab/coverArtThumb -->

    <owl:ObjectProperty rdf:about="&vocab;coverArtThumb">
        <rdfs:label>Thumbnail of cover art</rdfs:label>
        <rdfs:comment>Thumbnail version of cover art image.</rdfs:comment>
        <rdfs:domain rdf:resource="&vocab;CoverArt"/>
        <rdfs:subPropertyOf rdf:resource="&vocab;annotationBody"/>
        <rdfs:range rdf:resource="&rdfs;Resource"/>
    </owl:ObjectProperty>
    


    <!-- http://bibframe.org/vocab/creator -->

    <owl:ObjectProperty rdf:about="&vocab;creator">
        <rdfs:label>Creator role</rdfs:label>
        <rdfs:comment>Generalized creative responsibility role.</rdfs:comment>
        <rdfs:range rdf:resource="&vocab;Authority"/>
    </owl:ObjectProperty>
    


    <!-- http://bibframe.org/vocab/dataSource -->

    <owl:ObjectProperty rdf:about="&vocab;dataSource">
        <rdfs:label>Has data source</rdfs:label>
        <rdfs:comment>Work that is a data source to which the described resource is related. It may contain information about other files, printed sources, or collection procedures.</rdfs:comment>
        <rdfs:range rdf:resource="&vocab;Work"/>
        <rdfs:domain rdf:resource="&vocab;Work"/>
        <rdfs:subPropertyOf rdf:resource="&vocab;relatedTo"/>
    </owl:ObjectProperty>
    


    <!-- http://bibframe.org/vocab/derivedFrom -->

    <owl:ObjectProperty rdf:about="&vocab;derivedFrom">
        <rdfs:label>Source record</rdfs:label>
        <rdfs:comment>Link to the record that was the source of the data, when applicable.</rdfs:comment>
        <rdfs:range rdf:resource="&rdfs;Resource"/>
    </owl:ObjectProperty>
    


    <!-- http://bibframe.org/vocab/descriptionConventions -->

    <owl:ObjectProperty rdf:about="&vocab;descriptionConventions">
        <rdfs:label>Description conventions</rdfs:label>
        <dcterms:modified>2014-05-13 (updated)</dcterms:modified>
        <rdfs:comment>Rules used for the descriptive content of the description.</rdfs:comment>
        <rdfs:range rdf:resource="&rdfs;Resource"/>
    </owl:ObjectProperty>
    


    <!-- http://bibframe.org/vocab/descriptionLanguage -->

    <owl:ObjectProperty rdf:about="&vocab;descriptionLanguage">
        <rdfs:label>Description language</rdfs:label>
        <rdfs:comment>Language used for the metadata.</rdfs:comment>
        <rdfs:range rdf:resource="&rdfs;Resource"/>
    </owl:ObjectProperty>
    


    <!-- http://bibframe.org/vocab/descriptionModifier -->

    <owl:ObjectProperty rdf:about="&vocab;descriptionModifier">
        <rdfs:label>Description modifier</rdfs:label>
        <dcterms:modified>2014-10-27 (Updated)</dcterms:modified>
        <rdfs:comment>Agency that modified a description.</rdfs:comment>
        <rdfs:range rdf:resource="&rdfs;Resource"/>
    </owl:ObjectProperty>
    


    <!-- http://bibframe.org/vocab/descriptionSource -->

    <owl:ObjectProperty rdf:about="&vocab;descriptionSource">
        <rdfs:label>Description source</rdfs:label>
        <rdfs:comment>Entity that created or modified the metadata.</rdfs:comment>
        <rdfs:range rdf:resource="&rdfs;Resource"/>
    </owl:ObjectProperty>
    


    <!-- http://bibframe.org/vocab/dissertationIdentifier -->

    <owl:ObjectProperty rdf:about="&vocab;dissertationIdentifier">
        <rdfs:label>Dissertation identifier</rdfs:label>
        <rdfs:comment>Identifier assigned to a dissertation for identification purposes .</rdfs:comment>
        <rdfs:range rdf:resource="&vocab;Identifier"/>
        <rdfs:domain rdf:resource="&vocab;Work"/>
        <rdfs:subPropertyOf rdf:resource="&vocab;identifier"/>
    </owl:ObjectProperty>
    


    <!-- http://bibframe.org/vocab/dissertationInstitution -->

    <owl:ObjectProperty rdf:about="&vocab;dissertationInstitution">
        <rdfs:label>Degree issuing institution</rdfs:label>
        <rdfs:comment>Name of degree granting institution.</rdfs:comment>
        <rdfs:range rdf:resource="&vocab;Agent"/>
        <rdfs:domain rdf:resource="&vocab;Work"/>
    </owl:ObjectProperty>
    


    <!-- http://bibframe.org/vocab/distribution -->

    <owl:ObjectProperty rdf:about="&vocab;distribution">
        <rdfs:label>Distribution event</rdfs:label>
        <rdfs:comment>Information relating to distribution of an instance.</rdfs:comment>
        <rdfs:domain rdf:resource="&vocab;Instance"/>
        <rdfs:range rdf:resource="&vocab;Provider"/>
        <rdfs:subPropertyOf rdf:resource="&vocab;provider"/>
    </owl:ObjectProperty>
    


    <!-- http://bibframe.org/vocab/doi -->

    <owl:ObjectProperty rdf:about="&vocab;doi">
        <rdfs:label>DOI</rdfs:label>
        <rdfs:comment>Digital Object Identifier.</rdfs:comment>
        <rdfs:range rdf:resource="&vocab;Identifier"/>
        <rdfs:domain rdf:resource="&vocab;Instance"/>
        <rdfs:subPropertyOf rdf:resource="&vocab;identifier"/>
    </owl:ObjectProperty>
    


    <!-- http://bibframe.org/vocab/ean -->

    <owl:ObjectProperty rdf:about="&vocab;ean">
        <rdfs:label>EAN</rdfs:label>
        <rdfs:comment>International Article Identifier.</rdfs:comment>
        <rdfs:range rdf:resource="&vocab;Identifier"/>
        <rdfs:domain rdf:resource="&vocab;Instance"/>
        <rdfs:subPropertyOf rdf:resource="&vocab;identifier"/>
    </owl:ObjectProperty>
    


    <!-- http://bibframe.org/vocab/electronicLocator -->

    <owl:ObjectProperty rdf:about="&vocab;electronicLocator">
        <rdfs:label>Electronic location</rdfs:label>
        <dcterms:modified>2014-04-28 (New)</dcterms:modified>
        <rdfs:comment>Electronic location from which the resource is available.</rdfs:comment>
        <rdfs:domain rdf:resource="&vocab;HeldMaterial"/>
        <rdfs:range rdf:resource="&rdfs;Resource"/>
    </owl:ObjectProperty>
    


    <!-- http://bibframe.org/vocab/event -->

    <owl:ObjectProperty rdf:about="&vocab;event">
        <rdfs:label>Event associated with content</rdfs:label>
        <rdfs:comment>Information about the geographic area/or time period covered by an event (e.g., a report).</rdfs:comment>
        <dcterms:modified>2014-05-16 (Updated)</dcterms:modified>
        <rdfs:range rdf:resource="&vocab;Event"/>
        <rdfs:domain rdf:resource="&vocab;Work"/>
    </owl:ObjectProperty>
    


    <!-- http://bibframe.org/vocab/eventAgent -->

    <owl:ObjectProperty rdf:about="&vocab;eventAgent">
        <rdfs:label>Agent for event</rdfs:label>
        <dcterms:modified>2014-05-16 (Updated)</dcterms:modified>
        <rdfs:comment>Person or organization associated with event.</rdfs:comment>
        <rdfs:range rdf:resource="&vocab;Agent"/>
        <rdfs:domain rdf:resource="&vocab;Event"/>
    </owl:ObjectProperty>
    


    <!-- http://bibframe.org/vocab/eventPlace -->

    <owl:ObjectProperty rdf:about="&vocab;eventPlace">
        <rdfs:label>Place of event</rdfs:label>
        <rdfs:comment>Geographic area associated with event.</rdfs:comment>
        <rdfs:domain rdf:resource="&vocab;Event"/>
        <rdfs:range rdf:resource="&vocab;Place"/>
    </owl:ObjectProperty>
    


    <!-- http://bibframe.org/vocab/expressionOf -->

    <owl:ObjectProperty rdf:about="&vocab;expressionOf">
        <rdfs:label>Expression of</rdfs:label>
        <dcterms:modified>2014-04-10 (Updated subproperty)</dcterms:modified>
        <rdfs:comment>Expression has a related work. For use to connect Works under FRBR/RDA rules.</rdfs:comment>
        <rdfs:range rdf:resource="&vocab;Work"/>
        <rdfs:domain rdf:resource="&vocab;Work"/>
        <rdfs:subPropertyOf rdf:resource="&vocab;relatedTo"/>
    </owl:ObjectProperty>
    


    <!-- http://bibframe.org/vocab/findingAid -->

    <owl:ObjectProperty rdf:about="&vocab;findingAid">
        <rdfs:label>Has finding aid</rdfs:label>
        <rdfs:comment>Relationship is to a finding aid or similar control materials for archival, visual, and manuscript resources.</rdfs:comment>
        <rdfs:range rdf:resource="&vocab;Work"/>
        <rdfs:domain rdf:resource="&vocab;Work"/>
    </owl:ObjectProperty>
    


    <!-- http://bibframe.org/vocab/fingerprint -->

    <owl:ObjectProperty rdf:about="&vocab;fingerprint">
        <rdfs:label>Fingerprint identifier</rdfs:label>
        <rdfs:comment>Identifier that is used to assist in the identification of antiquarian books by recording information comprising groups of characters taken from specified positions on specified pages of the book.</rdfs:comment>
        <rdfs:range rdf:resource="&vocab;Identifier"/>
        <rdfs:domain rdf:resource="&vocab;Instance"/>
        <rdfs:subPropertyOf rdf:resource="&vocab;identifier"/>
    </owl:ObjectProperty>
    


    <!-- http://bibframe.org/vocab/genre -->

    <owl:ObjectProperty rdf:about="&vocab;genre">
        <rdfs:label>Genre</rdfs:label>
        <rdfs:comment>Genre and other general characteristics associated with genre and form.</rdfs:comment>
        <dcterms:modified>2014-03-21 (New)</dcterms:modified>
        <rdfs:range rdf:resource="&vocab;Category"/>
    </owl:ObjectProperty>
    


    <!-- http://bibframe.org/vocab/hasAnnotation -->

    <owl:ObjectProperty rdf:about="&vocab;hasAnnotation">
        <rdfs:label>Has annotation</rdfs:label>
        <rdfs:comment>Resource has an annotation.</rdfs:comment>
        <rdfs:range rdf:resource="&vocab;Annotation"/>
    </owl:ObjectProperty>
    


    <!-- http://bibframe.org/vocab/hasAuthority -->

    <owl:ObjectProperty rdf:about="&vocab;hasAuthority">
        <rdfs:label>Authority information</rdfs:label>
        <rdfs:comment>Link to controlled form of name or subject and other information about.</rdfs:comment>
        <dcterms:modified>2014-04-10 (Updated range)</dcterms:modified>
        <rdfs:domain rdf:resource="&vocab;Authority"/>
        <rdfs:range rdf:resource="&vocab;Resource"/>
    </owl:ObjectProperty>
    


    <!-- http://bibframe.org/vocab/hasExpression -->

    <owl:ObjectProperty rdf:about="&vocab;hasExpression">
        <rdfs:label>Expressed as</rdfs:label>
        <rdfs:comment>Work has a related expression. For use to connect Works under FRBR/RDA rules.</rdfs:comment>
        <dcterms:modified>2014-04-10 (Updated subproperty)</dcterms:modified>
        <rdfs:domain rdf:resource="&vocab;Work"/>
        <rdfs:range rdf:resource="&vocab;Work"/>
        <rdfs:subPropertyOf rdf:resource="&vocab;relatedTo"/>
    </owl:ObjectProperty>
    


    <!-- http://bibframe.org/vocab/hasInstance -->

    <owl:ObjectProperty rdf:about="&vocab;hasInstance">
        <rdfs:label>Instance of Work</rdfs:label>
        <rdfs:comment>Work has a related Instance/manifestation. For use to connect Works to Instances in the BIBFRAME structure.</rdfs:comment>
        <dcterms:modified>2014--03-21 (Updated definition)</dcterms:modified>
        <rdfs:range rdf:resource="&vocab;Instance"/>
        <rdfs:domain rdf:resource="&vocab;Work"/>
        <rdfs:subPropertyOf rdf:resource="&vocab;relatedTo"/>
    </owl:ObjectProperty>
    


    <!-- http://bibframe.org/vocab/hdl -->

    <owl:ObjectProperty rdf:about="&vocab;hdl">
        <rdfs:label>Handle</rdfs:label>
        <rdfs:comment>Unique and persistent identifier for digital objects developed by the Corporation for National Research Initiatives.</rdfs:comment>
        <rdfs:range rdf:resource="&vocab;Identifier"/>
        <rdfs:domain rdf:resource="&vocab;Instance"/>
        <rdfs:subPropertyOf rdf:resource="&vocab;identifier"/>
    </owl:ObjectProperty>
    


    <!-- http://bibframe.org/vocab/heldBy -->

    <owl:ObjectProperty rdf:about="&vocab;heldBy">
        <rdfs:label>Held by</rdfs:label>
        <rdfs:comment>Entity holding the item or from which it is available</rdfs:comment>
        <rdfs:range rdf:resource="&vocab;Agent"/>
        <rdfs:domain rdf:resource="&vocab;HeldMaterial"/>
    </owl:ObjectProperty>
    


    <!-- http://bibframe.org/vocab/holdingFor -->

    <owl:ObjectProperty rdf:about="&vocab;holdingFor">
        <rdfs:label>Holding for</rdfs:label>
        <rdfs:comment>Instance for which holding is reported</rdfs:comment>
        <rdfs:domain rdf:resource="&vocab;HeldMaterial"/>
        <rdfs:range rdf:resource="&vocab;Instance"/>
        <rdfs:subPropertyOf rdf:resource="&vocab;annotates"/>
    </owl:ObjectProperty>
    


    <!-- http://bibframe.org/vocab/identifier -->

    <owl:ObjectProperty rdf:about="&vocab;identifier">
        <rdfs:label>Identifier</rdfs:label>
        <rdfs:comment>Number or code that uniquely identifies an entity.</rdfs:comment>
        <rdfs:range rdf:resource="&vocab;Identifier"/>
        <rdfs:domain rdf:resource="&vocab;Resource"/>
    </owl:ObjectProperty>
    


    <!-- http://bibframe.org/vocab/identifierScheme -->

    <owl:ObjectProperty rdf:about="&vocab;identifierScheme">
        <rdfs:label>Identifier scheme</rdfs:label>
        <rdfs:comment>Scheme within which the identifier is unique.</rdfs:comment>
        <dcterms:modified>2014-06-04 (Updated mapping)</dcterms:modified>
        <dcterms:modified>&apos;2014-06-04 (Updated range)</dcterms:modified>
        <rdfs:domain rdf:resource="&vocab;Identifier"/>
        <rdfs:range rdf:resource="&rdfs;Resource"/>
    </owl:ObjectProperty>
    


    <!-- http://bibframe.org/vocab/index -->

    <owl:ObjectProperty rdf:about="&vocab;index">
        <rdfs:label>Index</rdfs:label>
        <rdfs:comment>Work has an accompanying index</rdfs:comment>
        <rdfs:domain rdf:resource="&vocab;Work"/>
        <rdfs:range rdf:resource="&vocab;Work"/>
    </owl:ObjectProperty>
    


    <!-- http://bibframe.org/vocab/instanceOf -->

    <owl:ObjectProperty rdf:about="&vocab;instanceOf">
        <rdfs:label>Instance of</rdfs:label>
        <rdfs:comment>Work this resource instantiates or manifests. For use to connect Instances to Works in the BIBFRAME structure.</rdfs:comment>
        <dcterms:modified>2014--03-21 (Updated definition)</dcterms:modified>
        <rdfs:domain rdf:resource="&vocab;Instance"/>
        <rdfs:range rdf:resource="&vocab;Work"/>
        <rdfs:subPropertyOf rdf:resource="&vocab;relatedTo"/>
    </owl:ObjectProperty>
    


    <!-- http://bibframe.org/vocab/instanceTitle -->

    <owl:ObjectProperty rdf:about="&vocab;instanceTitle">
        <rdfs:label>Instance title</rdfs:label>
        <rdfs:comment>Word, character, or group of words and/or characters that is the main name of an instance.</rdfs:comment>
        <rdfs:domain rdf:resource="&vocab;Instance"/>
        <rdfs:range rdf:resource="&vocab;Title"/>
    </owl:ObjectProperty>
    


    <!-- http://bibframe.org/vocab/intendedAudience -->

    <owl:ObjectProperty rdf:about="&vocab;intendedAudience">
        <rdfs:label>Intended audience</rdfs:label>
        <rdfs:comment>Information that identifies the specific audience or intellectual level for which the content of the resource is considered appropriate.</rdfs:comment>
        <rdfs:range rdf:resource="&vocab;IntendedAudience"/>
    </owl:ObjectProperty>
    


    <!-- http://bibframe.org/vocab/isan -->

    <owl:ObjectProperty rdf:about="&vocab;isan">
        <rdfs:label>ISAN</rdfs:label>
        <rdfs:comment>International Standard Audiovisual Number.</rdfs:comment>
        <rdfs:range rdf:resource="&vocab;Identifier"/>
        <rdfs:domain rdf:resource="&vocab;Work"/>
        <rdfs:subPropertyOf rdf:resource="&vocab;identifier"/>
    </owl:ObjectProperty>
    


    <!-- http://bibframe.org/vocab/isbn -->

    <owl:ObjectProperty rdf:about="&vocab;isbn">
        <rdfs:label>ISBN</rdfs:label>
        <rdfs:comment>International Standard Book Number.</rdfs:comment>
        <rdfs:range rdf:resource="&vocab;Identifier"/>
        <rdfs:domain rdf:resource="&vocab;Instance"/>
        <rdfs:subPropertyOf rdf:resource="&vocab;identifier"/>
    </owl:ObjectProperty>
    


    <!-- http://bibframe.org/vocab/isbn10 -->

    <owl:ObjectProperty rdf:about="&vocab;isbn10">
        <rdfs:label>ISBN-10</rdfs:label>
        <rdfs:comment>10 digit version of the International Standard Book Number.</rdfs:comment>
        <rdfs:range rdf:resource="&vocab;Identifier"/>
        <rdfs:domain rdf:resource="&vocab;Instance"/>
        <rdfs:subPropertyOf rdf:resource="&vocab;isbn"/>
    </owl:ObjectProperty>
    


    <!-- http://bibframe.org/vocab/isbn13 -->

    <owl:ObjectProperty rdf:about="&vocab;isbn13">
        <rdfs:label>ISBN-13</rdfs:label>
        <rdfs:comment>13 digit version of the International Standard Book Number.</rdfs:comment>
        <rdfs:range rdf:resource="&vocab;Identifier"/>
        <rdfs:domain rdf:resource="&vocab;Instance"/>
        <rdfs:subPropertyOf rdf:resource="&vocab;isbn"/>
    </owl:ObjectProperty>
    


    <!-- http://bibframe.org/vocab/ismn -->

    <owl:ObjectProperty rdf:about="&vocab;ismn">
        <rdfs:label>ISMN</rdfs:label>
        <rdfs:comment>International Standard Music Number.</rdfs:comment>
        <rdfs:range rdf:resource="&vocab;Identifier"/>
        <rdfs:domain rdf:resource="&vocab;Instance"/>
        <rdfs:subPropertyOf rdf:resource="&vocab;identifier"/>
    </owl:ObjectProperty>
    


    <!-- http://bibframe.org/vocab/iso -->

    <owl:ObjectProperty rdf:about="&vocab;iso">
        <rdfs:label>ISO number</rdfs:label>
        <rdfs:comment>International Organization for Standardization standard number.</rdfs:comment>
        <rdfs:range rdf:resource="&vocab;Identifier"/>
        <rdfs:domain rdf:resource="&vocab;Instance"/>
        <rdfs:subPropertyOf rdf:resource="&vocab;identifier"/>
    </owl:ObjectProperty>
    


    <!-- http://bibframe.org/vocab/issn -->

    <owl:ObjectProperty rdf:about="&vocab;issn">
        <rdfs:label>ISSN</rdfs:label>
        <rdfs:comment>International Standard Serial Number identifier.</rdfs:comment>
        <rdfs:range rdf:resource="&vocab;Identifier"/>
        <rdfs:domain rdf:resource="&vocab;Instance"/>
        <rdfs:subPropertyOf rdf:resource="&vocab;identifier"/>
    </owl:ObjectProperty>
    


    <!-- http://bibframe.org/vocab/issnL -->

    <owl:ObjectProperty rdf:about="&vocab;issnL">
        <rdfs:label>ISSN-L</rdfs:label>
        <rdfs:comment>International Standard Serial Number that links together various media versions of a continuing resource.</rdfs:comment>
        <rdfs:range rdf:resource="&vocab;Identifier"/>
        <rdfs:domain rdf:resource="&vocab;Work"/>
        <rdfs:subPropertyOf rdf:resource="&vocab;identifier"/>
    </owl:ObjectProperty>
    


    <!-- http://bibframe.org/vocab/issueNumber -->

    <owl:ObjectProperty rdf:about="&vocab;issueNumber">
        <rdfs:label>Audio issue number</rdfs:label>
        <rdfs:comment>Number used to identify the issue designation, or serial identification, assigned by a publisher to a sound recording.</rdfs:comment>
        <rdfs:range rdf:resource="&vocab;Identifier"/>
        <rdfs:domain rdf:resource="&vocab;Instance"/>
        <rdfs:subPropertyOf rdf:resource="&vocab;identifier"/>
    </owl:ObjectProperty>
    


    <!-- http://bibframe.org/vocab/issuedWith -->

    <owl:ObjectProperty rdf:about="&vocab;issuedWith">
        <rdfs:label>Issued with</rdfs:label>
        <rdfs:comment>Instance that is issued on the same carrier as the manifestation being described.</rdfs:comment>
        <rdfs:range rdf:resource="&vocab;Instance"/>
        <rdfs:domain rdf:resource="&vocab;Instance"/>
    </owl:ObjectProperty>
    


    <!-- http://bibframe.org/vocab/istc -->

    <owl:ObjectProperty rdf:about="&vocab;istc">
        <rdfs:label>ISTC</rdfs:label>
        <rdfs:comment>International Standard Text code, a numbering system developed to enable the unique identification of textual works.</rdfs:comment>
        <dcterms:modified>a,z</dcterms:modified>
        <rdfs:range rdf:resource="&vocab;Identifier"/>
        <rdfs:domain rdf:resource="&vocab;Work"/>
        <rdfs:subPropertyOf rdf:resource="&vocab;identifier"/>
    </owl:ObjectProperty>
    


    <!-- http://bibframe.org/vocab/iswc -->

    <owl:ObjectProperty rdf:about="&vocab;iswc">
        <rdfs:label>ISWC</rdfs:label>
        <rdfs:comment>International Standard Musical Work Code, a unique, persistent reference number for the identification of musical works.</rdfs:comment>
        <rdfs:range rdf:resource="&vocab;Identifier"/>
        <rdfs:domain rdf:resource="&vocab;Work"/>
        <rdfs:subPropertyOf rdf:resource="&vocab;identifier"/>
    </owl:ObjectProperty>
    


    <!-- http://bibframe.org/vocab/keyTitle -->

    <owl:ObjectProperty rdf:about="&vocab;keyTitle">
        <rdfs:label>Key title</rdfs:label>
        <rdfs:comment>Unique title for a continuing resource that is assigned by the ISSN International Center in conjunction with an ISSN.</rdfs:comment>
        <rdfs:domain rdf:resource="&vocab;Instance"/>
        <rdfs:range rdf:resource="&vocab;Title"/>
        <rdfs:subPropertyOf rdf:resource="&vocab;instanceTitle"/>
    </owl:ObjectProperty>
    


    <!-- http://bibframe.org/vocab/language -->

    <owl:ObjectProperty rdf:about="&vocab;language">
        <rdfs:label>Language</rdfs:label>
        <rdfs:comment>Languages associated with a resource including those for multilingual resources and translated resources.</rdfs:comment>
        <rdfs:range rdf:resource="&vocab;Language"/>
    </owl:ObjectProperty>
    


    <!-- http://bibframe.org/vocab/languageOfPartUri -->

    <owl:ObjectProperty rdf:about="&vocab;languageOfPartUri">
        <rdfs:label>Language of part URI</rdfs:label>
        <rdfs:comment>Language or notation system used to convey the content of the resource (associated with part or all of a resource).</rdfs:comment>
        <rdfs:domain rdf:resource="&vocab;Language"/>
        <rdfs:range rdf:resource="&rdfs;Resource"/>
    </owl:ObjectProperty>
    


    <!-- http://bibframe.org/vocab/lcOverseasAcq -->

    <owl:ObjectProperty rdf:about="&vocab;lcOverseasAcq">
        <rdfs:label>LC acquisition program</rdfs:label>
        <rdfs:comment>Identification number assigned by the Library of Congress to works acquired through one of its overseas acquisition programs.</rdfs:comment>
        <rdfs:range rdf:resource="&vocab;Identifier"/>
        <rdfs:domain rdf:resource="&vocab;Instance"/>
        <rdfs:subPropertyOf rdf:resource="&vocab;identifier"/>
    </owl:ObjectProperty>
    


    <!-- http://bibframe.org/vocab/lccn -->

    <owl:ObjectProperty rdf:about="&vocab;lccn">
        <rdfs:label>LCCN</rdfs:label>
        <rdfs:comment>Library of Congress Control Number, which identifies the resource description.</rdfs:comment>
        <rdfs:range rdf:resource="&vocab;Identifier"/>
        <rdfs:domain rdf:resource="&vocab;Instance"/>
        <rdfs:subPropertyOf rdf:resource="&vocab;identifier"/>
    </owl:ObjectProperty>
    


    <!-- http://bibframe.org/vocab/legalDeposit -->

    <owl:ObjectProperty rdf:about="&vocab;legalDeposit">
        <rdfs:label>Copyright number</rdfs:label>
        <rdfs:comment>Number assigned to a copyright or legal deposit, which Identifies a resource description.</rdfs:comment>
        <rdfs:range rdf:resource="&vocab;Identifier"/>
        <rdfs:domain rdf:resource="&vocab;Instance"/>
        <rdfs:subPropertyOf rdf:resource="&vocab;identifier"/>
    </owl:ObjectProperty>
    


    <!-- http://bibframe.org/vocab/local -->

    <owl:ObjectProperty rdf:about="&vocab;local">
        <rdfs:label>Local identifier</rdfs:label>
        <rdfs:comment>Identifier established locally and not a standard number.</rdfs:comment>
        <rdfs:range rdf:resource="&vocab;Identifier"/>
        <rdfs:subPropertyOf rdf:resource="&vocab;identifier"/>
    </owl:ObjectProperty>
    


    <!-- http://bibframe.org/vocab/manufacture -->

    <owl:ObjectProperty rdf:about="&vocab;manufacture">
        <rdfs:label>Manufacture event</rdfs:label>
        <rdfs:comment>Information relating to manufacture of an instance.</rdfs:comment>
        <rdfs:domain rdf:resource="&vocab;Instance"/>
        <rdfs:range rdf:resource="&vocab;Provider"/>
        <rdfs:subPropertyOf rdf:resource="&vocab;provider"/>
    </owl:ObjectProperty>
    


    <!-- http://bibframe.org/vocab/matrixNumber -->

    <owl:ObjectProperty rdf:about="&vocab;matrixNumber">
        <rdfs:label>Audio matrix number</rdfs:label>
        <rdfs:comment>Matrix number from the master from which a specific sound recording was pressed.</rdfs:comment>
        <rdfs:range rdf:resource="&vocab;Identifier"/>
        <rdfs:domain rdf:resource="&vocab;Instance"/>
        <rdfs:subPropertyOf rdf:resource="&vocab;identifier"/>
    </owl:ObjectProperty>
    


    <!-- http://bibframe.org/vocab/mediaCategory -->

    <owl:ObjectProperty rdf:about="&vocab;mediaCategory">
        <rdfs:label>Media type</rdfs:label>
        <rdfs:comment>Categorization reflecting the general type of intermediation device required to view, play, run, etc., the content of a resource.</rdfs:comment>
        <rdfs:range rdf:resource="&vocab;Category"/>
        <rdfs:domain rdf:resource="&vocab;Instance"/>
    </owl:ObjectProperty>
    


    <!-- http://bibframe.org/vocab/mergedToForm -->

    <owl:ObjectProperty rdf:about="&vocab;mergedToForm">
        <rdfs:label>Merged to form</rdfs:label>
        <rdfs:comment>One of two or more works that come together to form a new work.</rdfs:comment>
        <dcterms:modified>2014-04-10 (Updated subproperty)</dcterms:modified>
        <rdfs:domain rdf:resource="&vocab;Work"/>
        <rdfs:range rdf:resource="&vocab;Work"/>
    </owl:ObjectProperty>
    


    <!-- http://bibframe.org/vocab/musicMedium -->

    <owl:ObjectProperty rdf:about="&vocab;musicMedium">
        <rdfs:label>Music medium</rdfs:label>
        <rdfs:comment>Instrumental, vocal, and/or other medium of performance for which a musical resource was originally conceived, written or performed.</rdfs:comment>
        <rdfs:range rdf:resource="&rdfs;Resource"/>
    </owl:ObjectProperty>
    


    <!-- http://bibframe.org/vocab/musicPlate -->

    <owl:ObjectProperty rdf:about="&vocab;musicPlate">
        <rdfs:label>Music plate number</rdfs:label>
        <rdfs:comment>Number assigned by a music publisher to a specific music publication.</rdfs:comment>
        <rdfs:range rdf:resource="&vocab;Identifier"/>
        <rdfs:domain rdf:resource="&vocab;Instance"/>
        <rdfs:subPropertyOf rdf:resource="&vocab;identifier"/>
    </owl:ObjectProperty>
    


    <!-- http://bibframe.org/vocab/musicPublisherNumber -->

    <owl:ObjectProperty rdf:about="&vocab;musicPublisherNumber">
        <rdfs:label>Music publisher number</rdfs:label>
        <rdfs:comment>Number assigned to a music publication other than an issue, matrix, or plate number.</rdfs:comment>
        <rdfs:range rdf:resource="&vocab;Identifier"/>
        <rdfs:domain rdf:resource="&vocab;Instance"/>
        <rdfs:subPropertyOf rdf:resource="&vocab;identifier"/>
    </owl:ObjectProperty>
    


    <!-- http://bibframe.org/vocab/nban -->

    <owl:ObjectProperty rdf:about="&vocab;nban">
        <rdfs:label>NBAN</rdfs:label>
        <rdfs:comment>National Bibliography Agency Number, which identifies the resource description.</rdfs:comment>
        <rdfs:range rdf:resource="&vocab;Identifier"/>
        <rdfs:domain rdf:resource="&vocab;Instance"/>
        <rdfs:subPropertyOf rdf:resource="&vocab;identifier"/>
    </owl:ObjectProperty>
    


    <!-- http://bibframe.org/vocab/nbn -->

    <owl:ObjectProperty rdf:about="&vocab;nbn">
        <rdfs:label>NBN</rdfs:label>
        <rdfs:comment>National Bibliography Number, which identifies the resource description.</rdfs:comment>
        <rdfs:range rdf:resource="&vocab;Identifier"/>
        <rdfs:domain rdf:resource="&vocab;Instance"/>
        <rdfs:subPropertyOf rdf:resource="&vocab;identifier"/>
    </owl:ObjectProperty>
    


    <!-- http://bibframe.org/vocab/originPlace -->

    <owl:ObjectProperty rdf:about="&vocab;originPlace">
        <rdfs:label>Associated title place</rdfs:label>
        <rdfs:comment>Place from which the creation of the work originated.</rdfs:comment>
        <rdfs:range rdf:resource="&vocab;Place"/>
        <rdfs:domain rdf:resource="&vocab;Work"/>
    </owl:ObjectProperty>
    


    <!-- http://bibframe.org/vocab/originalVersion -->

    <owl:ObjectProperty rdf:about="&vocab;originalVersion">
        <rdfs:label>Has original version</rdfs:label>
        <rdfs:comment>Instance is the original version of which this resource is a reproduction.</rdfs:comment>
        <rdfs:domain rdf:resource="&vocab;Work"/>
        <rdfs:range rdf:resource="&vocab;Work"/>
    </owl:ObjectProperty>
    


    <!-- http://bibframe.org/vocab/otherEdition -->

    <owl:ObjectProperty rdf:about="&vocab;otherEdition">
        <rdfs:label>hasOtherEdition</rdfs:label>
        <rdfs:comment>Resource has other available editions, for example simultaneously published language editions or reprints.</rdfs:comment>
        <rdfs:domain rdf:resource="&vocab;Work"/>
        <rdfs:range rdf:resource="&vocab;Work"/>
    </owl:ObjectProperty>
    


    <!-- http://bibframe.org/vocab/otherPhysicalFormat -->

    <owl:ObjectProperty rdf:about="&vocab;otherPhysicalFormat">
        <rdfs:label>Has other physical format</rdfs:label>
        <dcterms:modified>2014-10-14 (Updated)</dcterms:modified>
        <rdfs:comment>Resource that is manifested in another physical carrier.</rdfs:comment>
        <rdfs:domain rdf:resource="&vocab;Instance"/>
        <rdfs:range rdf:resource="&vocab;Instance"/>
    </owl:ObjectProperty>
    


    <!-- http://bibframe.org/vocab/postalRegistration -->

    <owl:ObjectProperty rdf:about="&vocab;postalRegistration">
        <rdfs:label>Postal registration number</rdfs:label>
        <rdfs:comment>Number assigned to a publication for which the specified postal service permits the use of a special mailing class privilege.</rdfs:comment>
        <rdfs:range rdf:resource="&vocab;Identifier"/>
        <rdfs:domain rdf:resource="&vocab;Instance"/>
        <rdfs:subPropertyOf rdf:resource="&vocab;identifier"/>
    </owl:ObjectProperty>
    


    <!-- http://bibframe.org/vocab/production -->

    <owl:ObjectProperty rdf:about="&vocab;production">
        <rdfs:label>Production event</rdfs:label>
        <rdfs:comment>Information relating to production of an instance.</rdfs:comment>
        <rdfs:domain rdf:resource="&vocab;Instance"/>
        <rdfs:range rdf:resource="&vocab;Provider"/>
        <rdfs:subPropertyOf rdf:resource="&vocab;provider"/>
    </owl:ObjectProperty>
    


    <!-- http://bibframe.org/vocab/provider -->

    <owl:ObjectProperty rdf:about="&vocab;provider">
        <rdfs:label>Provider</rdfs:label>
        <rdfs:comment>Place, name, and/or date information relating to the publication, printing, distribution, issue, release, or production instance.</rdfs:comment>
        <rdfs:domain rdf:resource="&vocab;Instance"/>
        <rdfs:range rdf:resource="&vocab;Provider"/>
    </owl:ObjectProperty>
    


    <!-- http://bibframe.org/vocab/providerName -->

    <owl:ObjectProperty rdf:about="&vocab;providerName">
        <rdfs:label>Provider name</rdfs:label>
        <rdfs:comment>Name of the entity responsible for the publication, printing, distribution, issue, release or production of the instance.</rdfs:comment>
        <rdfs:range rdf:resource="&vocab;Agent"/>
        <rdfs:domain rdf:resource="&vocab;Provider"/>
    </owl:ObjectProperty>
    


    <!-- http://bibframe.org/vocab/providerPlace -->

    <owl:ObjectProperty rdf:about="&vocab;providerPlace">
        <rdfs:label>Provider place</rdfs:label>
        <rdfs:comment>Place associated with the publication, printing, distribution, issue, release or production of the instance.</rdfs:comment>
        <rdfs:range rdf:resource="&vocab;Place"/>
        <rdfs:domain rdf:resource="&vocab;Provider"/>
    </owl:ObjectProperty>
    


    <!-- http://bibframe.org/vocab/publication -->

    <owl:ObjectProperty rdf:about="&vocab;publication">
        <rdfs:label>Publication event</rdfs:label>
        <rdfs:comment>Information relating to publication of an instance.</rdfs:comment>
        <rdfs:domain rdf:resource="&vocab;Instance"/>
        <rdfs:range rdf:resource="&vocab;Provider"/>
        <rdfs:subPropertyOf rdf:resource="&vocab;provider"/>
    </owl:ObjectProperty>
    


    <!-- http://bibframe.org/vocab/publisherNumber -->

    <owl:ObjectProperty rdf:about="&vocab;publisherNumber">
        <rdfs:label>Other publisher number</rdfs:label>
        <rdfs:comment>Number assigned by a publisher that is not one of the specific defined types.</rdfs:comment>
        <rdfs:range rdf:resource="&vocab;Identifier"/>
        <rdfs:domain rdf:resource="&vocab;Instance"/>
        <rdfs:subPropertyOf rdf:resource="&vocab;identifier"/>
    </owl:ObjectProperty>
    


    <!-- http://bibframe.org/vocab/referenceAuthority -->

    <owl:ObjectProperty rdf:about="&vocab;referenceAuthority">
        <rdfs:label>Other authority information</rdfs:label>
        <rdfs:comment>Link to authority information</rdfs:comment>
        <dcterms:modified>2014-03-27 (Updated)</dcterms:modified>
        <rdfs:domain rdf:resource="&vocab;Authority"/>
        <rdfs:range rdf:resource="&vocab;Resource"/>
    </owl:ObjectProperty>
    


    <!-- http://bibframe.org/vocab/relatedInstance -->

    <owl:ObjectProperty rdf:about="&vocab;relatedInstance">
        <rdfs:label>Related Instance</rdfs:label>
        <rdfs:comment>General instance to instance relationship.</rdfs:comment>
        <rdfs:range rdf:resource="&vocab;Instance"/>
        <rdfs:domain rdf:resource="&vocab;Instance"/>
        <rdfs:subPropertyOf rdf:resource="&vocab;relatedTo"/>
    </owl:ObjectProperty>
    


    <!-- http://bibframe.org/vocab/relatedTo -->

    <owl:ObjectProperty rdf:about="&vocab;relatedTo">
        <rdfs:label>Related resource</rdfs:label>
        <rdfs:comment>Any relationship between work or instance resources.</rdfs:comment>
        <dcterms:modified>2014-04-10 (Range updated)</dcterms:modified>
        <rdfs:domain rdf:resource="&vocab;Resource"/>
        <rdfs:range rdf:resource="&vocab;Resource"/>
    </owl:ObjectProperty>
    


    <!-- http://bibframe.org/vocab/relatedWork -->

    <owl:ObjectProperty rdf:about="&vocab;relatedWork">
        <rdfs:label>Related Work</rdfs:label>
        <rdfs:comment>General work to work relationship.</rdfs:comment>
        <rdfs:domain rdf:resource="&vocab;Work"/>
        <rdfs:range rdf:resource="&vocab;Work"/>
        <rdfs:subPropertyOf rdf:resource="&vocab;relatedTo"/>
    </owl:ObjectProperty>
    


    <!-- http://bibframe.org/vocab/relator -->

    <owl:ObjectProperty rdf:about="&vocab;relator">
        <rdfs:label>Relationship of agent</rdfs:label>
        <dcterms:modified>2014-04-30 (New)</dcterms:modified>
        <rdfs:comment>link to role and agent information.</rdfs:comment>
        <rdfs:range rdf:resource="&vocab;Relator"/>
    </owl:ObjectProperty>
    


    <!-- http://bibframe.org/vocab/reportNumber -->

    <owl:ObjectProperty rdf:about="&vocab;reportNumber">
        <rdfs:label>Technical report number</rdfs:label>
        <rdfs:comment>Identification number of a report that is not a Standard Technical Report Number.</rdfs:comment>
        <rdfs:range rdf:resource="&vocab;Identifier"/>
        <rdfs:domain rdf:resource="&vocab;Instance"/>
        <rdfs:subPropertyOf rdf:resource="&vocab;identifier"/>
    </owl:ObjectProperty>
    


    <!-- http://bibframe.org/vocab/reproduction -->

    <owl:ObjectProperty rdf:about="&vocab;reproduction">
        <rdfs:label>Has reproduction</rdfs:label>
        <rdfs:comment>Instance that reproduces another Instance embodying the same work.</rdfs:comment>
        <rdfs:range rdf:resource="&vocab;Instance"/>
        <rdfs:domain rdf:resource="&vocab;Instance"/>
    </owl:ObjectProperty>
    


    <!-- http://bibframe.org/vocab/review -->

    <owl:ObjectProperty rdf:about="&vocab;review">
        <rdfs:label>Review content</rdfs:label>
        <rdfs:comment>Review content.</rdfs:comment>
        <rdfs:domain rdf:resource="&vocab;Review"/>
        <rdfs:subPropertyOf rdf:resource="&vocab;annotationBody"/>
        <rdfs:range rdf:resource="&rdfs;Resource"/>
    </owl:ObjectProperty>
    


    <!-- http://bibframe.org/vocab/reviewOf -->

    <owl:ObjectProperty rdf:about="&vocab;reviewOf">
        <rdfs:label>Resource reviewed</rdfs:label>
        <rdfs:comment>Resource to which the review pertains.</rdfs:comment>
        <rdfs:domain rdf:resource="&vocab;Review"/>
        <rdfs:range rdf:resource="&vocab;Work"/>
        <rdfs:subPropertyOf rdf:resource="&vocab;annotates"/>
    </owl:ObjectProperty>
    


    <!-- http://bibframe.org/vocab/separatedFrom -->

    <owl:ObjectProperty rdf:about="&vocab;separatedFrom">
        <rdfs:label>Separated from</rdfs:label>
        <rdfs:comment>Work that spun off a part of its content to form a new work.</rdfs:comment>
        <dcterms:modified>2014-04-10 (Updated subproperty)</dcterms:modified>
        <rdfs:domain rdf:resource="&vocab;Work"/>
        <rdfs:range rdf:resource="&vocab;Work"/>
    </owl:ObjectProperty>
    


    <!-- http://bibframe.org/vocab/series -->

    <owl:ObjectProperty rdf:about="&vocab;series">
        <rdfs:label>Has series</rdfs:label>
        <rdfs:comment>Work in which the part has been issued; the title of the larger work appears on the part.</rdfs:comment>
        <dcterms:modified>2014-10-14 (Updated)</dcterms:modified>
        <rdfs:range rdf:resource="&vocab;Work"/>
        <rdfs:domain rdf:resource="&vocab;Work"/>
    </owl:ObjectProperty>
    


    <!-- http://bibframe.org/vocab/sici -->

    <owl:ObjectProperty rdf:about="&vocab;sici">
        <rdfs:label>SICI</rdfs:label>
        <rdfs:comment>Serial Item and Contribution Identifier.</rdfs:comment>
        <rdfs:range rdf:resource="&vocab;Identifier"/>
        <rdfs:domain rdf:resource="&vocab;Instance"/>
        <rdfs:subPropertyOf rdf:resource="&vocab;identifier"/>
    </owl:ObjectProperty>
    


    <!-- http://bibframe.org/vocab/splitInto -->

    <owl:ObjectProperty rdf:about="&vocab;splitInto">
        <rdfs:label>Split into</rdfs:label>
        <dcterms:modified>2014-04-10 (Updated subproperty)</dcterms:modified>
        <rdfs:comment>One of two or more works resulting from the division of an earlier work into separate works.</rdfs:comment>
        <rdfs:domain rdf:resource="&vocab;Work"/>
        <rdfs:range rdf:resource="&vocab;Work"/>
    </owl:ObjectProperty>
    


    <!-- http://bibframe.org/vocab/stockNumber -->

    <owl:ObjectProperty rdf:about="&vocab;stockNumber">
        <rdfs:label>Stock number</rdfs:label>
        <rdfs:comment>Identification number such as distributor, publisher, or vendor number.</rdfs:comment>
        <rdfs:range rdf:resource="&vocab;Identifier"/>
        <rdfs:domain rdf:resource="&vocab;Instance"/>
        <rdfs:subPropertyOf rdf:resource="&vocab;identifier"/>
    </owl:ObjectProperty>
    


    <!-- http://bibframe.org/vocab/strn -->

    <owl:ObjectProperty rdf:about="&vocab;strn">
        <rdfs:label>STRN</rdfs:label>
        <rdfs:comment>Standard Technical Report Number.</rdfs:comment>
        <rdfs:range rdf:resource="&vocab;Identifier"/>
        <rdfs:domain rdf:resource="&vocab;Instance"/>
        <rdfs:subPropertyOf rdf:resource="&vocab;identifier"/>
    </owl:ObjectProperty>
    


    <!-- http://bibframe.org/vocab/studyNumber -->

    <owl:ObjectProperty rdf:about="&vocab;studyNumber">
        <rdfs:label>Study number</rdfs:label>
        <rdfs:comment>Identification number for a computer data file.</rdfs:comment>
        <rdfs:range rdf:resource="&vocab;Identifier"/>
        <rdfs:domain rdf:resource="&vocab;Instance"/>
        <rdfs:subPropertyOf rdf:resource="&vocab;identifier"/>
    </owl:ObjectProperty>
    


    <!-- http://bibframe.org/vocab/subject -->

    <owl:ObjectProperty rdf:about="&vocab;subject">
        <rdfs:label>Subject</rdfs:label>
        <rdfs:comment>Subject term(s) describing a resource.</rdfs:comment>
        <rdfs:range rdf:resource="&vocab;Authority"/>
        <rdfs:range rdf:resource="&vocab;Work"/>
        <rdfs:domain rdf:resource="&vocab;Work"/>
    </owl:ObjectProperty>
    


    <!-- http://bibframe.org/vocab/subseries -->

    <owl:ObjectProperty rdf:about="&vocab;subseries">
        <rdfs:label>Has subseries</rdfs:label>
        <rdfs:comment>Work, which is part of another series, in which the part has been issued.</rdfs:comment>
        <dcterms:modified>2014-10-14 (Updated)</dcterms:modified>
        <rdfs:domain rdf:resource="&vocab;Work"/>
        <rdfs:range rdf:resource="&vocab;Work"/>
    </owl:ObjectProperty>
    


    <!-- http://bibframe.org/vocab/subseriesOf -->

    <owl:ObjectProperty rdf:about="&vocab;subseriesOf">
        <rdfs:label>Subseries of</rdfs:label>
        <rdfs:comment>Work in which the part consistently appears; the title of the larger work appears on all issues or parts of the subseries).</rdfs:comment>
        <dcterms:modified>2014-10-14 (Updated)</dcterms:modified>
        <rdfs:domain rdf:resource="&vocab;Work"/>
        <rdfs:range rdf:resource="&vocab;Work"/>
    </owl:ObjectProperty>
    


    <!-- http://bibframe.org/vocab/summary -->

    <owl:ObjectProperty rdf:about="&vocab;summary">
        <rdfs:label>Summary content</rdfs:label>
        <rdfs:comment>Summary or abstract of the target work or instance.</rdfs:comment>
        <rdfs:domain rdf:resource="&vocab;Summary"/>
        <rdfs:subPropertyOf rdf:resource="&vocab;annotationBody"/>
        <rdfs:range rdf:resource="&rdfs;Resource"/>
    </owl:ObjectProperty>
    


    <!-- http://bibframe.org/vocab/supersededBy -->

    <owl:ObjectProperty rdf:about="&vocab;supersededBy">
        <rdfs:label>Superseded by</rdfs:label>
        <dcterms:modified>2014-04-10 (Updated subproperty)</dcterms:modified>
        <rdfs:comment>Later Work used in place of an earlier work, usually because the later work contains updated or new information.</rdfs:comment>
        <rdfs:domain rdf:resource="&vocab;Work"/>
        <rdfs:range rdf:resource="&vocab;Work"/>
    </owl:ObjectProperty>
    


    <!-- http://bibframe.org/vocab/supersededInPartBy -->

    <owl:ObjectProperty rdf:about="&vocab;supersededInPartBy">
        <rdfs:label>Superseded in part by</rdfs:label>
        <rdfs:comment>Later Work used in part in place of an earlier work, usually because the later work contains updated or new information.</rdfs:comment>
        <dcterms:modified>2014-04-10 (Updated subproperty)</dcterms:modified>
        <rdfs:domain rdf:resource="&vocab;Work"/>
        <rdfs:range rdf:resource="&vocab;Work"/>
    </owl:ObjectProperty>
    


    <!-- http://bibframe.org/vocab/supersedes -->

    <owl:ObjectProperty rdf:about="&vocab;supersedes">
        <rdfs:label>Supersedes</rdfs:label>
        <dcterms:modified>2014-04-10 (Updated subproperty)</dcterms:modified>
        <rdfs:comment>Earlier work whose content has been replaced by a later work, usually because the later work contains updated or new information.</rdfs:comment>
        <rdfs:domain rdf:resource="&vocab;Work"/>
        <rdfs:range rdf:resource="&vocab;Work"/>
    </owl:ObjectProperty>
    


    <!-- http://bibframe.org/vocab/supersedesInPart -->

    <owl:ObjectProperty rdf:about="&vocab;supersedesInPart">
        <rdfs:label>Supersedes in part</rdfs:label>
        <dcterms:modified>2014-04-10 (Updated subproperty)</dcterms:modified>
        <rdfs:comment>Earlier work whose content has been partially replaced by a later work, usually because the later work contains updated or new information.</rdfs:comment>
        <rdfs:domain rdf:resource="&vocab;Work"/>
        <rdfs:range rdf:resource="&vocab;Work"/>
    </owl:ObjectProperty>
    


    <!-- http://bibframe.org/vocab/supplement -->

    <owl:ObjectProperty rdf:about="&vocab;supplement">
        <rdfs:label>Has supplement</rdfs:label>
        <rdfs:comment>Work that updates or otherwise complements the predominant work.</rdfs:comment>
        <rdfs:range rdf:resource="&vocab;Work"/>
        <rdfs:domain rdf:resource="&vocab;Work"/>
    </owl:ObjectProperty>
    


    <!-- http://bibframe.org/vocab/supplementTo -->

    <owl:ObjectProperty rdf:about="&vocab;supplementTo">
        <rdfs:label>Supplement to</rdfs:label>
        <rdfs:comment>Work that is updated or otherwise complemented by the augmenting work.</rdfs:comment>
        <rdfs:range rdf:resource="&vocab;Work"/>
        <rdfs:domain rdf:resource="&vocab;Work"/>
    </owl:ObjectProperty>
    


    <!-- http://bibframe.org/vocab/systemNumber -->

    <owl:ObjectProperty rdf:about="&vocab;systemNumber">
        <rdfs:label>System control number</rdfs:label>
        <rdfs:comment>Control number of a system other than LCCN or NBAN, which Identifies a resource description.</rdfs:comment>
        <rdfs:range rdf:resource="&vocab;Identifier"/>
        <rdfs:subPropertyOf rdf:resource="&vocab;identifier"/>
    </owl:ObjectProperty>
    


    <!-- http://bibframe.org/vocab/tableOfContents -->

    <owl:ObjectProperty rdf:about="&vocab;tableOfContents">
        <rdfs:label>Table of contents content</rdfs:label>
        <rdfs:comment>Table of contents of the target work or instance.</rdfs:comment>
        <rdfs:domain rdf:resource="&vocab;TableOfContents"/>
        <rdfs:subPropertyOf rdf:resource="&vocab;annotationBody"/>
        <rdfs:range rdf:resource="&rdfs;Resource"/>
    </owl:ObjectProperty>
    


    <!-- http://bibframe.org/vocab/tableOfContentsFor -->

    <owl:ObjectProperty rdf:about="&vocab;tableOfContentsFor">
        <rdfs:label>Table of contents of resource</rdfs:label>
        <rdfs:comment>Resource to which the table of contents pertains.</rdfs:comment>
        <rdfs:domain rdf:resource="&vocab;TableOfContents"/>
        <rdfs:subPropertyOf rdf:resource="&vocab;annotates"/>
        <rdfs:range rdf:resource="&rdfs;Resource"/>
    </owl:ObjectProperty>
    


    <!-- http://bibframe.org/vocab/titleVariation -->

    <owl:ObjectProperty rdf:about="&vocab;titleVariation">
        <rdfs:label>Title variation</rdfs:label>
        <rdfs:comment>Title associated with the resource that is different from the main title.</rdfs:comment>
        <rdfs:range rdf:resource="&vocab;Title"/>
    </owl:ObjectProperty>
    


    <!-- http://bibframe.org/vocab/translation -->

    <owl:ObjectProperty rdf:about="&vocab;translation">
        <rdfs:label>Has translation</rdfs:label>
        <rdfs:comment>Work that translates the text of the source entity into a language different from that of the original.</rdfs:comment>
        <rdfs:range rdf:resource="&vocab;Work"/>
        <rdfs:domain rdf:resource="&vocab;Work"/>
    </owl:ObjectProperty>
    


    <!-- http://bibframe.org/vocab/translationOf -->

    <owl:ObjectProperty rdf:about="&vocab;translationOf">
        <rdfs:label>Translation of</rdfs:label>
        <rdfs:comment>Work that has been translated, i.e., the text expressed in a language different from that of the original work).</rdfs:comment>
        <rdfs:range rdf:resource="&vocab;Work"/>
        <rdfs:domain rdf:resource="&vocab;Work"/>
    </owl:ObjectProperty>
    


    <!-- http://bibframe.org/vocab/unionOf -->

    <owl:ObjectProperty rdf:about="&vocab;unionOf">
        <rdfs:label>Union of</rdfs:label>
        <dcterms:modified>2014-04-10 (Updated subproperty)</dcterms:modified>
        <rdfs:comment>One of two or more works which came together to form a new work.</rdfs:comment>
        <rdfs:domain rdf:resource="&vocab;Work"/>
        <rdfs:range rdf:resource="&vocab;Work"/>
    </owl:ObjectProperty>
    


    <!-- http://bibframe.org/vocab/upc -->

    <owl:ObjectProperty rdf:about="&vocab;upc">
        <rdfs:label>UPC</rdfs:label>
        <rdfs:comment>Universal Product Code.</rdfs:comment>
        <rdfs:range rdf:resource="&vocab;Identifier"/>
        <rdfs:domain rdf:resource="&vocab;Instance"/>
        <rdfs:subPropertyOf rdf:resource="&vocab;identifier"/>
    </owl:ObjectProperty>
    


    <!-- http://bibframe.org/vocab/uri -->

    <owl:ObjectProperty rdf:about="&vocab;uri">
        <rdfs:label>URI</rdfs:label>
        <rdfs:comment>Uniform Resource Identifier.</rdfs:comment>
        <rdfs:range rdf:resource="&vocab;Identifier"/>
        <rdfs:subPropertyOf rdf:resource="&vocab;identifier"/>
    </owl:ObjectProperty>
    


    <!-- http://bibframe.org/vocab/urn -->

    <owl:ObjectProperty rdf:about="&vocab;urn">
        <rdfs:label>URN</rdfs:label>
        <rdfs:comment>Uniform Resource Number.</rdfs:comment>
        <rdfs:range rdf:resource="&vocab;Identifier"/>
        <rdfs:domain rdf:resource="&vocab;Instance"/>
        <rdfs:subPropertyOf rdf:resource="&vocab;identifier"/>
    </owl:ObjectProperty>
    


    <!-- http://bibframe.org/vocab/videorecordingNumber -->

    <owl:ObjectProperty rdf:about="&vocab;videorecordingNumber">
        <rdfs:label>Videorecording number</rdfs:label>
        <rdfs:comment>Number assigned by a publisher to a videorecording.</rdfs:comment>
        <rdfs:range rdf:resource="&vocab;Identifier"/>
        <rdfs:domain rdf:resource="&vocab;Instance"/>
        <rdfs:subPropertyOf rdf:resource="&vocab;identifier"/>
    </owl:ObjectProperty>
    


    <!-- http://bibframe.org/vocab/workTitle -->

    <owl:ObjectProperty rdf:about="&vocab;workTitle">
        <rdfs:label>Work title</rdfs:label>
        <rdfs:comment>Title or form of title chosen to identify the work, such as a preferred title, preferred title with additions, uniform title, etc..</rdfs:comment>
        <rdfs:range rdf:resource="&vocab;Title"/>
        <rdfs:domain rdf:resource="&vocab;Work"/>
    </owl:ObjectProperty>
    


    <!-- http://purl.org/dc/terms/format -->

    <owl:ObjectProperty rdf:about="&dcterms;format">
        <rdfs:label xml:lang="en">Format</rdfs:label>
        <dcterms:modified rdf:datatype="&xsd;date">2008-01-14</dcterms:modified>
        <dcterms:issued rdf:datatype="&xsd;date">2008-01-14</dcterms:issued>
        <dcterms:description xml:lang="en">Examples of dimensions include size and duration. Recommended best practice is to use a controlled vocabulary such as the list of Internet Media Types [MIME].</dcterms:description>
        <rdfs:comment xml:lang="en">The file format, physical medium, or dimensions of the resource.</rdfs:comment>
        <dcterms:hasVersion rdf:resource="http://dublincore.org/usage/terms/history/#formatT-001"/>
        <rdfs:isDefinedBy rdf:resource="http://purl.org/dc/terms/"/>
    </owl:ObjectProperty>
    


    <!-- http://schema.org/accessibilityFeature -->

    <owl:ObjectProperty rdf:about="http://schema.org/accessibilityFeature">
        <rdfs:label xml:lang="en">Accessibility Feature</rdfs:label>
        <rdfs:comment xml:lang="en">Content features of the resource, such as accessible media, alternatives and supported enhancements for accessibility (WebSchemas wiki lists possible values).</rdfs:comment>
        <rdfs:isDefinedBy rdf:resource="http://schema.org/CreativeWork"/>
        <rdfs:range rdf:resource="&xsd;string"/>
    </owl:ObjectProperty>
    


    <!-- http://schema.org/audience -->

    <owl:ObjectProperty rdf:about="http://schema.org/audience">
        <rdfs:label xml:lang="en">Audience</rdfs:label>
        <rdfs:comment xml:lang="en">The intended audience of the item, i.e. the group for whom the item was created.</rdfs:comment>
        <rdfs:range rdf:resource="http://schema.org/Audience"/>
        <rdfs:isDefinedBy rdf:resource="http://schema.org/CreativeWork"/>
        <rdfs:isDefinedBy rdf:resource="http://schema.org/PlayAction"/>
        <rdfs:isDefinedBy rdf:resource="http://schema.org/Product"/>
    </owl:ObjectProperty>
    


    <!-- http://schema.org/permitAudience -->

    <owl:ObjectProperty rdf:about="http://schema.org/permitAudience">
        <rdfs:range rdf:resource="http://schema.org/Audience"/>
    </owl:ObjectProperty>
    


    <!-- http://schema.org/serviceAudience -->

    <owl:ObjectProperty rdf:about="http://schema.org/serviceAudience">
        <rdfs:range rdf:resource="http://schema.org/Audience"/>
    </owl:ObjectProperty>
    


    <!-- http://www.w3.org/ns/prov#atLocation -->

    <owl:ObjectProperty rdf:about="&prov;atLocation">
        <rdfs:label>atLocation</rdfs:label>
        <prov:category>expanded</prov:category>
        <rdfs:comment xml:lang="en">The Location of any resource.</rdfs:comment>
        <rdfs:comment>This property has multiple RDFS domains to suit multiple OWL Profiles. See &lt;a href=&quot;#owl-profile&quot;&gt;PROV-O OWL Profile&lt;/a&gt;.</rdfs:comment>
        <prov:editorialNote xml:lang="en">The naming of prov:atLocation parallels prov:atTime, and is not named prov:hadLocation to avoid conflicting with the convention that prov:had* properties are used on prov:Influence classes.</prov:editorialNote>
        <prov:editorialNote xml:lang="en">This property is not functional because the many values could be at a variety of granularies (In this building, in this room, in that chair).</prov:editorialNote>
        <prov:inverse>locationOf</prov:inverse>
        <rdfs:range rdf:resource="&prov;Location"/>
        <prov:sharesDefinitionWith rdf:resource="&prov;Location"/>
        <rdfs:isDefinedBy rdf:resource="http://www.w3.org/ns/prov-o#"/>
        <rdfs:domain>
            <owl:Class>
                <owl:unionOf rdf:parseType="Collection">
                    <rdf:Description rdf:about="&prov;Activity"/>
                    <rdf:Description rdf:about="&prov;Agent"/>
                    <rdf:Description rdf:about="&prov;Entity"/>
                    <rdf:Description rdf:about="&prov;InstantaneousEvent"/>
                </owl:unionOf>
            </owl:Class>
        </rdfs:domain>
    </owl:ObjectProperty>
    


    <!-- http://www.w3.org/ns/prov#locationOf -->

    <owl:ObjectProperty rdf:about="&prov;locationOf">
        <owl:inverseOf rdf:resource="&prov;atLocation"/>
    </owl:ObjectProperty>
    


    <!-- 
    ///////////////////////////////////////////////////////////////////////////////////////
    //
    // Data properties
    //
    ///////////////////////////////////////////////////////////////////////////////////////
     -->

    


    <!-- http://bibframe.org/vocab/accessCondition -->

    <owl:DatatypeProperty rdf:about="&vocab;accessCondition">
        <rdfs:label>Access condition</rdfs:label>
        <rdfs:comment>Allowances and restrictions on access.</rdfs:comment>
        <rdfs:range rdf:resource="&rdfs;Literal"/>
    </owl:DatatypeProperty>
    


    <!-- http://bibframe.org/vocab/aspectRatio -->

    <owl:DatatypeProperty rdf:about="&vocab;aspectRatio">
        <rdfs:label>Aspect ratio</rdfs:label>
        <rdfs:comment>Proportional relationship between an image&apos;s width and its height.</rdfs:comment>
        <rdfs:range rdf:resource="&rdfs;Literal"/>
    </owl:DatatypeProperty>
    


    <!-- http://bibframe.org/vocab/assertionDate -->

    <owl:DatatypeProperty rdf:about="&vocab;assertionDate">
        <rdfs:label>Annotation Assertion Date</rdfs:label>
        <rdfs:comment>Date when annotation was asserted.</rdfs:comment>
        <rdfs:range rdf:resource="&rdfs;Literal"/>
    </owl:DatatypeProperty>
    


    <!-- http://bibframe.org/vocab/audience -->

    <owl:DatatypeProperty rdf:about="&vocab;audience">
        <rdfs:label>Audience</rdfs:label>
        <rdfs:comment>Information that identifies the specific audience or intellectual level for which the content of the resource is considered appropriate.</rdfs:comment>
        <rdfs:range rdf:resource="&rdfs;Literal"/>
    </owl:DatatypeProperty>
    


    <!-- http://bibframe.org/vocab/audienceAssigner -->

    <owl:DatatypeProperty rdf:about="&vocab;audienceAssigner">
        <rdfs:label>Audience assigner</rdfs:label>
        <rdfs:comment>Entity that assigned the intended audience information.</rdfs:comment>
        <rdfs:range rdf:resource="&rdfs;Literal"/>
    </owl:DatatypeProperty>
    


    <!-- http://bibframe.org/vocab/authoritySource -->

    <owl:DatatypeProperty rdf:about="&vocab;authoritySource">
        <rdfs:label>Authority source</rdfs:label>
        <rdfs:comment>Authority list from which a value is taken.</rdfs:comment>
        <rdfs:range rdf:resource="&rdfs;Literal"/>
    </owl:DatatypeProperty>
    


    <!-- http://bibframe.org/vocab/authorizedAccessPoint -->

    <owl:DatatypeProperty rdf:about="&vocab;authorizedAccessPoint">
        <rdfs:label>Authorized access point</rdfs:label>
        <rdfs:comment>Controlled string form of a resource label intended to help uniquely identify it, such as a unique title or a unique name plus title.</rdfs:comment>
        <rdfs:range rdf:resource="&rdfs;Literal"/>
    </owl:DatatypeProperty>
    


    <!-- http://bibframe.org/vocab/awardNote -->

    <owl:DatatypeProperty rdf:about="&vocab;awardNote">
        <rdfs:label>Award note</rdfs:label>
        <rdfs:comment>Information on awards associated with the described resource.</rdfs:comment>
        <rdfs:range rdf:resource="&rdfs;Literal"/>
    </owl:DatatypeProperty>
    


    <!-- http://bibframe.org/vocab/barcode -->

    <owl:DatatypeProperty rdf:about="&vocab;barcode">
        <rdfs:label>Barcode</rdfs:label>
        <rdfs:comment>Identification number of the physical item.</rdfs:comment>
        <rdfs:range rdf:resource="&rdfs;Literal"/>
    </owl:DatatypeProperty>
    


    <!-- http://bibframe.org/vocab/cartographicAscensionAndDeclination -->

    <owl:DatatypeProperty rdf:about="&vocab;cartographicAscensionAndDeclination">
        <rdfs:label>Cartographic ascension and declination</rdfs:label>
        <rdfs:comment>System for identifying the location of a celestial object in the sky covered by the cartographic content of a resource using the angles of right ascension and declination.</rdfs:comment>
        <rdfs:range rdf:resource="&rdfs;Literal"/>
    </owl:DatatypeProperty>
    


    <!-- http://bibframe.org/vocab/cartographicCoordinates -->

    <owl:DatatypeProperty rdf:about="&vocab;cartographicCoordinates">
        <rdfs:label>Cartographic coordinates</rdfs:label>
        <rdfs:comment>Mathematical system for identifying the area covered by the cartographic content of a resource, Expressed either by means of longitude and latitude on the surface of planets or by the angles of right ascension and declination for celestial cartographic content.</rdfs:comment>
        <rdfs:range rdf:resource="&rdfs;Literal"/>
    </owl:DatatypeProperty>
    


    <!-- http://bibframe.org/vocab/cartographicEquinox -->

    <owl:DatatypeProperty rdf:about="&vocab;cartographicEquinox">
        <rdfs:label>Cartographic equinox</rdfs:label>
        <rdfs:comment>One of two points of intersection of the ecliptic and the celestial equator, occupied by the sun when its declination is 0 degrees.</rdfs:comment>
        <rdfs:range rdf:resource="&rdfs;Literal"/>
    </owl:DatatypeProperty>
    


    <!-- http://bibframe.org/vocab/cartographicExclusionGRing -->

    <owl:DatatypeProperty rdf:about="&vocab;cartographicExclusionGRing">
        <rdfs:label>Cartographic G ring area excluded</rdfs:label>
        <rdfs:comment>Coordinate pairs that identify the closed non-intersecting boundary of the area contained within the G-polygon outer ring that is excluded.</rdfs:comment>
        <rdfs:range rdf:resource="&rdfs;Literal"/>
    </owl:DatatypeProperty>
    


    <!-- http://bibframe.org/vocab/cartographicOuterGRing -->

    <owl:DatatypeProperty rdf:about="&vocab;cartographicOuterGRing">
        <rdfs:label>Cartographic outer G ring area covered</rdfs:label>
        <rdfs:comment>Coordinate pairs that identify the closed non-intersecting boundary of the area covered.</rdfs:comment>
        <rdfs:range rdf:resource="&rdfs;Literal"/>
    </owl:DatatypeProperty>
    


    <!-- http://bibframe.org/vocab/cartographicProjection -->

    <owl:DatatypeProperty rdf:about="&vocab;cartographicProjection">
        <rdfs:label>Cartographic projection</rdfs:label>
        <rdfs:comment>Method or system used to represent the surface of the Earth or of a celestial sphere on a plane.</rdfs:comment>
        <rdfs:range rdf:resource="&rdfs;Literal"/>
    </owl:DatatypeProperty>
    


    <!-- http://bibframe.org/vocab/cartographicScale -->

    <owl:DatatypeProperty rdf:about="&vocab;cartographicScale">
        <rdfs:label>Cartographic scale</rdfs:label>
        <rdfs:comment>Ratio of the dimensions of a form contained or embodied in a resource to the dimensions of the entity it represents.</rdfs:comment>
        <rdfs:range rdf:resource="&rdfs;Literal"/>
    </owl:DatatypeProperty>
    


    <!-- http://bibframe.org/vocab/categorySource -->

    <owl:DatatypeProperty rdf:about="&vocab;categorySource">
        <rdfs:label>Category source</rdfs:label>
        <rdfs:comment>Category list from which value is taken.</rdfs:comment>
        <rdfs:range rdf:resource="&rdfs;Literal"/>
    </owl:DatatypeProperty>
    


    <!-- http://bibframe.org/vocab/categoryType -->

    <owl:DatatypeProperty rdf:about="&vocab;categoryType">
        <rdfs:label>Type of category</rdfs:label>
        <rdfs:comment>Type of category recorded, e.g., content, genre, media, form, carrier.</rdfs:comment>
        <rdfs:range rdf:resource="&rdfs;Literal"/>
    </owl:DatatypeProperty>
    


    <!-- http://bibframe.org/vocab/categoryValue -->

    <owl:DatatypeProperty rdf:about="&vocab;categoryValue">
        <rdfs:label>Category</rdfs:label>
        <rdfs:comment>Category code or text.</rdfs:comment>
        <rdfs:range rdf:resource="&rdfs;Literal"/>
    </owl:DatatypeProperty>
    


    <!-- http://bibframe.org/vocab/changeDate -->

    <owl:DatatypeProperty rdf:about="&vocab;changeDate">
        <rdfs:label>Description change date</rdfs:label>
        <rdfs:comment>Date or date and time on which the metadata was modified.</rdfs:comment>
        <rdfs:range rdf:resource="&rdfs;Literal"/>
    </owl:DatatypeProperty>
    


    <!-- http://bibframe.org/vocab/circulationStatus -->

    <owl:DatatypeProperty rdf:about="&vocab;circulationStatus">
        <rdfs:label>Circulation status</rdfs:label>
        <rdfs:comment>Circulation status of an item.</rdfs:comment>
        <rdfs:range rdf:resource="&rdfs;Literal"/>
    </owl:DatatypeProperty>
    


    <!-- http://bibframe.org/vocab/classificationAssigner -->

    <owl:DatatypeProperty rdf:about="&vocab;classificationAssigner">
        <rdfs:label>Institution assigning classification</rdfs:label>
        <rdfs:comment>Entity that assigned the classification number.</rdfs:comment>
        <rdfs:range rdf:resource="&rdfs;Literal"/>
    </owl:DatatypeProperty>
    


    <!-- http://bibframe.org/vocab/classificationDesignation -->

    <owl:DatatypeProperty rdf:about="&vocab;classificationDesignation">
        <rdfs:label>Classification designation</rdfs:label>
        <rdfs:comment>Designates whether the classification number contained in the field is from the standard or optional part of the schedules or tables.</rdfs:comment>
        <rdfs:range rdf:resource="&rdfs;Literal"/>
    </owl:DatatypeProperty>
    


    <!-- http://bibframe.org/vocab/classificationEdition -->

    <owl:DatatypeProperty rdf:about="&vocab;classificationEdition">
        <rdfs:label>Classification scheme edition</rdfs:label>
        <rdfs:comment>Edition of the classification scheme, such as full, abridged or a number, when a classification scheme designates editions.</rdfs:comment>
        <dcterms:modified>2014-10-09 (Updated)</dcterms:modified>
        <rdfs:range rdf:resource="&rdfs;Literal"/>
    </owl:DatatypeProperty>
    


    <!-- http://bibframe.org/vocab/classificationItem -->

    <owl:DatatypeProperty rdf:about="&vocab;classificationItem">
        <rdfs:label>Classification item number</rdfs:label>
        <rdfs:comment>Number attached to a classification number that indicates a particular item.</rdfs:comment>
        <rdfs:range rdf:resource="&rdfs;Literal"/>
    </owl:DatatypeProperty>
    


    <!-- http://bibframe.org/vocab/classificationNumber -->

    <owl:DatatypeProperty rdf:about="&vocab;classificationNumber">
        <rdfs:label>Classification number</rdfs:label>
        <rdfs:comment>Classification number (single class number or beginning number of a span) that indicates the subject by applying a formal system of coding and organizing resources.</rdfs:comment>
        <rdfs:range rdf:resource="&rdfs;Literal"/>
    </owl:DatatypeProperty>
    


    <!-- http://bibframe.org/vocab/classificationScheme -->

    <owl:DatatypeProperty rdf:about="&vocab;classificationScheme">
        <rdfs:label>Classification scheme</rdfs:label>
        <rdfs:comment>Formal scheme from which a classification number is taken.</rdfs:comment>
        <rdfs:range rdf:resource="&rdfs;Literal"/>
    </owl:DatatypeProperty>
    


    <!-- http://bibframe.org/vocab/classificationSpanEnd -->

    <owl:DatatypeProperty rdf:about="&vocab;classificationSpanEnd">
        <rdfs:label>Classification number span end</rdfs:label>
        <rdfs:comment>Ending number of classification number span.</rdfs:comment>
        <rdfs:range rdf:resource="&rdfs;Literal"/>
    </owl:DatatypeProperty>
    


    <!-- http://bibframe.org/vocab/classificationStatus -->

    <owl:DatatypeProperty rdf:about="&vocab;classificationStatus">
        <rdfs:label>Classification status</rdfs:label>
        <rdfs:comment>Indicator that the classification number is canceled or invalid.</rdfs:comment>
        <rdfs:range rdf:resource="&rdfs;Literal"/>
    </owl:DatatypeProperty>
    


    <!-- http://bibframe.org/vocab/classificationTable -->

    <owl:DatatypeProperty rdf:about="&vocab;classificationTable">
        <rdfs:label>Classification table identification</rdfs:label>
        <rdfs:comment>DDC Table identification. Number of the table from which the classification number in a subdivision record is taken.</rdfs:comment>
        <rdfs:range rdf:resource="&rdfs;Literal"/>
    </owl:DatatypeProperty>
    


    <!-- http://bibframe.org/vocab/classificationTableSeq -->

    <owl:DatatypeProperty rdf:about="&vocab;classificationTableSeq">
        <rdfs:label>Classification table sequence number</rdfs:label>
        <rdfs:comment>Sequence number or other identifier for an internal classification subarrangement or add in a classification scheme.</rdfs:comment>
        <rdfs:range rdf:resource="&rdfs;Literal"/>
    </owl:DatatypeProperty>
    


    <!-- http://bibframe.org/vocab/colorContent -->

    <owl:DatatypeProperty rdf:about="&vocab;colorContent">
        <rdfs:label>Color content</rdfs:label>
        <rdfs:comment>Color characteristics, e.g. black and white, multicolored, etc.</rdfs:comment>
        <dcterms:modified>2014-10-14 (Updated)</dcterms:modified>
        <rdfs:range rdf:resource="&rdfs;Literal"/>
    </owl:DatatypeProperty>
    


    <!-- http://bibframe.org/vocab/contentAccessibility -->

    <owl:DatatypeProperty rdf:about="&vocab;contentAccessibility">
        <rdfs:label>Content accessibility note</rdfs:label>
        <rdfs:comment>Content that assists those with a sensory impairment for greater understanding of content, e.g., labels, captions.</rdfs:comment>
        <rdfs:range rdf:resource="&rdfs;Literal"/>
    </owl:DatatypeProperty>
    


    <!-- http://bibframe.org/vocab/contentsNote -->

    <owl:DatatypeProperty rdf:about="&vocab;contentsNote">
        <rdfs:label>Contents</rdfs:label>
        <rdfs:comment>List of subunits of the resource.</rdfs:comment>
        <rdfs:range rdf:resource="&rdfs;Literal"/>
    </owl:DatatypeProperty>
    


    <!-- http://bibframe.org/vocab/copyNote -->

    <owl:DatatypeProperty rdf:about="&vocab;copyNote">
        <rdfs:label>Copy note</rdfs:label>
        <rdfs:comment>Information about this copy.</rdfs:comment>
        <rdfs:range rdf:resource="&rdfs;Literal"/>
    </owl:DatatypeProperty>
    


    <!-- http://bibframe.org/vocab/copyrightDate -->

    <owl:DatatypeProperty rdf:about="&vocab;copyrightDate">
        <rdfs:label>Copyright date</rdfs:label>
        <rdfs:comment>Date associated with a claim of protection under copyright or a similar regime.</rdfs:comment>
        <rdfs:range rdf:resource="&rdfs;Literal"/>
    </owl:DatatypeProperty>
    


    <!-- http://bibframe.org/vocab/creationDate -->

    <owl:DatatypeProperty rdf:about="&vocab;creationDate">
        <rdfs:label>Description creation date</rdfs:label>
        <rdfs:comment>Date or date and time on which the original metadata first created.</rdfs:comment>
        <rdfs:range rdf:resource="&rdfs;Literal"/>
    </owl:DatatypeProperty>
    


    <!-- http://bibframe.org/vocab/creditsNote -->

    <owl:DatatypeProperty rdf:about="&vocab;creditsNote">
        <rdfs:label>Credits note</rdfs:label>
        <rdfs:comment>Credits for persons or organizations, other than members of the cast, who have participated in the creation and/or production of the.</rdfs:comment>
        <rdfs:range rdf:resource="&rdfs;Literal"/>
    </owl:DatatypeProperty>
    


    <!-- http://bibframe.org/vocab/custodialHistory -->

    <owl:DatatypeProperty rdf:about="&vocab;custodialHistory">
        <rdfs:label>Custodial history</rdfs:label>
        <rdfs:comment>Information about the provenance, such as origin, ownership and custodial history (chain of custody), of a resource.</rdfs:comment>
        <rdfs:range rdf:resource="&rdfs;Literal"/>
    </owl:DatatypeProperty>
    


    <!-- http://bibframe.org/vocab/descriptionAuthentication -->

    <owl:DatatypeProperty rdf:about="&vocab;descriptionAuthentication">
        <rdfs:label>Description authentication</rdfs:label>
        <rdfs:comment>Indication of specific types of reviews of description information.</rdfs:comment>
        <dcterms:modified>2014-10-27 (Updated)</dcterms:modified>
        <rdfs:range rdf:resource="&rdfs;Literal"/>
    </owl:DatatypeProperty>
    


    <!-- http://bibframe.org/vocab/descriptionStatus -->

    <owl:DatatypeProperty rdf:about="&vocab;descriptionStatus">
        <rdfs:label>Description status</rdfs:label>
        <rdfs:comment>Indicaton of whether the description is new or revised or in other states.</rdfs:comment>
        <dcterms:modified>2014-10-27 (Updated)</dcterms:modified>
        <rdfs:range rdf:resource="&rdfs;Literal"/>
    </owl:DatatypeProperty>
    


    <!-- http://bibframe.org/vocab/dimensions -->

    <owl:DatatypeProperty rdf:about="&vocab;dimensions">
        <rdfs:label>Dimensions</rdfs:label>
        <rdfs:comment>Measurements of the carrier or carriers and/or the container of a resource.</rdfs:comment>
        <rdfs:range rdf:resource="&rdfs;Literal"/>
    </owl:DatatypeProperty>
    


    <!-- http://bibframe.org/vocab/dissertationDegree -->

    <owl:DatatypeProperty rdf:about="&vocab;dissertationDegree">
        <rdfs:label>Degree</rdfs:label>
        <rdfs:comment>Degree for which author was a candidate.</rdfs:comment>
        <rdfs:range rdf:resource="&rdfs;Literal"/>
    </owl:DatatypeProperty>
    


    <!-- http://bibframe.org/vocab/dissertationNote -->

    <owl:DatatypeProperty rdf:about="&vocab;dissertationNote">
        <rdfs:label>Dissertation note</rdfs:label>
        <rdfs:comment>Textual information about the dissertation.</rdfs:comment>
        <rdfs:range rdf:resource="&rdfs;Literal"/>
    </owl:DatatypeProperty>
    


    <!-- http://bibframe.org/vocab/dissertationYear -->

    <owl:DatatypeProperty rdf:about="&vocab;dissertationYear">
        <rdfs:label>Year degree awarded</rdfs:label>
        <rdfs:comment>Year degree awarded.</rdfs:comment>
        <rdfs:range rdf:resource="&rdfs;Literal"/>
    </owl:DatatypeProperty>
    


    <!-- http://bibframe.org/vocab/duration -->

    <owl:DatatypeProperty rdf:about="&vocab;duration">
        <rdfs:label>Duration</rdfs:label>
        <rdfs:comment>Information about the playing time or duration in an unstructured form, e.g., &quot;2 hours&quot;.</rdfs:comment>
        <rdfs:range rdf:resource="&rdfs;Literal"/>
    </owl:DatatypeProperty>
    


    <!-- http://bibframe.org/vocab/edition -->

    <owl:DatatypeProperty rdf:about="&vocab;edition">
        <rdfs:label>Edition statement</rdfs:label>
        <rdfs:comment>Information identifying the edition or version of the resource.</rdfs:comment>
        <rdfs:range rdf:resource="&rdfs;Literal"/>
    </owl:DatatypeProperty>
    


    <!-- http://bibframe.org/vocab/editionResponsibility -->

    <owl:DatatypeProperty rdf:about="&vocab;editionResponsibility">
        <rdfs:label>Edition responsibility</rdfs:label>
        <rdfs:comment>Statement relating to the identification of any persons, families, or corporate bodies responsible for the edition being described.</rdfs:comment>
        <rdfs:range rdf:resource="&rdfs;Literal"/>
    </owl:DatatypeProperty>
    


    <!-- http://bibframe.org/vocab/enumerationAndChronology -->

    <owl:DatatypeProperty rdf:about="&vocab;enumerationAndChronology">
        <rdfs:label>Enumeration and chronology</rdfs:label>
        <rdfs:comment>Numbering and dates of holding.</rdfs:comment>
        <rdfs:range rdf:resource="&rdfs;Literal"/>
    </owl:DatatypeProperty>
    


    <!-- http://bibframe.org/vocab/eventDate -->

    <owl:DatatypeProperty rdf:about="&vocab;eventDate">
        <rdfs:label>Date(s) of event</rdfs:label>
        <rdfs:comment>Date, time or period of event.</rdfs:comment>
        <dcterms:modified>2014-05-16 (Updated)</dcterms:modified>
        <rdfs:range rdf:resource="&rdfs;Literal"/>
    </owl:DatatypeProperty>
    


    <!-- http://bibframe.org/vocab/extent -->

    <owl:DatatypeProperty rdf:about="&vocab;extent">
        <rdfs:label>Extent</rdfs:label>
        <rdfs:comment>Number and type of units and/or subunits making up a resource.</rdfs:comment>
        <rdfs:range rdf:resource="&rdfs;Literal"/>
    </owl:DatatypeProperty>
    


    <!-- http://bibframe.org/vocab/findingAidNote -->

    <owl:DatatypeProperty rdf:about="&vocab;findingAidNote">
        <rdfs:label>Index or finding aid note</rdfs:label>
        <rdfs:comment>Note about availability of an index or finding aid.</rdfs:comment>
        <rdfs:range rdf:resource="&rdfs;Literal"/>
    </owl:DatatypeProperty>
    


    <!-- http://bibframe.org/vocab/formDesignation -->

    <owl:DatatypeProperty rdf:about="&vocab;formDesignation">
        <rdfs:label>Form designation</rdfs:label>
        <rdfs:comment>Class or genre to which a Work or Instance belongs.</rdfs:comment>
        <dcterms:modified>2014-03-21 (Range updated)</dcterms:modified>
        <rdfs:range rdf:resource="&rdfs;Literal"/>
    </owl:DatatypeProperty>
    


    <!-- http://bibframe.org/vocab/format -->

    <owl:DatatypeProperty rdf:about="&vocab;format">
        <rdfs:label>Format</rdfs:label>
        <dcterms:modified>2014-10-27 (Updated)</dcterms:modified>
        <rdfs:comment>File format or physical medium of an instance.</rdfs:comment>
        <rdfs:range rdf:resource="&rdfs;Literal"/>
    </owl:DatatypeProperty>
    


    <!-- http://bibframe.org/vocab/formatOfMusic -->

    <owl:DatatypeProperty rdf:about="&vocab;formatOfMusic">
        <rdfs:label>Format of music</rdfs:label>
        <rdfs:comment>Format of a musical composition, e.g. full score, condensed score, vocal score, etc.</rdfs:comment>
        <rdfs:range rdf:resource="&rdfs;Literal"/>
    </owl:DatatypeProperty>
    


    <!-- http://bibframe.org/vocab/frequency -->

    <owl:DatatypeProperty rdf:about="&vocab;frequency">
        <rdfs:label>Frequency</rdfs:label>
        <rdfs:comment>Intervals at which the issues or parts of a serial or the updates to an integrating resource are issued.</rdfs:comment>
        <rdfs:range rdf:resource="&rdfs;Literal"/>
    </owl:DatatypeProperty>
    


    <!-- http://bibframe.org/vocab/frequencyNote -->

    <owl:DatatypeProperty rdf:about="&vocab;frequencyNote">
        <rdfs:label>Frequency note</rdfs:label>
        <rdfs:comment>Current or former publication frequency of a resource.</rdfs:comment>
        <rdfs:range rdf:resource="&rdfs;Literal"/>
    </owl:DatatypeProperty>
    


    <!-- http://bibframe.org/vocab/generationDate -->

    <owl:DatatypeProperty rdf:about="&vocab;generationDate">
        <rdfs:label>Date generated</rdfs:label>
        <dcterms:modified>2014-10-27 (Updated)</dcterms:modified>
        <rdfs:comment>Date of conversion of the data from another format.</rdfs:comment>
        <rdfs:range rdf:resource="&rdfs;Literal"/>
    </owl:DatatypeProperty>
    


    <!-- http://bibframe.org/vocab/generationProcess -->

    <owl:DatatypeProperty rdf:about="&vocab;generationProcess">
        <rdfs:label>Description generation</rdfs:label>
        <rdfs:comment>Indication of the program or process used to generate the description by application of a particular transformation.</rdfs:comment>
        <dcterms:modified>2014-10-27 (Updated)</dcterms:modified>
        <rdfs:range rdf:resource="&rdfs;Literal"/>
    </owl:DatatypeProperty>
    


    <!-- http://bibframe.org/vocab/geographicCoverageNote -->

    <owl:DatatypeProperty rdf:about="&vocab;geographicCoverageNote">
        <rdfs:label>Geographic coverage</rdfs:label>
        <rdfs:comment>Geographic entities covered by the resource.</rdfs:comment>
        <rdfs:range rdf:resource="&rdfs;Literal"/>
    </owl:DatatypeProperty>
    


    <!-- http://bibframe.org/vocab/graphicScaleNote -->

    <owl:DatatypeProperty rdf:about="&vocab;graphicScaleNote">
        <rdfs:label>Graphic scale</rdfs:label>
        <rdfs:comment>Textual information about scale, including the scale of graphic material item such as architectural drawings or three-dimensional artifacts.</rdfs:comment>
        <rdfs:range rdf:resource="&rdfs;Literal"/>
    </owl:DatatypeProperty>
    


    <!-- http://bibframe.org/vocab/identifierAssigner -->

    <owl:DatatypeProperty rdf:about="&vocab;identifierAssigner">
        <rdfs:label>Identifier assigner</rdfs:label>
        <rdfs:comment>Entity that assigned the identifier.</rdfs:comment>
        <rdfs:range rdf:resource="&rdfs;Literal"/>
    </owl:DatatypeProperty>
    


    <!-- http://bibframe.org/vocab/identifierQualifier -->

    <owl:DatatypeProperty rdf:about="&vocab;identifierQualifier">
        <rdfs:label>Identifier qualifier</rdfs:label>
        <rdfs:comment>Qualifying information associated with the identifier, e.g. specifying its applicability.</rdfs:comment>
        <rdfs:range rdf:resource="&rdfs;Literal"/>
    </owl:DatatypeProperty>
    


    <!-- http://bibframe.org/vocab/identifierStatus -->

    <owl:DatatypeProperty rdf:about="&vocab;identifierStatus">
        <rdfs:label>Identifier status</rdfs:label>
        <rdfs:comment>Indication of whether the identifier is canceled or invalid.</rdfs:comment>
        <rdfs:range rdf:resource="&rdfs;Literal"/>
    </owl:DatatypeProperty>
    


    <!-- http://bibframe.org/vocab/identifierValue -->

    <owl:DatatypeProperty rdf:about="&vocab;identifierValue">
        <rdfs:label>Identifier value</rdfs:label>
        <rdfs:comment>Value of the identifier.</rdfs:comment>
        <rdfs:range rdf:resource="&rdfs;Literal"/>
    </owl:DatatypeProperty>
    


    <!-- http://bibframe.org/vocab/illustrationNote -->

    <owl:DatatypeProperty rdf:about="&vocab;illustrationNote">
        <rdfs:label>Illustrative content note</rdfs:label>
        <rdfs:comment>Information about illustrative material in the resource.</rdfs:comment>
        <rdfs:range rdf:resource="&rdfs;Literal"/>
    </owl:DatatypeProperty>
    


    <!-- http://bibframe.org/vocab/immediateAcquisition -->

    <owl:DatatypeProperty rdf:about="&vocab;immediateAcquisition">
        <rdfs:label>Immediate acquisition</rdfs:label>
        <rdfs:comment>Information about the circumstances (e.g., source, date, method) under which the resource was directly acquired.</rdfs:comment>
        <rdfs:range rdf:resource="&rdfs;Literal"/>
    </owl:DatatypeProperty>
    


    <!-- http://bibframe.org/vocab/itemId -->

    <owl:DatatypeProperty rdf:about="&vocab;itemId">
        <rdfs:label>System item identifier</rdfs:label>
        <rdfs:comment>Identification number assigned to data about one item held.</rdfs:comment>
        <rdfs:range rdf:resource="&rdfs;Literal"/>
    </owl:DatatypeProperty>
    


    <!-- http://bibframe.org/vocab/label -->

    <owl:DatatypeProperty rdf:about="&vocab;label">
        <rdfs:label>Label</rdfs:label>
        <rdfs:comment>Text string expressing the property value.</rdfs:comment>
        <rdfs:range rdf:resource="&rdfs;Literal"/>
    </owl:DatatypeProperty>
    


    <!-- http://bibframe.org/vocab/languageNote -->

    <owl:DatatypeProperty rdf:about="&vocab;languageNote">
        <rdfs:label>Language note</rdfs:label>
        <rdfs:comment>Note concerning the language of the material or its parts.</rdfs:comment>
        <rdfs:range rdf:resource="&rdfs;Literal"/>
    </owl:DatatypeProperty>
    


    <!-- http://bibframe.org/vocab/languageOfPart -->

    <owl:DatatypeProperty rdf:about="&vocab;languageOfPart">
        <rdfs:label>Language of part</rdfs:label>
        <rdfs:comment>Language or notation system used to convey the content of the resource (associated with part or all of a resource).</rdfs:comment>
        <rdfs:range rdf:resource="&rdfs;Literal"/>
    </owl:DatatypeProperty>
    


    <!-- http://bibframe.org/vocab/languageSource -->

    <owl:DatatypeProperty rdf:about="&vocab;languageSource">
        <rdfs:label>Language source</rdfs:label>
        <rdfs:comment>Language code or name list from which value is taken.</rdfs:comment>
        <rdfs:range rdf:resource="&rdfs;Literal"/>
    </owl:DatatypeProperty>
    


    <!-- http://bibframe.org/vocab/legalDate -->

    <owl:DatatypeProperty rdf:about="&vocab;legalDate">
        <rdfs:label>Date of legal work</rdfs:label>
        <rdfs:comment>Date of legal work, or promulgation of a law, or signing of a treaty.</rdfs:comment>
        <rdfs:range rdf:resource="&rdfs;Literal"/>
    </owl:DatatypeProperty>
    


    <!-- http://bibframe.org/vocab/lendingPolicy -->

    <owl:DatatypeProperty rdf:about="&vocab;lendingPolicy">
        <rdfs:label>Lending policy</rdfs:label>
        <rdfs:comment>Policy statement about whether and with what restrictions the holding may be lent</rdfs:comment>
        <rdfs:range rdf:resource="&rdfs;Literal"/>
    </owl:DatatypeProperty>
    


    <!-- http://bibframe.org/vocab/materialArrangement -->

    <owl:DatatypeProperty rdf:about="&vocab;materialArrangement">
        <rdfs:label>Arrangement of material</rdfs:label>
        <rdfs:comment>Pattern of arrangement of materials within a unit.</rdfs:comment>
        <rdfs:range rdf:resource="&rdfs;Literal"/>
    </owl:DatatypeProperty>
    


    <!-- http://bibframe.org/vocab/materialHierarchicalLevel -->

    <owl:DatatypeProperty rdf:about="&vocab;materialHierarchicalLevel">
        <rdfs:label>Hierarchical level of material</rdfs:label>
        <rdfs:comment>Hierarchical position of the described materials relative to other material from the same source.</rdfs:comment>
        <rdfs:range rdf:resource="&rdfs;Literal"/>
    </owl:DatatypeProperty>
    


    <!-- http://bibframe.org/vocab/materialOrganization -->

    <owl:DatatypeProperty rdf:about="&vocab;materialOrganization">
        <rdfs:label>Organization of material</rdfs:label>
        <rdfs:comment>Manner in which resource is divided into smaller units.</rdfs:comment>
        <rdfs:range rdf:resource="&rdfs;Literal"/>
    </owl:DatatypeProperty>
    


    <!-- http://bibframe.org/vocab/materialPart -->

    <owl:DatatypeProperty rdf:about="&vocab;materialPart">
        <rdfs:label>Part of material</rdfs:label>
        <rdfs:comment>Part of the resource to which information applies.</rdfs:comment>
        <rdfs:range rdf:resource="&rdfs;Literal"/>
    </owl:DatatypeProperty>
    


    <!-- http://bibframe.org/vocab/modeOfIssuance -->

    <owl:DatatypeProperty rdf:about="&vocab;modeOfIssuance">
        <rdfs:label>Mode of issuance</rdfs:label>
        <rdfs:comment>Categorization reflecting whether a resource is issued in one or more parts, the way it is updated, and its intended termination.</rdfs:comment>
        <rdfs:range rdf:resource="&rdfs;Literal"/>
    </owl:DatatypeProperty>
    


    <!-- http://bibframe.org/vocab/musicKey -->

    <owl:DatatypeProperty rdf:about="&vocab;musicKey">
        <rdfs:label>Music Key</rdfs:label>
        <rdfs:comment>Pitch and mode for music.</rdfs:comment>
        <rdfs:range rdf:resource="&rdfs;Literal"/>
    </owl:DatatypeProperty>
    


    <!-- http://bibframe.org/vocab/musicMediumNote -->

    <owl:DatatypeProperty rdf:about="&vocab;musicMediumNote">
        <rdfs:label>Music medium note</rdfs:label>
        <rdfs:comment>Instrumental, vocal, and/or other medium of performance for which a musical resource was originally conceived, written or performed.</rdfs:comment>
        <rdfs:range rdf:resource="&rdfs;Literal"/>
    </owl:DatatypeProperty>
    


    <!-- http://bibframe.org/vocab/musicNumber -->

    <owl:DatatypeProperty rdf:about="&vocab;musicNumber">
        <rdfs:label>Music number</rdfs:label>
        <rdfs:comment>Serial, opus, or thematic number or code for music.</rdfs:comment>
        <rdfs:range rdf:resource="&rdfs;Literal"/>
    </owl:DatatypeProperty>
    


    <!-- http://bibframe.org/vocab/musicVersion -->

    <owl:DatatypeProperty rdf:about="&vocab;musicVersion">
        <rdfs:label>Music version</rdfs:label>
        <dcterms:modified>2014-06-19 (Example Added)</dcterms:modified>
        <rdfs:comment>Versions such as arrangements, transcriptions, etc. of music.</rdfs:comment>
        <rdfs:range rdf:resource="&rdfs;Literal"/>
    </owl:DatatypeProperty>
    


    <!-- http://bibframe.org/vocab/notation -->

    <owl:DatatypeProperty rdf:about="&vocab;notation">
        <rdfs:label>Notation system</rdfs:label>
        <rdfs:comment>Information on the alphabet, script, or symbol system used to convey the content of the resource, including specialized scripts, typefaces, tactile notation, and musical notation.</rdfs:comment>
        <rdfs:range rdf:resource="&rdfs;Literal"/>
    </owl:DatatypeProperty>
    


    <!-- http://bibframe.org/vocab/note -->

    <owl:DatatypeProperty rdf:about="&vocab;note">
        <rdfs:label>Note</rdfs:label>
        <rdfs:comment>General textual information relating to a resource.</rdfs:comment>
        <dcterms:modified>2014-10-14 (Updated)</dcterms:modified>
        <rdfs:range rdf:resource="&rdfs;Literal"/>
    </owl:DatatypeProperty>
    


    <!-- http://bibframe.org/vocab/originDate -->

    <owl:DatatypeProperty rdf:about="&vocab;originDate">
        <rdfs:label>Associated title date</rdfs:label>
        <dcterms:modified>2014-07-23 (Example added)</dcterms:modified>
        <rdfs:comment>Date or date range associated with the creation of the work.</rdfs:comment>
        <rdfs:range rdf:resource="&rdfs;Literal"/>
    </owl:DatatypeProperty>
    


    <!-- http://bibframe.org/vocab/partNumber -->

    <owl:DatatypeProperty rdf:about="&vocab;partNumber">
        <rdfs:label>Part number</rdfs:label>
        <rdfs:comment>Part or section number of a title.</rdfs:comment>
        <rdfs:range rdf:resource="&rdfs;Literal"/>
    </owl:DatatypeProperty>
    


    <!-- http://bibframe.org/vocab/partTitle -->

    <owl:DatatypeProperty rdf:about="&vocab;partTitle">
        <rdfs:label>Part title</rdfs:label>
        <rdfs:comment>Part or section name of a title.</rdfs:comment>
        <rdfs:range rdf:resource="&rdfs;Literal"/>
    </owl:DatatypeProperty>
    


    <!-- http://bibframe.org/vocab/performerNote -->

    <owl:DatatypeProperty rdf:about="&vocab;performerNote">
        <rdfs:label>Performer note</rdfs:label>
        <rdfs:comment>Information about the participants, players, narrators, presenters, or performers.</rdfs:comment>
        <rdfs:range rdf:resource="&rdfs;Literal"/>
    </owl:DatatypeProperty>
    


    <!-- http://bibframe.org/vocab/preferredCitation -->

    <owl:DatatypeProperty rdf:about="&vocab;preferredCitation">
        <rdfs:label>Preferred citation</rdfs:label>
        <rdfs:comment>Citation to the resource preferred by its custodian.</rdfs:comment>
        <rdfs:range rdf:resource="&rdfs;Literal"/>
    </owl:DatatypeProperty>
    


    <!-- http://bibframe.org/vocab/providerDate -->

    <owl:DatatypeProperty rdf:about="&vocab;providerDate">
        <rdfs:label>Provider date</rdfs:label>
        <rdfs:comment>Date associated with the publication, printing, distribution, issue, release or production of the instance.</rdfs:comment>
        <rdfs:range rdf:resource="&rdfs;Literal"/>
    </owl:DatatypeProperty>
    


    <!-- http://bibframe.org/vocab/providerRole -->

    <owl:DatatypeProperty rdf:about="&vocab;providerRole">
        <rdfs:label>Provider role</rdfs:label>
        <rdfs:comment>The type of role played by the provider of an instance, e.g. production, publication, manufacture, distribution.</rdfs:comment>
        <rdfs:range rdf:resource="&rdfs;Literal"/>
    </owl:DatatypeProperty>
    


    <!-- http://bibframe.org/vocab/providerStatement -->

    <owl:DatatypeProperty rdf:about="&vocab;providerStatement">
        <rdfs:label>Provider statement</rdfs:label>
        <rdfs:comment>Transcribed provider statement</rdfs:comment>
        <rdfs:range rdf:resource="&rdfs;Literal"/>
    </owl:DatatypeProperty>
    


    <!-- http://bibframe.org/vocab/relatorRole -->

    <owl:DatatypeProperty rdf:about="&vocab;relatorRole">
        <rdfs:label>Agent role</rdfs:label>
        <rdfs:comment>Specific role of agent.</rdfs:comment>
        <dcterms:modified>2014-04-30 (New)</dcterms:modified>
        <rdfs:range rdf:resource="&rdfs;Literal"/>
    </owl:DatatypeProperty>
    


    <!-- http://bibframe.org/vocab/reproductionPolicy -->

    <owl:DatatypeProperty rdf:about="&vocab;reproductionPolicy">
        <rdfs:label>Reproduction policy</rdfs:label>
        <rdfs:comment>Policy statement about whether reproductions of the holding can be made</rdfs:comment>
        <dcterms:modified>2014-10-21 (Added)</dcterms:modified>
        <rdfs:range rdf:resource="&rdfs;Literal"/>
    </owl:DatatypeProperty>
    


    <!-- http://bibframe.org/vocab/resourcePart -->

    <owl:DatatypeProperty rdf:about="&vocab;resourcePart">
        <rdfs:label>Resource part</rdfs:label>
        <rdfs:comment>Part of a resource for which language is being indicated.</rdfs:comment>
        <rdfs:range rdf:resource="&rdfs;Literal"/>
    </owl:DatatypeProperty>
    


    <!-- http://bibframe.org/vocab/responsibilityStatement -->

    <owl:DatatypeProperty rdf:about="&vocab;responsibilityStatement">
        <rdfs:label>Edition responsibility</rdfs:label>
        <rdfs:comment>Statement relating to the identification and/or function of any persons, families, or corporate bodies responsible for the creation of, or contributing to the content of a resource.</rdfs:comment>
        <rdfs:range rdf:resource="&rdfs;Literal"/>
    </owl:DatatypeProperty>
    


    <!-- http://bibframe.org/vocab/retentionPolicy -->

    <owl:DatatypeProperty rdf:about="&vocab;retentionPolicy">
        <rdfs:label>Retention policy</rdfs:label>
        <rdfs:comment>Policy statement about how many and/or how long the holdings are retained</rdfs:comment>
        <dcterms:modified>2014-10-21 (Added)</dcterms:modified>
        <rdfs:range rdf:resource="&rdfs;Literal"/>
    </owl:DatatypeProperty>
    


    <!-- http://bibframe.org/vocab/serialFirstIssue -->

    <owl:DatatypeProperty rdf:about="&vocab;serialFirstIssue">
        <rdfs:label>Serial first issue</rdfs:label>
        <rdfs:comment>Beginning date of an instance and/or the sequential designations.</rdfs:comment>
        <rdfs:range rdf:resource="&rdfs;Literal"/>
    </owl:DatatypeProperty>
    


    <!-- http://bibframe.org/vocab/serialLastIssue -->

    <owl:DatatypeProperty rdf:about="&vocab;serialLastIssue">
        <rdfs:label>Serial last issue</rdfs:label>
        <rdfs:comment>Ending date of an instance and/or the sequential designations.</rdfs:comment>
        <rdfs:range rdf:resource="&rdfs;Literal"/>
    </owl:DatatypeProperty>
    


    <!-- http://bibframe.org/vocab/shelfMark -->

    <owl:DatatypeProperty rdf:about="&vocab;shelfMark">
        <rdfs:label>Shelf Location</rdfs:label>
        <rdfs:comment>Physical location, such as a call number or a special shelf/location indicator.</rdfs:comment>
        <rdfs:range rdf:resource="&rdfs;Literal"/>
    </owl:DatatypeProperty>
    


    <!-- http://bibframe.org/vocab/shelfMarkDdc -->

    <owl:DatatypeProperty rdf:about="&vocab;shelfMarkDdc">
        <rdfs:label>DDC call number</rdfs:label>
        <rdfs:comment>Shelf mark based on Dewey Decimal Classification.</rdfs:comment>
        <rdfs:range rdf:resource="&rdfs;Literal"/>
    </owl:DatatypeProperty>
    


    <!-- http://bibframe.org/vocab/shelfMarkLcc -->

    <owl:DatatypeProperty rdf:about="&vocab;shelfMarkLcc">
        <rdfs:label>LCC call number</rdfs:label>
        <rdfs:comment>Shelf mark based on Library of Congress Classification.</rdfs:comment>
        <rdfs:range rdf:resource="&rdfs;Literal"/>
    </owl:DatatypeProperty>
    


    <!-- http://bibframe.org/vocab/shelfMarkNlm -->

    <owl:DatatypeProperty rdf:about="&vocab;shelfMarkNlm">
        <rdfs:label>NLM call number</rdfs:label>
        <rdfs:comment>Shelf mark based on National Library of Medicine Classification.</rdfs:comment>
        <rdfs:range rdf:resource="&rdfs;Literal"/>
    </owl:DatatypeProperty>
    


    <!-- http://bibframe.org/vocab/shelfMarkScheme -->

    <owl:DatatypeProperty rdf:about="&vocab;shelfMarkScheme">
        <rdfs:label>Shelf mark scheme</rdfs:label>
        <rdfs:comment>Scheme from which a shelf mark is taken.</rdfs:comment>
        <rdfs:range rdf:resource="&rdfs;Literal"/>
    </owl:DatatypeProperty>
    


    <!-- http://bibframe.org/vocab/shelfMarkUdc -->

    <owl:DatatypeProperty rdf:about="&vocab;shelfMarkUdc">
        <rdfs:label>UDC call number</rdfs:label>
        <rdfs:comment>Shelf mark based on Universal Decimal Classification.</rdfs:comment>
        <rdfs:range rdf:resource="&rdfs;Literal"/>
    </owl:DatatypeProperty>
    


    <!-- http://bibframe.org/vocab/soundContent -->

    <owl:DatatypeProperty rdf:about="&vocab;soundContent">
        <rdfs:label>Sound content</rdfs:label>
        <rdfs:comment>Indication of whether the production of sound is an integral part of the resource.</rdfs:comment>
        <rdfs:range rdf:resource="&rdfs;Literal"/>
    </owl:DatatypeProperty>
    


    <!-- http://bibframe.org/vocab/startOfReview -->

    <owl:DatatypeProperty rdf:about="&vocab;startOfReview">
        <rdfs:label>Review beginning</rdfs:label>
        <rdfs:comment>First part of review.</rdfs:comment>
        <rdfs:range rdf:resource="&rdfs;Literal"/>
    </owl:DatatypeProperty>
    


    <!-- http://bibframe.org/vocab/startOfSummary -->

    <owl:DatatypeProperty rdf:about="&vocab;startOfSummary">
        <rdfs:label>Summary beginning</rdfs:label>
        <rdfs:comment>First part of description.</rdfs:comment>
        <rdfs:range rdf:resource="&rdfs;Literal"/>
    </owl:DatatypeProperty>
    


    <!-- http://bibframe.org/vocab/subLocation -->

    <owl:DatatypeProperty rdf:about="&vocab;subLocation">
        <rdfs:label>Held in sublocation</rdfs:label>
        <dcterms:modified>2014-04-28 (Updated Mapping)</dcterms:modified>
        <rdfs:comment>Specific place within the holding entity where the item is located or made available</rdfs:comment>
        <rdfs:range rdf:resource="&rdfs;Literal"/>
    </owl:DatatypeProperty>
    


    <!-- http://bibframe.org/vocab/subtitle -->

    <owl:DatatypeProperty rdf:about="&vocab;subtitle">
        <rdfs:label>Subtitle</rdfs:label>
        <rdfs:comment>Word, character, or group of words and/or characters that contains the remainder of the title information after the main title.</rdfs:comment>
        <rdfs:range rdf:resource="&rdfs;Literal"/>
    </owl:DatatypeProperty>
    


    <!-- http://bibframe.org/vocab/supplementaryContentNote -->

    <owl:DatatypeProperty rdf:about="&vocab;supplementaryContentNote">
        <rdfs:label>Supplementary content note</rdfs:label>
        <rdfs:comment>Information on the presence of one or more bibliographies, discographies, filmographies, and/or other bibliographic references in a described resource or in accompanying material.</rdfs:comment>
        <rdfs:range rdf:resource="&rdfs;Literal"/>
    </owl:DatatypeProperty>
    


    <!-- http://bibframe.org/vocab/temporalCoverageNote -->

    <owl:DatatypeProperty rdf:about="&vocab;temporalCoverageNote">
        <rdfs:label>Temporal coverage</rdfs:label>
        <rdfs:comment>Time period covered by the resource.</rdfs:comment>
        <rdfs:range rdf:resource="&rdfs;Literal"/>
    </owl:DatatypeProperty>
    


    <!-- http://bibframe.org/vocab/title -->

    <owl:DatatypeProperty rdf:about="&vocab;title">
        <rdfs:label>Title</rdfs:label>
        <rdfs:comment>Word, character, or group of words and/or characters that is a name given to a resource</rdfs:comment>
        <rdfs:range rdf:resource="&rdfs;Literal"/>
    </owl:DatatypeProperty>
    


    <!-- http://bibframe.org/vocab/titleAttribute -->

    <owl:DatatypeProperty rdf:about="&vocab;titleAttribute">
        <rdfs:label>Other title attribute</rdfs:label>
        <rdfs:comment>Other distinguishing characteristic of a work, such as version, etc..</rdfs:comment>
        <rdfs:range rdf:resource="&rdfs;Literal"/>
    </owl:DatatypeProperty>
    


    <!-- http://bibframe.org/vocab/titleQualifier -->

    <owl:DatatypeProperty rdf:about="&vocab;titleQualifier">
        <rdfs:label>Title qualifier</rdfs:label>
        <rdfs:comment>Qualifier of title information to make it unique.</rdfs:comment>
        <rdfs:range rdf:resource="&rdfs;Literal"/>
    </owl:DatatypeProperty>
    


    <!-- http://bibframe.org/vocab/titleSource -->

    <owl:DatatypeProperty rdf:about="&vocab;titleSource">
        <rdfs:label>Title source</rdfs:label>
        <rdfs:comment>Title list from which title is taken, e.g., list of abbreviated titles.</rdfs:comment>
        <rdfs:range rdf:resource="&rdfs;Literal"/>
    </owl:DatatypeProperty>
    


    <!-- http://bibframe.org/vocab/titleStatement -->

    <owl:DatatypeProperty rdf:about="&vocab;titleStatement">
        <rdfs:label>Transcribed title</rdfs:label>
        <rdfs:comment>Title transcribed from an instance.</rdfs:comment>
        <dcterms:modified>2014-09-03 (Updated)</dcterms:modified>
        <rdfs:range rdf:resource="&rdfs;Literal"/>
    </owl:DatatypeProperty>
    


    <!-- http://bibframe.org/vocab/titleType -->

    <owl:DatatypeProperty rdf:about="&vocab;titleType">
        <rdfs:label>Variant title type</rdfs:label>
        <dcterms:modified>2014-08-07 (Example added)</dcterms:modified>
        <rdfs:comment>Type of title variation, e.g., acronym, cover, spine. .</rdfs:comment>
        <rdfs:range rdf:resource="&rdfs;Literal"/>
    </owl:DatatypeProperty>
    


    <!-- http://bibframe.org/vocab/titleValue -->

    <owl:DatatypeProperty rdf:about="&vocab;titleValue">
        <rdfs:label>Title</rdfs:label>
        <rdfs:comment>Title being addressed.</rdfs:comment>
        <rdfs:range rdf:resource="&rdfs;Literal"/>
    </owl:DatatypeProperty>
    


    <!-- http://bibframe.org/vocab/titleVariationDate -->

    <owl:DatatypeProperty rdf:about="&vocab;titleVariationDate">
        <rdfs:label>Variant title date</rdfs:label>
        <rdfs:comment>Date or sequential designation of title variation.</rdfs:comment>
        <rdfs:range rdf:resource="&rdfs;Literal"/>
    </owl:DatatypeProperty>
    


    <!-- http://bibframe.org/vocab/treatySignator -->

    <owl:DatatypeProperty rdf:about="&vocab;treatySignator">
        <rdfs:label>Signatory to a treaty</rdfs:label>
        <rdfs:comment>Government of other party that has formally signed a treaty.</rdfs:comment>
        <dcterms:modified>2014-03-21 (Range updated)</dcterms:modified>
        <rdfs:range rdf:resource="&rdfs;Literal"/>
    </owl:DatatypeProperty>
    


    <!-- http://www.w3.org/ns/prov#startedAtTime -->

    <owl:DatatypeProperty rdf:about="&prov;startedAtTime">
        <rdfs:label>startedAtTime</rdfs:label>
        <prov:editorialNote xml:lang="en">It is the intent that the property chain holds: (prov:qualifiedStart o prov:atTime) rdfs:subPropertyOf prov:startedAtTime.</prov:editorialNote>
        <rdfs:comment xml:lang="en">The time at which an activity started. See also prov:endedAtTime.</rdfs:comment>
        <prov:component>entities-activities</prov:component>
        <prov:category>starting-point</prov:category>
        <rdfs:range rdf:resource="&xsd;dateTime"/>
        <rdfs:domain rdf:resource="&prov;Activity"/>
        <prov:qualifiedForm rdf:resource="&prov;Start"/>
        <prov:qualifiedForm rdf:resource="&prov;atTime"/>
        <rdfs:isDefinedBy rdf:resource="http://www.w3.org/ns/prov-o#"/>
    </owl:DatatypeProperty>
    


    <!-- 
    ///////////////////////////////////////////////////////////////////////////////////////
    //
    // Classes
    //
    ///////////////////////////////////////////////////////////////////////////////////////
     -->

    


    <!-- http://bibframe.org/vocab/Agent -->

    <owl:Class rdf:about="&vocab;Agent">
        <rdfs:label>Agent</rdfs:label>
        <rdfs:subClassOf rdf:resource="&vocab;Authority"/>
        <rdfs:comment>Entity having a role in a resource (Person, Organization, etc.).</rdfs:comment>
    </owl:Class>
    


    <!-- http://bibframe.org/vocab/Annotation -->

    <owl:Class rdf:about="&vocab;Annotation">
        <rdfs:label>Annotation</rdfs:label>
        <rdfs:subClassOf rdf:resource="&vocab;Resource"/>
        <rdfs:comment>Resource that asserts additional information about other BIBFRAME resource.</rdfs:comment>
    </owl:Class>
    


    <!-- http://bibframe.org/vocab/Archival -->

    <owl:Class rdf:about="&vocab;Archival">
        <rdfs:label>Archival controlled</rdfs:label>
        <rdfs:subClassOf rdf:resource="&vocab;Instance"/>
        <dcterms:modified>2014-10-28 (Updated)</dcterms:modified>
        <rdfs:comment>Resources organically created, accumulated, and/or used by a person, family, or organization in the course of conduct of affairs and preserved because of their continuing value.</rdfs:comment>
    </owl:Class>
    


    <!-- http://bibframe.org/vocab/Arrangement -->

    <owl:Class rdf:about="&vocab;Arrangement">
        <rdfs:label>Organization of materials information</rdfs:label>
        <rdfs:subClassOf rdf:resource="&vocab;Resource"/>
        <rdfs:comment>Information about the organization and arrangement of a collection of items. For instance, for computer files, organization and arrangement information may be the file structure and sort sequence of a file; for visual materials, this information may be how a collection is arranged.</rdfs:comment>
    </owl:Class>
    


    <!-- http://bibframe.org/vocab/Audio -->

    <owl:Class rdf:about="&vocab;Audio">
        <rdfs:label>Audio</rdfs:label>
        <rdfs:subClassOf rdf:resource="&vocab;Work"/>
        <rdfs:comment>Resources expressed in an audible form, including music or other sounds.</rdfs:comment>
    </owl:Class>
    


    <!-- http://bibframe.org/vocab/Authority -->

    <owl:Class rdf:about="&vocab;Authority">
        <rdfs:label>Authority</rdfs:label>
        <rdfs:subClassOf rdf:resource="&vocab;Resource"/>
        <rdfs:comment>Representation of a key concept or thing. Works and Instances, for example, have defined relationships to these concepts and things.</rdfs:comment>
    </owl:Class>
    


    <!-- http://bibframe.org/vocab/Cartography -->

    <owl:Class rdf:about="&vocab;Cartography">
        <rdfs:label>Cartography</rdfs:label>
        <rdfs:subClassOf rdf:resource="&vocab;Work"/>
        <rdfs:comment>Resource that show spatial information, including maps, atlases, globes,digital maps, and other cartographic items.</rdfs:comment>
    </owl:Class>
    


    <!-- http://bibframe.org/vocab/Category -->

    <owl:Class rdf:about="&vocab;Category">
        <rdfs:label>Category</rdfs:label>
        <rdfs:subClassOf rdf:resource="&vocab;Resource"/>
        <rdfs:comment>Generic list of values information.</rdfs:comment>
        <dcterms:modified>2014-03-21 (Definition Updated)</dcterms:modified>
    </owl:Class>
    


    <!-- http://bibframe.org/vocab/Classification -->

    <owl:Class rdf:about="&vocab;Classification">
        <rdfs:label>Classification Entity</rdfs:label>
        <rdfs:subClassOf rdf:resource="&vocab;Resource"/>
        <rdfs:comment>System of coding, assorting and organizing materials according to their subject.</rdfs:comment>
    </owl:Class>
    


    <!-- http://bibframe.org/vocab/Collection -->

    <owl:Class rdf:about="&vocab;Collection">
        <rdfs:label>Collection</rdfs:label>
        <rdfs:subClassOf rdf:resource="&vocab;Instance"/>
        <rdfs:comment>Aggregation of resources, generally gathered together artificially.</rdfs:comment>
    </owl:Class>
    


    <!-- http://bibframe.org/vocab/CoverArt -->

    <owl:Class rdf:about="&vocab;CoverArt">
        <rdfs:label>Cover Art Annotation</rdfs:label>
        <rdfs:subClassOf rdf:resource="&vocab;Annotation"/>
        <rdfs:comment>Link to a cover illustration of an instance.</rdfs:comment>
    </owl:Class>
    


    <!-- http://bibframe.org/vocab/Dataset -->

    <owl:Class rdf:about="&vocab;Dataset">
        <rdfs:label>Dataset</rdfs:label>
        <rdfs:subClassOf rdf:resource="&vocab;Work"/>
        <rdfs:comment>Data encoded in a defined structure. Includes numeric data, environmental data,etc., used by applications software to calculate averages, correlations, etc., or to produce models, etc., but not normally displayed in its raw form.</rdfs:comment>
    </owl:Class>
    


    <!-- http://bibframe.org/vocab/DescriptionAdminInfo -->

    <owl:Class rdf:about="&vocab;DescriptionAdminInfo">
        <rdfs:label>Administrative metadata</rdfs:label>
        <rdfs:subClassOf rdf:resource="&vocab;Resource"/>
        <dcterms:modified>2014-03-21 (Definition Updated)</dcterms:modified>
        <rdfs:comment>Administrative metadata associated with the graph.</rdfs:comment>
    </owl:Class>
    


    <!-- http://bibframe.org/vocab/Electronic -->

    <owl:Class rdf:about="&vocab;Electronic">
        <rdfs:label>Electronic</rdfs:label>
        <rdfs:subClassOf rdf:resource="&vocab;Instance"/>
        <dcterms:modified>2014-10-28 (Updated)</dcterms:modified>
        <rdfs:comment>Resource that is intended for manipulation by a computer, residing in a carrier accessed either directly or remotely.</rdfs:comment>
    </owl:Class>
    


    <!-- http://bibframe.org/vocab/Event -->

    <owl:Class rdf:about="&vocab;Event">
        <rdfs:label>Event Entity</rdfs:label>
        <rdfs:subClassOf rdf:resource="&vocab;Resource"/>
        <rdfs:comment>Time or place of an event.</rdfs:comment>
        <dcterms:modified>2014-03-21 (Definition Updated)</dcterms:modified>
    </owl:Class>
    


    <!-- http://bibframe.org/vocab/Family -->

    <owl:Class rdf:about="&vocab;Family">
        <rdfs:label>Family</rdfs:label>
        <rdfs:subClassOf rdf:resource="&vocab;Agent"/>
        <rdfs:comment>Two or more persons related by birth, marriage, adoption, civil union, or similar legal status, or who otherwise present themselves as a family.</rdfs:comment>
    </owl:Class>
    


    <!-- http://bibframe.org/vocab/HeldItem -->

    <owl:Class rdf:about="&vocab;HeldItem">
        <rdfs:label>Item held</rdfs:label>
        <rdfs:subClassOf rdf:resource="&vocab;HeldMaterial"/>
        <rdfs:comment>Item holding information.</rdfs:comment>
        <dcterms:modified>2014-03-21 (Label Updated)</dcterms:modified>
    </owl:Class>
    


    <!-- http://bibframe.org/vocab/HeldMaterial -->

    <owl:Class rdf:about="&vocab;HeldMaterial">
        <rdfs:label>Material held</rdfs:label>
        <rdfs:subClassOf rdf:resource="&vocab;Annotation"/>
        <dcterms:modified>2014-03-21 (Label Updated)</dcterms:modified>
        <rdfs:comment>Summary holdings information.</rdfs:comment>
    </owl:Class>
    


    <!-- http://bibframe.org/vocab/Identifier -->

    <owl:Class rdf:about="&vocab;Identifier">
        <rdfs:label>Identifier</rdfs:label>
        <rdfs:subClassOf rdf:resource="&vocab;Resource"/>
        <rdfs:comment>Token or name that is associated with a resource, such as a URI, or an ISBN, etc..</rdfs:comment>
    </owl:Class>
    


    <!-- http://bibframe.org/vocab/Instance -->

    <owl:Class rdf:about="&vocab;Instance">
        <rdfs:label>Instance</rdfs:label>
        <rdfs:subClassOf rdf:resource="&vocab;Resource"/>
        <rdfs:comment>Resource reflecting an individual, material embodiment of the Work.</rdfs:comment>
    </owl:Class>
    


    <!-- http://bibframe.org/vocab/Integrating -->

    <owl:Class rdf:about="&vocab;Integrating">
        <rdfs:label>Integrating</rdfs:label>
        <rdfs:subClassOf rdf:resource="&vocab;Instance"/>
        <rdfs:comment>Cataloging resource that is added to or changed by means of updates that do not remain discrete but are integrated into the whole.</rdfs:comment>
    </owl:Class>
    


    <!-- http://bibframe.org/vocab/IntendedAudience -->

    <owl:Class rdf:about="&vocab;IntendedAudience">
        <rdfs:label>Intended Audience Information</rdfs:label>
        <rdfs:subClassOf rdf:resource="&vocab;Resource"/>
        <rdfs:comment>Information that identifies the specific intended or target audience or intellectual level for which the content described item is considered appropriate. Used to record interest and motivation levels and special learner characteristics.</rdfs:comment>
    </owl:Class>
    


    <!-- http://bibframe.org/vocab/Jurisdiction -->

    <owl:Class rdf:about="&vocab;Jurisdiction">
        <rdfs:label>Jurisdiction</rdfs:label>
        <rdfs:subClassOf rdf:resource="&vocab;Agent"/>
        <rdfs:comment>Legal or political unit administering a geographic area.</rdfs:comment>
    </owl:Class>
    


    <!-- http://bibframe.org/vocab/Language -->

    <owl:Class rdf:about="&vocab;Language">
        <rdfs:label>Language Entity</rdfs:label>
        <rdfs:subClassOf rdf:resource="&vocab;Resource"/>
        <rdfs:comment>Language entity.</rdfs:comment>
    </owl:Class>
    


    <!-- http://bibframe.org/vocab/Manuscript -->

    <owl:Class rdf:about="&vocab;Manuscript">
        <rdfs:label>Manuscript</rdfs:label>
        <rdfs:subClassOf rdf:resource="&vocab;Instance"/>
        <rdfs:comment>Resource that is written in handwriting or typescript. These are generally unique resources.</rdfs:comment>
    </owl:Class>
    


    <!-- http://bibframe.org/vocab/Meeting -->

    <owl:Class rdf:about="&vocab;Meeting">
        <rdfs:label>Meeting</rdfs:label>
        <rdfs:subClassOf rdf:resource="&vocab;Agent"/>
        <rdfs:comment>Gathering of individuals or representatives of various bodies for the purpose of discussing and/or acting on topics of common interest.</rdfs:comment>
    </owl:Class>
    


    <!-- http://bibframe.org/vocab/MixedMaterial -->

    <owl:Class rdf:about="&vocab;MixedMaterial">
        <rdfs:label>Mixed Material</rdfs:label>
        <rdfs:subClassOf rdf:resource="&vocab;Work"/>
        <rdfs:comment>Resource comprised of multiple types which are not driven by software. This may include materials in two or more forms that are related by virtue of their having been accumulated by or about a person or body, e.g. archival forms.</rdfs:comment>
    </owl:Class>
    


    <!-- http://bibframe.org/vocab/Monograph -->

    <owl:Class rdf:about="&vocab;Monograph">
        <rdfs:label>Single unit</rdfs:label>
        <rdfs:subClassOf rdf:resource="&vocab;Instance"/>
        <rdfs:comment>Single unit cataloging resource.</rdfs:comment>
    </owl:Class>
    


    <!-- http://bibframe.org/vocab/MovingImage -->

    <owl:Class rdf:about="&vocab;MovingImage">
        <rdfs:label>Moving Image</rdfs:label>
        <rdfs:subClassOf rdf:resource="&vocab;Work"/>
        <rdfs:comment>Images intended to be perceived as moving, including motion pictures (using liveaction and/or animation), film and video recordings of performances, events,etc.</rdfs:comment>
    </owl:Class>
    


    <!-- http://bibframe.org/vocab/Multimedia -->

    <owl:Class rdf:about="&vocab;Multimedia">
        <rdfs:label>Software or Multimedia</rdfs:label>
        <rdfs:subClassOf rdf:resource="&vocab;Work"/>
        <rdfs:comment>Electronic resource that is a computer program (i.e. digitally encoded instructions intended to be processed and performed by a computer) or which consist of multiple media types that are software driven. Examples include videogames and websites.</rdfs:comment>
    </owl:Class>
    


    <!-- http://bibframe.org/vocab/MultipartMonograph -->

    <owl:Class rdf:about="&vocab;MultipartMonograph">
        <rdfs:label>Multiple units</rdfs:label>
        <rdfs:subClassOf rdf:resource="&vocab;Instance"/>
        <rdfs:comment>Multiple unit cataloging resource that is complete or intended to be completed within a finite number of parts.</rdfs:comment>
    </owl:Class>
    


    <!-- http://bibframe.org/vocab/NotatedMovement -->

    <owl:Class rdf:about="&vocab;NotatedMovement">
        <rdfs:label>Notated Movement</rdfs:label>
        <rdfs:subClassOf rdf:resource="&vocab;Work"/>
        <rdfs:comment>Graphic, non-realized representations of movement intended to be perceived visually, e.g. dance.</rdfs:comment>
    </owl:Class>
    


    <!-- http://bibframe.org/vocab/NotatedMusic -->

    <owl:Class rdf:about="&vocab;NotatedMusic">
        <rdfs:label>Notated Music</rdfs:label>
        <rdfs:subClassOf rdf:resource="&vocab;Work"/>
        <rdfs:comment>Graphic, non-realized representations of musical works intended to be perceived visually.</rdfs:comment>
    </owl:Class>
    


    <!-- http://bibframe.org/vocab/Organization -->

    <owl:Class rdf:about="&vocab;Organization">
        <rdfs:label>Organization</rdfs:label>
        <rdfs:subClassOf rdf:resource="&vocab;Agent"/>
        <rdfs:comment>Corporation or group of persons and/or organizations that acts, or may act, as a unit.</rdfs:comment>
    </owl:Class>
    


    <!-- http://bibframe.org/vocab/Person -->

    <owl:Class rdf:about="&vocab;Person">
        <rdfs:label>Person</rdfs:label>
        <rdfs:subClassOf rdf:resource="&vocab;Agent"/>
        <rdfs:comment>Individual or identity established by an individual (either alone or in collaboration with one or more other individuals)</rdfs:comment>
    </owl:Class>
    


    <!-- http://bibframe.org/vocab/Place -->

    <owl:Class rdf:about="&vocab;Place">
        <rdfs:label>Place</rdfs:label>
        <rdfs:subClassOf rdf:resource="&vocab;Authority"/>
        <rdfs:comment>Geographic location.</rdfs:comment>
    </owl:Class>
    


    <!-- http://bibframe.org/vocab/Print -->

    <owl:Class rdf:about="&vocab;Print">
        <rdfs:label>Printed</rdfs:label>
        <rdfs:subClassOf rdf:resource="&vocab;Instance"/>
        <rdfs:comment>Resource that is printed.</rdfs:comment>
    </owl:Class>
    


    <!-- http://bibframe.org/vocab/Provider -->

    <owl:Class rdf:about="&vocab;Provider">
        <rdfs:label>Provider Entity</rdfs:label>
        <rdfs:subClassOf rdf:resource="&vocab;Resource"/>
        <rdfs:comment>Name of agent relating to the publication, printing, distribution, issue,release, or production of a resource.</rdfs:comment>
    </owl:Class>
    


    <!-- http://bibframe.org/vocab/Relator -->

    <owl:Class rdf:about="&vocab;Relator">
        <rdfs:label>Relationship</rdfs:label>
        <rdfs:subClassOf rdf:resource="&vocab;Resource"/>
        <rdfs:comment>How an agent is related to a resource.</rdfs:comment>
        <dcterms:modified>2014-04-30 (New)</dcterms:modified>
    </owl:Class>
    


    <!-- http://bibframe.org/vocab/Resource -->

    <owl:Class rdf:about="&vocab;Resource">
        <rdfs:label>Resource</rdfs:label>
        <rdfs:comment>Any BIBFRAME object.</rdfs:comment>
    </owl:Class>
    


    <!-- http://bibframe.org/vocab/Review -->

    <owl:Class rdf:about="&vocab;Review">
        <rdfs:label>Review Annotation</rdfs:label>
        <rdfs:subClassOf rdf:resource="&vocab;Annotation"/>
        <rdfs:comment>Critique of a resource, such as a book review, analysis, etc.</rdfs:comment>
    </owl:Class>
    


    <!-- http://bibframe.org/vocab/Serial -->

    <owl:Class rdf:about="&vocab;Serial">
        <rdfs:label>Serial</rdfs:label>
        <rdfs:subClassOf rdf:resource="&vocab;Instance"/>
        <rdfs:comment>Multiple unit cataloging resource issued in successive parts that has no predetermined conclusion.</rdfs:comment>
    </owl:Class>
    


    <!-- http://bibframe.org/vocab/StillImage -->

    <owl:Class rdf:about="&vocab;StillImage">
        <rdfs:label>Still Image</rdfs:label>
        <rdfs:subClassOf rdf:resource="&vocab;Work"/>
        <rdfs:comment>Resource expressed through line, shape, shading, etc., intended to be perceived visually as a still image or images in two dimensions. Includes two-dimensional images and slides and transparencies.</rdfs:comment>
    </owl:Class>
    


    <!-- http://bibframe.org/vocab/Summary -->

    <owl:Class rdf:about="&vocab;Summary">
        <rdfs:label>Summary Annotation</rdfs:label>
        <rdfs:subClassOf rdf:resource="&vocab;Annotation"/>
        <rdfs:comment>Description of the content of a resource, such as an abstract, summary, etc..</rdfs:comment>
    </owl:Class>
    


    <!-- http://bibframe.org/vocab/TableOfContents -->

    <owl:Class rdf:about="&vocab;TableOfContents">
        <rdfs:label>Table of Contents Annotation</rdfs:label>
        <rdfs:subClassOf rdf:resource="&vocab;Annotation"/>
        <rdfs:comment>Table of Contents information for a resource.</rdfs:comment>
        <dcterms:modified>2014-03-21 (Label Updated)</dcterms:modified>
    </owl:Class>
    


    <!-- http://bibframe.org/vocab/Tactile -->

    <owl:Class rdf:about="&vocab;Tactile">
        <rdfs:label>Tactile Material</rdfs:label>
        <rdfs:subClassOf rdf:resource="&vocab;Instance"/>
        <rdfs:comment>Resource that is intended to be perceived by touch.</rdfs:comment>
    </owl:Class>
    


    <!-- http://bibframe.org/vocab/Temporal -->

    <owl:Class rdf:about="&vocab;Temporal">
        <rdfs:label>Temporal Concept</rdfs:label>
        <rdfs:subClassOf rdf:resource="&vocab;Authority"/>
        <rdfs:comment>Chronological period.</rdfs:comment>
    </owl:Class>
    


    <!-- http://bibframe.org/vocab/Text -->

    <owl:Class rdf:about="&vocab;Text">
        <rdfs:label>Text</rdfs:label>
        <rdfs:subClassOf rdf:resource="&vocab;Work"/>
        <rdfs:comment>Form of notation for language intended to be perceived visually and understood through the use of language in written or spoken form.</rdfs:comment>
    </owl:Class>
    


    <!-- http://bibframe.org/vocab/ThreeDimensionalObject -->

    <owl:Class rdf:about="&vocab;ThreeDimensionalObject">
        <rdfs:label>Three-dimensional Object</rdfs:label>
        <rdfs:subClassOf rdf:resource="&vocab;Work"/>
        <rdfs:comment>Resource in a form intended to be perceived visually in three-dimensions.Includes man-made objects such as models, sculptures, clothing, and toys, as well as naturally occurring objects such as specimens mounted for viewing.</rdfs:comment>
    </owl:Class>
    


    <!-- http://bibframe.org/vocab/Title -->

    <owl:Class rdf:about="&vocab;Title">
        <rdfs:label>Title Entity</rdfs:label>
        <rdfs:subClassOf rdf:resource="&vocab;Resource"/>
        <rdfs:comment>Title information relating to a resource: title proper, translated title, or variant form of title.</rdfs:comment>
    </owl:Class>
    


    <!-- http://bibframe.org/vocab/Topic -->

    <owl:Class rdf:about="&vocab;Topic">
        <rdfs:label>Topic</rdfs:label>
        <rdfs:subClassOf rdf:resource="&vocab;Authority"/>
        <rdfs:comment>Concept or area of knowledge.</rdfs:comment>
    </owl:Class>
    


    <!-- http://bibframe.org/vocab/Work -->

    <owl:Class rdf:about="&vocab;Work">
        <rdfs:label>Work</rdfs:label>
        <rdfs:subClassOf rdf:resource="&vocab;Resource"/>
        <rdfs:comment>Resource reflecting a conceptual essence of the cataloging resource.</rdfs:comment>
    </owl:Class>
    


    <!-- http://schema.org/Audience -->

    <owl:Class rdf:about="http://schema.org/Audience">
        <rdfs:label xml:lang="en">Audience</rdfs:label>
        <rdfs:comment xml:lang="en"></rdfs:comment>
        <rdfs:isDefinedBy rdf:resource="http://schema.org/Audience"/>
    </owl:Class>
    


    <!-- http://schema.org/BusinessAudience -->

    <owl:Class rdf:about="http://schema.org/BusinessAudience">
        <rdfs:subClassOf rdf:resource="http://schema.org/Audience"/>
    </owl:Class>
    


    <!-- http://schema.org/EducationalAudience -->

    <owl:Class rdf:about="http://schema.org/EducationalAudience">
        <rdfs:subClassOf rdf:resource="http://schema.org/Audience"/>
    </owl:Class>
    


    <!-- http://schema.org/GovernmentOrganization -->

    <owl:Class rdf:about="http://schema.org/GovernmentOrganization">
        <rdfs:label xml:lang="en">Government Organization</rdfs:label>
        <rdfs:comment xml:lang="en"></rdfs:comment>
        <rdfs:isDefinedBy rdf:resource="http://schema.org/GovernmentOrganization"/>
    </owl:Class>
    


    <!-- http://schema.org/MedicalAudience -->

    <owl:Class rdf:about="http://schema.org/MedicalAudience">
        <rdfs:subClassOf rdf:resource="http://schema.org/Audience"/>
    </owl:Class>
    


    <!-- http://schema.org/PeopleAudience -->

    <owl:Class rdf:about="http://schema.org/PeopleAudience">
        <rdfs:subClassOf rdf:resource="http://schema.org/Audience"/>
    </owl:Class>
    


    <!-- http://www.w3.org/2000/01/rdf-schema#Resource -->

    <owl:Class rdf:about="&rdfs;Resource"/>
    


    <!-- http://www.w3.org/2001/XMLSchema#string -->

    <owl:Class rdf:about="&xsd;string"/>
    


    <!-- http://www.w3.org/ns/prov#Activity -->

    <owl:Class rdf:about="&prov;Activity"/>
    


    <!-- http://www.w3.org/ns/prov#Agent -->

    <owl:Class rdf:about="&prov;Agent"/>
    


    <!-- http://www.w3.org/ns/prov#Entity -->

    <owl:Class rdf:about="&prov;Entity"/>
    


    <!-- http://www.w3.org/ns/prov#InstantaneousEvent -->

    <owl:Class rdf:about="&prov;InstantaneousEvent"/>
    


    <!-- http://www.w3.org/ns/prov#Location -->

    <owl:Class rdf:about="&prov;Location"/>
</rdf:RDF>



<!-- Generated by the OWL API (version 3.4.2) http://owlapi.sourceforge.net -->

