<?xml version="1.0"?>


<!DOCTYPE rdf:RDF [
    <!ENTITY schema "http://schema.org/" >
    <!ENTITY rda-fields "http://bibframe.org/rda/" >
    <!ENTITY oa "http://www.w3.org/ns/oa#" >
    <!ENTITY marc-fields "http://bibframe.org/marc/" >
    <!ENTITY dcterms "http://purl.org/dc/terms/" >
    <!ENTITY foaf "http://xmlns.com/foaf/0.1/" >
    <!ENTITY prov-o "http://www.w3.org/ns/prov-o#" >
    <!ENTITY owl "http://www.w3.org/2002/07/owl#" >
    <!ENTITY bfmain "http://bibframe.org/vocab/main" >
    <!ENTITY bframe "http://bibframe.org/vocab/frame" >
    <!ENTITY skos2 "http://www.w3.org/2004/02/skos/" >
    <!ENTITY v1 "http://www.loc.gov/mads/rdf/v1#" >
    <!ENTITY dc "http://purl.org/dc/elements/1.1/" >
    <!ENTITY lingvoj "http://www.lingvoj.org/ontology#" >
    <!ENTITY xsd "http://www.w3.org/2001/XMLSchema#" >
    <!ENTITY event "http://purl.org/NET/c4dm/event.owl#" >
    <!ENTITY bf-abstract "http://bibframe.org/model-abstract/" >
    <!ENTITY skos "http://www.w3.org/2004/02/skos/core" >
    <!ENTITY rdfs "http://www.w3.org/2000/01/rdf-schema#" >
    <!ENTITY marcrel "http://id.loc.gov/vocabulary/relators/" >
    <!ENTITY RecordInfo "http://id.loc.gov/ontologies/RecordInfo#" >
    <!ENTITY rdf "http://www.w3.org/1999/02/22-rdf-syntax-ns#" >
]>


<rdf:RDF xmlns="http://bibframe.org/vocab/"
     xml:base="http://bibframe.org/vocab/"
     xmlns:v1="http://www.loc.gov/mads/rdf/v1#"
     xmlns:dc="http://purl.org/dc/elements/1.1/"
     xmlns:marcrel="http://id.loc.gov/vocabulary/relators/"
     xmlns:legacy="http://bibframe.org/vocab/legacy/"
     xmlns:prov-o="http://www.w3.org/ns/prov-o#"
     xmlns:foaf="http://xmlns.com/foaf/0.1/"
     xmlns:lingvoj="http://www.lingvoj.org/ontology#"
     xmlns:bf-abstract="http://bibframe.org/model-abstract/"
     xmlns:RecordInfo="http://id.loc.gov/ontologies/RecordInfo#"
     xmlns:bfmain="http://bibframe.org/vocab/main"
     xmlns:dcterms="http://purl.org/dc/terms/"
     xmlns:schema="http://schema.org/"
     xmlns:rdfs="http://www.w3.org/2000/01/rdf-schema#"
     xmlns:rda-fields="http://bibframe.org/rda/"
     xmlns:oa="http://www.w3.org/ns/oa#"
     xmlns:marc-fields="http://bibframe.org/marc/"
     xmlns:skos2="http://www.w3.org/2004/02/skos/"
     xmlns:event="http://purl.org/NET/c4dm/event.owl#"
     xmlns:owl="http://www.w3.org/2002/07/owl#"
     xmlns:xsd="http://www.w3.org/2001/XMLSchema#"
     xmlns:rdf="http://www.w3.org/1999/02/22-rdf-syntax-ns#"
     xmlns:skos="&skos2;core"
     xmlns:bframe="http://bibframe.org/vocab/frame">
    <owl:Ontology rdf:about="http://bibframe.org/vocab/">
        <owl:versionInfo rdf:datatype="&xsd;string">Initially automatically generated.</owl:versionInfo>
        <dcterms:modified>2015-04-10</dcterms:modified>
        <!--
        <owl:imports rdf:resource="http://motools.sourceforge.net/event/event.n3#"/>
        <owl:imports rdf:resource="http://schema.rdfs.org/all.rdf"/>
        <owl:imports rdf:resource="http://www.lingvoj.org/ontology_v2.3.ttl"/>
        <owl:imports rdf:resource="http://www.w3.org/TR/skos-reference/skos.rdf"/>
        <owl:imports rdf:resource="http://www.w3.org/ns/oa.owl"/>
        <owl:imports rdf:resource="http://www.w3.org/ns/prov-o#"/>
        <owl:imports rdf:resource="http://xmlns.com/foaf/spec/index.rdf"/>
        -->
    </owl:Ontology>
    


    <!-- 
    ///////////////////////////////////////////////////////////////////////////////////////
    //
    // Annotation properties
    //
    ///////////////////////////////////////////////////////////////////////////////////////
     -->

    


    <!-- http://id.loc.gov/ontologies/RecordInfo#recordContentSource -->

    <owl:AnnotationProperty rdf:about="&RecordInfo;recordContentSource"/>
    


    <!-- http://purl.org/dc/elements/1.1/contributor -->

    <owl:AnnotationProperty rdf:about="&dc;contributor"/>
    


    <!-- http://purl.org/dc/elements/1.1/coverage -->

    <owl:AnnotationProperty rdf:about="&dc;coverage"/>
    


    <!-- http://purl.org/dc/elements/1.1/creator -->

    <owl:AnnotationProperty rdf:about="&dc;creator"/>
    


    <!-- http://purl.org/dc/elements/1.1/format -->

    <owl:AnnotationProperty rdf:about="&dc;format"/>
    


    <!-- http://purl.org/dc/elements/1.1/identifier -->

    <owl:AnnotationProperty rdf:about="&dc;identifier"/>
    


    <!-- http://purl.org/dc/elements/1.1/language -->

    <owl:AnnotationProperty rdf:about="&dc;language"/>
    


    <!-- http://purl.org/dc/elements/1.1/publisher -->

    <owl:AnnotationProperty rdf:about="&dc;publisher"/>
    


    <!-- http://purl.org/dc/elements/1.1/relation -->

    <owl:AnnotationProperty rdf:about="&dc;relation"/>
    


    <!-- http://purl.org/dc/elements/1.1/rights -->

    <owl:AnnotationProperty rdf:about="&dc;rights"/>
    


    <!-- http://purl.org/dc/elements/1.1/source -->

    <owl:AnnotationProperty rdf:about="&dc;source"/>
    


    <!-- http://purl.org/dc/elements/1.1/subject -->

    <owl:AnnotationProperty rdf:about="&dc;subject"/>
    


    <!-- http://purl.org/dc/elements/1.1/type -->

    <owl:AnnotationProperty rdf:about="&dc;type"/>
    


    <!-- http://purl.org/dc/terms/abstract -->

    <owl:AnnotationProperty rdf:about="&dcterms;abstract">
        <rdfs:label xml:lang="en">Abstract</rdfs:label>
        <dcterms:issued rdf:datatype="&xsd;date">2000-07-11</dcterms:issued>
        <dcterms:modified rdf:datatype="&xsd;date">2008-01-14</dcterms:modified>
        <rdfs:comment xml:lang="en">A summary of the resource.</rdfs:comment>
        <dcterms:hasVersion rdf:resource="http://dublincore.org/usage/terms/history/#abstract-003"/>
        <rdfs:subPropertyOf rdf:resource="&dc;description"/>
        <rdfs:isDefinedBy rdf:resource="http://purl.org/dc/terms/"/>
        <rdfs:subPropertyOf rdf:resource="&dcterms;description"/>
    </owl:AnnotationProperty>
    


    <!-- http://purl.org/dc/terms/accessRights -->

    <owl:AnnotationProperty rdf:about="&dcterms;accessRights">
        <rdfs:label xml:lang="en">Access Rights</rdfs:label>
        <dcterms:issued rdf:datatype="&xsd;date">2003-02-15</dcterms:issued>
        <dcterms:modified rdf:datatype="&xsd;date">2008-01-14</dcterms:modified>
        <dcterms:description xml:lang="en">Access Rights may include information regarding access or restrictions based on privacy, security, or other policies.</dcterms:description>
        <rdfs:comment xml:lang="en">Information about who can access the resource or an indication of its security status.</rdfs:comment>
        <dcterms:hasVersion rdf:resource="http://dublincore.org/usage/terms/history/#accessRights-002"/>
        <rdfs:subPropertyOf rdf:resource="&dc;rights"/>
        <rdfs:isDefinedBy rdf:resource="http://purl.org/dc/terms/"/>
    </owl:AnnotationProperty>
    


    <!-- http://purl.org/dc/terms/accrualMethod -->

    <owl:AnnotationProperty rdf:about="&dcterms;accrualMethod">
        <rdfs:label xml:lang="en">Accrual Method</rdfs:label>
        <dcterms:issued rdf:datatype="&xsd;date">2005-06-13</dcterms:issued>
        <dcterms:modified rdf:datatype="&xsd;date">2010-10-11</dcterms:modified>
        <rdfs:comment xml:lang="en">The method by which items are added to a collection.</rdfs:comment>
        <dcterms:hasVersion rdf:resource="http://dublincore.org/usage/terms/history/#accrualMethod-003"/>
        <rdfs:domain rdf:resource="http://purl.org/dc/dcmitype/Collection"/>
        <rdfs:isDefinedBy rdf:resource="http://purl.org/dc/terms/"/>
    </owl:AnnotationProperty>
    


    <!-- http://purl.org/dc/terms/accrualPeriodicity -->

    <owl:AnnotationProperty rdf:about="&dcterms;accrualPeriodicity">
        <rdfs:label xml:lang="en">Accrual Periodicity</rdfs:label>
        <dcterms:issued rdf:datatype="&xsd;date">2005-06-13</dcterms:issued>
        <dcterms:modified rdf:datatype="&xsd;date">2010-10-11</dcterms:modified>
        <rdfs:comment xml:lang="en">The frequency with which items are added to a collection.</rdfs:comment>
        <dcterms:hasVersion rdf:resource="http://dublincore.org/usage/terms/history/#accrualPeriodicity-003"/>
        <rdfs:domain rdf:resource="http://purl.org/dc/dcmitype/Collection"/>
        <rdfs:isDefinedBy rdf:resource="http://purl.org/dc/terms/"/>
    </owl:AnnotationProperty>
    


    <!-- http://purl.org/dc/terms/accrualPolicy -->

    <owl:AnnotationProperty rdf:about="&dcterms;accrualPolicy">
        <rdfs:label xml:lang="en">Accrual Policy</rdfs:label>
        <dcterms:issued rdf:datatype="&xsd;date">2005-06-13</dcterms:issued>
        <dcterms:modified rdf:datatype="&xsd;date">2010-10-11</dcterms:modified>
        <rdfs:comment xml:lang="en">The policy governing the addition of items to a collection.</rdfs:comment>
        <dcterms:hasVersion rdf:resource="http://dublincore.org/usage/terms/history/#accrualPolicy-003"/>
        <rdfs:domain rdf:resource="http://purl.org/dc/dcmitype/Collection"/>
        <rdfs:isDefinedBy rdf:resource="http://purl.org/dc/terms/"/>
    </owl:AnnotationProperty>
    


    <!-- http://purl.org/dc/terms/alternative -->

    <owl:AnnotationProperty rdf:about="&dcterms;alternative">
        <rdfs:label xml:lang="en">Alternative Title</rdfs:label>
        <dcterms:issued rdf:datatype="&xsd;date">2000-07-11</dcterms:issued>
        <dcterms:modified rdf:datatype="&xsd;date">2010-10-11</dcterms:modified>
        <rdfs:comment xml:lang="en">An alternative name for the resource.</rdfs:comment>
        <dcterms:description xml:lang="en">The distinction between titles and alternative titles is application-specific.</dcterms:description>
        <dcterms:hasVersion rdf:resource="http://dublincore.org/usage/terms/history/#alternative-003"/>
        <rdfs:isDefinedBy rdf:resource="http://purl.org/dc/terms/"/>
    </owl:AnnotationProperty>
    


    <!-- http://purl.org/dc/terms/available -->

    <owl:AnnotationProperty rdf:about="&dcterms;available">
        <rdfs:label xml:lang="en">Date Available</rdfs:label>
        <dcterms:issued rdf:datatype="&xsd;date">2000-07-11</dcterms:issued>
        <dcterms:modified rdf:datatype="&xsd;date">2008-01-14</dcterms:modified>
        <rdfs:comment xml:lang="en">Date (often a range) that the resource became or will become available.</rdfs:comment>
        <dcterms:hasVersion rdf:resource="http://dublincore.org/usage/terms/history/#available-003"/>
        <rdfs:isDefinedBy rdf:resource="http://purl.org/dc/terms/"/>
    </owl:AnnotationProperty>
    


    <!-- http://purl.org/dc/terms/bibliographicCitation -->

    <owl:AnnotationProperty rdf:about="&dcterms;bibliographicCitation">
        <rdfs:label xml:lang="en">Bibliographic Citation</rdfs:label>
        <dcterms:issued rdf:datatype="&xsd;date">2003-02-15</dcterms:issued>
        <dcterms:modified rdf:datatype="&xsd;date">2008-01-14</dcterms:modified>
        <rdfs:comment xml:lang="en">A bibliographic reference for the resource.</rdfs:comment>
        <dcterms:description xml:lang="en">Recommended practice is to include sufficient bibliographic detail to identify the resource as unambiguously as possible.</dcterms:description>
        <dcterms:hasVersion rdf:resource="http://dublincore.org/usage/terms/history/#bibliographicCitation-002"/>
        <rdfs:subPropertyOf rdf:resource="&dc;identifier"/>
        <rdfs:isDefinedBy rdf:resource="http://purl.org/dc/terms/"/>
        <rdfs:domain rdf:resource="&dcterms;BibliographicResource"/>
    </owl:AnnotationProperty>
    


    <!-- http://purl.org/dc/terms/conformsTo -->

    <owl:AnnotationProperty rdf:about="&dcterms;conformsTo">
        <rdfs:label xml:lang="en">Conforms To</rdfs:label>
        <dcterms:issued rdf:datatype="&xsd;date">2001-05-21</dcterms:issued>
        <dcterms:modified rdf:datatype="&xsd;date">2008-01-14</dcterms:modified>
        <rdfs:comment xml:lang="en">An established standard to which the described resource conforms.</rdfs:comment>
        <dcterms:hasVersion rdf:resource="http://dublincore.org/usage/terms/history/#conformsTo-003"/>
        <rdfs:subPropertyOf rdf:resource="&dc;relation"/>
        <rdfs:isDefinedBy rdf:resource="http://purl.org/dc/terms/"/>
        <rdfs:subPropertyOf rdf:resource="&dcterms;relation"/>
    </owl:AnnotationProperty>
    


    <!-- http://purl.org/dc/terms/contributor -->

    <owl:AnnotationProperty rdf:about="&dcterms;contributor">
        <rdfs:label xml:lang="en">Contributor</rdfs:label>
        <dcterms:issued rdf:datatype="&xsd;date">2008-01-14</dcterms:issued>
        <dcterms:modified rdf:datatype="&xsd;date">2010-10-11</dcterms:modified>
        <rdfs:comment xml:lang="en">An entity responsible for making contributions to the resource.</rdfs:comment>
        <dcterms:description xml:lang="en">Examples of a Contributor include a person, an organization, or a service.</dcterms:description>
        <dcterms:hasVersion rdf:resource="http://dublincore.org/usage/terms/history/#contributorT-001"/>
        <rdfs:isDefinedBy rdf:resource="http://purl.org/dc/terms/"/>
    </owl:AnnotationProperty>
    


    <!-- http://purl.org/dc/terms/coverage -->

    <owl:AnnotationProperty rdf:about="&dcterms;coverage">
        <rdfs:label xml:lang="en">Coverage</rdfs:label>
        <dcterms:modified rdf:datatype="&xsd;date">2008-01-14</dcterms:modified>
        <dcterms:issued rdf:datatype="&xsd;date">2008-01-14</dcterms:issued>
        <dcterms:description xml:lang="en">Spatial topic and spatial applicability may be a named place or a location specified by its geographic coordinates. Temporal topic may be a named period, date, or date range. A jurisdiction may be a named administrative entity or a geographic place to which the resource applies. Recommended best practice is to use a controlled vocabulary such as the Thesaurus of Geographic Names [TGN]. Where appropriate, named places or time periods can be used in preference to numeric identifiers such as sets of coordinates or date ranges.</dcterms:description>
        <rdfs:comment xml:lang="en">The spatial or temporal topic of the resource, the spatial applicability of the resource, or the jurisdiction under which the resource is relevant.</rdfs:comment>
        <dcterms:hasVersion rdf:resource="http://dublincore.org/usage/terms/history/#coverageT-001"/>
        <rdfs:subPropertyOf rdf:resource="&dc;coverage"/>
        <rdfs:isDefinedBy rdf:resource="http://purl.org/dc/terms/"/>
    </owl:AnnotationProperty>
    


    <!-- http://purl.org/dc/terms/created -->

    <owl:AnnotationProperty rdf:about="&dcterms;created">
        <rdfs:label xml:lang="en">Date Created</rdfs:label>
        <dcterms:issued rdf:datatype="&xsd;date">2000-07-11</dcterms:issued>
        <dcterms:modified rdf:datatype="&xsd;date">2008-01-14</dcterms:modified>
        <rdfs:comment xml:lang="en">Date of creation of the resource.</rdfs:comment>
        <dcterms:hasVersion rdf:resource="http://dublincore.org/usage/terms/history/#created-003"/>
        <rdfs:isDefinedBy rdf:resource="http://purl.org/dc/terms/"/>
    </owl:AnnotationProperty>
    


    <!-- http://purl.org/dc/terms/creator -->

    <owl:AnnotationProperty rdf:about="&dcterms;creator">
        <rdfs:label xml:lang="en">Creator</rdfs:label>
        <dcterms:issued rdf:datatype="&xsd;date">2008-01-14</dcterms:issued>
        <dcterms:modified rdf:datatype="&xsd;date">2010-10-11</dcterms:modified>
        <rdfs:comment xml:lang="en">An entity primarily responsible for making the resource.</rdfs:comment>
        <dcterms:description xml:lang="en">Examples of a Creator include a person, an organization, or a service.</dcterms:description>
        <dcterms:hasVersion rdf:resource="http://dublincore.org/usage/terms/history/#creatorT-002"/>
        <rdfs:isDefinedBy rdf:resource="http://purl.org/dc/terms/"/>
    </owl:AnnotationProperty>
    


    <!-- http://purl.org/dc/terms/date -->

    <owl:AnnotationProperty rdf:about="&dcterms;date">
        <rdfs:label xml:lang="en">Date</rdfs:label>
        <dcterms:modified rdf:datatype="&xsd;date">2008-01-14</dcterms:modified>
        <dcterms:issued rdf:datatype="&xsd;date">2008-01-14</dcterms:issued>
        <rdfs:comment xml:lang="en">A point or period of time associated with an event in the lifecycle of the resource.</rdfs:comment>
        <dcterms:description xml:lang="en">Date may be used to express temporal information at any level of granularity.  Recommended best practice is to use an encoding scheme, such as the W3CDTF profile of ISO 8601 [W3CDTF].</dcterms:description>
        <dcterms:hasVersion rdf:resource="http://dublincore.org/usage/terms/history/#dateT-001"/>
        <rdfs:isDefinedBy rdf:resource="http://purl.org/dc/terms/"/>
    </owl:AnnotationProperty>
    


    <!-- http://purl.org/dc/terms/dateAccepted -->

    <owl:AnnotationProperty rdf:about="&dcterms;dateAccepted">
        <rdfs:label xml:lang="en">Date Accepted</rdfs:label>
        <dcterms:issued rdf:datatype="&xsd;date">2002-07-13</dcterms:issued>
        <dcterms:modified rdf:datatype="&xsd;date">2008-01-14</dcterms:modified>
        <rdfs:comment xml:lang="en">Date of acceptance of the resource.</rdfs:comment>
        <dcterms:description xml:lang="en">Examples of resources to which a Date Accepted may be relevant are a thesis (accepted by a university department) or an article (accepted by a journal).</dcterms:description>
        <dcterms:hasVersion rdf:resource="http://dublincore.org/usage/terms/history/#dateAccepted-002"/>
        <rdfs:isDefinedBy rdf:resource="http://purl.org/dc/terms/"/>
    </owl:AnnotationProperty>
    


    <!-- http://purl.org/dc/terms/dateCopyrighted -->

    <owl:AnnotationProperty rdf:about="&dcterms;dateCopyrighted">
        <rdfs:label xml:lang="en">Date Copyrighted</rdfs:label>
        <dcterms:issued rdf:datatype="&xsd;date">2002-07-13</dcterms:issued>
        <dcterms:modified rdf:datatype="&xsd;date">2008-01-14</dcterms:modified>
        <rdfs:comment xml:lang="en">Date of copyright.</rdfs:comment>
        <dcterms:hasVersion rdf:resource="http://dublincore.org/usage/terms/history/#dateCopyrighted-002"/>
        <rdfs:isDefinedBy rdf:resource="http://purl.org/dc/terms/"/>
    </owl:AnnotationProperty>
    


    <!-- http://purl.org/dc/terms/dateSubmitted -->

    <owl:AnnotationProperty rdf:about="&dcterms;dateSubmitted">
        <rdfs:label xml:lang="en">Date Submitted</rdfs:label>
        <dcterms:issued rdf:datatype="&xsd;date">2002-07-13</dcterms:issued>
        <dcterms:modified rdf:datatype="&xsd;date">2008-01-14</dcterms:modified>
        <rdfs:comment xml:lang="en">Date of submission of the resource.</rdfs:comment>
        <dcterms:description xml:lang="en">Examples of resources to which a Date Submitted may be relevant are a thesis (submitted to a university department) or an article (submitted to a journal).</dcterms:description>
        <dcterms:hasVersion rdf:resource="http://dublincore.org/usage/terms/history/#dateSubmitted-002"/>
        <rdfs:isDefinedBy rdf:resource="http://purl.org/dc/terms/"/>
    </owl:AnnotationProperty>
    


    <!-- http://purl.org/dc/terms/description -->

    <owl:AnnotationProperty rdf:about="&dcterms;description">
        <rdfs:label xml:lang="en">Description</rdfs:label>
        <dcterms:modified rdf:datatype="&xsd;date">2008-01-14</dcterms:modified>
        <dcterms:issued rdf:datatype="&xsd;date">2008-01-14</dcterms:issued>
        <rdfs:comment xml:lang="en">An account of the resource.</rdfs:comment>
        <dcterms:description xml:lang="en">Description may include but is not limited to: an abstract, a table of contents, a graphical representation, or a free-text account of the resource.</dcterms:description>
        <dcterms:hasVersion rdf:resource="http://dublincore.org/usage/terms/history/#descriptionT-001"/>
        <rdfs:subPropertyOf rdf:resource="&dc;description"/>
        <rdfs:isDefinedBy rdf:resource="http://purl.org/dc/terms/"/>
    </owl:AnnotationProperty>
    


    <!-- http://purl.org/dc/terms/educationLevel -->

    <owl:AnnotationProperty rdf:about="&dcterms;educationLevel">
        <rdfs:label xml:lang="en">Audience Education Level</rdfs:label>
        <dcterms:issued rdf:datatype="&xsd;date">2002-07-13</dcterms:issued>
        <dcterms:modified rdf:datatype="&xsd;date">2008-01-14</dcterms:modified>
        <rdfs:comment xml:lang="en">A class of entity, defined in terms of progression through an educational or training context, for which the described resource is intended.</rdfs:comment>
        <dcterms:hasVersion rdf:resource="http://dublincore.org/usage/terms/history/#educationLevel-002"/>
        <rdfs:isDefinedBy rdf:resource="http://purl.org/dc/terms/"/>
    </owl:AnnotationProperty>
    


    <!-- http://purl.org/dc/terms/extent -->

    <owl:AnnotationProperty rdf:about="&dcterms;extent">
        <rdfs:label xml:lang="en">Extent</rdfs:label>
        <dcterms:issued rdf:datatype="&xsd;date">2000-07-11</dcterms:issued>
        <dcterms:modified rdf:datatype="&xsd;date">2008-01-14</dcterms:modified>
        <rdfs:comment xml:lang="en">The size or duration of the resource.</rdfs:comment>
        <dcterms:hasVersion rdf:resource="http://dublincore.org/usage/terms/history/#extent-003"/>
        <rdfs:subPropertyOf rdf:resource="&dc;format"/>
        <rdfs:isDefinedBy rdf:resource="http://purl.org/dc/terms/"/>
    </owl:AnnotationProperty>
    


    <!-- http://purl.org/dc/terms/format -->

    <owl:AnnotationProperty rdf:about="&dcterms;format">
        <rdfs:label xml:lang="en">Format</rdfs:label>
        <dcterms:modified rdf:datatype="&xsd;date">2008-01-14</dcterms:modified>
        <dcterms:issued rdf:datatype="&xsd;date">2008-01-14</dcterms:issued>
        <dcterms:description xml:lang="en">Examples of dimensions include size and duration. Recommended best practice is to use a controlled vocabulary such as the list of Internet Media Types [MIME].</dcterms:description>
        <rdfs:comment xml:lang="en">The file format, physical medium, or dimensions of the resource.</rdfs:comment>
        <dcterms:hasVersion rdf:resource="http://dublincore.org/usage/terms/history/#formatT-001"/>
        <rdfs:subPropertyOf rdf:resource="&dc;format"/>
        <rdfs:isDefinedBy rdf:resource="http://purl.org/dc/terms/"/>
    </owl:AnnotationProperty>
    


    <!-- http://purl.org/dc/terms/hasFormat -->

    <owl:AnnotationProperty rdf:about="&dcterms;hasFormat">
        <rdfs:label xml:lang="en">Has Format</rdfs:label>
        <dcterms:issued rdf:datatype="&xsd;date">2000-07-11</dcterms:issued>
        <dcterms:modified rdf:datatype="&xsd;date">2008-01-14</dcterms:modified>
        <rdfs:comment xml:lang="en">A related resource that is substantially the same as the pre-existing described resource, but in another format.</rdfs:comment>
        <skos2:corenote xml:lang="en">This term is intended to be used with non-literal values as defined in the DCMI Abstract Model (http://dublincore.org/documents/abstract-model/).  As of December 2007, the DCMI Usage Board is seeking a way to express this intention with a formal range declaration.</skos2:corenote>
        <dcterms:hasVersion rdf:resource="http://dublincore.org/usage/terms/history/#hasFormat-003"/>
        <rdfs:subPropertyOf rdf:resource="&dc;relation"/>
        <rdfs:isDefinedBy rdf:resource="http://purl.org/dc/terms/"/>
        <rdfs:subPropertyOf rdf:resource="&dcterms;relation"/>
    </owl:AnnotationProperty>
    


    <!-- http://purl.org/dc/terms/hasPart -->

    <rdf:Description rdf:about="&dcterms;hasPart">
        <rdfs:label xml:lang="en">Has Part</rdfs:label>
        <dcterms:issued rdf:datatype="&xsd;date">2000-07-11</dcterms:issued>
        <dcterms:modified rdf:datatype="&xsd;date">2008-01-14</dcterms:modified>
        <rdfs:comment xml:lang="en">A related resource that is included either physically or logically in the described resource.</rdfs:comment>
        <skos2:corenote xml:lang="en">This term is intended to be used with non-literal values as defined in the DCMI Abstract Model (http://dublincore.org/documents/abstract-model/).  As of December 2007, the DCMI Usage Board is seeking a way to express this intention with a formal range declaration.</skos2:corenote>
        <dcterms:hasVersion rdf:resource="http://dublincore.org/usage/terms/history/#hasPart-003"/>
        <rdfs:subPropertyOf rdf:resource="&dc;relation"/>
        <rdfs:isDefinedBy rdf:resource="http://purl.org/dc/terms/"/>
        <rdfs:subPropertyOf rdf:resource="&dcterms;relation"/>
    </rdf:Description>
    


    <!-- http://purl.org/dc/terms/hasVersion -->

    <owl:AnnotationProperty rdf:about="&dcterms;hasVersion">
        <rdfs:label xml:lang="en">Has Version</rdfs:label>
        <dcterms:issued rdf:datatype="&xsd;date">2000-07-11</dcterms:issued>
        <dcterms:modified rdf:datatype="&xsd;date">2008-01-14</dcterms:modified>
        <rdfs:comment xml:lang="en">A related resource that is a version, edition, or adaptation of the described resource.</rdfs:comment>
        <skos2:corenote xml:lang="en">This term is intended to be used with non-literal values as defined in the DCMI Abstract Model (http://dublincore.org/documents/abstract-model/).  As of December 2007, the DCMI Usage Board is seeking a way to express this intention with a formal range declaration.</skos2:corenote>
        <dcterms:hasVersion rdf:resource="http://dublincore.org/usage/terms/history/#hasVersion-003"/>
        <rdfs:subPropertyOf rdf:resource="&dc;relation"/>
        <rdfs:isDefinedBy rdf:resource="http://purl.org/dc/terms/"/>
        <rdfs:subPropertyOf rdf:resource="&dcterms;relation"/>
    </owl:AnnotationProperty>
    


    <!-- http://purl.org/dc/terms/identifier -->

    <owl:AnnotationProperty rdf:about="&dcterms;identifier">
        <rdfs:label xml:lang="en">Identifier</rdfs:label>
        <dcterms:modified rdf:datatype="&xsd;date">2008-01-14</dcterms:modified>
        <dcterms:issued rdf:datatype="&xsd;date">2008-01-14</dcterms:issued>
        <rdfs:comment xml:lang="en">An unambiguous reference to the resource within a given context.</rdfs:comment>
        <dcterms:description xml:lang="en">Recommended best practice is to identify the resource by means of a string conforming to a formal identification system. </dcterms:description>
        <dcterms:hasVersion rdf:resource="http://dublincore.org/usage/terms/history/#identifierT-001"/>
        <rdfs:subPropertyOf rdf:resource="&dc;identifier"/>
        <rdfs:isDefinedBy rdf:resource="http://purl.org/dc/terms/"/>
    </owl:AnnotationProperty>
    


    <!-- http://purl.org/dc/terms/isFormatOf -->

    <owl:AnnotationProperty rdf:about="&dcterms;isFormatOf">
        <rdfs:label xml:lang="en">Is Format Of</rdfs:label>
        <dcterms:issued rdf:datatype="&xsd;date">2000-07-11</dcterms:issued>
        <dcterms:modified rdf:datatype="&xsd;date">2008-01-14</dcterms:modified>
        <rdfs:comment xml:lang="en">A related resource that is substantially the same as the described resource, but in another format.</rdfs:comment>
        <skos2:corenote xml:lang="en">This term is intended to be used with non-literal values as defined in the DCMI Abstract Model (http://dublincore.org/documents/abstract-model/).  As of December 2007, the DCMI Usage Board is seeking a way to express this intention with a formal range declaration.</skos2:corenote>
        <dcterms:hasVersion rdf:resource="http://dublincore.org/usage/terms/history/#isFormatOf-003"/>
        <rdfs:subPropertyOf rdf:resource="&dc;relation"/>
        <rdfs:isDefinedBy rdf:resource="http://purl.org/dc/terms/"/>
        <rdfs:subPropertyOf rdf:resource="&dcterms;relation"/>
    </owl:AnnotationProperty>
    


    <!-- http://purl.org/dc/terms/isPartOf -->

    <owl:AnnotationProperty rdf:about="&dcterms;isPartOf">
        <rdfs:label xml:lang="en">Is Part Of</rdfs:label>
        <dcterms:issued rdf:datatype="&xsd;date">2000-07-11</dcterms:issued>
        <dcterms:modified rdf:datatype="&xsd;date">2008-01-14</dcterms:modified>
        <rdfs:comment xml:lang="en">A related resource in which the described resource is physically or logically included.</rdfs:comment>
        <skos2:corenote xml:lang="en">This term is intended to be used with non-literal values as defined in the DCMI Abstract Model (http://dublincore.org/documents/abstract-model/).  As of December 2007, the DCMI Usage Board is seeking a way to express this intention with a formal range declaration.</skos2:corenote>
        <dcterms:hasVersion rdf:resource="http://dublincore.org/usage/terms/history/#isPartOf-003"/>
        <rdfs:subPropertyOf rdf:resource="&dc;relation"/>
        <rdfs:isDefinedBy rdf:resource="http://purl.org/dc/terms/"/>
        <rdfs:subPropertyOf rdf:resource="&dcterms;relation"/>
    </owl:AnnotationProperty>
    


    <!-- http://purl.org/dc/terms/isReferencedBy -->

    <owl:AnnotationProperty rdf:about="&dcterms;isReferencedBy">
        <rdfs:label xml:lang="en">Is Referenced By</rdfs:label>
        <dcterms:issued rdf:datatype="&xsd;date">2000-07-11</dcterms:issued>
        <dcterms:modified rdf:datatype="&xsd;date">2008-01-14</dcterms:modified>
        <rdfs:comment xml:lang="en">A related resource that references, cites, or otherwise points to the described resource.</rdfs:comment>
        <skos2:corenote xml:lang="en">This term is intended to be used with non-literal values as defined in the DCMI Abstract Model (http://dublincore.org/documents/abstract-model/).  As of December 2007, the DCMI Usage Board is seeking a way to express this intention with a formal range declaration.</skos2:corenote>
        <dcterms:hasVersion rdf:resource="http://dublincore.org/usage/terms/history/#isReferencedBy-003"/>
        <rdfs:subPropertyOf rdf:resource="&dc;relation"/>
        <rdfs:isDefinedBy rdf:resource="http://purl.org/dc/terms/"/>
        <rdfs:subPropertyOf rdf:resource="&dcterms;relation"/>
    </owl:AnnotationProperty>
    


    <!-- http://purl.org/dc/terms/isReplacedBy -->

    <rdf:Description rdf:about="&dcterms;isReplacedBy">
        <rdfs:label xml:lang="en">Is Replaced By</rdfs:label>
        <dcterms:issued rdf:datatype="&xsd;date">2000-07-11</dcterms:issued>
        <dcterms:modified rdf:datatype="&xsd;date">2008-01-14</dcterms:modified>
        <rdfs:comment xml:lang="en">A related resource that supplants, displaces, or supersedes the described resource.</rdfs:comment>
        <skos2:corenote xml:lang="en">This term is intended to be used with non-literal values as defined in the DCMI Abstract Model (http://dublincore.org/documents/abstract-model/).  As of December 2007, the DCMI Usage Board is seeking a way to express this intention with a formal range declaration.</skos2:corenote>
        <dcterms:hasVersion rdf:resource="http://dublincore.org/usage/terms/history/#isReplacedBy-003"/>
        <rdfs:subPropertyOf rdf:resource="&dc;relation"/>
        <rdfs:isDefinedBy rdf:resource="http://purl.org/dc/terms/"/>
        <rdfs:subPropertyOf rdf:resource="&dcterms;relation"/>
    </rdf:Description>
    


    <!-- http://purl.org/dc/terms/isRequiredBy -->

    <owl:AnnotationProperty rdf:about="&dcterms;isRequiredBy">
        <rdfs:label xml:lang="en">Is Required By</rdfs:label>
        <dcterms:issued rdf:datatype="&xsd;date">2000-07-11</dcterms:issued>
        <dcterms:modified rdf:datatype="&xsd;date">2008-01-14</dcterms:modified>
        <rdfs:comment xml:lang="en">A related resource that requires the described resource to support its function, delivery, or coherence.</rdfs:comment>
        <skos2:corenote xml:lang="en">This term is intended to be used with non-literal values as defined in the DCMI Abstract Model (http://dublincore.org/documents/abstract-model/).  As of December 2007, the DCMI Usage Board is seeking a way to express this intention with a formal range declaration.</skos2:corenote>
        <dcterms:hasVersion rdf:resource="http://dublincore.org/usage/terms/history/#isRequiredBy-003"/>
        <rdfs:subPropertyOf rdf:resource="&dc;relation"/>
        <rdfs:isDefinedBy rdf:resource="http://purl.org/dc/terms/"/>
        <rdfs:subPropertyOf rdf:resource="&dcterms;relation"/>
    </owl:AnnotationProperty>
    


    <!-- http://purl.org/dc/terms/isVersionOf -->

    <owl:AnnotationProperty rdf:about="&dcterms;isVersionOf">
        <rdfs:label xml:lang="en">Is Version Of</rdfs:label>
        <dcterms:issued rdf:datatype="&xsd;date">2000-07-11</dcterms:issued>
        <dcterms:modified rdf:datatype="&xsd;date">2008-01-14</dcterms:modified>
        <rdfs:comment xml:lang="en">A related resource of which the described resource is a version, edition, or adaptation.</rdfs:comment>
        <dcterms:description xml:lang="en">Changes in version imply substantive changes in content rather than differences in format.</dcterms:description>
        <skos2:corenote xml:lang="en">This term is intended to be used with non-literal values as defined in the DCMI Abstract Model (http://dublincore.org/documents/abstract-model/).  As of December 2007, the DCMI Usage Board is seeking a way to express this intention with a formal range declaration.</skos2:corenote>
        <dcterms:hasVersion rdf:resource="http://dublincore.org/usage/terms/history/#isVersionOf-003"/>
        <rdfs:subPropertyOf rdf:resource="&dc;relation"/>
        <rdfs:isDefinedBy rdf:resource="http://purl.org/dc/terms/"/>
        <rdfs:subPropertyOf rdf:resource="&dcterms;relation"/>
    </owl:AnnotationProperty>
    


    <!-- http://purl.org/dc/terms/issued -->

    <owl:AnnotationProperty rdf:about="&dcterms;issued">
        <rdfs:label xml:lang="en">Date Issued</rdfs:label>
        <dcterms:issued rdf:datatype="&xsd;date">2000-07-11</dcterms:issued>
        <dcterms:modified rdf:datatype="&xsd;date">2008-01-14</dcterms:modified>
        <rdfs:comment xml:lang="en">Date of formal issuance (e.g., publication) of the resource.</rdfs:comment>
        <dcterms:hasVersion rdf:resource="http://dublincore.org/usage/terms/history/#issued-003"/>
        <rdfs:isDefinedBy rdf:resource="http://purl.org/dc/terms/"/>
    </owl:AnnotationProperty>
    


    <!-- http://purl.org/dc/terms/language -->

    <owl:AnnotationProperty rdf:about="&dcterms;language">
        <rdfs:label xml:lang="en">Language</rdfs:label>
        <dcterms:issued rdf:datatype="&xsd;date">2008-01-14</dcterms:issued>
        <dcterms:modified rdf:datatype="&xsd;date">2008-01-14</dcterms:modified>
        <rdfs:comment xml:lang="en">A language of the resource.</rdfs:comment>
        <dcterms:description xml:lang="en">Recommended best practice is to use a controlled vocabulary such as RFC 4646 [RFC4646].</dcterms:description>
        <dcterms:hasVersion rdf:resource="http://dublincore.org/usage/terms/history/#languageT-001"/>
        <rdfs:subPropertyOf rdf:resource="&dc;language"/>
        <rdfs:isDefinedBy rdf:resource="http://purl.org/dc/terms/"/>
    </owl:AnnotationProperty>
    


    <!-- http://purl.org/dc/terms/license -->

    <owl:AnnotationProperty rdf:about="&dcterms;license">
        <rdfs:label xml:lang="en">License</rdfs:label>
        <dcterms:issued rdf:datatype="&xsd;date">2004-06-14</dcterms:issued>
        <dcterms:modified rdf:datatype="&xsd;date">2008-01-14</dcterms:modified>
        <rdfs:comment xml:lang="en">A legal document giving official permission to do something with the resource.</rdfs:comment>
        <dcterms:hasVersion rdf:resource="http://dublincore.org/usage/terms/history/#license-002"/>
        <rdfs:subPropertyOf rdf:resource="&dc;rights"/>
        <rdfs:isDefinedBy rdf:resource="http://purl.org/dc/terms/"/>
    </owl:AnnotationProperty>
    


    <!-- http://purl.org/dc/terms/mediator -->

    <owl:AnnotationProperty rdf:about="&dcterms;mediator">
        <rdfs:label xml:lang="en">Mediator</rdfs:label>
        <dcterms:issued rdf:datatype="&xsd;date">2001-05-21</dcterms:issued>
        <dcterms:modified rdf:datatype="&xsd;date">2008-01-14</dcterms:modified>
        <rdfs:comment xml:lang="en">An entity that mediates access to the resource and for whom the resource is intended or useful.</rdfs:comment>
        <dcterms:description xml:lang="en">In an educational context, a mediator might be a parent, teacher, teaching assistant, or care-giver.</dcterms:description>
        <dcterms:hasVersion rdf:resource="http://dublincore.org/usage/terms/history/#mediator-003"/>
        <rdfs:isDefinedBy rdf:resource="http://purl.org/dc/terms/"/>
    </owl:AnnotationProperty>
    


    <!-- http://purl.org/dc/terms/medium -->

    <owl:AnnotationProperty rdf:about="&dcterms;medium">
        <rdfs:label xml:lang="en">Medium</rdfs:label>
        <dcterms:issued rdf:datatype="&xsd;date">2000-07-11</dcterms:issued>
        <dcterms:modified rdf:datatype="&xsd;date">2008-01-14</dcterms:modified>
        <rdfs:comment xml:lang="en">The material or physical carrier of the resource.</rdfs:comment>
        <dcterms:hasVersion rdf:resource="http://dublincore.org/usage/terms/history/#medium-003"/>
        <rdfs:subPropertyOf rdf:resource="&dc;format"/>
        <rdfs:isDefinedBy rdf:resource="http://purl.org/dc/terms/"/>
    </owl:AnnotationProperty>
    


    <!-- http://purl.org/dc/terms/modified -->

    <owl:AnnotationProperty rdf:about="&dcterms;modified">
        <rdfs:label xml:lang="en">Date Modified</rdfs:label>
        <dcterms:issued rdf:datatype="&xsd;date">2000-07-11</dcterms:issued>
        <dcterms:modified rdf:datatype="&xsd;date">2008-01-14</dcterms:modified>
        <rdfs:comment xml:lang="en">Date on which the resource was changed.</rdfs:comment>
        <dcterms:hasVersion rdf:resource="http://dublincore.org/usage/terms/history/#modified-003"/>
        <rdfs:isDefinedBy rdf:resource="http://purl.org/dc/terms/"/>
    </owl:AnnotationProperty>
    


    <!-- http://purl.org/dc/terms/publisher -->

    <owl:AnnotationProperty rdf:about="&dcterms;publisher">
        <rdfs:label xml:lang="en">Publisher</rdfs:label>
        <dcterms:issued rdf:datatype="&xsd;date">2008-01-14</dcterms:issued>
        <dcterms:modified rdf:datatype="&xsd;date">2010-10-11</dcterms:modified>
        <rdfs:comment xml:lang="en">An entity responsible for making the resource available.</rdfs:comment>
        <dcterms:description xml:lang="en">Examples of a Publisher include a person, an organization, or a service.</dcterms:description>
        <dcterms:hasVersion rdf:resource="http://dublincore.org/usage/terms/history/#publisherT-001"/>
        <rdfs:subPropertyOf rdf:resource="&dc;publisher"/>
        <rdfs:isDefinedBy rdf:resource="http://purl.org/dc/terms/"/>
    </owl:AnnotationProperty>
    


    <!-- http://purl.org/dc/terms/references -->

    <owl:AnnotationProperty rdf:about="&dcterms;references">
        <rdfs:label xml:lang="en">References</rdfs:label>
        <dcterms:issued rdf:datatype="&xsd;date">2000-07-11</dcterms:issued>
        <dcterms:modified rdf:datatype="&xsd;date">2008-01-14</dcterms:modified>
        <rdfs:comment xml:lang="en">A related resource that is referenced, cited, or otherwise pointed to by the described resource.</rdfs:comment>
        <skos2:corenote xml:lang="en">This term is intended to be used with non-literal values as defined in the DCMI Abstract Model (http://dublincore.org/documents/abstract-model/).  As of December 2007, the DCMI Usage Board is seeking a way to express this intention with a formal range declaration.</skos2:corenote>
        <dcterms:hasVersion rdf:resource="http://dublincore.org/usage/terms/history/#references-003"/>
        <rdfs:subPropertyOf rdf:resource="&dc;relation"/>
        <rdfs:isDefinedBy rdf:resource="http://purl.org/dc/terms/"/>
        <rdfs:subPropertyOf rdf:resource="&dcterms;relation"/>
    </owl:AnnotationProperty>
    


    <!-- http://purl.org/dc/terms/relation -->

    <owl:AnnotationProperty rdf:about="&dcterms;relation">
        <rdfs:label xml:lang="en">Relation</rdfs:label>
        <dcterms:issued rdf:datatype="&xsd;date">2008-01-14</dcterms:issued>
        <dcterms:modified rdf:datatype="&xsd;date">2008-01-14</dcterms:modified>
        <rdfs:comment xml:lang="en">A related resource.</rdfs:comment>
        <dcterms:description xml:lang="en">Recommended best practice is to identify the related resource by means of a string conforming to a formal identification system. </dcterms:description>
        <skos2:corenote xml:lang="en">This term is intended to be used with non-literal values as defined in the DCMI Abstract Model (http://dublincore.org/documents/abstract-model/).  As of December 2007, the DCMI Usage Board is seeking a way to express this intention with a formal range declaration.</skos2:corenote>
        <dcterms:hasVersion rdf:resource="http://dublincore.org/usage/terms/history/#relationT-001"/>
        <rdfs:subPropertyOf rdf:resource="&dc;relation"/>
        <rdfs:isDefinedBy rdf:resource="http://purl.org/dc/terms/"/>
    </owl:AnnotationProperty>
    


    <!-- http://purl.org/dc/terms/replaces -->

    <rdf:Description rdf:about="&dcterms;replaces">
        <rdfs:label xml:lang="en">Replaces</rdfs:label>
        <dcterms:issued rdf:datatype="&xsd;date">2000-07-11</dcterms:issued>
        <dcterms:modified rdf:datatype="&xsd;date">2008-01-14</dcterms:modified>
        <rdfs:comment xml:lang="en">A related resource that is supplanted, displaced, or superseded by the described resource.</rdfs:comment>
        <skos2:corenote xml:lang="en">This term is intended to be used with non-literal values as defined in the DCMI Abstract Model (http://dublincore.org/documents/abstract-model/).  As of December 2007, the DCMI Usage Board is seeking a way to express this intention with a formal range declaration.</skos2:corenote>
        <dcterms:hasVersion rdf:resource="http://dublincore.org/usage/terms/history/#replaces-003"/>
        <rdfs:subPropertyOf rdf:resource="&dc;relation"/>
        <rdfs:isDefinedBy rdf:resource="http://purl.org/dc/terms/"/>
        <rdfs:subPropertyOf rdf:resource="&dcterms;relation"/>
    </rdf:Description>
    


    <!-- http://purl.org/dc/terms/requires -->

    <owl:AnnotationProperty rdf:about="&dcterms;requires">
        <rdfs:label xml:lang="en">Requires</rdfs:label>
        <dcterms:issued rdf:datatype="&xsd;date">2000-07-11</dcterms:issued>
        <dcterms:modified rdf:datatype="&xsd;date">2008-01-14</dcterms:modified>
        <rdfs:comment xml:lang="en">A related resource that is required by the described resource to support its function, delivery, or coherence.</rdfs:comment>
        <skos2:corenote xml:lang="en">This term is intended to be used with non-literal values as defined in the DCMI Abstract Model (http://dublincore.org/documents/abstract-model/).  As of December 2007, the DCMI Usage Board is seeking a way to express this intention with a formal range declaration.</skos2:corenote>
        <dcterms:hasVersion rdf:resource="http://dublincore.org/usage/terms/history/#requires-003"/>
        <rdfs:subPropertyOf rdf:resource="&dc;relation"/>
        <rdfs:isDefinedBy rdf:resource="http://purl.org/dc/terms/"/>
        <rdfs:subPropertyOf rdf:resource="&dcterms;relation"/>
    </owl:AnnotationProperty>
    


    <!-- http://purl.org/dc/terms/rights -->

    <owl:AnnotationProperty rdf:about="&dcterms;rights">
        <rdfs:label xml:lang="en">Rights</rdfs:label>
        <dcterms:modified rdf:datatype="&xsd;date">2008-01-14</dcterms:modified>
        <dcterms:issued rdf:datatype="&xsd;date">2008-01-14</dcterms:issued>
        <rdfs:comment xml:lang="en">Information about rights held in and over the resource.</rdfs:comment>
        <dcterms:description xml:lang="en">Typically, rights information includes a statement about various property rights associated with the resource, including intellectual property rights.</dcterms:description>
        <dcterms:hasVersion rdf:resource="http://dublincore.org/usage/terms/history/#rightsT-001"/>
        <rdfs:subPropertyOf rdf:resource="&dc;rights"/>
        <rdfs:isDefinedBy rdf:resource="http://purl.org/dc/terms/"/>
    </owl:AnnotationProperty>
    


    <!-- http://purl.org/dc/terms/source -->

    <owl:AnnotationProperty rdf:about="&dcterms;source">
        <rdfs:label xml:lang="en">Source</rdfs:label>
        <dcterms:modified rdf:datatype="&xsd;date">2008-01-14</dcterms:modified>
        <dcterms:issued rdf:datatype="&xsd;date">2008-01-14</dcterms:issued>
        <rdfs:comment xml:lang="en">A related resource from which the described resource is derived.</rdfs:comment>
        <dcterms:description xml:lang="en">The described resource may be derived from the related resource in whole or in part. Recommended best practice is to identify the related resource by means of a string conforming to a formal identification system.</dcterms:description>
        <skos2:corenote xml:lang="en">This term is intended to be used with non-literal values as defined in the DCMI Abstract Model (http://dublincore.org/documents/abstract-model/).  As of December 2007, the DCMI Usage Board is seeking a way to express this intention with a formal range declaration.</skos2:corenote>
        <dcterms:hasVersion rdf:resource="http://dublincore.org/usage/terms/history/#sourceT-001"/>
        <rdfs:subPropertyOf rdf:resource="&dc;source"/>
        <rdfs:isDefinedBy rdf:resource="http://purl.org/dc/terms/"/>
        <rdfs:subPropertyOf rdf:resource="&dcterms;relation"/>
    </owl:AnnotationProperty>
    


    <!-- http://purl.org/dc/terms/spatial -->

    <owl:AnnotationProperty rdf:about="&dcterms;spatial">
        <rdfs:label xml:lang="en">Spatial Coverage</rdfs:label>
        <dcterms:issued rdf:datatype="&xsd;date">2000-07-11</dcterms:issued>
        <dcterms:modified rdf:datatype="&xsd;date">2008-01-14</dcterms:modified>
        <rdfs:comment xml:lang="en">Spatial characteristics of the resource.</rdfs:comment>
        <dcterms:hasVersion rdf:resource="http://dublincore.org/usage/terms/history/#spatial-003"/>
        <rdfs:subPropertyOf rdf:resource="&dc;coverage"/>
        <rdfs:isDefinedBy rdf:resource="http://purl.org/dc/terms/"/>
    </owl:AnnotationProperty>
    


    <!-- http://purl.org/dc/terms/subject -->

    <owl:AnnotationProperty rdf:about="&dcterms;subject">
        <rdfs:label xml:lang="en">Subject</rdfs:label>
        <dcterms:issued rdf:datatype="&xsd;date">2008-01-14</dcterms:issued>
        <dcterms:modified rdf:datatype="&xsd;date">2012-06-14</dcterms:modified>
        <rdfs:comment xml:lang="en">The topic of the resource.</rdfs:comment>
        <skos2:corenote xml:lang="en">This term is intended to be used with non-literal values as defined in the DCMI Abstract Model (http://dublincore.org/documents/abstract-model/).  As of December 2007, the DCMI Usage Board is seeking a way to express this intention with a formal range declaration.</skos2:corenote>
        <dcterms:description xml:lang="en">Typically, the subject will be represented using keywords, key phrases, or classification codes. Recommended best practice is to use a controlled vocabulary.</dcterms:description>
        <dcterms:hasVersion rdf:resource="http://dublincore.org/usage/terms/history/#subjectT-002"/>
        <rdfs:subPropertyOf rdf:resource="&dc;subject"/>
        <rdfs:isDefinedBy rdf:resource="http://purl.org/dc/terms/"/>
    </owl:AnnotationProperty>
    


    <!-- http://purl.org/dc/terms/tableOfContents -->

    <owl:AnnotationProperty rdf:about="&dcterms;tableOfContents">
        <rdfs:label xml:lang="en">Table Of Contents</rdfs:label>
        <dcterms:issued rdf:datatype="&xsd;date">2000-07-11</dcterms:issued>
        <dcterms:modified rdf:datatype="&xsd;date">2008-01-14</dcterms:modified>
        <rdfs:comment xml:lang="en">A list of subunits of the resource.</rdfs:comment>
        <dcterms:hasVersion rdf:resource="http://dublincore.org/usage/terms/history/#tableOfContents-003"/>
        <rdfs:subPropertyOf rdf:resource="&dc;description"/>
        <rdfs:isDefinedBy rdf:resource="http://purl.org/dc/terms/"/>
        <rdfs:subPropertyOf rdf:resource="&dcterms;description"/>
    </owl:AnnotationProperty>
    


    <!-- http://purl.org/dc/terms/temporal -->

    <owl:AnnotationProperty rdf:about="&dcterms;temporal">
        <rdfs:label xml:lang="en">Temporal Coverage</rdfs:label>
        <dcterms:issued rdf:datatype="&xsd;date">2000-07-11</dcterms:issued>
        <dcterms:modified rdf:datatype="&xsd;date">2008-01-14</dcterms:modified>
        <rdfs:comment xml:lang="en">Temporal characteristics of the resource.</rdfs:comment>
        <dcterms:hasVersion rdf:resource="http://dublincore.org/usage/terms/history/#temporal-003"/>
        <rdfs:subPropertyOf rdf:resource="&dc;coverage"/>
        <rdfs:isDefinedBy rdf:resource="http://purl.org/dc/terms/"/>
    </owl:AnnotationProperty>
    


    <!-- http://purl.org/dc/terms/title -->

    <owl:AnnotationProperty rdf:about="&dcterms;title">
        <rdfs:label xml:lang="en">Title</rdfs:label>
        <dcterms:issued rdf:datatype="&xsd;date">2008-01-14</dcterms:issued>
        <dcterms:modified rdf:datatype="&xsd;date">2010-10-11</dcterms:modified>
        <rdfs:comment xml:lang="en">A name given to the resource.</rdfs:comment>
        <dcterms:hasVersion rdf:resource="http://dublincore.org/usage/terms/history/#titleT-002"/>
        <rdfs:isDefinedBy rdf:resource="http://purl.org/dc/terms/"/>
    </owl:AnnotationProperty>
    


    <!-- http://purl.org/dc/terms/type -->

    <owl:AnnotationProperty rdf:about="&dcterms;type">
        <rdfs:label xml:lang="en">Type</rdfs:label>
        <dcterms:issued rdf:datatype="&xsd;date">2008-01-14</dcterms:issued>
        <dcterms:modified rdf:datatype="&xsd;date">2008-01-14</dcterms:modified>
        <dcterms:description xml:lang="en">Recommended best practice is to use a controlled vocabulary such as the DCMI Type Vocabulary [DCMITYPE]. To describe the file format, physical medium, or dimensions of the resource, use the Format element.</dcterms:description>
        <rdfs:comment xml:lang="en">The nature or genre of the resource.</rdfs:comment>
        <dcterms:hasVersion rdf:resource="http://dublincore.org/usage/terms/history/#typeT-001"/>
        <rdfs:subPropertyOf rdf:resource="&dc;type"/>
        <rdfs:isDefinedBy rdf:resource="http://purl.org/dc/terms/"/>
    </owl:AnnotationProperty>
    


    <!-- http://purl.org/dc/terms/valid -->

    <owl:AnnotationProperty rdf:about="&dcterms;valid">
        <rdfs:label xml:lang="en">Date Valid</rdfs:label>
        <dcterms:issued rdf:datatype="&xsd;date">2000-07-11</dcterms:issued>
        <dcterms:modified rdf:datatype="&xsd;date">2008-01-14</dcterms:modified>
        <rdfs:comment xml:lang="en">Date (often a range) of validity of a resource.</rdfs:comment>
        <dcterms:hasVersion rdf:resource="http://dublincore.org/usage/terms/history/#valid-003"/>
        <rdfs:isDefinedBy rdf:resource="http://purl.org/dc/terms/"/>
    </owl:AnnotationProperty>
    


    <!-- http://www.loc.gov/mads/rdf/v1#adminMetadata -->

    <owl:AnnotationProperty rdf:about="&v1;adminMetadata"/>
    


    <!-- http://www.loc.gov/mads/rdf/v1#authoritativeLabel -->

    <owl:AnnotationProperty rdf:about="&v1;authoritativeLabel"/>
    


    <!-- http://www.loc.gov/mads/rdf/v1#code -->

    <owl:AnnotationProperty rdf:about="&v1;code"/>
    


    <!-- http://www.loc.gov/mads/rdf/v1#definitionNote -->

    <owl:AnnotationProperty rdf:about="&v1;definitionNote"/>
    


    <!-- http://www.loc.gov/mads/rdf/v1#editorialNote -->

    <owl:AnnotationProperty rdf:about="&v1;editorialNote"/>
    


    <!-- http://www.loc.gov/mads/rdf/v1#hasVariant -->

    <owl:AnnotationProperty rdf:about="&v1;hasVariant"/>
    


    <!-- http://www.loc.gov/mads/rdf/v1#isMemberOfMADSCollection -->

    <owl:AnnotationProperty rdf:about="&v1;isMemberOfMADSCollection"/>
    


    <!-- http://www.loc.gov/mads/rdf/v1#isMemberOfMADSScheme -->

    <owl:AnnotationProperty rdf:about="&v1;isMemberOfMADSScheme"/>
    


    <!-- http://www.w3.org/2004/02/skos/corenote -->

    <owl:AnnotationProperty rdf:about="&skos2;corenote"/>
    


    <!-- 
    ///////////////////////////////////////////////////////////////////////////////////////
    //
    // Datatypes
    //
    ///////////////////////////////////////////////////////////////////////////////////////
     -->

    


    <!-- http://purl.org/dc/terms/Box -->

    <rdfs:Datatype rdf:about="&dcterms;Box">
        <rdfs:label xml:lang="en">DCMI Box</rdfs:label>
        <dcterms:issued rdf:datatype="&xsd;date">2000-07-11</dcterms:issued>
        <dcterms:modified rdf:datatype="&xsd;date">2008-01-14</dcterms:modified>
        <rdfs:comment xml:lang="en">The set of regions in space defined by their geographic coordinates according to the DCMI Box Encoding Scheme.</rdfs:comment>
        <rdfs:seeAlso rdf:resource="http://dublincore.org/documents/dcmi-box/"/>
        <dcterms:hasVersion rdf:resource="http://dublincore.org/usage/terms/history/#Box-003"/>
        <rdfs:isDefinedBy rdf:resource="http://purl.org/dc/terms/"/>
    </rdfs:Datatype>
    


    <!-- http://purl.org/dc/terms/ISO3166 -->

    <rdfs:Datatype rdf:about="&dcterms;ISO3166">
        <rdfs:label xml:lang="en">ISO 3166</rdfs:label>
        <dcterms:issued rdf:datatype="&xsd;date">2000-07-11</dcterms:issued>
        <dcterms:modified rdf:datatype="&xsd;date">2008-01-14</dcterms:modified>
        <rdfs:comment xml:lang="en">The set of codes listed in ISO 3166-1 for the representation of names of countries.</rdfs:comment>
        <dcterms:hasVersion rdf:resource="http://dublincore.org/usage/terms/history/#ISO3166-004"/>
        <rdfs:isDefinedBy rdf:resource="http://purl.org/dc/terms/"/>
        <rdfs:seeAlso rdf:resource="http://www.iso.org/iso/en/prods-services/iso3166ma/02iso-3166-code-lists/list-en1.html"/>
    </rdfs:Datatype>
    


    <!-- http://purl.org/dc/terms/ISO639-2 -->

    <rdfs:Datatype rdf:about="&dcterms;ISO639-2">
        <rdfs:label xml:lang="en">ISO 639-2</rdfs:label>
        <dcterms:issued rdf:datatype="&xsd;date">2000-07-11</dcterms:issued>
        <dcterms:modified rdf:datatype="&xsd;date">2008-01-14</dcterms:modified>
        <rdfs:comment xml:lang="en">The three-letter alphabetic codes listed in ISO639-2 for the representation of names of languages.</rdfs:comment>
        <dcterms:hasVersion rdf:resource="http://dublincore.org/usage/terms/history/#ISO639-2-003"/>
        <rdfs:seeAlso rdf:resource="http://lcweb.loc.gov/standards/iso639-2/langhome.html"/>
        <rdfs:isDefinedBy rdf:resource="http://purl.org/dc/terms/"/>
    </rdfs:Datatype>
    


    <!-- http://purl.org/dc/terms/ISO639-3 -->

    <rdfs:Datatype rdf:about="&dcterms;ISO639-3">
        <rdfs:label xml:lang="en">ISO 639-3</rdfs:label>
        <dcterms:issued rdf:datatype="&xsd;date">2008-01-14</dcterms:issued>
        <rdfs:comment xml:lang="en">The set of three-letter codes listed in ISO 639-3 for the representation of names of languages.</rdfs:comment>
        <dcterms:hasVersion rdf:resource="http://dublincore.org/usage/terms/history/#ISO639-3-001"/>
        <rdfs:isDefinedBy rdf:resource="http://purl.org/dc/terms/"/>
        <rdfs:seeAlso rdf:resource="http://www.sil.org/iso639-3/"/>
    </rdfs:Datatype>
    


    <!-- http://purl.org/dc/terms/Period -->

    <rdfs:Datatype rdf:about="&dcterms;Period">
        <rdfs:label xml:lang="en">DCMI Period</rdfs:label>
        <dcterms:issued rdf:datatype="&xsd;date">2000-07-11</dcterms:issued>
        <dcterms:modified rdf:datatype="&xsd;date">2008-01-14</dcterms:modified>
        <rdfs:comment xml:lang="en">The set of time intervals defined by their limits according to the DCMI Period Encoding Scheme.</rdfs:comment>
        <rdfs:seeAlso rdf:resource="http://dublincore.org/documents/dcmi-period/"/>
        <dcterms:hasVersion rdf:resource="http://dublincore.org/usage/terms/history/#Period-003"/>
        <rdfs:isDefinedBy rdf:resource="http://purl.org/dc/terms/"/>
    </rdfs:Datatype>
    


    <!-- http://purl.org/dc/terms/Point -->

    <rdfs:Datatype rdf:about="&dcterms;Point">
        <rdfs:label xml:lang="en">DCMI Point</rdfs:label>
        <dcterms:issued rdf:datatype="&xsd;date">2000-07-11</dcterms:issued>
        <dcterms:modified rdf:datatype="&xsd;date">2008-01-14</dcterms:modified>
        <rdfs:comment xml:lang="en">The set of points in space defined by their geographic coordinates according to the DCMI Point Encoding Scheme.</rdfs:comment>
        <rdfs:seeAlso rdf:resource="http://dublincore.org/documents/dcmi-point/"/>
        <dcterms:hasVersion rdf:resource="http://dublincore.org/usage/terms/history/#Point-003"/>
        <rdfs:isDefinedBy rdf:resource="http://purl.org/dc/terms/"/>
    </rdfs:Datatype>
    


    <!-- http://purl.org/dc/terms/RFC1766 -->

    <rdfs:Datatype rdf:about="&dcterms;RFC1766">
        <rdfs:label xml:lang="en">RFC 1766</rdfs:label>
        <dcterms:issued rdf:datatype="&xsd;date">2000-07-11</dcterms:issued>
        <dcterms:modified rdf:datatype="&xsd;date">2008-01-14</dcterms:modified>
        <rdfs:comment xml:lang="en">The set of tags, constructed according to RFC 1766, for the identification of languages.</rdfs:comment>
        <dcterms:hasVersion rdf:resource="http://dublincore.org/usage/terms/history/#RFC1766-003"/>
        <rdfs:isDefinedBy rdf:resource="http://purl.org/dc/terms/"/>
        <rdfs:seeAlso rdf:resource="http://www.ietf.org/rfc/rfc1766.txt"/>
    </rdfs:Datatype>
    


    <!-- http://purl.org/dc/terms/RFC3066 -->

    <rdfs:Datatype rdf:about="&dcterms;RFC3066">
        <rdfs:label xml:lang="en">RFC 3066</rdfs:label>
        <dcterms:issued rdf:datatype="&xsd;date">2002-07-13</dcterms:issued>
        <dcterms:modified rdf:datatype="&xsd;date">2008-01-14</dcterms:modified>
        <dcterms:description xml:lang="en">RFC 3066 has been obsoleted by RFC 4646.</dcterms:description>
        <rdfs:comment xml:lang="en">The set of tags constructed according to RFC 3066 for the identification of languages.</rdfs:comment>
        <dcterms:hasVersion rdf:resource="http://dublincore.org/usage/terms/history/#RFC3066-002"/>
        <rdfs:isDefinedBy rdf:resource="http://purl.org/dc/terms/"/>
        <rdfs:seeAlso rdf:resource="http://www.ietf.org/rfc/rfc3066.txt"/>
    </rdfs:Datatype>
    


    <!-- http://purl.org/dc/terms/RFC4646 -->

    <rdfs:Datatype rdf:about="&dcterms;RFC4646">
        <rdfs:label xml:lang="en">RFC 4646</rdfs:label>
        <dcterms:issued rdf:datatype="&xsd;date">2008-01-14</dcterms:issued>
        <dcterms:description xml:lang="en">RFC 4646 obsoletes RFC 3066.</dcterms:description>
        <rdfs:comment xml:lang="en">The set of tags constructed according to RFC 4646 for the identification of languages.</rdfs:comment>
        <dcterms:hasVersion rdf:resource="http://dublincore.org/usage/terms/history/#RFC4646-001"/>
        <rdfs:isDefinedBy rdf:resource="http://purl.org/dc/terms/"/>
        <rdfs:seeAlso rdf:resource="http://www.ietf.org/rfc/rfc4646.txt"/>
    </rdfs:Datatype>
    


    <!-- http://purl.org/dc/terms/RFC5646 -->

    <rdfs:Datatype rdf:about="&dcterms;RFC5646">
        <rdfs:label xml:lang="en">RFC 5646</rdfs:label>
        <dcterms:issued rdf:datatype="&xsd;date">2010-10-11</dcterms:issued>
        <dcterms:description xml:lang="en">RFC 5646 obsoletes RFC 4646.</dcterms:description>
        <rdfs:comment xml:lang="en">The set of tags constructed according to RFC 5646 for the identification of languages.</rdfs:comment>
        <dcterms:hasVersion rdf:resource="http://dublincore.org/usage/terms/history/#RFC5646-001"/>
        <rdfs:isDefinedBy rdf:resource="http://purl.org/dc/terms/"/>
        <rdfs:seeAlso rdf:resource="http://www.ietf.org/rfc/rfc5646.txt"/>
    </rdfs:Datatype>
    


    <!-- http://purl.org/dc/terms/URI -->

    <rdfs:Datatype rdf:about="&dcterms;URI">
        <rdfs:label xml:lang="en">URI</rdfs:label>
        <dcterms:issued rdf:datatype="&xsd;date">2000-07-11</dcterms:issued>
        <dcterms:modified rdf:datatype="&xsd;date">2008-01-14</dcterms:modified>
        <rdfs:comment xml:lang="en">The set of identifiers constructed according to the generic syntax for Uniform Resource Identifiers as specified by the Internet Engineering Task Force.</rdfs:comment>
        <dcterms:hasVersion rdf:resource="http://dublincore.org/usage/terms/history/#URI-003"/>
        <rdfs:isDefinedBy rdf:resource="http://purl.org/dc/terms/"/>
        <rdfs:seeAlso rdf:resource="http://www.ietf.org/rfc/rfc3986.txt"/>
    </rdfs:Datatype>
    


    <!-- http://purl.org/dc/terms/W3CDTF -->

    <rdfs:Datatype rdf:about="&dcterms;W3CDTF">
        <rdfs:label xml:lang="en">W3C-DTF</rdfs:label>
        <dcterms:issued rdf:datatype="&xsd;date">2000-07-11</dcterms:issued>
        <dcterms:modified rdf:datatype="&xsd;date">2008-01-14</dcterms:modified>
        <rdfs:comment xml:lang="en">The set of dates and times constructed according to the W3C Date and Time Formats Specification.</rdfs:comment>
        <dcterms:hasVersion rdf:resource="http://dublincore.org/usage/terms/history/#W3CDTF-003"/>
        <rdfs:isDefinedBy rdf:resource="http://purl.org/dc/terms/"/>
        <rdfs:seeAlso rdf:resource="http://www.w3.org/TR/NOTE-datetime"/>
    </rdfs:Datatype>
    


    <!-- 
    ///////////////////////////////////////////////////////////////////////////////////////
    //
    // Object Properties
    //
    ///////////////////////////////////////////////////////////////////////////////////////
     -->

    


    <!-- http://bibframe.org/vocab/abbreviatedTitle -->

    <owl:ObjectProperty rdf:about="http://bibframe.org/vocab/abbreviatedTitle">
        <rdfs:label>Abbreviated title</rdfs:label>
        <rdfs:comment>Title as abbreviated for indexing or identification.</rdfs:comment>
        <rdfs:domain rdf:resource="http://bibframe.org/vocab/Instance"/>
        <rdfs:range rdf:resource="http://bibframe.org/vocab/Title"/>
        <rdfs:subPropertyOf rdf:resource="http://bibframe.org/vocab/instanceTitle"/>
    </owl:ObjectProperty>
    


    <!-- http://bibframe.org/vocab/absorbed -->

    <owl:ObjectProperty rdf:about="http://bibframe.org/vocab/absorbed">
        <rdfs:label>Absorbed</rdfs:label>
        <rdfs:comment>Work that has been incorporated into another Work</rdfs:comment>
        <dcterms:modified>2014-04-10 (Updated subproperty)</dcterms:modified>
        <rdfs:range rdf:resource="http://bibframe.org/vocab/Work"/>
        <rdfs:domain rdf:resource="http://bibframe.org/vocab/Work"/>
        <rdfs:subPropertyOf rdf:resource="http://bibframe.org/vocab/precededBy"/>
    </owl:ObjectProperty>
    


    <!-- http://bibframe.org/vocab/absorbedBy -->

    <owl:ObjectProperty rdf:about="http://bibframe.org/vocab/absorbedBy">
        <rdfs:label>Absorbed by</rdfs:label>
        <dcterms:modified>2014-04-10 (Updated subproperty)</dcterms:modified>
        <rdfs:comment>Work that incorporates another work.</rdfs:comment>
        <rdfs:range rdf:resource="http://bibframe.org/vocab/Work"/>
        <rdfs:domain rdf:resource="http://bibframe.org/vocab/Work"/>
        <owl:inverseOf rdf:resource="http://bibframe.org/vocab/absorbed"/>
        <rdfs:subPropertyOf rdf:resource="http://bibframe.org/vocab/succeededBy"/>
    </owl:ObjectProperty>
    


    <!-- http://bibframe.org/vocab/absorbedInPart -->

    <owl:ObjectProperty rdf:about="http://bibframe.org/vocab/absorbedInPart">
        <rdfs:label>Absorbed in part</rdfs:label>
        <rdfs:comment>Work that has been partially incorporated into another work.</rdfs:comment>
        <dcterms:modified>2014-04-10 (Updated subproperty)</dcterms:modified>
        <rdfs:range rdf:resource="http://bibframe.org/vocab/Work"/>
        <rdfs:domain rdf:resource="http://bibframe.org/vocab/Work"/>
        <rdfs:subPropertyOf rdf:resource="http://bibframe.org/vocab/precededBy"/>
    </owl:ObjectProperty>
    


    <!-- http://bibframe.org/vocab/absorbedInPartBy -->

    <owl:ObjectProperty rdf:about="http://bibframe.org/vocab/absorbedInPartBy">
        <rdfs:label>Absorbed in part by</rdfs:label>
        <dcterms:modified>2014-04-10 (Updated subproperty)</dcterms:modified>
        <rdfs:comment>Work that incorporates part of the content of another work.</rdfs:comment>
        <rdfs:domain rdf:resource="http://bibframe.org/vocab/Work"/>
        <rdfs:range rdf:resource="http://bibframe.org/vocab/Work"/>
        <owl:inverseOf rdf:resource="http://bibframe.org/vocab/absorbedInPart"/>
        <rdfs:subPropertyOf rdf:resource="http://bibframe.org/vocab/succeededBy"/>
    </owl:ObjectProperty>
    


    <!-- http://bibframe.org/vocab/accompaniedBy -->

    <owl:ObjectProperty rdf:about="http://bibframe.org/vocab/accompaniedBy">
        <rdfs:label>Accompanied by</rdfs:label>
        <dcterms:modified>2014-04-10 (Range updated)</dcterms:modified>
        <rdfs:comment>Resource that has an accompanying resource which adds to it</rdfs:comment>
        <owl:inverseOf rdf:resource="http://bibframe.org/vocab/accompanies"/>
        <rdfs:subPropertyOf rdf:resource="http://bibframe.org/vocab/relatedTo"/>
    </owl:ObjectProperty>
    


    <!-- http://bibframe.org/vocab/accompanies -->

    <owl:ObjectProperty rdf:about="http://bibframe.org/vocab/accompanies">
        <rdfs:label>Accompanies</rdfs:label>
        <rdfs:comment>Resource that adds to or is issued with the described resource</rdfs:comment>
        <dcterms:modified>2014-04-10 (Range updated)</dcterms:modified>
        <rdfs:subPropertyOf rdf:resource="http://bibframe.org/vocab/relatedTo"/>
    </owl:ObjectProperty>
    


    <!-- http://bibframe.org/vocab/agent -->

    <owl:ObjectProperty rdf:about="http://bibframe.org/vocab/agent">
        <rdfs:label>Associated agent</rdfs:label>
        <rdfs:comment>Entity associated with a resource or element of description</rdfs:comment>
    </owl:ObjectProperty>
    


    <!-- http://bibframe.org/vocab/agentOf -->

    <owl:ObjectProperty rdf:about="http://bibframe.org/vocab/agentOf">
        <rdfs:label>agent of</rdfs:label>
        <rdfs:comment>Relates an Authority to a Resource it is associated with.</rdfs:comment>
        <owl:inverseOf rdf:resource="http://bibframe.org/vocab/agent"/>
    </owl:ObjectProperty>
    


    <!-- http://bibframe.org/vocab/annotates -->

    <owl:ObjectProperty rdf:about="http://bibframe.org/vocab/annotates">
        <rdfs:label>Target of Annotation</rdfs:label>
        <rdfs:comment>Resource to which the annotation relates.</rdfs:comment>
        <rdfs:range rdf:resource="&rdfs;Resource"/>
    </owl:ObjectProperty>
    


    <!-- http://bibframe.org/vocab/annotationAssertedBy -->

    <owl:ObjectProperty rdf:about="http://bibframe.org/vocab/annotationAssertedBy">
        <rdfs:label>Annotation asserted by</rdfs:label>
        <rdfs:comment>Annotation was asserted by the given entity.</rdfs:comment>
    </owl:ObjectProperty>
    


    <!-- http://bibframe.org/vocab/annotationBody -->

    <owl:ObjectProperty rdf:about="http://bibframe.org/vocab/annotationBody">
        <rdfs:label>Annotation Body</rdfs:label>
        <rdfs:comment>Content of the annotation about the resource.</rdfs:comment>
        <rdfs:range rdf:resource="&rdfs;Resource"/>
    </owl:ObjectProperty>
    


    <!-- http://bibframe.org/vocab/annotationSource -->

    <owl:ObjectProperty rdf:about="http://bibframe.org/vocab/annotationSource">
        <rdfs:label>Annotation Source</rdfs:label>
        <rdfs:comment>Source of the annotation.</rdfs:comment>
    </owl:ObjectProperty>
    


    <!-- http://bibframe.org/vocab/ansi -->

    <owl:ObjectProperty rdf:about="http://bibframe.org/vocab/ansi">
        <rdfs:label>ANSI number</rdfs:label>
        <rdfs:comment>American National Standards Institute identifier.</rdfs:comment>
        <rdfs:range rdf:resource="http://bibframe.org/vocab/Identifier"/>
        <rdfs:domain rdf:resource="http://bibframe.org/vocab/Instance"/>
        <rdfs:subPropertyOf rdf:resource="http://bibframe.org/vocab/identifier"/>
    </owl:ObjectProperty>
    


    <!-- http://bibframe.org/vocab/arrangement -->

    <owl:ObjectProperty rdf:about="http://bibframe.org/vocab/arrangement">
        <rdfs:label>Organization and Arrangement</rdfs:label>
        <rdfs:comment>Information about the organization and arrangement of a collection of resources.</rdfs:comment>
        <rdfs:range rdf:resource="http://bibframe.org/vocab/Arrangement"/>
        <rdfs:domain rdf:resource="http://bibframe.org/vocab/Instance"/>
    </owl:ObjectProperty>
    


    <!-- http://bibframe.org/vocab/arrangementOf -->

    <owl:ObjectProperty rdf:about="http://bibframe.org/vocab/arrangementOf">
        <rdfs:label>arrangement of</rdfs:label>
        <rdfs:comment>Relates an Arrangement to an Instance it is an arrangement of.</rdfs:comment>
        <rdfs:domain rdf:resource="http://bibframe.org/vocab/Arrangement"/>
        <rdfs:range rdf:resource="http://bibframe.org/vocab/Instance"/>
        <owl:inverseOf rdf:resource="http://bibframe.org/vocab/arrangement"/>
    </owl:ObjectProperty>
    


    <!-- http://bibframe.org/vocab/authorityAssigner -->

    <owl:ObjectProperty rdf:about="http://bibframe.org/vocab/authorityAssigner">
        <rdfs:label>Authority assigner</rdfs:label>
        <rdfs:comment>Entity that assigned the information.</rdfs:comment>
    </owl:ObjectProperty>
    


    <!-- http://bibframe.org/vocab/authorityFor -->

    <owl:ObjectProperty rdf:about="http://bibframe.org/vocab/authorityFor">
        <rdfs:label>authority for</rdfs:label>
        <rdfs:comment>Links an external Authority to a bf:Authority.</rdfs:comment>
        <owl:inverseOf rdf:resource="http://bibframe.org/vocab/hasAuthority"/>
    </owl:ObjectProperty>
    


    <!-- http://bibframe.org/vocab/carrierCategory -->

    <owl:ObjectProperty rdf:about="http://bibframe.org/vocab/carrierCategory">
        <rdfs:label>Carrier type</rdfs:label>
        <rdfs:comment>Categorization reflecting the format of the storage medium and housing of a carrier.</rdfs:comment>
        <rdfs:range rdf:resource="http://bibframe.org/vocab/Category"/>
        <rdfs:domain rdf:resource="http://bibframe.org/vocab/Instance"/>
    </owl:ObjectProperty>
    


    <!-- http://bibframe.org/vocab/carrierCategoryOf -->

    <owl:ObjectProperty rdf:about="http://bibframe.org/vocab/carrierCategoryOf">
        <rdfs:label>carrier category of</rdfs:label>
        <rdfs:comment>Relates a Category to an Instance of that content type.</rdfs:comment>
        <rdfs:domain rdf:resource="http://bibframe.org/vocab/Category"/>
        <rdfs:range rdf:resource="http://bibframe.org/vocab/Instance"/>
        <owl:inverseOf rdf:resource="http://bibframe.org/vocab/carrierCategory"/>
    </owl:ObjectProperty>
    


    <!-- http://bibframe.org/vocab/cartography -->

    <owl:ObjectProperty rdf:about="http://bibframe.org/vocab/cartography">
        <rdfs:label>Cartographic data</rdfs:label>
        <dcterms:modified>2014-03-27 (Updated)</dcterms:modified>
        <rdfs:comment>Cartographic data that identifies scale, coordinates, etc.</rdfs:comment>
        <rdfs:range rdf:resource="http://bibframe.org/vocab/Cartography"/>
    </owl:ObjectProperty>
    


    <!-- http://bibframe.org/vocab/classification -->

    <owl:ObjectProperty rdf:about="http://bibframe.org/vocab/classification">
        <rdfs:label>Classification</rdfs:label>
        <rdfs:comment>Classification number in any scheme.</rdfs:comment>
        <rdfs:range rdf:resource="http://bibframe.org/vocab/Classification"/>
        <rdfs:domain rdf:resource="http://bibframe.org/vocab/Work"/>
    </owl:ObjectProperty>
    


    <!-- http://bibframe.org/vocab/classificationDdc -->

    <owl:ObjectProperty rdf:about="http://bibframe.org/vocab/classificationDdc">
        <rdfs:label>DDC Classification</rdfs:label>
        <rdfs:comment>Dewey Decimal Classification number used for subject access.</rdfs:comment>
        <rdfs:range rdf:resource="http://bibframe.org/vocab/Classification"/>
        <rdfs:domain rdf:resource="http://bibframe.org/vocab/Work"/>
        <rdfs:subPropertyOf rdf:resource="http://bibframe.org/vocab/classification"/>
    </owl:ObjectProperty>
    


    <!-- http://bibframe.org/vocab/classificationLcc -->

    <owl:ObjectProperty rdf:about="http://bibframe.org/vocab/classificationLcc">
        <rdfs:label>LCC Classification</rdfs:label>
        <rdfs:comment>Library of Congress Classification number used for subject access.</rdfs:comment>
        <rdfs:range rdf:resource="http://bibframe.org/vocab/Classification"/>
        <rdfs:domain rdf:resource="http://bibframe.org/vocab/Work"/>
        <rdfs:subPropertyOf rdf:resource="http://bibframe.org/vocab/classification"/>
    </owl:ObjectProperty>
    


    <!-- http://bibframe.org/vocab/classificationNlm -->

    <owl:ObjectProperty rdf:about="http://bibframe.org/vocab/classificationNlm">
        <rdfs:label>NLM classification</rdfs:label>
        <rdfs:comment>National Library of Medicine Classification number used for subject access</rdfs:comment>
        <rdfs:range rdf:resource="http://bibframe.org/vocab/Classification"/>
        <rdfs:domain rdf:resource="http://bibframe.org/vocab/Work"/>
        <rdfs:subPropertyOf rdf:resource="http://bibframe.org/vocab/classification"/>
    </owl:ObjectProperty>
    


    <!-- http://bibframe.org/vocab/classificationNumberUri -->

    <owl:ObjectProperty rdf:about="http://bibframe.org/vocab/classificationNumberUri">
        <rdfs:label>Classification number URI</rdfs:label>
        <rdfs:comment>Classification number represented as a URI.</rdfs:comment>
        <rdfs:domain rdf:resource="http://bibframe.org/vocab/Classification"/>
        <rdfs:range rdf:resource="&rdfs;Resource"/>
    </owl:ObjectProperty>
    


    <!-- http://bibframe.org/vocab/classificationUdc -->

    <owl:ObjectProperty rdf:about="http://bibframe.org/vocab/classificationUdc">
        <rdfs:label>UDC Classification</rdfs:label>
        <rdfs:comment>Universal Decimal Classification number used for subject access.</rdfs:comment>
        <rdfs:range rdf:resource="http://bibframe.org/vocab/Classification"/>
        <rdfs:domain rdf:resource="http://bibframe.org/vocab/Work"/>
        <rdfs:subPropertyOf rdf:resource="http://bibframe.org/vocab/classification"/>
    </owl:ObjectProperty>
    


    <!-- http://bibframe.org/vocab/coden -->

    <owl:ObjectProperty rdf:about="http://bibframe.org/vocab/coden">
        <rdfs:label>CODEN</rdfs:label>
        <rdfs:comment>Identifier for scientific and technical periodical titles assigned by the International CODEN Section of Chemical Abstracts Service.</rdfs:comment>
        <rdfs:range rdf:resource="http://bibframe.org/vocab/Identifier"/>
        <rdfs:domain rdf:resource="http://bibframe.org/vocab/Instance"/>
        <rdfs:subPropertyOf rdf:resource="http://bibframe.org/vocab/identifier"/>
    </owl:ObjectProperty>
    


    <!-- http://bibframe.org/vocab/componentOf -->

    <owl:ObjectProperty rdf:about="http://bibframe.org/vocab/componentOf">
        <rdfs:label>Held item</rdfs:label>
        <rdfs:comment>Link to held material</rdfs:comment>
    </owl:ObjectProperty>
    


    <!-- http://bibframe.org/vocab/contentCategory -->

    <owl:ObjectProperty rdf:about="http://bibframe.org/vocab/contentCategory">
        <rdfs:label>Content type</rdfs:label>
        <rdfs:comment>Categorization reflecting the fundamental form of communication in which the content is expressed and the human sense through which it is intended to be perceived.</rdfs:comment>
        <rdfs:range rdf:resource="http://bibframe.org/vocab/Category"/>
        <rdfs:domain rdf:resource="http://bibframe.org/vocab/Work"/>
    </owl:ObjectProperty>
    


    <!-- http://bibframe.org/vocab/contentCategoryOf -->

    <owl:ObjectProperty rdf:about="http://bibframe.org/vocab/contentCategoryOf">
        <rdfs:label>content category of</rdfs:label>
        <rdfs:comment>Relates a Category to a Work of that content type.</rdfs:comment>
        <rdfs:domain rdf:resource="http://bibframe.org/vocab/Category"/>
        <rdfs:range rdf:resource="http://bibframe.org/vocab/Work"/>
        <owl:inverseOf rdf:resource="http://bibframe.org/vocab/contentCategory"/>
    </owl:ObjectProperty>
    


    <!-- http://bibframe.org/vocab/continuedBy -->

    <owl:ObjectProperty rdf:about="http://bibframe.org/vocab/continuedBy">
        <rdfs:label>Continued by</rdfs:label>
        <dcterms:modified>2014-04-10 (Updated subproperty)</dcterms:modified>
        <rdfs:comment>Work whose content continues an earlier work under a new title.</rdfs:comment>
        <rdfs:domain rdf:resource="http://bibframe.org/vocab/Work"/>
        <rdfs:range rdf:resource="http://bibframe.org/vocab/Work"/>
        <owl:inverseOf rdf:resource="http://bibframe.org/vocab/continues"/>
        <rdfs:subPropertyOf rdf:resource="http://bibframe.org/vocab/succeededBy"/>
    </owl:ObjectProperty>
    


    <!-- http://bibframe.org/vocab/continuedInPartBy -->

    <owl:ObjectProperty rdf:about="http://bibframe.org/vocab/continuedInPartBy">
        <rdfs:label>Continued in part by</rdfs:label>
        <rdfs:comment>Work part of whose content separated from an earlier work to form a new work.</rdfs:comment>
        <dcterms:modified>2014-04-10 (Updated subproperty)</dcterms:modified>
        <rdfs:domain rdf:resource="http://bibframe.org/vocab/Work"/>
        <rdfs:range rdf:resource="http://bibframe.org/vocab/Work"/>
        <owl:inverseOf rdf:resource="http://bibframe.org/vocab/continuesInPart"/>
        <rdfs:subPropertyOf rdf:resource="http://bibframe.org/vocab/succeededBy"/>
    </owl:ObjectProperty>
    


    <!-- http://bibframe.org/vocab/continues -->

    <owl:ObjectProperty rdf:about="http://bibframe.org/vocab/continues">
        <rdfs:label>Continues</rdfs:label>
        <rdfs:comment>Work that is continued by the content of a later work under a new title.</rdfs:comment>
        <dcterms:modified>2014-04-10 (Updated subproperty)</dcterms:modified>
        <rdfs:domain rdf:resource="http://bibframe.org/vocab/Work"/>
        <rdfs:range rdf:resource="http://bibframe.org/vocab/Work"/>
        <rdfs:subPropertyOf rdf:resource="http://bibframe.org/vocab/precededBy"/>
    </owl:ObjectProperty>
    


    <!-- http://bibframe.org/vocab/continuesInPart -->

    <owl:ObjectProperty rdf:about="http://bibframe.org/vocab/continuesInPart">
        <rdfs:label>Continues in part</rdfs:label>
        <rdfs:comment>Work that split into two or more separate works with new titles.</rdfs:comment>
        <dcterms:modified>2014-04-10 (Updated subproperty)</dcterms:modified>
        <rdfs:domain rdf:resource="http://bibframe.org/vocab/Work"/>
        <rdfs:range rdf:resource="http://bibframe.org/vocab/Work"/>
        <rdfs:subPropertyOf rdf:resource="http://bibframe.org/vocab/precededBy"/>
    </owl:ObjectProperty>
    


    <!-- http://bibframe.org/vocab/contributor -->

    <owl:ObjectProperty rdf:about="http://bibframe.org/vocab/contributor">
        <rdfs:label>Contributor role</rdfs:label>
        <rdfs:comment>Generalized expressive responsibility role.</rdfs:comment>
    </owl:ObjectProperty>
    


    <!-- http://bibframe.org/vocab/contributorTo -->

    <owl:ObjectProperty rdf:about="http://bibframe.org/vocab/contributorTo">
        <rdfs:label>contributor to</rdfs:label>
        <rdfs:comment>Relates an Authority to a Resource it contributed to.</rdfs:comment>
        <owl:inverseOf rdf:resource="http://bibframe.org/vocab/contributor"/>
    </owl:ObjectProperty>
    


    <!-- http://bibframe.org/vocab/coverArt -->

    <owl:ObjectProperty rdf:about="http://bibframe.org/vocab/coverArt">
        <rdfs:label>Cover art</rdfs:label>
        <rdfs:comment>Cover art image.</rdfs:comment>
        <rdfs:subPropertyOf rdf:resource="http://bibframe.org/vocab/annotationBody"/>
        <rdfs:range rdf:resource="&rdfs;Resource"/>
    </owl:ObjectProperty>
    


    <!-- http://bibframe.org/vocab/coverArtFor -->

    <owl:ObjectProperty rdf:about="http://bibframe.org/vocab/coverArtFor">
        <rdfs:label>Cover art of instance</rdfs:label>
        <rdfs:comment>Resource to which the cover art pertains.</rdfs:comment>
        <rdfs:range rdf:resource="http://bibframe.org/vocab/Instance"/>
        <rdfs:subPropertyOf rdf:resource="http://bibframe.org/vocab/annotates"/>
    </owl:ObjectProperty>
    


    <!-- http://bibframe.org/vocab/coverArtThumb -->

    <owl:ObjectProperty rdf:about="http://bibframe.org/vocab/coverArtThumb">
        <rdfs:label>Thumbnail of cover art</rdfs:label>
        <rdfs:comment>Thumbnail version of cover art image.</rdfs:comment>
        <rdfs:subPropertyOf rdf:resource="http://bibframe.org/vocab/annotationBody"/>
        <rdfs:range rdf:resource="&rdfs;Resource"/>
    </owl:ObjectProperty>
    


    <!-- http://bibframe.org/vocab/creator -->

    <owl:ObjectProperty rdf:about="http://bibframe.org/vocab/creator">
        <rdfs:label>Creator role</rdfs:label>
        <rdfs:comment>Generalized creative responsibility role.</rdfs:comment>
    </owl:ObjectProperty>
    


    <!-- http://bibframe.org/vocab/creatorOf -->

    <owl:ObjectProperty rdf:about="http://bibframe.org/vocab/creatorOf">
        <rdfs:label>creator of</rdfs:label>
        <rdfs:comment>Relates an Authority to a Resource it created.</rdfs:comment>
        <owl:inverseOf rdf:resource="http://bibframe.org/vocab/creator"/>
    </owl:ObjectProperty>
    


    <!-- http://bibframe.org/vocab/dataSource -->

    <owl:ObjectProperty rdf:about="http://bibframe.org/vocab/dataSource">
        <rdfs:label>Has data source</rdfs:label>
        <rdfs:comment>Work that is a data source to which the described resource is related. It may contain information about other files, printed sources, or collection procedures.</rdfs:comment>
        <rdfs:range rdf:resource="http://bibframe.org/vocab/Work"/>
        <rdfs:domain rdf:resource="http://bibframe.org/vocab/Work"/>
        <rdfs:subPropertyOf rdf:resource="http://bibframe.org/vocab/relatedTo"/>
    </owl:ObjectProperty>
    


    <!-- http://bibframe.org/vocab/dataSourceFor -->

    <owl:ObjectProperty rdf:about="http://bibframe.org/vocab/dataSourceFor">
        <rdfs:label>data source for</rdfs:label>
        <rdfs:comment>Relates a Work to another Work for which it is the data source.</rdfs:comment>
        <rdfs:range rdf:resource="http://bibframe.org/vocab/Work"/>
        <rdfs:domain rdf:resource="http://bibframe.org/vocab/Work"/>
        <owl:inverseOf rdf:resource="http://bibframe.org/vocab/dataSource"/>
    </owl:ObjectProperty>
    


    <!-- http://bibframe.org/vocab/derivativeOf -->

    <owl:ObjectProperty rdf:about="http://bibframe.org/vocab/derivativeOf">
        <rdfs:label>Is derivative of</rdfs:label>
        <rdfs:comment>Work is a modification of a source work.</rdfs:comment>
        <dcterms:modified>2014-04-30 (New)</dcterms:modified>
        <owl:inverseOf rdf:resource="http://bibframe.org/vocab/hasDerivative"/>
        <rdfs:subPropertyOf rdf:resource="http://bibframe.org/vocab/relatedTo"/>
    </owl:ObjectProperty>
    


    <!-- http://bibframe.org/vocab/derivedFrom -->

    <owl:ObjectProperty rdf:about="http://bibframe.org/vocab/derivedFrom">
        <rdfs:label>Source record</rdfs:label>
        <rdfs:comment>Link to the record that was the source of the data, when applicable.</rdfs:comment>
        <rdfs:range rdf:resource="&rdfs;Resource"/>
    </owl:ObjectProperty>
    


    <!-- http://bibframe.org/vocab/descriptionConventions -->

    <owl:ObjectProperty rdf:about="http://bibframe.org/vocab/descriptionConventions">
        <rdfs:label>Description conventions</rdfs:label>
        <dcterms:modified>2014-05-13 (updated)</dcterms:modified>
        <rdfs:comment>Rules used for the descriptive content of the description.</rdfs:comment>
        <rdfs:range rdf:resource="&rdfs;Resource"/>
    </owl:ObjectProperty>
    


    <!-- http://bibframe.org/vocab/descriptionLanguage -->

    <owl:ObjectProperty rdf:about="http://bibframe.org/vocab/descriptionLanguage">
        <rdfs:label>Description language</rdfs:label>
        <rdfs:comment>Language used for the metadata.</rdfs:comment>
        <rdfs:range rdf:resource="&rdfs;Resource"/>
    </owl:ObjectProperty>
    


    <!-- http://bibframe.org/vocab/descriptionModifier -->

    <owl:ObjectProperty rdf:about="http://bibframe.org/vocab/descriptionModifier">
        <rdfs:label>Description modifier</rdfs:label>
        <dcterms:modified>2014-10-27 (Updated)</dcterms:modified>
        <rdfs:comment>Agency that modified a description.</rdfs:comment>
        <rdfs:range rdf:resource="&rdfs;Resource"/>
    </owl:ObjectProperty>
    


    <!-- http://bibframe.org/vocab/descriptionOf -->

    <owl:ObjectProperty rdf:about="http://bibframe.org/vocab/descriptionOf">
        <rdfs:label>Is description of</rdfs:label>
        <rdfs:comment>Related resource that is analyzed, commented upon, critiqued, evaluated, reviewed, or otherwise described by the resource.</rdfs:comment>
        <dcterms:modified>2014-04-30 (New)</dcterms:modified>
        <owl:inverseOf rdf:resource="http://bibframe.org/vocab/hasDescription"/>
        <rdfs:subPropertyOf rdf:resource="http://bibframe.org/vocab/relatedTo"/>
    </owl:ObjectProperty>
    


    <!-- http://bibframe.org/vocab/descriptionSource -->

    <owl:ObjectProperty rdf:about="http://bibframe.org/vocab/descriptionSource">
        <rdfs:label>Description source</rdfs:label>
        <rdfs:comment>Entity that created or modified the metadata.</rdfs:comment>
        <rdfs:range rdf:resource="&rdfs;Resource"/>
    </owl:ObjectProperty>
    


    <!-- http://bibframe.org/vocab/dissertationIdentifier -->

    <owl:ObjectProperty rdf:about="http://bibframe.org/vocab/dissertationIdentifier">
        <rdfs:label>Dissertation identifier</rdfs:label>
        <rdfs:comment>Identifier assigned to a dissertation for identification purposes .</rdfs:comment>
        <rdfs:range rdf:resource="http://bibframe.org/vocab/Identifier"/>
        <rdfs:domain rdf:resource="http://bibframe.org/vocab/Work"/>
        <rdfs:subPropertyOf rdf:resource="http://bibframe.org/vocab/identifier"/>
    </owl:ObjectProperty>
    


    <!-- http://bibframe.org/vocab/dissertationInstitution -->

    <owl:ObjectProperty rdf:about="http://bibframe.org/vocab/dissertationInstitution">
        <rdfs:label>Degree issuing institution</rdfs:label>
        <rdfs:comment>Name of degree granting institution.</rdfs:comment>
        <rdfs:domain rdf:resource="http://bibframe.org/vocab/Work"/>
    </owl:ObjectProperty>
    


    <!-- http://bibframe.org/vocab/dissertationInstitutionOf -->

    <owl:ObjectProperty rdf:about="http://bibframe.org/vocab/dissertationInstitutionOf">
        <rdfs:label>dissertation issued</rdfs:label>
        <rdfs:comment>Relates an institution to a disseration issued there.</rdfs:comment>
        <rdfs:range rdf:resource="http://bibframe.org/vocab/Work"/>
        <owl:inverseOf rdf:resource="http://bibframe.org/vocab/dissertationInstitution"/>
    </owl:ObjectProperty>
    


    <!-- http://bibframe.org/vocab/distribution -->

    <owl:ObjectProperty rdf:about="http://bibframe.org/vocab/distribution">
        <rdfs:label>Distribution event</rdfs:label>
        <rdfs:comment>Information relating to distribution of an instance.</rdfs:comment>
        <rdfs:domain rdf:resource="http://bibframe.org/vocab/Instance"/>
        <rdfs:range rdf:resource="http://bibframe.org/vocab/Provider"/>
        <rdfs:subPropertyOf rdf:resource="http://bibframe.org/vocab/provider"/>
    </owl:ObjectProperty>
    


    <!-- http://bibframe.org/vocab/doi -->

    <owl:ObjectProperty rdf:about="http://bibframe.org/vocab/doi">
        <rdfs:label>DOI</rdfs:label>
        <rdfs:comment>Digital Object Identifier.</rdfs:comment>
        <rdfs:range rdf:resource="http://bibframe.org/vocab/Identifier"/>
        <rdfs:domain rdf:resource="http://bibframe.org/vocab/Instance"/>
        <rdfs:subPropertyOf rdf:resource="http://bibframe.org/vocab/identifier"/>
    </owl:ObjectProperty>
    


    <!-- http://bibframe.org/vocab/ean -->

    <owl:ObjectProperty rdf:about="http://bibframe.org/vocab/ean">
        <rdfs:label>EAN</rdfs:label>
        <rdfs:comment>International Article Identifier.</rdfs:comment>
        <rdfs:range rdf:resource="http://bibframe.org/vocab/Identifier"/>
        <rdfs:domain rdf:resource="http://bibframe.org/vocab/Instance"/>
        <rdfs:subPropertyOf rdf:resource="http://bibframe.org/vocab/identifier"/>
    </owl:ObjectProperty>
    


    <!-- http://bibframe.org/vocab/electronicLocation -->

    <owl:ObjectProperty rdf:about="http://bibframe.org/vocab/electronicLocation">
        <rdfs:label>electronic location</rdfs:label>
        <rdfs:comment>Electronic location of a Resource.</rdfs:comment>
        <owl:inverseOf rdf:resource="http://bibframe.org/vocab/electronicLocator"/>
    </owl:ObjectProperty>
    


    <!-- http://bibframe.org/vocab/electronicLocator -->

    <owl:ObjectProperty rdf:about="http://bibframe.org/vocab/electronicLocator">
        <rdfs:label>Electronic location</rdfs:label>
        <dcterms:modified>2014-04-28 (New)</dcterms:modified>
        <rdfs:comment>Electronic location from which the resource is available.</rdfs:comment>
        <rdfs:range rdf:resource="&rdfs;Resource"/>
    </owl:ObjectProperty>
    


    <!-- http://bibframe.org/vocab/event -->

    <owl:ObjectProperty rdf:about="http://bibframe.org/vocab/event">
        <rdfs:label>Event associated with content</rdfs:label>
        <rdfs:comment>Information about the geographic area/or time period covered by an event (e.g., a report).</rdfs:comment>
        <dcterms:modified>2014-05-16 (Updated)</dcterms:modified>
        <rdfs:domain rdf:resource="http://bibframe.org/vocab/Work"/>
    </owl:ObjectProperty>
    


    <!-- http://bibframe.org/vocab/eventOf -->

    <owl:ObjectProperty rdf:about="http://bibframe.org/vocab/eventOf">
        <rdfs:label>event of</rdfs:label>
        <rdfs:comment>Relates an Event to an associated Work.</rdfs:comment>
        <rdfs:range rdf:resource="http://bibframe.org/vocab/Work"/>
        <owl:inverseOf rdf:resource="http://bibframe.org/vocab/event"/>
    </owl:ObjectProperty>
    


    <!-- http://bibframe.org/vocab/expressionOf -->

    <owl:ObjectProperty rdf:about="http://bibframe.org/vocab/expressionOf">
        <rdfs:label>Expression of</rdfs:label>
        <dcterms:modified>2014-04-10 (Updated subproperty)</dcterms:modified>
        <rdfs:comment>Expression has a related work. For use to connect Works under FRBR/RDA rules.</rdfs:comment>
        <rdfs:range rdf:resource="http://bibframe.org/vocab/Work"/>
        <rdfs:domain rdf:resource="http://bibframe.org/vocab/Work"/>
        <owl:inverseOf rdf:resource="http://bibframe.org/vocab/hasExpression"/>
        <rdfs:subPropertyOf rdf:resource="http://bibframe.org/vocab/relatedTo"/>
    </owl:ObjectProperty>
    


    <!-- http://bibframe.org/vocab/findingAid -->

    <owl:ObjectProperty rdf:about="http://bibframe.org/vocab/findingAid">
        <rdfs:label>Has finding aid</rdfs:label>
        <rdfs:comment>Relationship is to a finding aid or similar control materials for archival, visual, and manuscript resources.</rdfs:comment>
        <rdfs:range rdf:resource="http://bibframe.org/vocab/Work"/>
        <rdfs:domain rdf:resource="http://bibframe.org/vocab/Work"/>
        <rdfs:subPropertyOf rdf:resource="http://bibframe.org/vocab/accompaniedBy"/>
    </owl:ObjectProperty>
    


    <!-- http://bibframe.org/vocab/fingerprint -->

    <owl:ObjectProperty rdf:about="http://bibframe.org/vocab/fingerprint">
        <rdfs:label>Fingerprint identifier</rdfs:label>
        <rdfs:comment>Identifier that is used to assist in the identification of antiquarian books by recording information comprising groups of characters taken from specified positions on specified pages of the book.</rdfs:comment>
        <rdfs:range rdf:resource="http://bibframe.org/vocab/Identifier"/>
        <rdfs:domain rdf:resource="http://bibframe.org/vocab/Instance"/>
        <rdfs:subPropertyOf rdf:resource="http://bibframe.org/vocab/identifier"/>
    </owl:ObjectProperty>
    


    <!-- http://bibframe.org/vocab/genre -->

    <owl:ObjectProperty rdf:about="http://bibframe.org/vocab/genre">
        <rdfs:label>hasGenre</rdfs:label>
        <rdfs:comment>Genre and other general characteristics associated with genre and form.</rdfs:comment>
        <dcterms:modified>2014-03-21 (New)</dcterms:modified>
        <rdfs:range rdf:resource="http://bibframe.org/vocab/Category"/>
    </owl:ObjectProperty>
    


    <!-- http://bibframe.org/vocab/genreOf -->

    <owl:ObjectProperty rdf:about="http://bibframe.org/vocab/genreOf">
        <rdfs:label>genreOf</rdfs:label>
        <rdfs:comment>Relates a Category to a Resource of that genre.</rdfs:comment>
        <rdfs:domain rdf:resource="http://bibframe.org/vocab/Category"/>
        <owl:inverseOf rdf:resource="http://bibframe.org/vocab/genre"/>
    </owl:ObjectProperty>
    


    <!-- http://bibframe.org/vocab/hasAccompaniment -->

    <owl:ObjectProperty rdf:about="http://bibframe.org/vocab/hasAccompaniment"/>
    


    <!-- http://bibframe.org/vocab/hasAnnotation -->

    <owl:ObjectProperty rdf:about="http://bibframe.org/vocab/hasAnnotation">
        <rdfs:label>Has annotation</rdfs:label>
        <rdfs:comment>Resource has an annotation.</rdfs:comment>
        <owl:inverseOf rdf:resource="http://bibframe.org/vocab/annotates"/>
    </owl:ObjectProperty>
    


    <!-- http://bibframe.org/vocab/hasAuthority -->

    <owl:ObjectProperty rdf:about="http://bibframe.org/vocab/hasAuthority">
        <rdfs:label>Authority information</rdfs:label>
        <rdfs:comment>Link to controlled form of name or subject and other information about.</rdfs:comment>
        <dcterms:modified>2014-04-10 (Updated range)</dcterms:modified>
    </owl:ObjectProperty>
    


    <!-- http://bibframe.org/vocab/hasDerivative -->

    <owl:ObjectProperty rdf:about="http://bibframe.org/vocab/hasDerivative">
        <rdfs:label>Has derivative</rdfs:label>
        <rdfs:comment>Work has a modification for which it is the source.</rdfs:comment>
        <dcterms:modified>2014-04-10 (Range updated)</dcterms:modified>
        <rdfs:subPropertyOf rdf:resource="http://bibframe.org/vocab/relatedTo"/>
    </owl:ObjectProperty>
    


    <!-- http://bibframe.org/vocab/hasDescription -->

    <owl:ObjectProperty rdf:about="http://bibframe.org/vocab/hasDescription">
        <rdfs:label>Has description</rdfs:label>
        <rdfs:comment>Related resource that analyzes, comments on, critiques, evaluates, reviews, or otherwise describes the resource.</rdfs:comment>
        <dcterms:modified>2014-04-10 (Range updated)</dcterms:modified>
        <rdfs:subPropertyOf rdf:resource="http://bibframe.org/vocab/relatedTo"/>
    </owl:ObjectProperty>
    


    <!-- http://bibframe.org/vocab/hasEquivalent -->

    <owl:ObjectProperty rdf:about="http://bibframe.org/vocab/hasEquivalent">
        <rdf:type rdf:resource="&owl;SymmetricProperty"/>
        <rdfs:label>Equivalence</rdfs:label>
        <rdfs:comment>Instance embodies the same expression of a work as the resource being described.</rdfs:comment>
        <dcterms:modified>2014-04-10 (Range updated)</dcterms:modified>
        <rdfs:subPropertyOf rdf:resource="http://bibframe.org/vocab/relatedTo"/>
    </owl:ObjectProperty>
    


    <!-- http://bibframe.org/vocab/hasExpression -->

    <owl:ObjectProperty rdf:about="http://bibframe.org/vocab/hasExpression">
        <rdfs:label>Expressed as</rdfs:label>
        <rdfs:comment>Work has a related expression. For use to connect Works under FRBR/RDA rules.</rdfs:comment>
        <dcterms:modified>2014-04-10 (Updated subproperty)</dcterms:modified>
        <rdfs:domain rdf:resource="http://bibframe.org/vocab/Work"/>
        <rdfs:range rdf:resource="http://bibframe.org/vocab/Work"/>
        <rdfs:subPropertyOf rdf:resource="http://bibframe.org/vocab/relatedTo"/>
    </owl:ObjectProperty>
    


    <!-- http://bibframe.org/vocab/hasInstance -->

    <owl:ObjectProperty rdf:about="http://bibframe.org/vocab/hasInstance">
        <rdfs:label>Instance of Work</rdfs:label>
        <rdfs:comment>Work has a related Instance/manifestation. For use to connect Works to Instances in the BIBFRAME structure.</rdfs:comment>
        <dcterms:modified>2014--03-21 (Updated definition)</dcterms:modified>
        <rdfs:range rdf:resource="http://bibframe.org/vocab/Instance"/>
        <rdfs:domain rdf:resource="http://bibframe.org/vocab/Work"/>
        <rdfs:subPropertyOf rdf:resource="http://bibframe.org/vocab/relatedTo"/>
    </owl:ObjectProperty>
    


    <!-- http://bibframe.org/vocab/hasPart -->

    <owl:ObjectProperty rdf:about="http://bibframe.org/vocab/hasPart">
        <rdfs:label>Has part</rdfs:label>
        <rdfs:comment>Resource that is included either physically or logically contained in the described resource</rdfs:comment>
        <dcterms:modified>2014-04-10 (Range updated)</dcterms:modified>
        <rdfs:subPropertyOf rdf:resource="http://bibframe.org/vocab/relatedTo"/>
    </owl:ObjectProperty>
    


    <!-- http://bibframe.org/vocab/hasSeries -->

    <owl:ObjectProperty rdf:about="http://bibframe.org/vocab/hasSeries"/>
    


    <!-- http://bibframe.org/vocab/hdl -->

    <owl:ObjectProperty rdf:about="http://bibframe.org/vocab/hdl">
        <rdfs:label>Handle</rdfs:label>
        <rdfs:comment>Unique and persistent identifier for digital objects developed by the Corporation for National Research Initiatives.</rdfs:comment>
        <rdfs:range rdf:resource="http://bibframe.org/vocab/Identifier"/>
        <rdfs:domain rdf:resource="http://bibframe.org/vocab/Instance"/>
        <rdfs:subPropertyOf rdf:resource="http://bibframe.org/vocab/identifier"/>
    </owl:ObjectProperty>
    


    <!-- http://bibframe.org/vocab/heldBy -->

    <owl:ObjectProperty rdf:about="http://bibframe.org/vocab/heldBy">
        <rdfs:label>Held by</rdfs:label>
        <rdfs:comment>Entity holding the item or from which it is available</rdfs:comment>
    </owl:ObjectProperty>
    


    <!-- http://bibframe.org/vocab/holding -->

    <owl:ObjectProperty rdf:about="http://bibframe.org/vocab/holding">
        <rdfs:label>holding</rdfs:label>
        <rdfs:comment>Holding of an Instance.</rdfs:comment>
        <rdfs:domain rdf:resource="http://bibframe.org/vocab/Instance"/>
        <owl:inverseOf rdf:resource="http://bibframe.org/vocab/holdingFor"/>
    </owl:ObjectProperty>
    


    <!-- http://bibframe.org/vocab/holdingFor -->

    <owl:ObjectProperty rdf:about="http://bibframe.org/vocab/holdingFor">
        <rdfs:label>Holding for</rdfs:label>
        <rdfs:comment>Instance for which holding is reported</rdfs:comment>
        <rdfs:range rdf:resource="http://bibframe.org/vocab/Instance"/>
        <rdfs:subPropertyOf rdf:resource="http://bibframe.org/vocab/annotates"/>
    </owl:ObjectProperty>
    


    <!-- http://bibframe.org/vocab/holds -->

    <owl:ObjectProperty rdf:about="http://bibframe.org/vocab/holds">
        <rdfs:label>holds</rdfs:label>
        <rdfs:comment>Entity holding the item or from which it is available.</rdfs:comment>
        <owl:inverseOf rdf:resource="http://bibframe.org/vocab/heldBy"/>
    </owl:ObjectProperty>
    


    <!-- http://bibframe.org/vocab/identifier -->

    <owl:ObjectProperty rdf:about="http://bibframe.org/vocab/identifier">
        <rdfs:label>Identifier</rdfs:label>
        <rdfs:comment>Number or code that uniquely identifies an entity.</rdfs:comment>
        <rdfs:range rdf:resource="http://bibframe.org/vocab/Identifier"/>
    </owl:ObjectProperty>
    


    <!-- http://bibframe.org/vocab/identifierScheme -->

    <owl:ObjectProperty rdf:about="http://bibframe.org/vocab/identifierScheme">
        <rdfs:label>Identifier scheme</rdfs:label>
        <rdfs:comment>Scheme within which the identifier is unique.</rdfs:comment>
        <dcterms:modified>2014-06-04 (Updated mapping)</dcterms:modified>
        <dcterms:modified>&apos;2014-06-04 (Updated range)</dcterms:modified>
        <rdfs:domain rdf:resource="http://bibframe.org/vocab/Identifier"/>
        <rdfs:range rdf:resource="&rdfs;Resource"/>
    </owl:ObjectProperty>
    


    <!-- http://bibframe.org/vocab/index -->

    <owl:ObjectProperty rdf:about="http://bibframe.org/vocab/index">
        <rdfs:label>Index</rdfs:label>
        <rdfs:comment>Work has an accompanying index</rdfs:comment>
        <rdfs:domain rdf:resource="http://bibframe.org/vocab/Work"/>
        <rdfs:range rdf:resource="http://bibframe.org/vocab/Work"/>
        <rdfs:subPropertyOf rdf:resource="http://bibframe.org/vocab/accompaniedBy"/>
    </owl:ObjectProperty>
    


    <!-- http://bibframe.org/vocab/instanceOf -->

    <owl:ObjectProperty rdf:about="http://bibframe.org/vocab/instanceOf">
        <rdfs:label>Instance of</rdfs:label>
        <rdfs:comment>Work this resource instantiates or manifests. For use to connect Instances to Works in the BIBFRAME structure.</rdfs:comment>
        <dcterms:modified>2014--03-21 (Updated definition)</dcterms:modified>
        <rdfs:domain rdf:resource="http://bibframe.org/vocab/Instance"/>
        <rdfs:range rdf:resource="http://bibframe.org/vocab/Work"/>
        <owl:inverseOf rdf:resource="http://bibframe.org/vocab/hasInstance"/>
        <rdfs:subPropertyOf rdf:resource="http://bibframe.org/vocab/relatedTo"/>
    </owl:ObjectProperty>
    


    <!-- http://bibframe.org/vocab/instanceTitle -->

    <owl:ObjectProperty rdf:about="http://bibframe.org/vocab/instanceTitle">
        <rdfs:label>Instance title</rdfs:label>
        <rdfs:comment>Word, character, or group of words and/or characters that is the main name of an instance.</rdfs:comment>
        <rdfs:domain rdf:resource="http://bibframe.org/vocab/Instance"/>
        <rdfs:range rdf:resource="http://bibframe.org/vocab/Title"/>
    </owl:ObjectProperty>
    


    <!-- http://bibframe.org/vocab/intendedAudience -->

    <owl:ObjectProperty rdf:about="http://bibframe.org/vocab/intendedAudience">
        <rdfs:label>Intended audience</rdfs:label>
        <rdfs:comment>Information that identifies the specific audience or intellectual level for which the content of the resource is considered appropriate.</rdfs:comment>
        <rdfs:range rdf:resource="http://bibframe.org/vocab/IntendedAudience"/>
    </owl:ObjectProperty>
    


    <!-- http://bibframe.org/vocab/intendedAudienceOf -->

    <owl:ObjectProperty rdf:about="http://bibframe.org/vocab/intendedAudienceOf">
        <rdfs:label>intended audience of</rdfs:label>
        <rdfs:comment>Relates an IntendedAudience to a Resource containing content considered appropriate for it.</rdfs:comment>
        <rdfs:domain rdf:resource="http://bibframe.org/vocab/IntendedAudience"/>
        <owl:inverseOf rdf:resource="http://bibframe.org/vocab/intendedAudience"/>
    </owl:ObjectProperty>
    


    <!-- http://bibframe.org/vocab/isan -->

    <owl:ObjectProperty rdf:about="http://bibframe.org/vocab/isan">
        <rdfs:label>ISAN</rdfs:label>
        <rdfs:comment>International Standard Audiovisual Number.</rdfs:comment>
        <rdfs:range rdf:resource="http://bibframe.org/vocab/Identifier"/>
        <rdfs:domain rdf:resource="http://bibframe.org/vocab/Work"/>
        <rdfs:subPropertyOf rdf:resource="http://bibframe.org/vocab/identifier"/>
    </owl:ObjectProperty>
    


    <!-- http://bibframe.org/vocab/isbn -->

    <owl:ObjectProperty rdf:about="http://bibframe.org/vocab/isbn">
        <rdfs:label>ISBN</rdfs:label>
        <rdfs:comment>International Standard Book Number.</rdfs:comment>
        <rdfs:range rdf:resource="http://bibframe.org/vocab/Identifier"/>
        <rdfs:domain rdf:resource="http://bibframe.org/vocab/Instance"/>
        <rdfs:subPropertyOf rdf:resource="http://bibframe.org/vocab/identifier"/>
    </owl:ObjectProperty>
    


    <!-- http://bibframe.org/vocab/isbn10 -->

    <owl:ObjectProperty rdf:about="http://bibframe.org/vocab/isbn10">
        <rdfs:label>ISBN-10</rdfs:label>
        <rdfs:comment>10 digit version of the International Standard Book Number.</rdfs:comment>
        <rdfs:range rdf:resource="http://bibframe.org/vocab/Identifier"/>
        <rdfs:domain rdf:resource="http://bibframe.org/vocab/Instance"/>
        <rdfs:subPropertyOf rdf:resource="http://bibframe.org/vocab/isbn"/>
    </owl:ObjectProperty>
    


    <!-- http://bibframe.org/vocab/isbn13 -->

    <owl:ObjectProperty rdf:about="http://bibframe.org/vocab/isbn13">
        <rdfs:label>ISBN-13</rdfs:label>
        <rdfs:comment>13 digit version of the International Standard Book Number.</rdfs:comment>
        <rdfs:range rdf:resource="http://bibframe.org/vocab/Identifier"/>
        <rdfs:domain rdf:resource="http://bibframe.org/vocab/Instance"/>
        <rdfs:subPropertyOf rdf:resource="http://bibframe.org/vocab/isbn"/>
    </owl:ObjectProperty>
    


    <!-- http://bibframe.org/vocab/ismn -->

    <owl:ObjectProperty rdf:about="http://bibframe.org/vocab/ismn">
        <rdfs:label>ISMN</rdfs:label>
        <rdfs:comment>International Standard Music Number.</rdfs:comment>
        <rdfs:range rdf:resource="http://bibframe.org/vocab/Identifier"/>
        <rdfs:domain rdf:resource="http://bibframe.org/vocab/Instance"/>
        <rdfs:subPropertyOf rdf:resource="http://bibframe.org/vocab/identifier"/>
    </owl:ObjectProperty>
    


    <!-- http://bibframe.org/vocab/iso -->

    <owl:ObjectProperty rdf:about="http://bibframe.org/vocab/iso">
        <rdfs:label>ISO number</rdfs:label>
        <rdfs:comment>International Organization for Standardization standard number.</rdfs:comment>
        <rdfs:range rdf:resource="http://bibframe.org/vocab/Identifier"/>
        <rdfs:domain rdf:resource="http://bibframe.org/vocab/Instance"/>
        <rdfs:subPropertyOf rdf:resource="http://bibframe.org/vocab/identifier"/>
    </owl:ObjectProperty>
    


    <!-- http://bibframe.org/vocab/issn -->

    <owl:ObjectProperty rdf:about="http://bibframe.org/vocab/issn">
        <rdfs:label>ISSN</rdfs:label>
        <rdfs:comment>International Standard Serial Number identifier.</rdfs:comment>
        <rdfs:range rdf:resource="http://bibframe.org/vocab/Identifier"/>
        <rdfs:domain rdf:resource="http://bibframe.org/vocab/Instance"/>
        <rdfs:subPropertyOf rdf:resource="http://bibframe.org/vocab/identifier"/>
    </owl:ObjectProperty>
    


    <!-- http://bibframe.org/vocab/issnL -->

    <owl:ObjectProperty rdf:about="http://bibframe.org/vocab/issnL">
        <rdfs:label>ISSN-L</rdfs:label>
        <rdfs:comment>International Standard Serial Number that links together various media versions of a continuing resource.</rdfs:comment>
        <rdfs:range rdf:resource="http://bibframe.org/vocab/Identifier"/>
        <rdfs:domain rdf:resource="http://bibframe.org/vocab/Work"/>
        <rdfs:subPropertyOf rdf:resource="http://bibframe.org/vocab/identifier"/>
    </owl:ObjectProperty>
    


    <!-- http://bibframe.org/vocab/issueNumber -->

    <owl:ObjectProperty rdf:about="http://bibframe.org/vocab/issueNumber">
        <rdfs:label>Audio issue number</rdfs:label>
        <rdfs:comment>Number used to identify the issue designation, or serial identification, assigned by a publisher to a sound recording.</rdfs:comment>
        <rdfs:range rdf:resource="http://bibframe.org/vocab/Identifier"/>
        <rdfs:domain rdf:resource="http://bibframe.org/vocab/Instance"/>
        <rdfs:subPropertyOf rdf:resource="http://bibframe.org/vocab/identifier"/>
    </owl:ObjectProperty>
    


    <!-- http://bibframe.org/vocab/issuedWith -->

    <owl:ObjectProperty rdf:about="http://bibframe.org/vocab/issuedWith">
        <rdf:type rdf:resource="&owl;SymmetricProperty"/>
        <rdfs:label>Issued with</rdfs:label>
        <rdfs:comment>Instance that is issued on the same carrier as the manifestation being described.</rdfs:comment>
        <rdfs:range rdf:resource="http://bibframe.org/vocab/Instance"/>
        <rdfs:domain rdf:resource="http://bibframe.org/vocab/Instance"/>
        <rdfs:subPropertyOf rdf:resource="http://bibframe.org/vocab/hasAccompaniment"/>
    </owl:ObjectProperty>
    


    <!-- http://bibframe.org/vocab/istc -->

    <owl:ObjectProperty rdf:about="http://bibframe.org/vocab/istc">
        <rdfs:label>ISTC</rdfs:label>
        <rdfs:comment>International Standard Text code, a numbering system developed to enable the unique identification of textual works.</rdfs:comment>
        <dcterms:modified>a,z</dcterms:modified>
        <rdfs:range rdf:resource="http://bibframe.org/vocab/Identifier"/>
        <rdfs:domain rdf:resource="http://bibframe.org/vocab/Work"/>
        <rdfs:subPropertyOf rdf:resource="http://bibframe.org/vocab/identifier"/>
    </owl:ObjectProperty>
    


    <!-- http://bibframe.org/vocab/iswc -->

    <owl:ObjectProperty rdf:about="http://bibframe.org/vocab/iswc">
        <rdfs:label>ISWC</rdfs:label>
        <rdfs:comment>International Standard Musical Work Code, a unique, persistent reference number for the identification of musical works.</rdfs:comment>
        <rdfs:range rdf:resource="http://bibframe.org/vocab/Identifier"/>
        <rdfs:domain rdf:resource="http://bibframe.org/vocab/Work"/>
        <rdfs:subPropertyOf rdf:resource="http://bibframe.org/vocab/identifier"/>
    </owl:ObjectProperty>
    


    <!-- http://bibframe.org/vocab/keyTitle -->

    <owl:ObjectProperty rdf:about="http://bibframe.org/vocab/keyTitle">
        <rdfs:label>Key title</rdfs:label>
        <rdfs:comment>Unique title for a continuing resource that is assigned by the ISSN International Center in conjunction with an ISSN.</rdfs:comment>
        <rdfs:domain rdf:resource="http://bibframe.org/vocab/Instance"/>
        <rdfs:range rdf:resource="http://bibframe.org/vocab/Title"/>
        <rdfs:subPropertyOf rdf:resource="http://bibframe.org/vocab/instanceTitle"/>
    </owl:ObjectProperty>
    


    <!-- http://bibframe.org/vocab/language -->

    <owl:ObjectProperty rdf:about="http://bibframe.org/vocab/language">
        <rdfs:label>Language</rdfs:label>
        <rdfs:comment>Languages associated with a resource including those for multilingual resources and translated resources.</rdfs:comment>
        <rdfs:range rdf:resource="http://bibframe.org/vocab/Language"/>
        <rdfs:domain rdf:resource="http://bibframe.org/vocab/Language"/>
    </owl:ObjectProperty>
    


    <!-- http://bibframe.org/vocab/languageOfPartUri -->

    <owl:ObjectProperty rdf:about="http://bibframe.org/vocab/languageOfPartUri">
        <rdfs:label>Language of part URI</rdfs:label>
        <rdfs:comment>Language or notation system used to convey the content of the resource (associated with part or all of a resource).</rdfs:comment>
        <rdfs:domain rdf:resource="http://bibframe.org/vocab/Language"/>
        <owl:inverseOf rdf:resource="http://bibframe.org/vocab/language"/>
        <rdfs:range rdf:resource="&rdfs;Resource"/>
    </owl:ObjectProperty>
    


    <!-- http://bibframe.org/vocab/lcOverseasAcq -->

    <owl:ObjectProperty rdf:about="http://bibframe.org/vocab/lcOverseasAcq">
        <rdfs:label>LC acquisition program</rdfs:label>
        <rdfs:comment>Identification number assigned by the Library of Congress to works acquired through one of its overseas acquisition programs.</rdfs:comment>
        <rdfs:range rdf:resource="http://bibframe.org/vocab/Identifier"/>
        <rdfs:domain rdf:resource="http://bibframe.org/vocab/Instance"/>
        <rdfs:subPropertyOf rdf:resource="http://bibframe.org/vocab/identifier"/>
    </owl:ObjectProperty>
    


    <!-- http://bibframe.org/vocab/lccn -->

    <owl:ObjectProperty rdf:about="http://bibframe.org/vocab/lccn">
        <rdfs:label>LCCN</rdfs:label>
        <rdfs:comment>Library of Congress Control Number, which identifies the resource description.</rdfs:comment>
        <rdfs:range rdf:resource="http://bibframe.org/vocab/Identifier"/>
        <rdfs:domain rdf:resource="http://bibframe.org/vocab/Instance"/>
        <rdfs:subPropertyOf rdf:resource="http://bibframe.org/vocab/identifier"/>
    </owl:ObjectProperty>
    


    <!-- http://bibframe.org/vocab/legalDeposit -->

    <owl:ObjectProperty rdf:about="http://bibframe.org/vocab/legalDeposit">
        <rdfs:label>Copyright number</rdfs:label>
        <rdfs:comment>Number assigned to a copyright or legal deposit, which Identifies a resource description.</rdfs:comment>
        <rdfs:range rdf:resource="http://bibframe.org/vocab/Identifier"/>
        <rdfs:domain rdf:resource="http://bibframe.org/vocab/Instance"/>
        <rdfs:subPropertyOf rdf:resource="http://bibframe.org/vocab/identifier"/>
    </owl:ObjectProperty>
    


    <!-- http://bibframe.org/vocab/local -->

    <owl:ObjectProperty rdf:about="http://bibframe.org/vocab/local">
        <rdfs:label>Local identifier</rdfs:label>
        <rdfs:comment>Identifier established locally and not a standard number.</rdfs:comment>
        <rdfs:range rdf:resource="http://bibframe.org/vocab/Identifier"/>
        <rdfs:subPropertyOf rdf:resource="http://bibframe.org/vocab/identifier"/>
    </owl:ObjectProperty>
    


    <!-- http://bibframe.org/vocab/manufacture -->

    <owl:ObjectProperty rdf:about="http://bibframe.org/vocab/manufacture">
        <rdfs:label>Manufacture event</rdfs:label>
        <rdfs:comment>Information relating to manufacture of an instance.</rdfs:comment>
        <rdfs:domain rdf:resource="http://bibframe.org/vocab/Instance"/>
        <rdfs:range rdf:resource="http://bibframe.org/vocab/Provider"/>
        <rdfs:subPropertyOf rdf:resource="http://bibframe.org/vocab/provider"/>
    </owl:ObjectProperty>
    


    <!-- http://bibframe.org/vocab/matrixNumber -->

    <owl:ObjectProperty rdf:about="http://bibframe.org/vocab/matrixNumber">
        <rdfs:label>Audio matrix number</rdfs:label>
        <rdfs:comment>Matrix number from the master from which a specific sound recording was pressed.</rdfs:comment>
        <rdfs:range rdf:resource="http://bibframe.org/vocab/Identifier"/>
        <rdfs:domain rdf:resource="http://bibframe.org/vocab/Instance"/>
        <rdfs:subPropertyOf rdf:resource="http://bibframe.org/vocab/identifier"/>
    </owl:ObjectProperty>
    


    <!-- http://bibframe.org/vocab/mediaCategory -->

    <owl:ObjectProperty rdf:about="http://bibframe.org/vocab/mediaCategory">
        <rdfs:label>Media type</rdfs:label>
        <rdfs:comment>Categorization reflecting the general type of intermediation device required to view, play, run, etc., the content of a resource.</rdfs:comment>
        <rdfs:range rdf:resource="http://bibframe.org/vocab/Category"/>
        <rdfs:domain rdf:resource="http://bibframe.org/vocab/Instance"/>
    </owl:ObjectProperty>
    


    <!-- http://bibframe.org/vocab/mediaCategoryOf -->

    <owl:ObjectProperty rdf:about="http://bibframe.org/vocab/mediaCategoryOf">
        <rdfs:label>media category of</rdfs:label>
        <rdfs:comment>Relates a Category to an Instance of that media type.</rdfs:comment>
        <rdfs:domain rdf:resource="http://bibframe.org/vocab/Category"/>
        <rdfs:range rdf:resource="http://bibframe.org/vocab/Instance"/>
        <owl:inverseOf rdf:resource="http://bibframe.org/vocab/mediaCategory"/>
    </owl:ObjectProperty>
    


    <!-- http://bibframe.org/vocab/mergedToForm -->

    <owl:ObjectProperty rdf:about="http://bibframe.org/vocab/mergedToForm">
        <rdfs:label>Merged to form</rdfs:label>
        <rdfs:comment>One of two or more works that come together to form a new work.</rdfs:comment>
        <dcterms:modified>2014-04-10 (Updated subproperty)</dcterms:modified>
        <rdfs:domain rdf:resource="http://bibframe.org/vocab/Work"/>
        <rdfs:range rdf:resource="http://bibframe.org/vocab/Work"/>
        <rdfs:subPropertyOf rdf:resource="http://bibframe.org/vocab/succeededBy"/>
    </owl:ObjectProperty>
    


    <!-- http://bibframe.org/vocab/musicMedium -->

    <owl:ObjectProperty rdf:about="http://bibframe.org/vocab/musicMedium">
        <rdfs:label>Music medium</rdfs:label>
        <rdfs:comment>Instrumental, vocal, and/or other medium of performance for which a musical resource was originally conceived, written or performed.</rdfs:comment>
        <rdfs:range rdf:resource="&rdfs;Resource"/>
    </owl:ObjectProperty>
    


    <!-- http://bibframe.org/vocab/musicMediumOf -->

    <owl:ObjectProperty rdf:about="http://bibframe.org/vocab/musicMediumOf">
        <rdfs:label>music medium of</rdfs:label>
        <rdfs:comment>Relates a music medium to a Resource.</rdfs:comment>
        <owl:inverseOf rdf:resource="http://bibframe.org/vocab/musicMedium"/>
    </owl:ObjectProperty>
    


    <!-- http://bibframe.org/vocab/musicPlate -->

    <owl:ObjectProperty rdf:about="http://bibframe.org/vocab/musicPlate">
        <rdfs:label>Music plate number</rdfs:label>
        <rdfs:comment>Number assigned by a music publisher to a specific music publication.</rdfs:comment>
        <rdfs:range rdf:resource="http://bibframe.org/vocab/Identifier"/>
        <rdfs:domain rdf:resource="http://bibframe.org/vocab/Instance"/>
        <rdfs:subPropertyOf rdf:resource="http://bibframe.org/vocab/identifier"/>
    </owl:ObjectProperty>
    


    <!-- http://bibframe.org/vocab/musicPublisherNumber -->

    <owl:ObjectProperty rdf:about="http://bibframe.org/vocab/musicPublisherNumber">
        <rdfs:label>Music publisher number</rdfs:label>
        <rdfs:comment>Number assigned to a music publication other than an issue, matrix, or plate number.</rdfs:comment>
        <rdfs:range rdf:resource="http://bibframe.org/vocab/Identifier"/>
        <rdfs:domain rdf:resource="http://bibframe.org/vocab/Instance"/>
        <rdfs:subPropertyOf rdf:resource="http://bibframe.org/vocab/identifier"/>
    </owl:ObjectProperty>
    


    <!-- http://bibframe.org/vocab/nban -->

    <owl:ObjectProperty rdf:about="http://bibframe.org/vocab/nban">
        <rdfs:label>NBAN</rdfs:label>
        <rdfs:comment>National Bibliography Agency Number, which identifies the resource description.</rdfs:comment>
        <rdfs:range rdf:resource="http://bibframe.org/vocab/Identifier"/>
        <rdfs:domain rdf:resource="http://bibframe.org/vocab/Instance"/>
        <rdfs:subPropertyOf rdf:resource="http://bibframe.org/vocab/identifier"/>
    </owl:ObjectProperty>
    


    <!-- http://bibframe.org/vocab/nbn -->

    <owl:ObjectProperty rdf:about="http://bibframe.org/vocab/nbn">
        <rdfs:label>NBN</rdfs:label>
        <rdfs:comment>National Bibliography Number, which identifies the resource description.</rdfs:comment>
        <rdfs:range rdf:resource="http://bibframe.org/vocab/Identifier"/>
        <rdfs:domain rdf:resource="http://bibframe.org/vocab/Instance"/>
        <rdfs:subPropertyOf rdf:resource="http://bibframe.org/vocab/identifier"/>
    </owl:ObjectProperty>
    


    <!-- http://bibframe.org/vocab/originPlace -->

    <owl:ObjectProperty rdf:about="http://bibframe.org/vocab/originPlace">
        <rdfs:label>Associated title place</rdfs:label>
        <rdfs:comment>Place from which the creation of the work originated.</rdfs:comment>
        <rdfs:domain rdf:resource="http://bibframe.org/vocab/Work"/>
    </owl:ObjectProperty>
    


    <!-- http://bibframe.org/vocab/originPlaceOf -->

    <owl:ObjectProperty rdf:about="http://bibframe.org/vocab/originPlaceOf">
        <rdfs:label>place of origin of</rdfs:label>
        <rdfs:comment>Relates a place to a Work created there.</rdfs:comment>
        <rdfs:range rdf:resource="http://bibframe.org/vocab/Work"/>
        <owl:inverseOf rdf:resource="http://bibframe.org/vocab/originPlace"/>
    </owl:ObjectProperty>
    


    <!-- http://bibframe.org/vocab/originalVersion -->

    <owl:ObjectProperty rdf:about="http://bibframe.org/vocab/originalVersion">
        <rdfs:label>Has original version</rdfs:label>
        <rdfs:comment>Instance is the original version of which this resource is a reproduction.</rdfs:comment>
        <rdfs:domain rdf:resource="http://bibframe.org/vocab/Work"/>
        <rdfs:range rdf:resource="http://bibframe.org/vocab/Work"/>
        <rdfs:subPropertyOf rdf:resource="http://bibframe.org/vocab/derivativeOf"/>
    </owl:ObjectProperty>
    


    <!-- http://bibframe.org/vocab/originalVersionOf -->

    <owl:ObjectProperty rdf:about="http://bibframe.org/vocab/originalVersionOf">
        <rdfs:label>original version of</rdfs:label>
        <rdfs:comment>Relates an original Work to a reproduction (Work).</rdfs:comment>
        <rdfs:domain rdf:resource="http://bibframe.org/vocab/Work"/>
        <rdfs:range rdf:resource="http://bibframe.org/vocab/Work"/>
        <owl:inverseOf rdf:resource="http://bibframe.org/vocab/originalVersion"/>
    </owl:ObjectProperty>
    


    <!-- http://bibframe.org/vocab/otherEdition -->

    <owl:ObjectProperty rdf:about="http://bibframe.org/vocab/otherEdition">
        <rdfs:label>hasOtherEdition</rdfs:label>
        <rdfs:comment>Resource has other available editions, for example simultaneously published language editions or reprints.</rdfs:comment>
        <rdfs:domain rdf:resource="http://bibframe.org/vocab/Work"/>
        <rdfs:range rdf:resource="http://bibframe.org/vocab/Work"/>
        <rdfs:subPropertyOf rdf:resource="http://bibframe.org/vocab/derivativeOf"/>
    </owl:ObjectProperty>
    


    <!-- http://bibframe.org/vocab/otherPhysicalFormat -->

    <owl:ObjectProperty rdf:about="http://bibframe.org/vocab/otherPhysicalFormat">
        <rdf:type rdf:resource="&owl;SymmetricProperty"/>
        <rdfs:label>Has other physical format</rdfs:label>
        <dcterms:modified>2014-10-14 (Updated)</dcterms:modified>
        <rdfs:comment>Resource that is manifested in another physical carrier.</rdfs:comment>
        <rdfs:domain rdf:resource="http://bibframe.org/vocab/Instance"/>
        <rdfs:range rdf:resource="http://bibframe.org/vocab/Instance"/>
        <rdfs:subPropertyOf rdf:resource="http://bibframe.org/vocab/hasEquivalent"/>
    </owl:ObjectProperty>
    


    <!-- http://bibframe.org/vocab/partOf -->

    <owl:ObjectProperty rdf:about="http://bibframe.org/vocab/partOf">
        <rdfs:label>Is part of</rdfs:label>
        <rdfs:comment>Resource in which the described resource is physically or logically contained.</rdfs:comment>
        <dcterms:modified>2014-04-30 (New)</dcterms:modified>
        <owl:inverseOf rdf:resource="http://bibframe.org/vocab/hasPart"/>
        <rdfs:subPropertyOf rdf:resource="http://bibframe.org/vocab/relatedTo"/>
    </owl:ObjectProperty>
    


    <!-- http://bibframe.org/vocab/postalRegistration -->

    <owl:ObjectProperty rdf:about="http://bibframe.org/vocab/postalRegistration">
        <rdfs:label>Postal registration number</rdfs:label>
        <rdfs:comment>Number assigned to a publication for which the specified postal service permits the use of a special mailing class privilege.</rdfs:comment>
        <rdfs:range rdf:resource="http://bibframe.org/vocab/Identifier"/>
        <rdfs:domain rdf:resource="http://bibframe.org/vocab/Instance"/>
        <rdfs:subPropertyOf rdf:resource="http://bibframe.org/vocab/identifier"/>
    </owl:ObjectProperty>
    


    <!-- http://bibframe.org/vocab/precededBy -->

    <owl:ObjectProperty rdf:about="http://bibframe.org/vocab/precededBy">
        <rdfs:label>Preceded By</rdfs:label>
        <dcterms:modified>2014-04-10 (Renamed)</dcterms:modified>
        <rdfs:comment>Resource that precedes the resource being described (e.g., is earlier in time or before in narrative).</rdfs:comment>
        <rdfs:subPropertyOf rdf:resource="http://bibframe.org/vocab/relatedTo"/>
        <owl:inverseOf rdf:resource="http://bibframe.org/vocab/succeededBy"/>
    </owl:ObjectProperty>
    


    <!-- http://bibframe.org/vocab/production -->

    <owl:ObjectProperty rdf:about="http://bibframe.org/vocab/production">
        <rdfs:label>Production event</rdfs:label>
        <rdfs:comment>Information relating to production of an instance.</rdfs:comment>
        <rdfs:domain rdf:resource="http://bibframe.org/vocab/Instance"/>
        <rdfs:range rdf:resource="http://bibframe.org/vocab/Provider"/>
        <rdfs:subPropertyOf rdf:resource="http://bibframe.org/vocab/provider"/>
    </owl:ObjectProperty>
    


    <!-- http://bibframe.org/vocab/provider -->

    <owl:ObjectProperty rdf:about="http://bibframe.org/vocab/provider">
        <rdfs:label>Provider</rdfs:label>
        <rdfs:comment>Place, name, and/or date information relating to the publication, printing, distribution, issue, release, or production instance.</rdfs:comment>
        <rdfs:domain rdf:resource="http://bibframe.org/vocab/Instance"/>
        <rdfs:range rdf:resource="http://bibframe.org/vocab/Provider"/>
    </owl:ObjectProperty>
    


    <!-- http://bibframe.org/vocab/providerName -->

    <owl:ObjectProperty rdf:about="http://bibframe.org/vocab/providerName">
        <rdfs:label>Provider name</rdfs:label>
        <rdfs:comment>Name of the entity responsible for the publication, printing, distribution, issue, release or production of the instance.</rdfs:comment>
        <rdfs:domain rdf:resource="http://bibframe.org/vocab/Provider"/>
    </owl:ObjectProperty>
    


    <!-- http://bibframe.org/vocab/providerPlace -->

    <owl:ObjectProperty rdf:about="http://bibframe.org/vocab/providerPlace">
        <rdfs:label>Provider place</rdfs:label>
        <rdfs:comment>Place associated with the publication, printing, distribution, issue, release or production of the instance.</rdfs:comment>
        <rdfs:domain rdf:resource="http://bibframe.org/vocab/Provider"/>
    </owl:ObjectProperty>
    


    <!-- http://bibframe.org/vocab/publication -->

    <owl:ObjectProperty rdf:about="http://bibframe.org/vocab/publication">
        <rdfs:label>Publication event</rdfs:label>
        <rdfs:comment>Information relating to publication of an instance.</rdfs:comment>
        <rdfs:domain rdf:resource="http://bibframe.org/vocab/Instance"/>
        <rdfs:range rdf:resource="http://bibframe.org/vocab/Provider"/>
        <rdfs:subPropertyOf rdf:resource="http://bibframe.org/vocab/provider"/>
    </owl:ObjectProperty>
    


    <!-- http://bibframe.org/vocab/publisherNumber -->

    <owl:ObjectProperty rdf:about="http://bibframe.org/vocab/publisherNumber">
        <rdfs:label>Other publisher number</rdfs:label>
        <rdfs:comment>Number assigned by a publisher that is not one of the specific defined types.</rdfs:comment>
        <rdfs:range rdf:resource="http://bibframe.org/vocab/Identifier"/>
        <rdfs:domain rdf:resource="http://bibframe.org/vocab/Instance"/>
        <rdfs:subPropertyOf rdf:resource="http://bibframe.org/vocab/identifier"/>
    </owl:ObjectProperty>
    


    <!-- http://bibframe.org/vocab/referenceAuthority -->

    <owl:ObjectProperty rdf:about="http://bibframe.org/vocab/referenceAuthority">
        <rdfs:label>Other authority information</rdfs:label>
        <rdfs:comment>Link to authority information</rdfs:comment>
        <dcterms:modified>2014-03-27 (Updated)</dcterms:modified>
    </owl:ObjectProperty>
    


    <!-- http://bibframe.org/vocab/relatedInstance -->

    <owl:ObjectProperty rdf:about="http://bibframe.org/vocab/relatedInstance">
        <rdf:type rdf:resource="&owl;SymmetricProperty"/>
        <rdfs:label>Related Instance</rdfs:label>
        <rdfs:comment>General instance to instance relationship.</rdfs:comment>
        <rdfs:range rdf:resource="http://bibframe.org/vocab/Instance"/>
        <rdfs:domain rdf:resource="http://bibframe.org/vocab/Instance"/>
        <rdfs:subPropertyOf rdf:resource="http://bibframe.org/vocab/relatedTo"/>
    </owl:ObjectProperty>
    


    <!-- http://bibframe.org/vocab/relatedTo -->

    <owl:ObjectProperty rdf:about="http://bibframe.org/vocab/relatedTo">
        <rdf:type rdf:resource="&owl;SymmetricProperty"/>
        <rdfs:label>Related resource</rdfs:label>
        <rdfs:comment>Any relationship between work or instance resources.</rdfs:comment>
        <dcterms:modified>2014-04-10 (Range updated)</dcterms:modified>
    </owl:ObjectProperty>
    


    <!-- http://bibframe.org/vocab/relatedWork -->

    <owl:ObjectProperty rdf:about="http://bibframe.org/vocab/relatedWork">
        <rdf:type rdf:resource="&owl;SymmetricProperty"/>
        <rdfs:label>Related Work</rdfs:label>
        <rdfs:comment>General work to work relationship.</rdfs:comment>
        <rdfs:domain rdf:resource="http://bibframe.org/vocab/Work"/>
        <rdfs:range rdf:resource="http://bibframe.org/vocab/Work"/>
        <rdfs:subPropertyOf rdf:resource="http://bibframe.org/vocab/relatedTo"/>
    </owl:ObjectProperty>
    


    <!-- http://bibframe.org/vocab/relator -->

    <owl:ObjectProperty rdf:about="http://bibframe.org/vocab/relator">
        <rdfs:label>Relationship of agent</rdfs:label>
        <dcterms:modified>2014-04-30 (New)</dcterms:modified>
        <rdfs:comment>link to role and agent information.</rdfs:comment>
        <rdfs:range rdf:resource="http://bibframe.org/vocab/Relator"/>
    </owl:ObjectProperty>
    


    <!-- http://bibframe.org/vocab/reportNumber -->

    <owl:ObjectProperty rdf:about="http://bibframe.org/vocab/reportNumber">
        <rdfs:label>Technical report number</rdfs:label>
        <rdfs:comment>Identification number of a report that is not a Standard Technical Report Number.</rdfs:comment>
        <rdfs:range rdf:resource="http://bibframe.org/vocab/Identifier"/>
        <rdfs:domain rdf:resource="http://bibframe.org/vocab/Instance"/>
        <rdfs:subPropertyOf rdf:resource="http://bibframe.org/vocab/identifier"/>
    </owl:ObjectProperty>
    


    <!-- http://bibframe.org/vocab/reproduction -->

    <owl:ObjectProperty rdf:about="http://bibframe.org/vocab/reproduction">
        <rdfs:label>Has reproduction</rdfs:label>
        <rdfs:comment>Instance that reproduces another Instance embodying the same work.</rdfs:comment>
        <rdfs:range rdf:resource="http://bibframe.org/vocab/Instance"/>
        <rdfs:domain rdf:resource="http://bibframe.org/vocab/Instance"/>
        <rdfs:subPropertyOf rdf:resource="http://bibframe.org/vocab/hasEquivalent"/>
    </owl:ObjectProperty>
    


    <!-- http://bibframe.org/vocab/reproductionOf -->

    <owl:ObjectProperty rdf:about="http://bibframe.org/vocab/reproductionOf">
        <rdfs:label>reproduction of</rdfs:label>
        <rdfs:comment>Relates a reproduction (Instance) to the original Instance.</rdfs:comment>
        <rdfs:range rdf:resource="http://bibframe.org/vocab/Instance"/>
        <rdfs:domain rdf:resource="http://bibframe.org/vocab/Instance"/>
        <owl:inverseOf rdf:resource="http://bibframe.org/vocab/reproduction"/>
    </owl:ObjectProperty>
    


    <!-- http://bibframe.org/vocab/review -->

    <owl:ObjectProperty rdf:about="http://bibframe.org/vocab/review">
        <rdfs:label>Review content</rdfs:label>
        <rdfs:comment>Review content.</rdfs:comment>
        <rdfs:subPropertyOf rdf:resource="http://bibframe.org/vocab/annotationBody"/>
        <rdfs:range rdf:resource="&rdfs;Resource"/>
    </owl:ObjectProperty>
    


    <!-- http://bibframe.org/vocab/reviewOf -->

    <owl:ObjectProperty rdf:about="http://bibframe.org/vocab/reviewOf">
        <rdfs:label>Resource reviewed</rdfs:label>
        <rdfs:comment>Resource to which the review pertains.</rdfs:comment>
        <rdfs:range rdf:resource="http://bibframe.org/vocab/Work"/>
        <rdfs:subPropertyOf rdf:resource="http://bibframe.org/vocab/annotates"/>
        <owl:inverseOf rdf:resource="http://bibframe.org/vocab/review"/>
    </owl:ObjectProperty>
    


    <!-- http://bibframe.org/vocab/separatedFrom -->

    <owl:ObjectProperty rdf:about="http://bibframe.org/vocab/separatedFrom">
        <rdfs:label>Separated from</rdfs:label>
        <rdfs:comment>Work that spun off a part of its content to form a new work.</rdfs:comment>
        <dcterms:modified>2014-04-10 (Updated subproperty)</dcterms:modified>
        <rdfs:domain rdf:resource="http://bibframe.org/vocab/Work"/>
        <rdfs:range rdf:resource="http://bibframe.org/vocab/Work"/>
        <rdfs:subPropertyOf rdf:resource="http://bibframe.org/vocab/precededBy"/>
    </owl:ObjectProperty>
    


    <!-- http://bibframe.org/vocab/series -->

    <owl:ObjectProperty rdf:about="http://bibframe.org/vocab/series">
        <rdfs:label>Has series</rdfs:label>
        <rdfs:comment>Work in which the part has been issued; the title of the larger work appears on the part.</rdfs:comment>
        <dcterms:modified>2014-10-14 (Updated)</dcterms:modified>
        <rdfs:range rdf:resource="http://bibframe.org/vocab/Work"/>
        <rdfs:domain rdf:resource="http://bibframe.org/vocab/Work"/>
        <rdfs:subPropertyOf rdf:resource="http://bibframe.org/vocab/partOf"/>
    </owl:ObjectProperty>
    


    <!-- http://bibframe.org/vocab/seriesOf -->

    <owl:ObjectProperty rdf:about="http://bibframe.org/vocab/seriesOf">
        <rdfs:label>series of</rdfs:label>
        <rdfs:comment>Relates a series (Work) to a member (Work).</rdfs:comment>
        <rdfs:range rdf:resource="http://bibframe.org/vocab/Work"/>
        <rdfs:domain rdf:resource="http://bibframe.org/vocab/Work"/>
        <owl:inverseOf rdf:resource="http://bibframe.org/vocab/hasSeries"/>
    </owl:ObjectProperty>
    


    <!-- http://bibframe.org/vocab/sici -->

    <owl:ObjectProperty rdf:about="http://bibframe.org/vocab/sici">
        <rdfs:label>SICI</rdfs:label>
        <rdfs:comment>Serial Item and Contribution Identifier.</rdfs:comment>
        <rdfs:range rdf:resource="http://bibframe.org/vocab/Identifier"/>
        <rdfs:domain rdf:resource="http://bibframe.org/vocab/Instance"/>
        <rdfs:subPropertyOf rdf:resource="http://bibframe.org/vocab/identifier"/>
    </owl:ObjectProperty>
    


    <!-- http://bibframe.org/vocab/split -->

    <owl:ObjectProperty rdf:about="http://bibframe.org/vocab/split">
        <rdfs:label>holding</rdfs:label>
        <rdfs:comment>Earlier Work split to form two or more Works.</rdfs:comment>
        <rdfs:range rdf:resource="http://bibframe.org/vocab/Work"/>
        <rdfs:domain rdf:resource="http://bibframe.org/vocab/Work"/>
        <owl:inverseOf rdf:resource="http://bibframe.org/vocab/splitInto"/>
    </owl:ObjectProperty>
    


    <!-- http://bibframe.org/vocab/splitInto -->

    <owl:ObjectProperty rdf:about="http://bibframe.org/vocab/splitInto">
        <rdfs:label>Split into</rdfs:label>
        <dcterms:modified>2014-04-10 (Updated subproperty)</dcterms:modified>
        <rdfs:comment>One of two or more works resulting from the division of an earlier work into separate works.</rdfs:comment>
        <rdfs:domain rdf:resource="http://bibframe.org/vocab/Work"/>
        <rdfs:range rdf:resource="http://bibframe.org/vocab/Work"/>
        <rdfs:subPropertyOf rdf:resource="http://bibframe.org/vocab/succeededBy"/>
    </owl:ObjectProperty>
    


    <!-- http://bibframe.org/vocab/stockNumber -->

    <owl:ObjectProperty rdf:about="http://bibframe.org/vocab/stockNumber">
        <rdfs:label>Stock number</rdfs:label>
        <rdfs:comment>Identification number such as distributor, publisher, or vendor number.</rdfs:comment>
        <rdfs:range rdf:resource="http://bibframe.org/vocab/Identifier"/>
        <rdfs:domain rdf:resource="http://bibframe.org/vocab/Instance"/>
        <rdfs:subPropertyOf rdf:resource="http://bibframe.org/vocab/identifier"/>
    </owl:ObjectProperty>
    


    <!-- http://bibframe.org/vocab/strn -->

    <owl:ObjectProperty rdf:about="http://bibframe.org/vocab/strn">
        <rdfs:label>STRN</rdfs:label>
        <rdfs:comment>Standard Technical Report Number.</rdfs:comment>
        <rdfs:range rdf:resource="http://bibframe.org/vocab/Identifier"/>
        <rdfs:domain rdf:resource="http://bibframe.org/vocab/Instance"/>
        <rdfs:subPropertyOf rdf:resource="http://bibframe.org/vocab/identifier"/>
    </owl:ObjectProperty>
    


    <!-- http://bibframe.org/vocab/studyNumber -->

    <owl:ObjectProperty rdf:about="http://bibframe.org/vocab/studyNumber">
        <rdfs:label>Study number</rdfs:label>
        <rdfs:comment>Identification number for a computer data file.</rdfs:comment>
        <rdfs:range rdf:resource="http://bibframe.org/vocab/Identifier"/>
        <rdfs:domain rdf:resource="http://bibframe.org/vocab/Instance"/>
        <rdfs:subPropertyOf rdf:resource="http://bibframe.org/vocab/identifier"/>
    </owl:ObjectProperty>
    


    <!-- http://bibframe.org/vocab/subject -->

    <owl:ObjectProperty rdf:about="http://bibframe.org/vocab/subject">
        <rdfs:label>Subject</rdfs:label>
        <rdfs:comment>Subject term(s) describing a resource.</rdfs:comment>
        <rdfs:range rdf:resource="http://bibframe.org/vocab/Work"/>
        <rdfs:domain rdf:resource="http://bibframe.org/vocab/Work"/>
    </owl:ObjectProperty>
    


    <!-- http://bibframe.org/vocab/subjectOf -->

    <owl:ObjectProperty rdf:about="http://bibframe.org/vocab/subjectOf">
        <rdfs:label>subject of</rdfs:label>
        <rdfs:comment>Relates a subject to a Work it is the subject of.</rdfs:comment>
        <rdfs:range rdf:resource="http://bibframe.org/vocab/Work"/>
        <rdfs:domain rdf:resource="http://bibframe.org/vocab/Work"/>
        <owl:inverseOf rdf:resource="http://bibframe.org/vocab/subject"/>
    </owl:ObjectProperty>
    


    <!-- http://bibframe.org/vocab/subseries -->

    <owl:ObjectProperty rdf:about="http://bibframe.org/vocab/subseries">
        <rdfs:label>Has subseries</rdfs:label>
        <rdfs:comment>Work, which is part of another series, in which the part has been issued.</rdfs:comment>
        <dcterms:modified>2014-10-14 (Updated)</dcterms:modified>
        <rdfs:domain rdf:resource="http://bibframe.org/vocab/Work"/>
        <rdfs:range rdf:resource="http://bibframe.org/vocab/Work"/>
        <rdfs:subPropertyOf rdf:resource="http://bibframe.org/vocab/hasPart"/>
    </owl:ObjectProperty>
    


    <!-- http://bibframe.org/vocab/subseriesOf -->

    <owl:ObjectProperty rdf:about="http://bibframe.org/vocab/subseriesOf">
        <rdfs:label>Subseries of</rdfs:label>
        <rdfs:comment>Work in which the part consistently appears; the title of the larger work appears on all issues or parts of the subseries).</rdfs:comment>
        <dcterms:modified>2014-10-14 (Updated)</dcterms:modified>
        <rdfs:domain rdf:resource="http://bibframe.org/vocab/Work"/>
        <rdfs:range rdf:resource="http://bibframe.org/vocab/Work"/>
        <rdfs:subPropertyOf rdf:resource="http://bibframe.org/vocab/partOf"/>
        <owl:inverseOf rdf:resource="http://bibframe.org/vocab/subseries"/>
    </owl:ObjectProperty>
    


    <!-- http://bibframe.org/vocab/succeededBy -->

    <owl:ObjectProperty rdf:about="http://bibframe.org/vocab/succeededBy">
        <rdfs:label>Succeeded By</rdfs:label>
        <dcterms:modified>2014-04-10 (Renamed)</dcterms:modified>
        <rdfs:comment>Resource that succeeds the resource being described (e.g., later in time or after in a narrative).</rdfs:comment>
        <rdfs:subPropertyOf rdf:resource="http://bibframe.org/vocab/relatedTo"/>
    </owl:ObjectProperty>
    


    <!-- http://bibframe.org/vocab/summary -->

    <owl:ObjectProperty rdf:about="http://bibframe.org/vocab/summary">
        <rdfs:label>Summary content</rdfs:label>
        <rdfs:comment>Summary or abstract of the target work or instance.</rdfs:comment>
        <rdfs:subPropertyOf rdf:resource="http://bibframe.org/vocab/annotationBody"/>
        <rdfs:range rdf:resource="&rdfs;Resource"/>
    </owl:ObjectProperty>
    


    <!-- http://bibframe.org/vocab/summaryOf -->

    <owl:ObjectProperty rdf:about="http://bibframe.org/vocab/summaryOf">
        <rdfs:label>Resource summarized</rdfs:label>
        <rdfs:comment>Resource to which the description pertains.</rdfs:comment>
        <rdfs:subPropertyOf rdf:resource="http://bibframe.org/vocab/annotates"/>
    </owl:ObjectProperty>
    


    <!-- http://bibframe.org/vocab/supersededBy -->

    <owl:ObjectProperty rdf:about="http://bibframe.org/vocab/supersededBy">
        <rdfs:label>Superseded by</rdfs:label>
        <dcterms:modified>2014-04-10 (Updated subproperty)</dcterms:modified>
        <rdfs:comment>Later Work used in place of an earlier work, usually because the later work contains updated or new information.</rdfs:comment>
        <rdfs:domain rdf:resource="http://bibframe.org/vocab/Work"/>
        <rdfs:range rdf:resource="http://bibframe.org/vocab/Work"/>
        <rdfs:subPropertyOf rdf:resource="http://bibframe.org/vocab/succeededBy"/>
        <owl:inverseOf rdf:resource="http://bibframe.org/vocab/supersedes"/>
    </owl:ObjectProperty>
    


    <!-- http://bibframe.org/vocab/supersededInPartBy -->

    <owl:ObjectProperty rdf:about="http://bibframe.org/vocab/supersededInPartBy">
        <rdfs:label>Superseded in part by</rdfs:label>
        <rdfs:comment>Later Work used in part in place of an earlier work, usually because the later work contains updated or new information.</rdfs:comment>
        <dcterms:modified>2014-04-10 (Updated subproperty)</dcterms:modified>
        <rdfs:domain rdf:resource="http://bibframe.org/vocab/Work"/>
        <rdfs:range rdf:resource="http://bibframe.org/vocab/Work"/>
        <rdfs:subPropertyOf rdf:resource="http://bibframe.org/vocab/succeededBy"/>
        <owl:inverseOf rdf:resource="http://bibframe.org/vocab/supersedesInPart"/>
    </owl:ObjectProperty>
    


    <!-- http://bibframe.org/vocab/supersedes -->

    <owl:ObjectProperty rdf:about="http://bibframe.org/vocab/supersedes">
        <rdfs:label>Supersedes</rdfs:label>
        <dcterms:modified>2014-04-10 (Updated subproperty)</dcterms:modified>
        <rdfs:comment>Earlier work whose content has been replaced by a later work, usually because the later work contains updated or new information.</rdfs:comment>
        <rdfs:domain rdf:resource="http://bibframe.org/vocab/Work"/>
        <rdfs:range rdf:resource="http://bibframe.org/vocab/Work"/>
        <rdfs:subPropertyOf rdf:resource="http://bibframe.org/vocab/precededBy"/>
    </owl:ObjectProperty>
    


    <!-- http://bibframe.org/vocab/supersedesInPart -->

    <owl:ObjectProperty rdf:about="http://bibframe.org/vocab/supersedesInPart">
        <rdfs:label>Supersedes in part</rdfs:label>
        <dcterms:modified>2014-04-10 (Updated subproperty)</dcterms:modified>
        <rdfs:comment>Earlier work whose content has been partially replaced by a later work, usually because the later work contains updated or new information.</rdfs:comment>
        <rdfs:domain rdf:resource="http://bibframe.org/vocab/Work"/>
        <rdfs:range rdf:resource="http://bibframe.org/vocab/Work"/>
        <rdfs:subPropertyOf rdf:resource="http://bibframe.org/vocab/precededBy"/>
    </owl:ObjectProperty>
    


    <!-- http://bibframe.org/vocab/supplement -->

    <owl:ObjectProperty rdf:about="http://bibframe.org/vocab/supplement">
        <rdfs:label>Has supplement</rdfs:label>
        <rdfs:comment>Work that updates or otherwise complements the predominant work.</rdfs:comment>
        <rdfs:range rdf:resource="http://bibframe.org/vocab/Work"/>
        <rdfs:domain rdf:resource="http://bibframe.org/vocab/Work"/>
        <rdfs:subPropertyOf rdf:resource="http://bibframe.org/vocab/accompaniedBy"/>
    </owl:ObjectProperty>
    


    <!-- http://bibframe.org/vocab/supplementTo -->

    <owl:ObjectProperty rdf:about="http://bibframe.org/vocab/supplementTo">
        <rdfs:label>Supplement to</rdfs:label>
        <rdfs:comment>Work that is updated or otherwise complemented by the augmenting work.</rdfs:comment>
        <rdfs:range rdf:resource="http://bibframe.org/vocab/Work"/>
        <rdfs:domain rdf:resource="http://bibframe.org/vocab/Work"/>
        <rdfs:subPropertyOf rdf:resource="http://bibframe.org/vocab/accompanies"/>
        <owl:inverseOf rdf:resource="http://bibframe.org/vocab/supplement"/>
    </owl:ObjectProperty>
    


    <!-- http://bibframe.org/vocab/systemNumber -->

    <owl:ObjectProperty rdf:about="http://bibframe.org/vocab/systemNumber">
        <rdfs:label>System control number</rdfs:label>
        <rdfs:comment>Control number of a system other than LCCN or NBAN, which Identifies a resource description.</rdfs:comment>
        <rdfs:range rdf:resource="http://bibframe.org/vocab/Identifier"/>
        <rdfs:subPropertyOf rdf:resource="http://bibframe.org/vocab/identifier"/>
    </owl:ObjectProperty>
    


    <!-- http://bibframe.org/vocab/tableOfContents -->

    <owl:ObjectProperty rdf:about="http://bibframe.org/vocab/tableOfContents">
        <rdfs:label>Table of contents content</rdfs:label>
        <rdfs:comment>Table of contents of the target work or instance.</rdfs:comment>
        <rdfs:subPropertyOf rdf:resource="http://bibframe.org/vocab/annotationBody"/>
        <rdfs:range rdf:resource="&rdfs;Resource"/>
    </owl:ObjectProperty>
    


    <!-- http://bibframe.org/vocab/tableOfContentsFor -->

    <owl:ObjectProperty rdf:about="http://bibframe.org/vocab/tableOfContentsFor">
        <rdfs:label>Table of contents of resource</rdfs:label>
        <rdfs:comment>Resource to which the table of contents pertains.</rdfs:comment>
        <rdfs:subPropertyOf rdf:resource="http://bibframe.org/vocab/annotates"/>
        <owl:inverseOf rdf:resource="http://bibframe.org/vocab/tableOfContents"/>
        <rdfs:range rdf:resource="&rdfs;Resource"/>
    </owl:ObjectProperty>
    


    <!-- http://bibframe.org/vocab/titleVariation -->

    <owl:ObjectProperty rdf:about="http://bibframe.org/vocab/titleVariation">
        <rdfs:label>Title variation</rdfs:label>
        <rdfs:comment>Title associated with the resource that is different from the main title.</rdfs:comment>
        <rdfs:range rdf:resource="http://bibframe.org/vocab/Title"/>
    </owl:ObjectProperty>
    


    <!-- http://bibframe.org/vocab/translation -->

    <owl:ObjectProperty rdf:about="http://bibframe.org/vocab/translation">
        <rdfs:label>Has translation</rdfs:label>
        <rdfs:comment>Work that translates the text of the source entity into a language different from that of the original.</rdfs:comment>
        <rdfs:range rdf:resource="http://bibframe.org/vocab/Work"/>
        <rdfs:domain rdf:resource="http://bibframe.org/vocab/Work"/>
        <rdfs:subPropertyOf rdf:resource="http://bibframe.org/vocab/derivativeOf"/>
    </owl:ObjectProperty>
    


    <!-- http://bibframe.org/vocab/translationOf -->

    <owl:ObjectProperty rdf:about="http://bibframe.org/vocab/translationOf">
        <rdfs:label>Translation of</rdfs:label>
        <rdfs:comment>Work that has been translated, i.e., the text expressed in a language different from that of the original work).</rdfs:comment>
        <rdfs:range rdf:resource="http://bibframe.org/vocab/Work"/>
        <rdfs:domain rdf:resource="http://bibframe.org/vocab/Work"/>
        <rdfs:subPropertyOf rdf:resource="http://bibframe.org/vocab/hasDerivative"/>
        <owl:inverseOf rdf:resource="http://bibframe.org/vocab/translation"/>
    </owl:ObjectProperty>
    


    <!-- http://bibframe.org/vocab/unionOf -->

    <owl:ObjectProperty rdf:about="http://bibframe.org/vocab/unionOf">
        <rdfs:label>Union of</rdfs:label>
        <dcterms:modified>2014-04-10 (Updated subproperty)</dcterms:modified>
        <rdfs:comment>One of two or more works which came together to form a new work.</rdfs:comment>
        <rdfs:domain rdf:resource="http://bibframe.org/vocab/Work"/>
        <rdfs:range rdf:resource="http://bibframe.org/vocab/Work"/>
        <owl:inverseOf rdf:resource="http://bibframe.org/vocab/mergedToForm"/>
        <rdfs:subPropertyOf rdf:resource="http://bibframe.org/vocab/precededBy"/>
    </owl:ObjectProperty>
    


    <!-- http://bibframe.org/vocab/upc -->

    <owl:ObjectProperty rdf:about="http://bibframe.org/vocab/upc">
        <rdfs:label>UPC</rdfs:label>
        <rdfs:comment>Universal Product Code.</rdfs:comment>
        <rdfs:range rdf:resource="http://bibframe.org/vocab/Identifier"/>
        <rdfs:domain rdf:resource="http://bibframe.org/vocab/Instance"/>
        <rdfs:subPropertyOf rdf:resource="http://bibframe.org/vocab/identifier"/>
    </owl:ObjectProperty>
    


    <!-- http://bibframe.org/vocab/uri -->

    <owl:ObjectProperty rdf:about="http://bibframe.org/vocab/uri">
        <rdfs:label>URI</rdfs:label>
        <rdfs:comment>Uniform Resource Identifier.</rdfs:comment>
        <rdfs:range rdf:resource="http://bibframe.org/vocab/Identifier"/>
        <rdfs:subPropertyOf rdf:resource="http://bibframe.org/vocab/identifier"/>
    </owl:ObjectProperty>
    


    <!-- http://bibframe.org/vocab/urn -->

    <owl:ObjectProperty rdf:about="http://bibframe.org/vocab/urn">
        <rdfs:label>URN</rdfs:label>
        <rdfs:comment>Uniform Resource Number.</rdfs:comment>
        <rdfs:range rdf:resource="http://bibframe.org/vocab/Identifier"/>
        <rdfs:domain rdf:resource="http://bibframe.org/vocab/Instance"/>
        <rdfs:subPropertyOf rdf:resource="http://bibframe.org/vocab/identifier"/>
    </owl:ObjectProperty>
    


    <!-- http://bibframe.org/vocab/videorecordingNumber -->

    <owl:ObjectProperty rdf:about="http://bibframe.org/vocab/videorecordingNumber">
        <rdfs:label>Videorecording number</rdfs:label>
        <rdfs:comment>Number assigned by a publisher to a videorecording.</rdfs:comment>
        <rdfs:range rdf:resource="http://bibframe.org/vocab/Identifier"/>
        <rdfs:domain rdf:resource="http://bibframe.org/vocab/Instance"/>
        <rdfs:subPropertyOf rdf:resource="http://bibframe.org/vocab/identifier"/>
    </owl:ObjectProperty>
    


    <!-- http://bibframe.org/vocab/workTitle -->

    <owl:ObjectProperty rdf:about="http://bibframe.org/vocab/workTitle">
        <rdfs:label>Work title</rdfs:label>
        <rdfs:comment>Title or form of title chosen to identify the work, such as a preferred title, preferred title with additions, uniform title, etc..</rdfs:comment>
        <rdfs:range rdf:resource="http://bibframe.org/vocab/Title"/>
        <rdfs:domain rdf:resource="http://bibframe.org/vocab/Work"/>
    </owl:ObjectProperty>
    


    <!-- http://id.loc.gov/vocabulary/relators/cre -->

    <owl:ObjectProperty rdf:about="&marcrel;cre">
        <v1:code>cre</v1:code>
        <v1:definitionNote>A person or organization responsible for the intellectual or artistic content of a resource</v1:definitionNote>
        <v1:authoritativeLabel xml:lang="en">Creator</v1:authoritativeLabel>
        <v1:isMemberOfMADSScheme rdf:resource="http://id.loc.gov/vocabulary/relators"/>
        <v1:isMemberOfMADSCollection rdf:resource="&marcrel;collection_BIBFRAMEWork"/>
        <v1:isMemberOfMADSCollection rdf:resource="&marcrel;collection_RDA"/>
        <v1:isMemberOfMADSCollection rdf:resource="&marcrel;collection_RDACreator"/>
        <v1:isMemberOfMADSCollection rdf:resource="&marcrel;collection_RDAWork"/>
        <rdfs:subPropertyOf rdf:resource="&marcrel;role"/>
        <rdfs:subPropertyOf rdf:resource="&dc;contributor"/>
        <rdfs:subPropertyOf rdf:resource="&dc;creator"/>
        <v1:adminMetadata>
            <rdf:Description>
                <rdf:type rdf:resource="&RecordInfo;RecordInfo"/>
                <RecordInfo:recordContentSource rdf:resource="http://id.loc.gov/vocabulary/organizations/dlcmrc"/>
            </rdf:Description>
        </v1:adminMetadata>
        <v1:adminMetadata>
            <rdf:Description>
                <rdf:type rdf:resource="&RecordInfo;RecordInfo"/>
                <RecordInfo:recordContentSource rdf:resource="http://id.loc.gov/vocabulary/organizations/dlcmrc"/>
            </rdf:Description>
        </v1:adminMetadata>
        <v1:adminMetadata>
            <rdf:Description>
                <rdf:type rdf:resource="&RecordInfo;RecordInfo"/>
                <RecordInfo:recordContentSource rdf:resource="http://id.loc.gov/vocabulary/organizations/dlcmrc"/>
            </rdf:Description>
        </v1:adminMetadata>
        <v1:adminMetadata>
            <rdf:Description>
                <rdf:type rdf:resource="&RecordInfo;RecordInfo"/>
                <RecordInfo:recordContentSource rdf:resource="http://id.loc.gov/vocabulary/organizations/dlcmrc"/>
            </rdf:Description>
        </v1:adminMetadata>
        <v1:adminMetadata>
            <rdf:Description>
                <rdf:type rdf:resource="&RecordInfo;RecordInfo"/>
                <RecordInfo:recordContentSource rdf:resource="http://id.loc.gov/vocabulary/organizations/dlcmrc"/>
            </rdf:Description>
        </v1:adminMetadata>
        <v1:adminMetadata>
            <rdf:Description>
                <rdf:type rdf:resource="&RecordInfo;RecordInfo"/>
                <RecordInfo:recordContentSource rdf:resource="http://id.loc.gov/vocabulary/organizations/dlcmrc"/>
            </rdf:Description>
        </v1:adminMetadata>
        <v1:adminMetadata>
            <rdf:Description>
                <rdf:type rdf:resource="&RecordInfo;RecordInfo"/>
                <RecordInfo:recordContentSource rdf:resource="http://id.loc.gov/vocabulary/organizations/dlcmrc"/>
            </rdf:Description>
        </v1:adminMetadata>
        <v1:adminMetadata>
            <rdf:Description>
                <rdf:type rdf:resource="&RecordInfo;RecordInfo"/>
                <RecordInfo:recordContentSource rdf:resource="http://id.loc.gov/vocabulary/organizations/dlcmrc"/>
            </rdf:Description>
        </v1:adminMetadata>
    </owl:ObjectProperty>
    


    <!-- http://id.loc.gov/vocabulary/relators/ctb -->

    <owl:ObjectProperty rdf:about="&marcrel;ctb">
        <v1:definitionNote>A person, family or organization responsible for making contributions to the resource. This includes those whose work has been contributed to a larger work, such as an anthology, serial publication, or other compilation of individual works. If a more specific role is available, prefer that, e.g. editor, compiler, illustrator</v1:definitionNote>
        <v1:editorialNote>Changed MARC def; Collaborator deprecated in MARC list and reference made</v1:editorialNote>
        <v1:code>ctb</v1:code>
        <v1:authoritativeLabel xml:lang="en">Contributor</v1:authoritativeLabel>
        <v1:isMemberOfMADSScheme rdf:resource="http://id.loc.gov/vocabulary/relators"/>
        <v1:isMemberOfMADSCollection rdf:resource="&marcrel;collection_BIBFRAMEWork"/>
        <v1:isMemberOfMADSCollection rdf:resource="&marcrel;collection_RDA"/>
        <v1:isMemberOfMADSCollection rdf:resource="&marcrel;collection_RDAContributor"/>
        <v1:isMemberOfMADSCollection rdf:resource="&marcrel;collection_RDAExpression"/>
        <rdfs:subPropertyOf rdf:resource="&marcrel;role"/>
        <rdfs:subPropertyOf rdf:resource="&dc;contributor"/>
        <v1:hasVariant>
            <rdf:Description>
                <rdf:type rdf:resource="&v1;Topic"/>
            </rdf:Description>
        </v1:hasVariant>
        <v1:hasVariant>
            <rdf:Description>
                <rdf:type rdf:resource="&v1;Topic"/>
            </rdf:Description>
        </v1:hasVariant>
        <v1:adminMetadata>
            <rdf:Description>
                <rdf:type rdf:resource="&RecordInfo;RecordInfo"/>
                <RecordInfo:recordContentSource rdf:resource="http://id.loc.gov/vocabulary/organizations/dlcmrc"/>
            </rdf:Description>
        </v1:adminMetadata>
        <v1:adminMetadata>
            <rdf:Description>
                <rdf:type rdf:resource="&RecordInfo;RecordInfo"/>
                <RecordInfo:recordContentSource rdf:resource="http://id.loc.gov/vocabulary/organizations/dlcmrc"/>
            </rdf:Description>
        </v1:adminMetadata>
        <v1:adminMetadata>
            <rdf:Description>
                <rdf:type rdf:resource="&RecordInfo;RecordInfo"/>
                <RecordInfo:recordContentSource rdf:resource="http://id.loc.gov/vocabulary/organizations/dlcmrc"/>
            </rdf:Description>
        </v1:adminMetadata>
        <v1:hasVariant>
            <rdf:Description>
                <rdf:type rdf:resource="&v1;Topic"/>
            </rdf:Description>
        </v1:hasVariant>
        <v1:adminMetadata>
            <rdf:Description>
                <rdf:type rdf:resource="&RecordInfo;RecordInfo"/>
                <RecordInfo:recordContentSource rdf:resource="http://id.loc.gov/vocabulary/organizations/dlcmrc"/>
            </rdf:Description>
        </v1:adminMetadata>
        <v1:adminMetadata>
            <rdf:Description>
                <rdf:type rdf:resource="&RecordInfo;RecordInfo"/>
                <RecordInfo:recordContentSource rdf:resource="http://id.loc.gov/vocabulary/organizations/dlcmrc"/>
            </rdf:Description>
        </v1:adminMetadata>
        <v1:adminMetadata>
            <rdf:Description>
                <rdf:type rdf:resource="&RecordInfo;RecordInfo"/>
                <RecordInfo:recordContentSource rdf:resource="http://id.loc.gov/vocabulary/organizations/dlcmrc"/>
            </rdf:Description>
        </v1:adminMetadata>
        <v1:adminMetadata>
            <rdf:Description>
                <rdf:type rdf:resource="&RecordInfo;RecordInfo"/>
                <RecordInfo:recordContentSource rdf:resource="http://id.loc.gov/vocabulary/organizations/dlcmrc"/>
            </rdf:Description>
        </v1:adminMetadata>
        <v1:adminMetadata>
            <rdf:Description>
                <rdf:type rdf:resource="&RecordInfo;RecordInfo"/>
                <RecordInfo:recordContentSource rdf:resource="http://id.loc.gov/vocabulary/organizations/dlcmrc"/>
            </rdf:Description>
        </v1:adminMetadata>
        <v1:hasVariant>
            <rdf:Description>
                <rdf:type rdf:resource="&v1;Topic"/>
            </rdf:Description>
        </v1:hasVariant>
    </owl:ObjectProperty>
    


    <!-- http://id.loc.gov/vocabulary/relators/role -->

    <owl:ObjectProperty rdf:about="&marcrel;role"/>
    


    <!-- http://purl.org/dc/elements/1.1/contributor -->

    <owl:ObjectProperty rdf:about="&dc;contributor"/>
    


    <!-- http://purl.org/dc/elements/1.1/creator -->

    <owl:ObjectProperty rdf:about="&dc;creator"/>
    


    <!-- http://purl.org/dc/terms/accessRights -->

    <owl:ObjectProperty rdf:about="&dcterms;accessRights">
        <rdfs:label xml:lang="en">Access Rights</rdfs:label>
        <dcterms:issued rdf:datatype="&xsd;date">2003-02-15</dcterms:issued>
        <dcterms:modified rdf:datatype="&xsd;date">2008-01-14</dcterms:modified>
        <dcterms:description xml:lang="en">Access Rights may include information regarding access or restrictions based on privacy, security, or other policies.</dcterms:description>
        <rdfs:comment xml:lang="en">Information about who can access the resource or an indication of its security status.</rdfs:comment>
        <dcterms:hasVersion rdf:resource="http://dublincore.org/usage/terms/history/#accessRights-002"/>
        <rdfs:isDefinedBy rdf:resource="http://purl.org/dc/terms/"/>
        <rdfs:range rdf:resource="&dcterms;RightsStatement"/>
        <rdfs:subPropertyOf rdf:resource="&dcterms;rights"/>
    </owl:ObjectProperty>
    


    <!-- http://purl.org/dc/terms/accrualMethod -->

    <owl:ObjectProperty rdf:about="&dcterms;accrualMethod">
        <rdfs:label xml:lang="en">Accrual Method</rdfs:label>
        <dcterms:issued rdf:datatype="&xsd;date">2005-06-13</dcterms:issued>
        <dcterms:modified rdf:datatype="&xsd;date">2010-10-11</dcterms:modified>
        <rdfs:comment xml:lang="en">The method by which items are added to a collection.</rdfs:comment>
        <dcterms:hasVersion rdf:resource="http://dublincore.org/usage/terms/history/#accrualMethod-003"/>
        <rdfs:isDefinedBy rdf:resource="http://purl.org/dc/terms/"/>
        <rdfs:range rdf:resource="&dcterms;MethodOfAccrual"/>
    </owl:ObjectProperty>
    


    <!-- http://purl.org/dc/terms/accrualPeriodicity -->

    <owl:ObjectProperty rdf:about="&dcterms;accrualPeriodicity">
        <rdfs:label xml:lang="en">Accrual Periodicity</rdfs:label>
        <dcterms:issued rdf:datatype="&xsd;date">2005-06-13</dcterms:issued>
        <dcterms:modified rdf:datatype="&xsd;date">2010-10-11</dcterms:modified>
        <rdfs:comment xml:lang="en">The frequency with which items are added to a collection.</rdfs:comment>
        <dcterms:hasVersion rdf:resource="http://dublincore.org/usage/terms/history/#accrualPeriodicity-003"/>
        <rdfs:isDefinedBy rdf:resource="http://purl.org/dc/terms/"/>
        <rdfs:range rdf:resource="&dcterms;Frequency"/>
    </owl:ObjectProperty>
    


    <!-- http://purl.org/dc/terms/accrualPolicy -->

    <owl:ObjectProperty rdf:about="&dcterms;accrualPolicy">
        <rdfs:label xml:lang="en">Accrual Policy</rdfs:label>
        <dcterms:issued rdf:datatype="&xsd;date">2005-06-13</dcterms:issued>
        <dcterms:modified rdf:datatype="&xsd;date">2010-10-11</dcterms:modified>
        <rdfs:comment xml:lang="en">The policy governing the addition of items to a collection.</rdfs:comment>
        <dcterms:hasVersion rdf:resource="http://dublincore.org/usage/terms/history/#accrualPolicy-003"/>
        <rdfs:isDefinedBy rdf:resource="http://purl.org/dc/terms/"/>
        <rdfs:range rdf:resource="&dcterms;Policy"/>
    </owl:ObjectProperty>
    


    <!-- http://purl.org/dc/terms/audience -->

    <owl:ObjectProperty rdf:about="&dcterms;audience">
        <rdfs:label xml:lang="en">Audience</rdfs:label>
        <dcterms:issued rdf:datatype="&xsd;date">2001-05-21</dcterms:issued>
        <dcterms:modified rdf:datatype="&xsd;date">2008-01-14</dcterms:modified>
        <rdfs:comment xml:lang="en">A class of entity for whom the resource is intended or useful.</rdfs:comment>
        <dcterms:hasVersion rdf:resource="http://dublincore.org/usage/terms/history/#audience-003"/>
        <rdfs:isDefinedBy rdf:resource="http://purl.org/dc/terms/"/>
        <rdfs:range rdf:resource="&dcterms;AgentClass"/>
    </owl:ObjectProperty>
    


    <!-- http://purl.org/dc/terms/conformsTo -->

    <owl:ObjectProperty rdf:about="&dcterms;conformsTo">
        <rdfs:label xml:lang="en">Conforms To</rdfs:label>
        <dcterms:issued rdf:datatype="&xsd;date">2001-05-21</dcterms:issued>
        <dcterms:modified rdf:datatype="&xsd;date">2008-01-14</dcterms:modified>
        <rdfs:comment xml:lang="en">An established standard to which the described resource conforms.</rdfs:comment>
        <dcterms:hasVersion rdf:resource="http://dublincore.org/usage/terms/history/#conformsTo-003"/>
        <rdfs:isDefinedBy rdf:resource="http://purl.org/dc/terms/"/>
        <rdfs:range rdf:resource="&dcterms;Standard"/>
    </owl:ObjectProperty>
    


    <!-- http://purl.org/dc/terms/contributor -->

    <owl:ObjectProperty rdf:about="&dcterms;contributor">
        <rdfs:label xml:lang="en">Contributor</rdfs:label>
        <dcterms:issued rdf:datatype="&xsd;date">2008-01-14</dcterms:issued>
        <dcterms:modified rdf:datatype="&xsd;date">2010-10-11</dcterms:modified>
        <rdfs:comment xml:lang="en">An entity responsible for making contributions to the resource.</rdfs:comment>
        <dcterms:description xml:lang="en">Examples of a Contributor include a person, an organization, or a service.</dcterms:description>
        <dcterms:hasVersion rdf:resource="http://dublincore.org/usage/terms/history/#contributorT-001"/>
        <rdfs:subPropertyOf rdf:resource="&dc;contributor"/>
        <rdfs:isDefinedBy rdf:resource="http://purl.org/dc/terms/"/>
        <rdfs:range rdf:resource="&dcterms;Agent"/>
    </owl:ObjectProperty>
    


    <!-- http://purl.org/dc/terms/coverage -->

    <owl:ObjectProperty rdf:about="&dcterms;coverage">
        <rdfs:label xml:lang="en">Coverage</rdfs:label>
        <dcterms:modified rdf:datatype="&xsd;date">2008-01-14</dcterms:modified>
        <dcterms:issued rdf:datatype="&xsd;date">2008-01-14</dcterms:issued>
        <dcterms:description xml:lang="en">Spatial topic and spatial applicability may be a named place or a location specified by its geographic coordinates. Temporal topic may be a named period, date, or date range. A jurisdiction may be a named administrative entity or a geographic place to which the resource applies. Recommended best practice is to use a controlled vocabulary such as the Thesaurus of Geographic Names [TGN]. Where appropriate, named places or time periods can be used in preference to numeric identifiers such as sets of coordinates or date ranges.</dcterms:description>
        <rdfs:comment xml:lang="en">The spatial or temporal topic of the resource, the spatial applicability of the resource, or the jurisdiction under which the resource is relevant.</rdfs:comment>
        <dcterms:hasVersion rdf:resource="http://dublincore.org/usage/terms/history/#coverageT-001"/>
        <rdfs:isDefinedBy rdf:resource="http://purl.org/dc/terms/"/>
        <rdfs:range rdf:resource="&dcterms;LocationPeriodOrJurisdiction"/>
    </owl:ObjectProperty>
    


    <!-- http://purl.org/dc/terms/creator -->

    <owl:ObjectProperty rdf:about="&dcterms;creator">
        <rdfs:label xml:lang="en">Creator</rdfs:label>
        <dcterms:issued rdf:datatype="&xsd;date">2008-01-14</dcterms:issued>
        <dcterms:modified rdf:datatype="&xsd;date">2010-10-11</dcterms:modified>
        <rdfs:comment xml:lang="en">An entity primarily responsible for making the resource.</rdfs:comment>
        <dcterms:description xml:lang="en">Examples of a Creator include a person, an organization, or a service.</dcterms:description>
        <dcterms:hasVersion rdf:resource="http://dublincore.org/usage/terms/history/#creatorT-002"/>
        <rdfs:subPropertyOf rdf:resource="&dc;creator"/>
        <rdfs:isDefinedBy rdf:resource="http://purl.org/dc/terms/"/>
        <rdfs:range rdf:resource="&dcterms;Agent"/>
        <rdfs:subPropertyOf rdf:resource="&dcterms;contributor"/>
    </owl:ObjectProperty>
    


    <!-- http://purl.org/dc/terms/educationLevel -->

    <owl:ObjectProperty rdf:about="&dcterms;educationLevel">
        <rdfs:label xml:lang="en">Audience Education Level</rdfs:label>
        <dcterms:issued rdf:datatype="&xsd;date">2002-07-13</dcterms:issued>
        <dcterms:modified rdf:datatype="&xsd;date">2008-01-14</dcterms:modified>
        <rdfs:comment xml:lang="en">A class of entity, defined in terms of progression through an educational or training context, for which the described resource is intended.</rdfs:comment>
        <dcterms:hasVersion rdf:resource="http://dublincore.org/usage/terms/history/#educationLevel-002"/>
        <rdfs:isDefinedBy rdf:resource="http://purl.org/dc/terms/"/>
        <rdfs:range rdf:resource="&dcterms;AgentClass"/>
        <rdfs:subPropertyOf rdf:resource="&dcterms;audience"/>
    </owl:ObjectProperty>
    


    <!-- http://purl.org/dc/terms/extent -->

    <owl:ObjectProperty rdf:about="&dcterms;extent">
        <rdfs:label xml:lang="en">Extent</rdfs:label>
        <dcterms:issued rdf:datatype="&xsd;date">2000-07-11</dcterms:issued>
        <dcterms:modified rdf:datatype="&xsd;date">2008-01-14</dcterms:modified>
        <rdfs:comment xml:lang="en">The size or duration of the resource.</rdfs:comment>
        <dcterms:hasVersion rdf:resource="http://dublincore.org/usage/terms/history/#extent-003"/>
        <rdfs:isDefinedBy rdf:resource="http://purl.org/dc/terms/"/>
        <rdfs:range rdf:resource="&dcterms;SizeOrDuration"/>
        <rdfs:subPropertyOf rdf:resource="&dcterms;format"/>
    </owl:ObjectProperty>
    


    <!-- http://purl.org/dc/terms/format -->

    <owl:ObjectProperty rdf:about="&dcterms;format">
        <rdfs:label xml:lang="en">Format</rdfs:label>
        <dcterms:modified rdf:datatype="&xsd;date">2008-01-14</dcterms:modified>
        <dcterms:issued rdf:datatype="&xsd;date">2008-01-14</dcterms:issued>
        <dcterms:description xml:lang="en">Examples of dimensions include size and duration. Recommended best practice is to use a controlled vocabulary such as the list of Internet Media Types [MIME].</dcterms:description>
        <rdfs:comment xml:lang="en">The file format, physical medium, or dimensions of the resource.</rdfs:comment>
        <dcterms:hasVersion rdf:resource="http://dublincore.org/usage/terms/history/#formatT-001"/>
        <rdfs:isDefinedBy rdf:resource="http://purl.org/dc/terms/"/>
        <rdfs:range rdf:resource="&dcterms;MediaTypeOrExtent"/>
    </owl:ObjectProperty>
    


    <!-- http://purl.org/dc/terms/instructionalMethod -->

    <owl:ObjectProperty rdf:about="&dcterms;instructionalMethod">
        <rdfs:label xml:lang="en">Instructional Method</rdfs:label>
        <dcterms:issued rdf:datatype="&xsd;date">2005-06-13</dcterms:issued>
        <dcterms:modified rdf:datatype="&xsd;date">2008-01-14</dcterms:modified>
        <rdfs:comment xml:lang="en">A process, used to engender knowledge, attitudes and skills, that the described resource is designed to support.</rdfs:comment>
        <dcterms:description xml:lang="en">Instructional Method will typically include ways of presenting instructional materials or conducting instructional activities, patterns of learner-to-learner and learner-to-instructor interactions, and mechanisms by which group and individual levels of learning are measured.  Instructional methods include all aspects of the instruction and learning processes from planning and implementation through evaluation and feedback.</dcterms:description>
        <dcterms:hasVersion rdf:resource="http://dublincore.org/usage/terms/history/#instructionalMethod-002"/>
        <rdfs:isDefinedBy rdf:resource="http://purl.org/dc/terms/"/>
        <rdfs:range rdf:resource="&dcterms;MethodOfInstruction"/>
    </owl:ObjectProperty>
    


    <!-- http://purl.org/dc/terms/language -->

    <owl:ObjectProperty rdf:about="&dcterms;language">
        <rdfs:label xml:lang="en">Language</rdfs:label>
        <dcterms:issued rdf:datatype="&xsd;date">2008-01-14</dcterms:issued>
        <dcterms:modified rdf:datatype="&xsd;date">2008-01-14</dcterms:modified>
        <rdfs:comment xml:lang="en">A language of the resource.</rdfs:comment>
        <dcterms:description xml:lang="en">Recommended best practice is to use a controlled vocabulary such as RFC 4646 [RFC4646].</dcterms:description>
        <dcterms:hasVersion rdf:resource="http://dublincore.org/usage/terms/history/#languageT-001"/>
        <rdfs:isDefinedBy rdf:resource="http://purl.org/dc/terms/"/>
        <rdfs:range rdf:resource="&dcterms;LinguisticSystem"/>
    </owl:ObjectProperty>
    


    <!-- http://purl.org/dc/terms/license -->

    <owl:ObjectProperty rdf:about="&dcterms;license">
        <rdfs:label xml:lang="en">License</rdfs:label>
        <dcterms:issued rdf:datatype="&xsd;date">2004-06-14</dcterms:issued>
        <dcterms:modified rdf:datatype="&xsd;date">2008-01-14</dcterms:modified>
        <rdfs:comment xml:lang="en">A legal document giving official permission to do something with the resource.</rdfs:comment>
        <dcterms:hasVersion rdf:resource="http://dublincore.org/usage/terms/history/#license-002"/>
        <rdfs:isDefinedBy rdf:resource="http://purl.org/dc/terms/"/>
        <rdfs:range rdf:resource="&dcterms;LicenseDocument"/>
        <rdfs:subPropertyOf rdf:resource="&dcterms;rights"/>
    </owl:ObjectProperty>
    


    <!-- http://purl.org/dc/terms/mediator -->

    <owl:ObjectProperty rdf:about="&dcterms;mediator">
        <rdfs:label xml:lang="en">Mediator</rdfs:label>
        <dcterms:issued rdf:datatype="&xsd;date">2001-05-21</dcterms:issued>
        <dcterms:modified rdf:datatype="&xsd;date">2008-01-14</dcterms:modified>
        <rdfs:comment xml:lang="en">An entity that mediates access to the resource and for whom the resource is intended or useful.</rdfs:comment>
        <dcterms:description xml:lang="en">In an educational context, a mediator might be a parent, teacher, teaching assistant, or care-giver.</dcterms:description>
        <dcterms:hasVersion rdf:resource="http://dublincore.org/usage/terms/history/#mediator-003"/>
        <rdfs:isDefinedBy rdf:resource="http://purl.org/dc/terms/"/>
        <rdfs:range rdf:resource="&dcterms;AgentClass"/>
        <rdfs:subPropertyOf rdf:resource="&dcterms;audience"/>
    </owl:ObjectProperty>
    


    <!-- http://purl.org/dc/terms/medium -->

    <owl:ObjectProperty rdf:about="&dcterms;medium">
        <rdfs:label xml:lang="en">Medium</rdfs:label>
        <dcterms:issued rdf:datatype="&xsd;date">2000-07-11</dcterms:issued>
        <dcterms:modified rdf:datatype="&xsd;date">2008-01-14</dcterms:modified>
        <rdfs:comment xml:lang="en">The material or physical carrier of the resource.</rdfs:comment>
        <dcterms:hasVersion rdf:resource="http://dublincore.org/usage/terms/history/#medium-003"/>
        <rdfs:isDefinedBy rdf:resource="http://purl.org/dc/terms/"/>
        <rdfs:range rdf:resource="&dcterms;PhysicalMedium"/>
        <rdfs:domain rdf:resource="&dcterms;PhysicalResource"/>
        <rdfs:subPropertyOf rdf:resource="&dcterms;format"/>
    </owl:ObjectProperty>
    


    <!-- http://purl.org/dc/terms/provenance -->

    <owl:ObjectProperty rdf:about="&dcterms;provenance">
        <rdfs:label xml:lang="en">Provenance</rdfs:label>
        <dcterms:issued rdf:datatype="&xsd;date">2004-09-20</dcterms:issued>
        <dcterms:modified rdf:datatype="&xsd;date">2008-01-14</dcterms:modified>
        <rdfs:comment xml:lang="en">A statement of any changes in ownership and custody of the resource since its creation that are significant for its authenticity, integrity, and interpretation.</rdfs:comment>
        <dcterms:description xml:lang="en">The statement may include a description of any changes successive custodians made to the resource.</dcterms:description>
        <dcterms:hasVersion rdf:resource="http://dublincore.org/usage/terms/history/#provenance-002"/>
        <rdfs:isDefinedBy rdf:resource="http://purl.org/dc/terms/"/>
        <rdfs:range rdf:resource="&dcterms;ProvenanceStatement"/>
    </owl:ObjectProperty>
    


    <!-- http://purl.org/dc/terms/publisher -->

    <owl:ObjectProperty rdf:about="&dcterms;publisher">
        <rdfs:label xml:lang="en">Publisher</rdfs:label>
        <dcterms:issued rdf:datatype="&xsd;date">2008-01-14</dcterms:issued>
        <dcterms:modified rdf:datatype="&xsd;date">2010-10-11</dcterms:modified>
        <rdfs:comment xml:lang="en">An entity responsible for making the resource available.</rdfs:comment>
        <dcterms:description xml:lang="en">Examples of a Publisher include a person, an organization, or a service.</dcterms:description>
        <dcterms:hasVersion rdf:resource="http://dublincore.org/usage/terms/history/#publisherT-001"/>
        <rdfs:isDefinedBy rdf:resource="http://purl.org/dc/terms/"/>
        <rdfs:range rdf:resource="&dcterms;Agent"/>
    </owl:ObjectProperty>
    


    <!-- http://purl.org/dc/terms/rights -->

    <owl:ObjectProperty rdf:about="&dcterms;rights">
        <rdfs:label xml:lang="en">Rights</rdfs:label>
        <dcterms:modified rdf:datatype="&xsd;date">2008-01-14</dcterms:modified>
        <dcterms:issued rdf:datatype="&xsd;date">2008-01-14</dcterms:issued>
        <rdfs:comment xml:lang="en">Information about rights held in and over the resource.</rdfs:comment>
        <dcterms:description xml:lang="en">Typically, rights information includes a statement about various property rights associated with the resource, including intellectual property rights.</dcterms:description>
        <dcterms:hasVersion rdf:resource="http://dublincore.org/usage/terms/history/#rightsT-001"/>
        <rdfs:isDefinedBy rdf:resource="http://purl.org/dc/terms/"/>
        <rdfs:range rdf:resource="&dcterms;RightsStatement"/>
    </owl:ObjectProperty>
    


    <!-- http://purl.org/dc/terms/rightsHolder -->

    <owl:ObjectProperty rdf:about="&dcterms;rightsHolder">
        <rdfs:label xml:lang="en">Rights Holder</rdfs:label>
        <dcterms:issued rdf:datatype="&xsd;date">2004-06-14</dcterms:issued>
        <dcterms:modified rdf:datatype="&xsd;date">2008-01-14</dcterms:modified>
        <rdfs:comment xml:lang="en">A person or organization owning or managing rights over the resource.</rdfs:comment>
        <dcterms:hasVersion rdf:resource="http://dublincore.org/usage/terms/history/#rightsHolder-002"/>
        <rdfs:isDefinedBy rdf:resource="http://purl.org/dc/terms/"/>
        <rdfs:range rdf:resource="&dcterms;Agent"/>
    </owl:ObjectProperty>
    


    <!-- http://purl.org/dc/terms/spatial -->

    <owl:ObjectProperty rdf:about="&dcterms;spatial">
        <rdfs:label xml:lang="en">Spatial Coverage</rdfs:label>
        <dcterms:issued rdf:datatype="&xsd;date">2000-07-11</dcterms:issued>
        <dcterms:modified rdf:datatype="&xsd;date">2008-01-14</dcterms:modified>
        <rdfs:comment xml:lang="en">Spatial characteristics of the resource.</rdfs:comment>
        <dcterms:hasVersion rdf:resource="http://dublincore.org/usage/terms/history/#spatial-003"/>
        <rdfs:isDefinedBy rdf:resource="http://purl.org/dc/terms/"/>
        <rdfs:range rdf:resource="&dcterms;Location"/>
        <rdfs:subPropertyOf rdf:resource="&dcterms;coverage"/>
    </owl:ObjectProperty>
    


    <!-- http://purl.org/dc/terms/temporal -->

    <owl:ObjectProperty rdf:about="&dcterms;temporal">
        <rdfs:label xml:lang="en">Temporal Coverage</rdfs:label>
        <dcterms:issued rdf:datatype="&xsd;date">2000-07-11</dcterms:issued>
        <dcterms:modified rdf:datatype="&xsd;date">2008-01-14</dcterms:modified>
        <rdfs:comment xml:lang="en">Temporal characteristics of the resource.</rdfs:comment>
        <dcterms:hasVersion rdf:resource="http://dublincore.org/usage/terms/history/#temporal-003"/>
        <rdfs:isDefinedBy rdf:resource="http://purl.org/dc/terms/"/>
        <rdfs:range rdf:resource="&dcterms;PeriodOfTime"/>
        <rdfs:subPropertyOf rdf:resource="&dcterms;coverage"/>
    </owl:ObjectProperty>
    


    <!-- http://purl.org/dc/terms/type -->

    <owl:ObjectProperty rdf:about="&dcterms;type">
        <rdfs:label xml:lang="en">Type</rdfs:label>
        <dcterms:issued rdf:datatype="&xsd;date">2008-01-14</dcterms:issued>
        <dcterms:modified rdf:datatype="&xsd;date">2008-01-14</dcterms:modified>
        <dcterms:description xml:lang="en">Recommended best practice is to use a controlled vocabulary such as the DCMI Type Vocabulary [DCMITYPE]. To describe the file format, physical medium, or dimensions of the resource, use the Format element.</dcterms:description>
        <rdfs:comment xml:lang="en">The nature or genre of the resource.</rdfs:comment>
        <dcterms:hasVersion rdf:resource="http://dublincore.org/usage/terms/history/#typeT-001"/>
        <rdfs:isDefinedBy rdf:resource="http://purl.org/dc/terms/"/>
        <rdfs:range rdf:resource="&rdfs;Class"/>
    </owl:ObjectProperty>
    


    <!-- 
    ///////////////////////////////////////////////////////////////////////////////////////
    //
    // Data properties
    //
    ///////////////////////////////////////////////////////////////////////////////////////
     -->

    


    <!-- http://bibframe.org/vocab/accessCondition -->

    <owl:DatatypeProperty rdf:about="http://bibframe.org/vocab/accessCondition">
        <rdfs:label>Access condition</rdfs:label>
        <rdfs:comment>Allowances and restrictions on access.</rdfs:comment>
        <rdfs:range rdf:resource="&rdfs;Literal"/>
    </owl:DatatypeProperty>
    


    <!-- http://bibframe.org/vocab/aspectRatio -->

    <owl:DatatypeProperty rdf:about="http://bibframe.org/vocab/aspectRatio">
        <rdfs:label>Aspect ratio</rdfs:label>
        <rdfs:comment>Proportional relationship between an image&apos;s width and its height.</rdfs:comment>
        <rdfs:domain rdf:resource="http://bibframe.org/vocab/Instance"/>
        <rdfs:range rdf:resource="&rdfs;Literal"/>
    </owl:DatatypeProperty>
    


    <!-- http://bibframe.org/vocab/assertionDate -->

    <owl:DatatypeProperty rdf:about="http://bibframe.org/vocab/assertionDate">
        <rdfs:label>Annotation Assertion Date</rdfs:label>
        <rdfs:comment>Date when annotation was asserted.</rdfs:comment>
        <rdfs:range rdf:resource="&rdfs;Literal"/>
    </owl:DatatypeProperty>
    


    <!-- http://bibframe.org/vocab/audience -->

    <owl:DatatypeProperty rdf:about="http://bibframe.org/vocab/audience">
        <rdfs:label>Audience</rdfs:label>
        <rdfs:comment>Information that identifies the specific audience or intellectual level for which the content of the resource is considered appropriate.</rdfs:comment>
        <rdfs:domain rdf:resource="http://bibframe.org/vocab/IntendedAudience"/>
        <rdfs:range rdf:resource="&rdfs;Literal"/>
    </owl:DatatypeProperty>
    


    <!-- http://bibframe.org/vocab/audienceAssigner -->

    <owl:DatatypeProperty rdf:about="http://bibframe.org/vocab/audienceAssigner">
        <rdfs:label>Audience assigner</rdfs:label>
        <rdfs:comment>Entity that assigned the intended audience information.</rdfs:comment>
        <rdfs:domain rdf:resource="http://bibframe.org/vocab/IntendedAudience"/>
        <rdfs:range rdf:resource="&rdfs;Literal"/>
    </owl:DatatypeProperty>
    


    <!-- http://bibframe.org/vocab/authoritySource -->

    <owl:DatatypeProperty rdf:about="http://bibframe.org/vocab/authoritySource">
        <rdfs:label>Authority source</rdfs:label>
        <rdfs:comment>Authority list from which a value is taken.</rdfs:comment>
        <rdfs:range rdf:resource="&rdfs;Literal"/>
    </owl:DatatypeProperty>
    


    <!-- http://bibframe.org/vocab/authorizedAccessPoint -->

    <owl:DatatypeProperty rdf:about="http://bibframe.org/vocab/authorizedAccessPoint">
        <rdfs:label>Authorized access point</rdfs:label>
        <rdfs:comment>Controlled string form of a resource label intended to help uniquely identify it, such as a unique title or a unique name plus title.</rdfs:comment>
        <rdfs:range rdf:resource="&rdfs;Literal"/>
    </owl:DatatypeProperty>
    


    <!-- http://bibframe.org/vocab/awardNote -->

    <owl:DatatypeProperty rdf:about="http://bibframe.org/vocab/awardNote">
        <rdfs:label>Award note</rdfs:label>
        <rdfs:comment>Information on awards associated with the described resource.</rdfs:comment>
        <rdfs:domain rdf:resource="http://bibframe.org/vocab/Instance"/>
        <rdfs:range rdf:resource="&rdfs;Literal"/>
    </owl:DatatypeProperty>
    


    <!-- http://bibframe.org/vocab/barcode -->

    <owl:DatatypeProperty rdf:about="http://bibframe.org/vocab/barcode">
        <rdfs:label>Barcode</rdfs:label>
        <rdfs:comment>Identification number of the physical item.</rdfs:comment>
        <rdfs:range rdf:resource="&rdfs;Literal"/>
    </owl:DatatypeProperty>
    


    <!-- http://bibframe.org/vocab/cartographicAscensionAndDeclination -->

    <owl:DatatypeProperty rdf:about="http://bibframe.org/vocab/cartographicAscensionAndDeclination">
        <rdfs:label>Cartographic ascension and declination</rdfs:label>
        <rdfs:comment>System for identifying the location of a celestial object in the sky covered by the cartographic content of a resource using the angles of right ascension and declination.</rdfs:comment>
        <rdfs:domain rdf:resource="http://bibframe.org/vocab/Cartography"/>
        <rdfs:range rdf:resource="&rdfs;Literal"/>
    </owl:DatatypeProperty>
    


    <!-- http://bibframe.org/vocab/cartographicCoordinates -->

    <owl:DatatypeProperty rdf:about="http://bibframe.org/vocab/cartographicCoordinates">
        <rdfs:label>Cartographic coordinates</rdfs:label>
        <rdfs:comment>Mathematical system for identifying the area covered by the cartographic content of a resource, Expressed either by means of longitude and latitude on the surface of planets or by the angles of right ascension and declination for celestial cartographic content.</rdfs:comment>
        <rdfs:domain rdf:resource="http://bibframe.org/vocab/Cartography"/>
        <rdfs:range rdf:resource="&rdfs;Literal"/>
    </owl:DatatypeProperty>
    


    <!-- http://bibframe.org/vocab/cartographicEquinox -->

    <owl:DatatypeProperty rdf:about="http://bibframe.org/vocab/cartographicEquinox">
        <rdfs:label>Cartographic equinox</rdfs:label>
        <rdfs:comment>One of two points of intersection of the ecliptic and the celestial equator, occupied by the sun when its declination is 0 degrees.</rdfs:comment>
        <rdfs:domain rdf:resource="http://bibframe.org/vocab/Cartography"/>
        <rdfs:range rdf:resource="&rdfs;Literal"/>
    </owl:DatatypeProperty>
    


    <!-- http://bibframe.org/vocab/cartographicExclusionGRing -->

    <owl:DatatypeProperty rdf:about="http://bibframe.org/vocab/cartographicExclusionGRing">
        <rdfs:label>Cartographic G ring area excluded</rdfs:label>
        <rdfs:comment>Coordinate pairs that identify the closed non-intersecting boundary of the area contained within the G-polygon outer ring that is excluded.</rdfs:comment>
        <rdfs:domain rdf:resource="http://bibframe.org/vocab/Cartography"/>
        <rdfs:range rdf:resource="&rdfs;Literal"/>
    </owl:DatatypeProperty>
    


    <!-- http://bibframe.org/vocab/cartographicOuterGRing -->

    <owl:DatatypeProperty rdf:about="http://bibframe.org/vocab/cartographicOuterGRing">
        <rdfs:label>Cartographic outer G ring area covered</rdfs:label>
        <rdfs:comment>Coordinate pairs that identify the closed non-intersecting boundary of the area covered.</rdfs:comment>
        <rdfs:domain rdf:resource="http://bibframe.org/vocab/Cartography"/>
        <rdfs:range rdf:resource="&rdfs;Literal"/>
    </owl:DatatypeProperty>
    


    <!-- http://bibframe.org/vocab/cartographicProjection -->

    <owl:DatatypeProperty rdf:about="http://bibframe.org/vocab/cartographicProjection">
        <rdfs:label>Cartographic projection</rdfs:label>
        <rdfs:comment>Method or system used to represent the surface of the Earth or of a celestial sphere on a plane.</rdfs:comment>
        <rdfs:domain rdf:resource="http://bibframe.org/vocab/Cartography"/>
        <rdfs:range rdf:resource="&rdfs;Literal"/>
    </owl:DatatypeProperty>
    


    <!-- http://bibframe.org/vocab/cartographicScale -->

    <owl:DatatypeProperty rdf:about="http://bibframe.org/vocab/cartographicScale">
        <rdfs:label>Cartographic scale</rdfs:label>
        <rdfs:comment>Ratio of the dimensions of a form contained or embodied in a resource to the dimensions of the entity it represents.</rdfs:comment>
        <rdfs:domain rdf:resource="http://bibframe.org/vocab/Cartography"/>
        <rdfs:range rdf:resource="&rdfs;Literal"/>
    </owl:DatatypeProperty>
    


    <!-- http://bibframe.org/vocab/categorySource -->

    <owl:DatatypeProperty rdf:about="http://bibframe.org/vocab/categorySource">
        <rdfs:label>Category source</rdfs:label>
        <rdfs:comment>Category list from which value is taken.</rdfs:comment>
        <rdfs:domain rdf:resource="http://bibframe.org/vocab/Category"/>
        <rdfs:range rdf:resource="&rdfs;Literal"/>
    </owl:DatatypeProperty>
    


    <!-- http://bibframe.org/vocab/categoryType -->

    <owl:DatatypeProperty rdf:about="http://bibframe.org/vocab/categoryType">
        <rdfs:label>Type of category</rdfs:label>
        <rdfs:comment>Type of category recorded, e.g., content, genre, media, form, carrier.</rdfs:comment>
        <rdfs:domain rdf:resource="http://bibframe.org/vocab/Category"/>
        <rdfs:range rdf:resource="&rdfs;Literal"/>
    </owl:DatatypeProperty>
    


    <!-- http://bibframe.org/vocab/categoryValue -->

    <owl:DatatypeProperty rdf:about="http://bibframe.org/vocab/categoryValue">
        <rdfs:label>Category</rdfs:label>
        <rdfs:comment>Category code or text.</rdfs:comment>
        <rdfs:domain rdf:resource="http://bibframe.org/vocab/Category"/>
        <rdfs:range rdf:resource="&rdfs;Literal"/>
    </owl:DatatypeProperty>
    


    <!-- http://bibframe.org/vocab/changeDate -->

    <owl:DatatypeProperty rdf:about="http://bibframe.org/vocab/changeDate">
        <rdfs:label>Description change date</rdfs:label>
        <rdfs:comment>Date or date and time on which the metadata was modified.</rdfs:comment>
        <rdfs:range rdf:resource="&rdfs;Literal"/>
    </owl:DatatypeProperty>
    


    <!-- http://bibframe.org/vocab/circulationStatus -->

    <owl:DatatypeProperty rdf:about="http://bibframe.org/vocab/circulationStatus">
        <rdfs:label>Circulation status</rdfs:label>
        <rdfs:comment>Circulation status of an item.</rdfs:comment>
        <rdfs:range rdf:resource="&rdfs;Literal"/>
    </owl:DatatypeProperty>
    


    <!-- http://bibframe.org/vocab/classificationAssigner -->

    <owl:DatatypeProperty rdf:about="http://bibframe.org/vocab/classificationAssigner">
        <rdfs:label>Institution assigning classification</rdfs:label>
        <rdfs:comment>Entity that assigned the classification number.</rdfs:comment>
        <rdfs:domain rdf:resource="http://bibframe.org/vocab/Classification"/>
        <rdfs:range rdf:resource="&rdfs;Literal"/>
    </owl:DatatypeProperty>
    


    <!-- http://bibframe.org/vocab/classificationDesignation -->

    <owl:DatatypeProperty rdf:about="http://bibframe.org/vocab/classificationDesignation">
        <rdfs:label>Classification designation</rdfs:label>
        <rdfs:comment>Designates whether the classification number contained in the field is from the standard or optional part of the schedules or tables.</rdfs:comment>
        <rdfs:domain rdf:resource="http://bibframe.org/vocab/Classification"/>
        <rdfs:range rdf:resource="&rdfs;Literal"/>
    </owl:DatatypeProperty>
    


    <!-- http://bibframe.org/vocab/classificationEdition -->

    <owl:DatatypeProperty rdf:about="http://bibframe.org/vocab/classificationEdition">
        <rdfs:label>Classification scheme edition</rdfs:label>
        <rdfs:comment>Edition of the classification scheme, such as full, abridged or a number, when a classification scheme designates editions.</rdfs:comment>
        <dcterms:modified>2014-10-09 (Updated)</dcterms:modified>
        <rdfs:domain rdf:resource="http://bibframe.org/vocab/Classification"/>
        <rdfs:range rdf:resource="&rdfs;Literal"/>
    </owl:DatatypeProperty>
    


    <!-- http://bibframe.org/vocab/classificationItem -->

    <owl:DatatypeProperty rdf:about="http://bibframe.org/vocab/classificationItem">
        <rdfs:label>Classification item number</rdfs:label>
        <rdfs:comment>Number attached to a classification number that indicates a particular item.</rdfs:comment>
        <rdfs:domain rdf:resource="http://bibframe.org/vocab/Classification"/>
        <rdfs:range rdf:resource="&rdfs;Literal"/>
    </owl:DatatypeProperty>
    


    <!-- http://bibframe.org/vocab/classificationNumber -->

    <owl:DatatypeProperty rdf:about="http://bibframe.org/vocab/classificationNumber">
        <rdfs:label>Classification number</rdfs:label>
        <rdfs:comment>Classification number (single class number or beginning number of a span) that indicates the subject by applying a formal system of coding and organizing resources.</rdfs:comment>
        <rdfs:domain rdf:resource="http://bibframe.org/vocab/Classification"/>
        <rdfs:range rdf:resource="&rdfs;Literal"/>
    </owl:DatatypeProperty>
    


    <!-- http://bibframe.org/vocab/classificationScheme -->

    <owl:DatatypeProperty rdf:about="http://bibframe.org/vocab/classificationScheme">
        <rdfs:label>Classification scheme</rdfs:label>
        <rdfs:comment>Formal scheme from which a classification number is taken.</rdfs:comment>
        <rdfs:domain rdf:resource="http://bibframe.org/vocab/Classification"/>
        <rdfs:range rdf:resource="&rdfs;Literal"/>
    </owl:DatatypeProperty>
    


    <!-- http://bibframe.org/vocab/classificationSpanEnd -->

    <owl:DatatypeProperty rdf:about="http://bibframe.org/vocab/classificationSpanEnd">
        <rdfs:label>Classification number span end</rdfs:label>
        <rdfs:comment>Ending number of classification number span.</rdfs:comment>
        <rdfs:domain rdf:resource="http://bibframe.org/vocab/Classification"/>
        <rdfs:range rdf:resource="&rdfs;Literal"/>
    </owl:DatatypeProperty>
    


    <!-- http://bibframe.org/vocab/classificationStatus -->

    <owl:DatatypeProperty rdf:about="http://bibframe.org/vocab/classificationStatus">
        <rdfs:label>Classification status</rdfs:label>
        <rdfs:comment>Indicator that the classification number is canceled or invalid.</rdfs:comment>
        <rdfs:domain rdf:resource="http://bibframe.org/vocab/Classification"/>
        <rdfs:range rdf:resource="&rdfs;Literal"/>
    </owl:DatatypeProperty>
    


    <!-- http://bibframe.org/vocab/classificationTable -->

    <owl:DatatypeProperty rdf:about="http://bibframe.org/vocab/classificationTable">
        <rdfs:label>Classification table identification</rdfs:label>
        <rdfs:comment>DDC Table identification. Number of the table from which the classification number in a subdivision record is taken.</rdfs:comment>
        <rdfs:domain rdf:resource="http://bibframe.org/vocab/Classification"/>
        <rdfs:range rdf:resource="&rdfs;Literal"/>
    </owl:DatatypeProperty>
    


    <!-- http://bibframe.org/vocab/classificationTableSeq -->

    <owl:DatatypeProperty rdf:about="http://bibframe.org/vocab/classificationTableSeq">
        <rdfs:label>Classification table sequence number</rdfs:label>
        <rdfs:comment>Sequence number or other identifier for an internal classification subarrangement or add in a classification scheme.</rdfs:comment>
        <rdfs:domain rdf:resource="http://bibframe.org/vocab/Classification"/>
        <rdfs:range rdf:resource="&rdfs;Literal"/>
    </owl:DatatypeProperty>
    


    <!-- http://bibframe.org/vocab/colorContent -->

    <owl:DatatypeProperty rdf:about="http://bibframe.org/vocab/colorContent">
        <rdfs:label>Color content</rdfs:label>
        <rdfs:comment>Color characteristics, e.g. black and white, multicolored, etc.</rdfs:comment>
        <dcterms:modified>2014-10-14 (Updated)</dcterms:modified>
        <rdfs:domain rdf:resource="http://bibframe.org/vocab/Instance"/>
        <rdfs:range rdf:resource="&rdfs;Literal"/>
    </owl:DatatypeProperty>
    


    <!-- http://bibframe.org/vocab/contentAccessibility -->

    <owl:DatatypeProperty rdf:about="http://bibframe.org/vocab/contentAccessibility">
        <rdfs:label>Content accessibility note</rdfs:label>
        <rdfs:comment>Content that assists those with a sensory impairment for greater understanding of content, e.g., labels, captions.</rdfs:comment>
        <rdfs:domain rdf:resource="http://bibframe.org/vocab/Instance"/>
        <rdfs:range rdf:resource="&rdfs;Literal"/>
    </owl:DatatypeProperty>
    


    <!-- http://bibframe.org/vocab/contentsNote -->

    <owl:DatatypeProperty rdf:about="http://bibframe.org/vocab/contentsNote">
        <rdfs:label>Contents</rdfs:label>
        <rdfs:comment>List of subunits of the resource.</rdfs:comment>
        <rdfs:domain rdf:resource="http://bibframe.org/vocab/Instance"/>
        <rdfs:range rdf:resource="&rdfs;Literal"/>
    </owl:DatatypeProperty>
    


    <!-- http://bibframe.org/vocab/copyNote -->

    <owl:DatatypeProperty rdf:about="http://bibframe.org/vocab/copyNote">
        <rdfs:label>Copy note</rdfs:label>
        <rdfs:comment>Information about this copy.</rdfs:comment>
        <rdfs:range rdf:resource="&rdfs;Literal"/>
    </owl:DatatypeProperty>
    


    <!-- http://bibframe.org/vocab/copyrightDate -->

    <owl:DatatypeProperty rdf:about="http://bibframe.org/vocab/copyrightDate">
        <rdfs:label>Copyright date</rdfs:label>
        <rdfs:comment>Date associated with a claim of protection under copyright or a similar regime.</rdfs:comment>
        <rdfs:domain rdf:resource="http://bibframe.org/vocab/Provider"/>
        <rdfs:range rdf:resource="&rdfs;Literal"/>
    </owl:DatatypeProperty>
    


    <!-- http://bibframe.org/vocab/creationDate -->

    <owl:DatatypeProperty rdf:about="http://bibframe.org/vocab/creationDate">
        <rdfs:label>Description creation date</rdfs:label>
        <rdfs:comment>Date or date and time on which the original metadata first created.</rdfs:comment>
        <rdfs:range rdf:resource="&rdfs;Literal"/>
    </owl:DatatypeProperty>
    


    <!-- http://bibframe.org/vocab/creditsNote -->

    <owl:DatatypeProperty rdf:about="http://bibframe.org/vocab/creditsNote">
        <rdfs:label>Credits note</rdfs:label>
        <rdfs:comment>Credits for persons or organizations, other than members of the cast, who have participated in the creation and/or production of the.</rdfs:comment>
        <rdfs:range rdf:resource="&rdfs;Literal"/>
    </owl:DatatypeProperty>
    


    <!-- http://bibframe.org/vocab/custodialHistory -->

    <owl:DatatypeProperty rdf:about="http://bibframe.org/vocab/custodialHistory">
        <rdfs:label>Custodial history</rdfs:label>
        <rdfs:comment>Information about the provenance, such as origin, ownership and custodial history (chain of custody), of a resource.</rdfs:comment>
        <rdfs:domain rdf:resource="http://bibframe.org/vocab/Instance"/>
        <rdfs:range rdf:resource="&rdfs;Literal"/>
    </owl:DatatypeProperty>
    


    <!-- http://bibframe.org/vocab/descriptionAuthentication -->

    <owl:DatatypeProperty rdf:about="http://bibframe.org/vocab/descriptionAuthentication">
        <rdfs:label>Description authentication</rdfs:label>
        <rdfs:comment>Indication of specific types of reviews of description information.</rdfs:comment>
        <dcterms:modified>2014-10-27 (Updated)</dcterms:modified>
        <rdfs:range rdf:resource="&rdfs;Literal"/>
    </owl:DatatypeProperty>
    


    <!-- http://bibframe.org/vocab/descriptionStatus -->

    <owl:DatatypeProperty rdf:about="http://bibframe.org/vocab/descriptionStatus">
        <rdfs:label>Description status</rdfs:label>
        <rdfs:comment>Indicaton of whether the description is new or revised or in other states.</rdfs:comment>
        <dcterms:modified>2014-10-27 (Updated)</dcterms:modified>
        <rdfs:range rdf:resource="&rdfs;Literal"/>
    </owl:DatatypeProperty>
    


    <!-- http://bibframe.org/vocab/dimensions -->

    <owl:DatatypeProperty rdf:about="http://bibframe.org/vocab/dimensions">
        <rdfs:label>Dimensions</rdfs:label>
        <rdfs:comment>Measurements of the carrier or carriers and/or the container of a resource.</rdfs:comment>
        <rdfs:domain rdf:resource="http://bibframe.org/vocab/Instance"/>
        <rdfs:range rdf:resource="&rdfs;Literal"/>
    </owl:DatatypeProperty>
    


    <!-- http://bibframe.org/vocab/dissertationDegree -->

    <owl:DatatypeProperty rdf:about="http://bibframe.org/vocab/dissertationDegree">
        <rdfs:label>Degree</rdfs:label>
        <rdfs:comment>Degree for which author was a candidate.</rdfs:comment>
        <rdfs:domain rdf:resource="http://bibframe.org/vocab/Work"/>
        <rdfs:range rdf:resource="&rdfs;Literal"/>
    </owl:DatatypeProperty>
    


    <!-- http://bibframe.org/vocab/dissertationNote -->

    <owl:DatatypeProperty rdf:about="http://bibframe.org/vocab/dissertationNote">
        <rdfs:label>Dissertation note</rdfs:label>
        <rdfs:comment>Textual information about the dissertation.</rdfs:comment>
        <rdfs:domain rdf:resource="http://bibframe.org/vocab/Work"/>
        <rdfs:range rdf:resource="&rdfs;Literal"/>
    </owl:DatatypeProperty>
    


    <!-- http://bibframe.org/vocab/dissertationYear -->

    <owl:DatatypeProperty rdf:about="http://bibframe.org/vocab/dissertationYear">
        <rdfs:label>Year degree awarded</rdfs:label>
        <rdfs:comment>Year degree awarded.</rdfs:comment>
        <rdfs:domain rdf:resource="http://bibframe.org/vocab/Work"/>
        <rdfs:range rdf:resource="&rdfs;Literal"/>
    </owl:DatatypeProperty>
    


    <!-- http://bibframe.org/vocab/duration -->

    <owl:DatatypeProperty rdf:about="http://bibframe.org/vocab/duration">
        <rdfs:label>Duration</rdfs:label>
        <rdfs:comment>Information about the playing time or duration in an unstructured form, e.g., &quot;2 hours&quot;.</rdfs:comment>
        <rdfs:domain rdf:resource="http://bibframe.org/vocab/Instance"/>
        <rdfs:range rdf:resource="&rdfs;Literal"/>
    </owl:DatatypeProperty>
    


    <!-- http://bibframe.org/vocab/edition -->

    <owl:DatatypeProperty rdf:about="http://bibframe.org/vocab/edition">
        <rdfs:label>Edition statement</rdfs:label>
        <rdfs:comment>Information identifying the edition or version of the resource.</rdfs:comment>
        <rdfs:domain rdf:resource="http://bibframe.org/vocab/Instance"/>
        <rdfs:range rdf:resource="&rdfs;Literal"/>
    </owl:DatatypeProperty>
    


    <!-- http://bibframe.org/vocab/editionResponsibility -->

    <owl:DatatypeProperty rdf:about="http://bibframe.org/vocab/editionResponsibility">
        <rdfs:label>Edition responsibility</rdfs:label>
        <rdfs:comment>Statement relating to the identification of any persons, families, or corporate bodies responsible for the edition being described.</rdfs:comment>
        <rdfs:domain rdf:resource="http://bibframe.org/vocab/Instance"/>
        <rdfs:range rdf:resource="&rdfs;Literal"/>
    </owl:DatatypeProperty>
    


    <!-- http://bibframe.org/vocab/enumerationAndChronology -->

    <owl:DatatypeProperty rdf:about="http://bibframe.org/vocab/enumerationAndChronology">
        <rdfs:label>Enumeration and chronology</rdfs:label>
        <rdfs:comment>Numbering and dates of holding.</rdfs:comment>
        <rdfs:range rdf:resource="&rdfs;Literal"/>
    </owl:DatatypeProperty>
    


    <!-- http://bibframe.org/vocab/eventDate -->

    <owl:DatatypeProperty rdf:about="http://bibframe.org/vocab/eventDate">
        <rdfs:label>Date(s) of event</rdfs:label>
        <rdfs:comment>Date, time or period of event.</rdfs:comment>
        <dcterms:modified>2014-05-16 (Updated)</dcterms:modified>
        <rdfs:range rdf:resource="&rdfs;Literal"/>
    </owl:DatatypeProperty>
    


    <!-- http://bibframe.org/vocab/extent -->

    <owl:DatatypeProperty rdf:about="http://bibframe.org/vocab/extent">
        <rdfs:label>Extent</rdfs:label>
        <rdfs:comment>Number and type of units and/or subunits making up a resource.</rdfs:comment>
        <rdfs:domain rdf:resource="http://bibframe.org/vocab/Instance"/>
        <rdfs:range rdf:resource="&rdfs;Literal"/>
    </owl:DatatypeProperty>
    


    <!-- http://bibframe.org/vocab/findingAidNote -->

    <owl:DatatypeProperty rdf:about="http://bibframe.org/vocab/findingAidNote">
        <rdfs:label>Index or finding aid note</rdfs:label>
        <rdfs:comment>Note about availability of an index or finding aid.</rdfs:comment>
        <rdfs:range rdf:resource="&rdfs;Literal"/>
    </owl:DatatypeProperty>
    


    <!-- http://bibframe.org/vocab/formDesignation -->

    <owl:DatatypeProperty rdf:about="http://bibframe.org/vocab/formDesignation">
        <rdfs:label>Form designation</rdfs:label>
        <rdfs:comment>Class or genre to which a Work or Instance belongs.</rdfs:comment>
        <dcterms:modified>2014-03-21 (Range updated)</dcterms:modified>
        <rdfs:domain rdf:resource="http://bibframe.org/vocab/Title"/>
        <rdfs:range rdf:resource="&rdfs;Literal"/>
    </owl:DatatypeProperty>
    


    <!-- http://bibframe.org/vocab/format -->

    <owl:DatatypeProperty rdf:about="http://bibframe.org/vocab/format">
        <rdfs:label>Format</rdfs:label>
        <dcterms:modified>2014-10-27 (Updated)</dcterms:modified>
        <rdfs:comment>File format or physical medium of an instance.</rdfs:comment>
        <rdfs:domain rdf:resource="http://bibframe.org/vocab/Instance"/>
        <rdfs:range rdf:resource="&rdfs;Literal"/>
    </owl:DatatypeProperty>
    


    <!-- http://bibframe.org/vocab/formatOfMusic -->

    <owl:DatatypeProperty rdf:about="http://bibframe.org/vocab/formatOfMusic">
        <rdfs:label>Format of music</rdfs:label>
        <rdfs:comment>Format of a musical composition, e.g. full score, condensed score, vocal score, etc.</rdfs:comment>
        <rdfs:domain rdf:resource="http://bibframe.org/vocab/Instance"/>
        <rdfs:range rdf:resource="&rdfs;Literal"/>
    </owl:DatatypeProperty>
    


    <!-- http://bibframe.org/vocab/frequency -->

    <owl:DatatypeProperty rdf:about="http://bibframe.org/vocab/frequency">
        <rdfs:label>Frequency</rdfs:label>
        <rdfs:comment>Intervals at which the issues or parts of a serial or the updates to an integrating resource are issued.</rdfs:comment>
        <rdfs:domain rdf:resource="http://bibframe.org/vocab/Instance"/>
        <rdfs:range rdf:resource="&rdfs;Literal"/>
    </owl:DatatypeProperty>
    


    <!-- http://bibframe.org/vocab/frequencyNote -->

    <owl:DatatypeProperty rdf:about="http://bibframe.org/vocab/frequencyNote">
        <rdfs:label>Frequency note</rdfs:label>
        <rdfs:comment>Current or former publication frequency of a resource.</rdfs:comment>
        <rdfs:domain rdf:resource="http://bibframe.org/vocab/Instance"/>
        <rdfs:range rdf:resource="&rdfs;Literal"/>
    </owl:DatatypeProperty>
    


    <!-- http://bibframe.org/vocab/generationDate -->

    <owl:DatatypeProperty rdf:about="http://bibframe.org/vocab/generationDate">
        <rdfs:label>Date generated</rdfs:label>
        <dcterms:modified>2014-10-27 (Updated)</dcterms:modified>
        <rdfs:comment>Date of conversion of the data from another format.</rdfs:comment>
        <rdfs:range rdf:resource="&rdfs;Literal"/>
    </owl:DatatypeProperty>
    


    <!-- http://bibframe.org/vocab/generationProcess -->

    <owl:DatatypeProperty rdf:about="http://bibframe.org/vocab/generationProcess">
        <rdfs:label>Description generation</rdfs:label>
        <rdfs:comment>Indication of the program or process used to generate the description by application of a particular transformation.</rdfs:comment>
        <dcterms:modified>2014-10-27 (Updated)</dcterms:modified>
        <rdfs:range rdf:resource="&rdfs;Literal"/>
    </owl:DatatypeProperty>
    


    <!-- http://bibframe.org/vocab/geographicCoverageNote -->

    <owl:DatatypeProperty rdf:about="http://bibframe.org/vocab/geographicCoverageNote">
        <rdfs:label>Geographic coverage</rdfs:label>
        <rdfs:comment>Geographic entities covered by the resource.</rdfs:comment>
        <rdfs:domain rdf:resource="http://bibframe.org/vocab/Work"/>
        <rdfs:range rdf:resource="&rdfs;Literal"/>
    </owl:DatatypeProperty>
    


    <!-- http://bibframe.org/vocab/graphicScaleNote -->

    <owl:DatatypeProperty rdf:about="http://bibframe.org/vocab/graphicScaleNote">
        <rdfs:label>Graphic scale</rdfs:label>
        <rdfs:comment>Textual information about scale, including the scale of graphic material item such as architectural drawings or three-dimensional artifacts.</rdfs:comment>
        <rdfs:domain rdf:resource="http://bibframe.org/vocab/Instance"/>
        <rdfs:range rdf:resource="&rdfs;Literal"/>
    </owl:DatatypeProperty>
    


    <!-- http://bibframe.org/vocab/identifierAssigner -->

    <owl:DatatypeProperty rdf:about="http://bibframe.org/vocab/identifierAssigner">
        <rdfs:label>Identifier assigner</rdfs:label>
        <rdfs:comment>Entity that assigned the identifier.</rdfs:comment>
        <rdfs:domain rdf:resource="http://bibframe.org/vocab/Identifier"/>
        <rdfs:range rdf:resource="&rdfs;Literal"/>
    </owl:DatatypeProperty>
    


    <!-- http://bibframe.org/vocab/identifierQualifier -->

    <owl:DatatypeProperty rdf:about="http://bibframe.org/vocab/identifierQualifier">
        <rdfs:label>Identifier qualifier</rdfs:label>
        <rdfs:comment>Qualifying information associated with the identifier, e.g. specifying its applicability.</rdfs:comment>
        <rdfs:domain rdf:resource="http://bibframe.org/vocab/Identifier"/>
        <rdfs:range rdf:resource="&rdfs;Literal"/>
    </owl:DatatypeProperty>
    


    <!-- http://bibframe.org/vocab/identifierStatus -->

    <owl:DatatypeProperty rdf:about="http://bibframe.org/vocab/identifierStatus">
        <rdfs:label>Identifier status</rdfs:label>
        <rdfs:comment>Indication of whether the identifier is canceled or invalid.</rdfs:comment>
        <rdfs:domain rdf:resource="http://bibframe.org/vocab/Identifier"/>
        <rdfs:range rdf:resource="&rdfs;Literal"/>
    </owl:DatatypeProperty>
    


    <!-- http://bibframe.org/vocab/identifierValue -->

    <owl:DatatypeProperty rdf:about="http://bibframe.org/vocab/identifierValue">
        <rdfs:label>Identifier value</rdfs:label>
        <rdfs:comment>Value of the identifier.</rdfs:comment>
        <rdfs:domain rdf:resource="http://bibframe.org/vocab/Identifier"/>
        <rdfs:range rdf:resource="&rdfs;Literal"/>
    </owl:DatatypeProperty>
    


    <!-- http://bibframe.org/vocab/illustrationNote -->

    <owl:DatatypeProperty rdf:about="http://bibframe.org/vocab/illustrationNote">
        <rdfs:label>Illustrative content note</rdfs:label>
        <rdfs:comment>Information about illustrative material in the resource.</rdfs:comment>
        <rdfs:domain rdf:resource="http://bibframe.org/vocab/Instance"/>
        <rdfs:range rdf:resource="&rdfs;Literal"/>
    </owl:DatatypeProperty>
    


    <!-- http://bibframe.org/vocab/immediateAcquisition -->

    <owl:DatatypeProperty rdf:about="http://bibframe.org/vocab/immediateAcquisition">
        <rdfs:label>Immediate acquisition</rdfs:label>
        <rdfs:comment>Information about the circumstances (e.g., source, date, method) under which the resource was directly acquired.</rdfs:comment>
        <rdfs:range rdf:resource="&rdfs;Literal"/>
    </owl:DatatypeProperty>
    


    <!-- http://bibframe.org/vocab/itemId -->

    <owl:DatatypeProperty rdf:about="http://bibframe.org/vocab/itemId">
        <rdfs:label>System item identifier</rdfs:label>
        <rdfs:comment>Identification number assigned to data about one item held.</rdfs:comment>
        <rdfs:range rdf:resource="&rdfs;Literal"/>
    </owl:DatatypeProperty>
    


    <!-- http://bibframe.org/vocab/label -->

    <owl:DatatypeProperty rdf:about="http://bibframe.org/vocab/label">
        <rdfs:label>Label</rdfs:label>
        <rdfs:comment>Text string expressing the property value.</rdfs:comment>
        <rdfs:range rdf:resource="&rdfs;Literal"/>
    </owl:DatatypeProperty>
    


    <!-- http://bibframe.org/vocab/languageNote -->

    <owl:DatatypeProperty rdf:about="http://bibframe.org/vocab/languageNote">
        <rdfs:label>Language note</rdfs:label>
        <rdfs:comment>Note concerning the language of the material or its parts.</rdfs:comment>
        <rdfs:domain rdf:resource="http://bibframe.org/vocab/Work"/>
        <rdfs:range rdf:resource="&rdfs;Literal"/>
    </owl:DatatypeProperty>
    


    <!-- http://bibframe.org/vocab/languageOfPart -->

    <owl:DatatypeProperty rdf:about="http://bibframe.org/vocab/languageOfPart">
        <rdfs:label>Language of part</rdfs:label>
        <rdfs:comment>Language or notation system used to convey the content of the resource (associated with part or all of a resource).</rdfs:comment>
        <rdfs:domain rdf:resource="http://bibframe.org/vocab/Language"/>
        <rdfs:range rdf:resource="&rdfs;Literal"/>
    </owl:DatatypeProperty>
    


    <!-- http://bibframe.org/vocab/languageSource -->

    <owl:DatatypeProperty rdf:about="http://bibframe.org/vocab/languageSource">
        <rdfs:label>Language source</rdfs:label>
        <rdfs:comment>Language code or name list from which value is taken.</rdfs:comment>
        <rdfs:domain rdf:resource="http://bibframe.org/vocab/Language"/>
        <rdfs:range rdf:resource="&rdfs;Literal"/>
    </owl:DatatypeProperty>
    


    <!-- http://bibframe.org/vocab/legalDate -->

    <owl:DatatypeProperty rdf:about="http://bibframe.org/vocab/legalDate">
        <rdfs:label>Date of legal work</rdfs:label>
        <rdfs:comment>Date of legal work, or promulgation of a law, or signing of a treaty.</rdfs:comment>
        <rdfs:range rdf:resource="&rdfs;Literal"/>
    </owl:DatatypeProperty>
    


    <!-- http://bibframe.org/vocab/lendingPolicy -->

    <owl:DatatypeProperty rdf:about="http://bibframe.org/vocab/lendingPolicy">
        <rdfs:label>Lending policy</rdfs:label>
        <rdfs:comment>Policy statement about whether and with what restrictions the holding may be lent</rdfs:comment>
        <rdfs:range rdf:resource="&rdfs;Literal"/>
    </owl:DatatypeProperty>
    


    <!-- http://bibframe.org/vocab/materialArrangement -->

    <owl:DatatypeProperty rdf:about="http://bibframe.org/vocab/materialArrangement">
        <rdfs:label>Arrangement of material</rdfs:label>
        <rdfs:comment>Pattern of arrangement of materials within a unit.</rdfs:comment>
        <rdfs:domain rdf:resource="http://bibframe.org/vocab/Arrangement"/>
        <rdfs:range rdf:resource="&rdfs;Literal"/>
    </owl:DatatypeProperty>
    


    <!-- http://bibframe.org/vocab/materialHierarchicalLevel -->

    <owl:DatatypeProperty rdf:about="http://bibframe.org/vocab/materialHierarchicalLevel">
        <rdfs:label>Hierarchical level of material</rdfs:label>
        <rdfs:comment>Hierarchical position of the described materials relative to other material from the same source.</rdfs:comment>
        <rdfs:domain rdf:resource="http://bibframe.org/vocab/Arrangement"/>
        <rdfs:range rdf:resource="&rdfs;Literal"/>
    </owl:DatatypeProperty>
    


    <!-- http://bibframe.org/vocab/materialOrganization -->

    <owl:DatatypeProperty rdf:about="http://bibframe.org/vocab/materialOrganization">
        <rdfs:label>Organization of material</rdfs:label>
        <rdfs:comment>Manner in which resource is divided into smaller units.</rdfs:comment>
        <rdfs:domain rdf:resource="http://bibframe.org/vocab/Arrangement"/>
        <rdfs:range rdf:resource="&rdfs;Literal"/>
    </owl:DatatypeProperty>
    


    <!-- http://bibframe.org/vocab/materialPart -->

    <owl:DatatypeProperty rdf:about="http://bibframe.org/vocab/materialPart">
        <rdfs:label>Part of material</rdfs:label>
        <rdfs:comment>Part of the resource to which information applies.</rdfs:comment>
        <rdfs:domain rdf:resource="http://bibframe.org/vocab/Arrangement"/>
        <rdfs:range rdf:resource="&rdfs;Literal"/>
    </owl:DatatypeProperty>
    


    <!-- http://bibframe.org/vocab/modeOfIssuance -->

    <owl:DatatypeProperty rdf:about="http://bibframe.org/vocab/modeOfIssuance">
        <rdfs:label>Mode of issuance</rdfs:label>
        <rdfs:comment>Categorization reflecting whether a resource is issued in one or more parts, the way it is updated, and its intended termination.</rdfs:comment>
        <rdfs:domain rdf:resource="http://bibframe.org/vocab/Instance"/>
        <rdfs:range rdf:resource="&rdfs;Literal"/>
    </owl:DatatypeProperty>
    


    <!-- http://bibframe.org/vocab/musicKey -->

    <owl:DatatypeProperty rdf:about="http://bibframe.org/vocab/musicKey">
        <rdfs:label>Music Key</rdfs:label>
        <rdfs:comment>Pitch and mode for music.</rdfs:comment>
        <rdfs:range rdf:resource="&rdfs;Literal"/>
    </owl:DatatypeProperty>
    


    <!-- http://bibframe.org/vocab/musicMediumNote -->

    <owl:DatatypeProperty rdf:about="http://bibframe.org/vocab/musicMediumNote">
        <rdfs:label>Music medium note</rdfs:label>
        <rdfs:comment>Instrumental, vocal, and/or other medium of performance for which a musical resource was originally conceived, written or performed.</rdfs:comment>
        <rdfs:range rdf:resource="&rdfs;Literal"/>
    </owl:DatatypeProperty>
    


    <!-- http://bibframe.org/vocab/musicNumber -->

    <owl:DatatypeProperty rdf:about="http://bibframe.org/vocab/musicNumber">
        <rdfs:label>Music number</rdfs:label>
        <rdfs:comment>Serial, opus, or thematic number or code for music.</rdfs:comment>
        <rdfs:range rdf:resource="&rdfs;Literal"/>
    </owl:DatatypeProperty>
    


    <!-- http://bibframe.org/vocab/musicVersion -->

    <owl:DatatypeProperty rdf:about="http://bibframe.org/vocab/musicVersion">
        <rdfs:label>Music version</rdfs:label>
        <dcterms:modified>2014-06-19 (Example Added)</dcterms:modified>
        <rdfs:comment>Versions such as arrangements, transcriptions, etc. of music.</rdfs:comment>
        <rdfs:range rdf:resource="&rdfs;Literal"/>
    </owl:DatatypeProperty>
    


    <!-- http://bibframe.org/vocab/notation -->

    <owl:DatatypeProperty rdf:about="http://bibframe.org/vocab/notation">
        <rdfs:label>Notation system</rdfs:label>
        <rdfs:comment>Information on the alphabet, script, or symbol system used to convey the content of the resource, including specialized scripts, typefaces, tactile notation, and musical notation.</rdfs:comment>
        <rdfs:domain rdf:resource="http://bibframe.org/vocab/Instance"/>
        <rdfs:range rdf:resource="&rdfs;Literal"/>
    </owl:DatatypeProperty>
    


    <!-- http://bibframe.org/vocab/note -->

    <owl:DatatypeProperty rdf:about="http://bibframe.org/vocab/note">
        <rdfs:label>Note</rdfs:label>
        <rdfs:comment>General textual information relating to a resource.</rdfs:comment>
        <dcterms:modified>2014-10-14 (Updated)</dcterms:modified>
        <rdfs:range rdf:resource="&rdfs;Literal"/>
    </owl:DatatypeProperty>
    


    <!-- http://bibframe.org/vocab/originDate -->

    <owl:DatatypeProperty rdf:about="http://bibframe.org/vocab/originDate">
        <rdfs:label>Associated title date</rdfs:label>
        <dcterms:modified>2014-07-23 (Example added)</dcterms:modified>
        <rdfs:comment>Date or date range associated with the creation of the work.</rdfs:comment>
        <rdfs:domain rdf:resource="http://bibframe.org/vocab/Work"/>
        <rdfs:range rdf:resource="&rdfs;Literal"/>
    </owl:DatatypeProperty>
    


    <!-- http://bibframe.org/vocab/partNumber -->

    <owl:DatatypeProperty rdf:about="http://bibframe.org/vocab/partNumber">
        <rdfs:label>Part number</rdfs:label>
        <rdfs:comment>Part or section number of a title.</rdfs:comment>
        <rdfs:domain rdf:resource="http://bibframe.org/vocab/Title"/>
        <rdfs:range rdf:resource="&rdfs;Literal"/>
    </owl:DatatypeProperty>
    


    <!-- http://bibframe.org/vocab/partTitle -->

    <owl:DatatypeProperty rdf:about="http://bibframe.org/vocab/partTitle">
        <rdfs:label>Part title</rdfs:label>
        <rdfs:comment>Part or section name of a title.</rdfs:comment>
        <rdfs:domain rdf:resource="http://bibframe.org/vocab/Title"/>
        <rdfs:range rdf:resource="&rdfs;Literal"/>
    </owl:DatatypeProperty>
    


    <!-- http://bibframe.org/vocab/performerNote -->

    <owl:DatatypeProperty rdf:about="http://bibframe.org/vocab/performerNote">
        <rdfs:label>Performer note</rdfs:label>
        <rdfs:comment>Information about the participants, players, narrators, presenters, or performers.</rdfs:comment>
        <rdfs:range rdf:resource="&rdfs;Literal"/>
    </owl:DatatypeProperty>
    


    <!-- http://bibframe.org/vocab/preferredCitation -->

    <owl:DatatypeProperty rdf:about="http://bibframe.org/vocab/preferredCitation">
        <rdfs:label>Preferred citation</rdfs:label>
        <rdfs:comment>Citation to the resource preferred by its custodian.</rdfs:comment>
        <rdfs:domain rdf:resource="http://bibframe.org/vocab/Instance"/>
        <rdfs:range rdf:resource="&rdfs;Literal"/>
    </owl:DatatypeProperty>
    


    <!-- http://bibframe.org/vocab/providerDate -->

    <owl:DatatypeProperty rdf:about="http://bibframe.org/vocab/providerDate">
        <rdfs:label>Provider date</rdfs:label>
        <rdfs:comment>Date associated with the publication, printing, distribution, issue, release or production of the instance.</rdfs:comment>
        <rdfs:domain rdf:resource="http://bibframe.org/vocab/Provider"/>
        <rdfs:range rdf:resource="&rdfs;Literal"/>
    </owl:DatatypeProperty>
    


    <!-- http://bibframe.org/vocab/providerRole -->

    <owl:DatatypeProperty rdf:about="http://bibframe.org/vocab/providerRole">
        <rdfs:label>Provider role</rdfs:label>
        <rdfs:comment>The type of role played by the provider of an instance, e.g. production, publication, manufacture, distribution.</rdfs:comment>
        <rdfs:domain rdf:resource="http://bibframe.org/vocab/Provider"/>
        <rdfs:range rdf:resource="&rdfs;Literal"/>
    </owl:DatatypeProperty>
    


    <!-- http://bibframe.org/vocab/providerStatement -->

    <owl:DatatypeProperty rdf:about="http://bibframe.org/vocab/providerStatement">
        <rdfs:label>Provider statement</rdfs:label>
        <rdfs:comment>Transcribed provider statement</rdfs:comment>
        <rdfs:domain rdf:resource="http://bibframe.org/vocab/Instance"/>
        <rdfs:range rdf:resource="&rdfs;Literal"/>
    </owl:DatatypeProperty>
    


    <!-- http://bibframe.org/vocab/relatorRole -->

    <owl:DatatypeProperty rdf:about="http://bibframe.org/vocab/relatorRole">
        <rdfs:label>Agent role</rdfs:label>
        <rdfs:comment>Specific role of agent.</rdfs:comment>
        <dcterms:modified>2014-04-30 (New)</dcterms:modified>
        <rdfs:domain rdf:resource="http://bibframe.org/vocab/Relator"/>
        <rdfs:range rdf:resource="&rdfs;Literal"/>
    </owl:DatatypeProperty>
    


    <!-- http://bibframe.org/vocab/reproductionPolicy -->

    <owl:DatatypeProperty rdf:about="http://bibframe.org/vocab/reproductionPolicy">
        <rdfs:label>Reproduction policy</rdfs:label>
        <rdfs:comment>Policy statement about whether reproductions of the holding can be made</rdfs:comment>
        <dcterms:modified>2014-10-21 (Added)</dcterms:modified>
        <rdfs:range rdf:resource="&rdfs;Literal"/>
    </owl:DatatypeProperty>
    


    <!-- http://bibframe.org/vocab/resourcePart -->

    <owl:DatatypeProperty rdf:about="http://bibframe.org/vocab/resourcePart">
        <rdfs:label>Resource part</rdfs:label>
        <rdfs:comment>Part of a resource for which language is being indicated.</rdfs:comment>
        <rdfs:domain rdf:resource="http://bibframe.org/vocab/Language"/>
        <rdfs:range rdf:resource="&rdfs;Literal"/>
    </owl:DatatypeProperty>
    


    <!-- http://bibframe.org/vocab/responsibilityStatement -->

    <owl:DatatypeProperty rdf:about="http://bibframe.org/vocab/responsibilityStatement">
        <rdfs:label>Edition responsibility</rdfs:label>
        <rdfs:comment>Statement relating to the identification and/or function of any persons, families, or corporate bodies responsible for the creation of, or contributing to the content of a resource.</rdfs:comment>
        <rdfs:domain rdf:resource="http://bibframe.org/vocab/Instance"/>
        <rdfs:range rdf:resource="&rdfs;Literal"/>
    </owl:DatatypeProperty>
    


    <!-- http://bibframe.org/vocab/retentionPolicy -->

    <owl:DatatypeProperty rdf:about="http://bibframe.org/vocab/retentionPolicy">
        <rdfs:label>Retention policy</rdfs:label>
        <rdfs:comment>Policy statement about how many and/or how long the holdings are retained</rdfs:comment>
        <dcterms:modified>2014-10-21 (Added)</dcterms:modified>
        <rdfs:range rdf:resource="&rdfs;Literal"/>
    </owl:DatatypeProperty>
    


    <!-- http://bibframe.org/vocab/serialFirstIssue -->

    <owl:DatatypeProperty rdf:about="http://bibframe.org/vocab/serialFirstIssue">
        <rdfs:label>Serial first issue</rdfs:label>
        <rdfs:comment>Beginning date of an instance and/or the sequential designations.</rdfs:comment>
        <rdfs:domain rdf:resource="http://bibframe.org/vocab/Instance"/>
        <rdfs:range rdf:resource="&rdfs;Literal"/>
    </owl:DatatypeProperty>
    


    <!-- http://bibframe.org/vocab/serialLastIssue -->

    <owl:DatatypeProperty rdf:about="http://bibframe.org/vocab/serialLastIssue">
        <rdfs:label>Serial last issue</rdfs:label>
        <rdfs:comment>Ending date of an instance and/or the sequential designations.</rdfs:comment>
        <rdfs:domain rdf:resource="http://bibframe.org/vocab/Instance"/>
        <rdfs:range rdf:resource="&rdfs;Literal"/>
    </owl:DatatypeProperty>
    


    <!-- http://bibframe.org/vocab/shelfMark -->

    <owl:DatatypeProperty rdf:about="http://bibframe.org/vocab/shelfMark">
        <rdfs:label>Shelf Location</rdfs:label>
        <rdfs:comment>Physical location, such as a call number or a special shelf/location indicator.</rdfs:comment>
        <rdfs:range rdf:resource="&rdfs;Literal"/>
    </owl:DatatypeProperty>
    


    <!-- http://bibframe.org/vocab/shelfMarkDdc -->

    <owl:DatatypeProperty rdf:about="http://bibframe.org/vocab/shelfMarkDdc">
        <rdfs:label>DDC call number</rdfs:label>
        <rdfs:comment>Shelf mark based on Dewey Decimal Classification.</rdfs:comment>
        <rdfs:range rdf:resource="&rdfs;Literal"/>
    </owl:DatatypeProperty>
    


    <!-- http://bibframe.org/vocab/shelfMarkLcc -->

    <owl:DatatypeProperty rdf:about="http://bibframe.org/vocab/shelfMarkLcc">
        <rdfs:label>LCC call number</rdfs:label>
        <rdfs:comment>Shelf mark based on Library of Congress Classification.</rdfs:comment>
        <rdfs:range rdf:resource="&rdfs;Literal"/>
    </owl:DatatypeProperty>
    


    <!-- http://bibframe.org/vocab/shelfMarkNlm -->

    <owl:DatatypeProperty rdf:about="http://bibframe.org/vocab/shelfMarkNlm">
        <rdfs:label>NLM call number</rdfs:label>
        <rdfs:comment>Shelf mark based on National Library of Medicine Classification.</rdfs:comment>
        <rdfs:range rdf:resource="&rdfs;Literal"/>
    </owl:DatatypeProperty>
    


    <!-- http://bibframe.org/vocab/shelfMarkScheme -->

    <owl:DatatypeProperty rdf:about="http://bibframe.org/vocab/shelfMarkScheme">
        <rdfs:label>Shelf mark scheme</rdfs:label>
        <rdfs:comment>Scheme from which a shelf mark is taken.</rdfs:comment>
        <rdfs:range rdf:resource="&rdfs;Literal"/>
    </owl:DatatypeProperty>
    


    <!-- http://bibframe.org/vocab/shelfMarkUdc -->

    <owl:DatatypeProperty rdf:about="http://bibframe.org/vocab/shelfMarkUdc">
        <rdfs:label>UDC call number</rdfs:label>
        <rdfs:comment>Shelf mark based on Universal Decimal Classification.</rdfs:comment>
        <rdfs:range rdf:resource="&rdfs;Literal"/>
    </owl:DatatypeProperty>
    


    <!-- http://bibframe.org/vocab/soundContent -->

    <owl:DatatypeProperty rdf:about="http://bibframe.org/vocab/soundContent">
        <rdfs:label>Sound content</rdfs:label>
        <rdfs:comment>Indication of whether the production of sound is an integral part of the resource.</rdfs:comment>
        <rdfs:domain rdf:resource="http://bibframe.org/vocab/Instance"/>
        <rdfs:range rdf:resource="&rdfs;Literal"/>
    </owl:DatatypeProperty>
    


    <!-- http://bibframe.org/vocab/startOfReview -->

    <owl:DatatypeProperty rdf:about="http://bibframe.org/vocab/startOfReview">
        <rdfs:label>Review beginning</rdfs:label>
        <rdfs:comment>First part of review.</rdfs:comment>
        <rdfs:range rdf:resource="&rdfs;Literal"/>
    </owl:DatatypeProperty>
    


    <!-- http://bibframe.org/vocab/startOfSummary -->

    <owl:DatatypeProperty rdf:about="http://bibframe.org/vocab/startOfSummary">
        <rdfs:label>Summary beginning</rdfs:label>
        <rdfs:comment>First part of description.</rdfs:comment>
        <rdfs:range rdf:resource="&rdfs;Literal"/>
    </owl:DatatypeProperty>
    


    <!-- http://bibframe.org/vocab/subLocation -->

    <owl:DatatypeProperty rdf:about="http://bibframe.org/vocab/subLocation">
        <rdfs:label>Held in sublocation</rdfs:label>
        <dcterms:modified>2014-04-28 (Updated Mapping)</dcterms:modified>
        <rdfs:comment>Specific place within the holding entity where the item is located or made available</rdfs:comment>
        <rdfs:range rdf:resource="&rdfs;Literal"/>
    </owl:DatatypeProperty>
    


    <!-- http://bibframe.org/vocab/subtitle -->

    <owl:DatatypeProperty rdf:about="http://bibframe.org/vocab/subtitle">
        <rdfs:label>Subtitle</rdfs:label>
        <rdfs:comment>Word, character, or group of words and/or characters that contains the remainder of the title information after the main title.</rdfs:comment>
        <rdfs:domain rdf:resource="http://bibframe.org/vocab/Title"/>
        <rdfs:range rdf:resource="&rdfs;Literal"/>
    </owl:DatatypeProperty>
    


    <!-- http://bibframe.org/vocab/supplementaryContentNote -->

    <owl:DatatypeProperty rdf:about="http://bibframe.org/vocab/supplementaryContentNote">
        <rdfs:label>Supplementary content note</rdfs:label>
        <rdfs:comment>Information on the presence of one or more bibliographies, discographies, filmographies, and/or other bibliographic references in a described resource or in accompanying material.</rdfs:comment>
        <rdfs:domain rdf:resource="http://bibframe.org/vocab/Instance"/>
        <rdfs:range rdf:resource="&rdfs;Literal"/>
    </owl:DatatypeProperty>
    


    <!-- http://bibframe.org/vocab/temporalCoverageNote -->

    <owl:DatatypeProperty rdf:about="http://bibframe.org/vocab/temporalCoverageNote">
        <rdfs:label>Temporal coverage</rdfs:label>
        <rdfs:comment>Time period covered by the resource.</rdfs:comment>
        <rdfs:domain rdf:resource="http://bibframe.org/vocab/Work"/>
        <rdfs:range rdf:resource="&rdfs;Literal"/>
    </owl:DatatypeProperty>
    


    <!-- http://bibframe.org/vocab/title -->

    <owl:DatatypeProperty rdf:about="http://bibframe.org/vocab/title">
        <rdfs:label>Title</rdfs:label>
        <rdfs:comment>Word, character, or group of words and/or characters that is a name given to a resource</rdfs:comment>
        <rdfs:range rdf:resource="&rdfs;Literal"/>
    </owl:DatatypeProperty>
    


    <!-- http://bibframe.org/vocab/titleAttribute -->

    <owl:DatatypeProperty rdf:about="http://bibframe.org/vocab/titleAttribute">
        <rdfs:label>Other title attribute</rdfs:label>
        <rdfs:comment>Other distinguishing characteristic of a work, such as version, etc..</rdfs:comment>
        <rdfs:domain rdf:resource="http://bibframe.org/vocab/Title"/>
        <rdfs:range rdf:resource="&rdfs;Literal"/>
    </owl:DatatypeProperty>
    


    <!-- http://bibframe.org/vocab/titleQualifier -->

    <owl:DatatypeProperty rdf:about="http://bibframe.org/vocab/titleQualifier">
        <rdfs:label>Title qualifier</rdfs:label>
        <rdfs:comment>Qualifier of title information to make it unique.</rdfs:comment>
        <rdfs:domain rdf:resource="http://bibframe.org/vocab/Title"/>
        <rdfs:range rdf:resource="&rdfs;Literal"/>
    </owl:DatatypeProperty>
    


    <!-- http://bibframe.org/vocab/titleSource -->

    <owl:DatatypeProperty rdf:about="http://bibframe.org/vocab/titleSource">
        <rdfs:label>Title source</rdfs:label>
        <rdfs:comment>Title list from which title is taken, e.g., list of abbreviated titles.</rdfs:comment>
        <rdfs:domain rdf:resource="http://bibframe.org/vocab/Title"/>
        <rdfs:range rdf:resource="&rdfs;Literal"/>
    </owl:DatatypeProperty>
    


    <!-- http://bibframe.org/vocab/titleStatement -->

    <owl:DatatypeProperty rdf:about="http://bibframe.org/vocab/titleStatement">
        <rdfs:label>Transcribed title</rdfs:label>
        <rdfs:comment>Title transcribed from an instance.</rdfs:comment>
        <dcterms:modified>2014-09-03 (Updated)</dcterms:modified>
        <rdfs:domain rdf:resource="http://bibframe.org/vocab/Instance"/>
        <rdfs:range rdf:resource="&rdfs;Literal"/>
    </owl:DatatypeProperty>
    


    <!-- http://bibframe.org/vocab/titleType -->

    <owl:DatatypeProperty rdf:about="http://bibframe.org/vocab/titleType">
        <rdfs:label>Variant title type</rdfs:label>
        <dcterms:modified>2014-08-07 (Example added)</dcterms:modified>
        <rdfs:comment>Type of title variation, e.g., acronym, cover, spine. .</rdfs:comment>
        <rdfs:domain rdf:resource="http://bibframe.org/vocab/Title"/>
        <rdfs:range rdf:resource="&rdfs;Literal"/>
    </owl:DatatypeProperty>
    


    <!-- http://bibframe.org/vocab/titleValue -->

    <owl:DatatypeProperty rdf:about="http://bibframe.org/vocab/titleValue">
        <rdfs:label>Title</rdfs:label>
        <rdfs:comment>Title being addressed.</rdfs:comment>
        <rdfs:domain rdf:resource="http://bibframe.org/vocab/Title"/>
        <rdfs:range rdf:resource="&rdfs;Literal"/>
    </owl:DatatypeProperty>
    


    <!-- http://bibframe.org/vocab/titleVariationDate -->

    <owl:DatatypeProperty rdf:about="http://bibframe.org/vocab/titleVariationDate">
        <rdfs:label>Variant title date</rdfs:label>
        <rdfs:comment>Date or sequential designation of title variation.</rdfs:comment>
        <rdfs:domain rdf:resource="http://bibframe.org/vocab/Title"/>
        <rdfs:range rdf:resource="&rdfs;Literal"/>
    </owl:DatatypeProperty>
    


    <!-- http://bibframe.org/vocab/treatySignator -->

    <owl:DatatypeProperty rdf:about="http://bibframe.org/vocab/treatySignator">
        <rdfs:label>Signatory to a treaty</rdfs:label>
        <rdfs:comment>Government of other party that has formally signed a treaty.</rdfs:comment>
        <dcterms:modified>2014-03-21 (Range updated)</dcterms:modified>
        <rdfs:range rdf:resource="&rdfs;Literal"/>
    </owl:DatatypeProperty>
    


    <!-- http://purl.org/dc/terms/alternative -->

    <owl:DatatypeProperty rdf:about="&dcterms;alternative">
        <rdfs:label xml:lang="en">Alternative Title</rdfs:label>
        <dcterms:issued rdf:datatype="&xsd;date">2000-07-11</dcterms:issued>
        <dcterms:modified rdf:datatype="&xsd;date">2010-10-11</dcterms:modified>
        <rdfs:comment xml:lang="en">An alternative name for the resource.</rdfs:comment>
        <dcterms:description xml:lang="en">The distinction between titles and alternative titles is application-specific.</dcterms:description>
        <dcterms:hasVersion rdf:resource="http://dublincore.org/usage/terms/history/#alternative-003"/>
        <rdfs:subPropertyOf rdf:resource="&dc;title"/>
        <rdfs:isDefinedBy rdf:resource="http://purl.org/dc/terms/"/>
        <rdfs:subPropertyOf rdf:resource="&dcterms;title"/>
        <rdfs:range rdf:resource="&rdfs;Literal"/>
    </owl:DatatypeProperty>
    


    <!-- http://purl.org/dc/terms/available -->

    <owl:DatatypeProperty rdf:about="&dcterms;available">
        <rdfs:label xml:lang="en">Date Available</rdfs:label>
        <dcterms:issued rdf:datatype="&xsd;date">2000-07-11</dcterms:issued>
        <dcterms:modified rdf:datatype="&xsd;date">2008-01-14</dcterms:modified>
        <rdfs:comment xml:lang="en">Date (often a range) that the resource became or will become available.</rdfs:comment>
        <dcterms:hasVersion rdf:resource="http://dublincore.org/usage/terms/history/#available-003"/>
        <rdfs:subPropertyOf rdf:resource="&dc;date"/>
        <rdfs:isDefinedBy rdf:resource="http://purl.org/dc/terms/"/>
        <rdfs:subPropertyOf rdf:resource="&dcterms;date"/>
        <rdfs:range rdf:resource="&rdfs;Literal"/>
    </owl:DatatypeProperty>
    


    <!-- http://purl.org/dc/terms/bibliographicCitation -->

    <owl:DatatypeProperty rdf:about="&dcterms;bibliographicCitation">
        <rdfs:label xml:lang="en">Bibliographic Citation</rdfs:label>
        <dcterms:issued rdf:datatype="&xsd;date">2003-02-15</dcterms:issued>
        <dcterms:modified rdf:datatype="&xsd;date">2008-01-14</dcterms:modified>
        <rdfs:comment xml:lang="en">A bibliographic reference for the resource.</rdfs:comment>
        <dcterms:description xml:lang="en">Recommended practice is to include sufficient bibliographic detail to identify the resource as unambiguously as possible.</dcterms:description>
        <dcterms:hasVersion rdf:resource="http://dublincore.org/usage/terms/history/#bibliographicCitation-002"/>
        <rdfs:isDefinedBy rdf:resource="http://purl.org/dc/terms/"/>
        <rdfs:subPropertyOf rdf:resource="&dcterms;identifier"/>
        <rdfs:range rdf:resource="&rdfs;Literal"/>
    </owl:DatatypeProperty>
    


    <!-- http://purl.org/dc/terms/created -->

    <owl:DatatypeProperty rdf:about="&dcterms;created">
        <rdfs:label xml:lang="en">Date Created</rdfs:label>
        <dcterms:issued rdf:datatype="&xsd;date">2000-07-11</dcterms:issued>
        <dcterms:modified rdf:datatype="&xsd;date">2008-01-14</dcterms:modified>
        <rdfs:comment xml:lang="en">Date of creation of the resource.</rdfs:comment>
        <dcterms:hasVersion rdf:resource="http://dublincore.org/usage/terms/history/#created-003"/>
        <rdfs:subPropertyOf rdf:resource="&dc;date"/>
        <rdfs:isDefinedBy rdf:resource="http://purl.org/dc/terms/"/>
        <rdfs:subPropertyOf rdf:resource="&dcterms;date"/>
        <rdfs:range rdf:resource="&rdfs;Literal"/>
    </owl:DatatypeProperty>
    


    <!-- http://purl.org/dc/terms/date -->

    <owl:DatatypeProperty rdf:about="&dcterms;date">
        <rdfs:label xml:lang="en">Date</rdfs:label>
        <dcterms:modified rdf:datatype="&xsd;date">2008-01-14</dcterms:modified>
        <dcterms:issued rdf:datatype="&xsd;date">2008-01-14</dcterms:issued>
        <rdfs:comment xml:lang="en">A point or period of time associated with an event in the lifecycle of the resource.</rdfs:comment>
        <dcterms:description xml:lang="en">Date may be used to express temporal information at any level of granularity.  Recommended best practice is to use an encoding scheme, such as the W3CDTF profile of ISO 8601 [W3CDTF].</dcterms:description>
        <dcterms:hasVersion rdf:resource="http://dublincore.org/usage/terms/history/#dateT-001"/>
        <rdfs:subPropertyOf rdf:resource="&dc;date"/>
        <rdfs:isDefinedBy rdf:resource="http://purl.org/dc/terms/"/>
        <rdfs:range rdf:resource="&rdfs;Literal"/>
    </owl:DatatypeProperty>
    


    <!-- http://purl.org/dc/terms/dateAccepted -->

    <owl:DatatypeProperty rdf:about="&dcterms;dateAccepted">
        <rdfs:label xml:lang="en">Date Accepted</rdfs:label>
        <dcterms:issued rdf:datatype="&xsd;date">2002-07-13</dcterms:issued>
        <dcterms:modified rdf:datatype="&xsd;date">2008-01-14</dcterms:modified>
        <rdfs:comment xml:lang="en">Date of acceptance of the resource.</rdfs:comment>
        <dcterms:description xml:lang="en">Examples of resources to which a Date Accepted may be relevant are a thesis (accepted by a university department) or an article (accepted by a journal).</dcterms:description>
        <dcterms:hasVersion rdf:resource="http://dublincore.org/usage/terms/history/#dateAccepted-002"/>
        <rdfs:subPropertyOf rdf:resource="&dc;date"/>
        <rdfs:isDefinedBy rdf:resource="http://purl.org/dc/terms/"/>
        <rdfs:subPropertyOf rdf:resource="&dcterms;date"/>
        <rdfs:range rdf:resource="&rdfs;Literal"/>
    </owl:DatatypeProperty>
    


    <!-- http://purl.org/dc/terms/dateCopyrighted -->

    <owl:DatatypeProperty rdf:about="&dcterms;dateCopyrighted">
        <rdfs:label xml:lang="en">Date Copyrighted</rdfs:label>
        <dcterms:issued rdf:datatype="&xsd;date">2002-07-13</dcterms:issued>
        <dcterms:modified rdf:datatype="&xsd;date">2008-01-14</dcterms:modified>
        <rdfs:comment xml:lang="en">Date of copyright.</rdfs:comment>
        <dcterms:hasVersion rdf:resource="http://dublincore.org/usage/terms/history/#dateCopyrighted-002"/>
        <rdfs:subPropertyOf rdf:resource="&dc;date"/>
        <rdfs:isDefinedBy rdf:resource="http://purl.org/dc/terms/"/>
        <rdfs:subPropertyOf rdf:resource="&dcterms;date"/>
        <rdfs:range rdf:resource="&rdfs;Literal"/>
    </owl:DatatypeProperty>
    


    <!-- http://purl.org/dc/terms/dateSubmitted -->

    <owl:DatatypeProperty rdf:about="&dcterms;dateSubmitted">
        <rdfs:label xml:lang="en">Date Submitted</rdfs:label>
        <dcterms:issued rdf:datatype="&xsd;date">2002-07-13</dcterms:issued>
        <dcterms:modified rdf:datatype="&xsd;date">2008-01-14</dcterms:modified>
        <rdfs:comment xml:lang="en">Date of submission of the resource.</rdfs:comment>
        <dcterms:description xml:lang="en">Examples of resources to which a Date Submitted may be relevant are a thesis (submitted to a university department) or an article (submitted to a journal).</dcterms:description>
        <dcterms:hasVersion rdf:resource="http://dublincore.org/usage/terms/history/#dateSubmitted-002"/>
        <rdfs:subPropertyOf rdf:resource="&dc;date"/>
        <rdfs:isDefinedBy rdf:resource="http://purl.org/dc/terms/"/>
        <rdfs:subPropertyOf rdf:resource="&dcterms;date"/>
        <rdfs:range rdf:resource="&rdfs;Literal"/>
    </owl:DatatypeProperty>
    


    <!-- http://purl.org/dc/terms/identifier -->

    <rdf:Description rdf:about="&dcterms;identifier">
        <rdfs:label xml:lang="en">Identifier</rdfs:label>
        <dcterms:modified rdf:datatype="&xsd;date">2008-01-14</dcterms:modified>
        <dcterms:issued rdf:datatype="&xsd;date">2008-01-14</dcterms:issued>
        <rdfs:comment xml:lang="en">An unambiguous reference to the resource within a given context.</rdfs:comment>
        <dcterms:description xml:lang="en">Recommended best practice is to identify the resource by means of a string conforming to a formal identification system. </dcterms:description>
        <dcterms:hasVersion rdf:resource="http://dublincore.org/usage/terms/history/#identifierT-001"/>
        <rdfs:isDefinedBy rdf:resource="http://purl.org/dc/terms/"/>
        <rdfs:range rdf:resource="&rdfs;Literal"/>
    </rdf:Description>
    


    <!-- http://purl.org/dc/terms/issued -->

    <owl:DatatypeProperty rdf:about="&dcterms;issued">
        <rdfs:label xml:lang="en">Date Issued</rdfs:label>
        <dcterms:issued rdf:datatype="&xsd;date">2000-07-11</dcterms:issued>
        <dcterms:modified rdf:datatype="&xsd;date">2008-01-14</dcterms:modified>
        <rdfs:comment xml:lang="en">Date of formal issuance (e.g., publication) of the resource.</rdfs:comment>
        <dcterms:hasVersion rdf:resource="http://dublincore.org/usage/terms/history/#issued-003"/>
        <rdfs:subPropertyOf rdf:resource="&dc;date"/>
        <rdfs:isDefinedBy rdf:resource="http://purl.org/dc/terms/"/>
        <rdfs:subPropertyOf rdf:resource="&dcterms;date"/>
        <rdfs:range rdf:resource="&rdfs;Literal"/>
    </owl:DatatypeProperty>
    


    <!-- http://purl.org/dc/terms/modified -->

    <owl:DatatypeProperty rdf:about="&dcterms;modified">
        <rdfs:label xml:lang="en">Date Modified</rdfs:label>
        <dcterms:issued rdf:datatype="&xsd;date">2000-07-11</dcterms:issued>
        <dcterms:modified rdf:datatype="&xsd;date">2008-01-14</dcterms:modified>
        <rdfs:comment xml:lang="en">Date on which the resource was changed.</rdfs:comment>
        <dcterms:hasVersion rdf:resource="http://dublincore.org/usage/terms/history/#modified-003"/>
        <rdfs:subPropertyOf rdf:resource="&dc;date"/>
        <rdfs:isDefinedBy rdf:resource="http://purl.org/dc/terms/"/>
        <rdfs:subPropertyOf rdf:resource="&dcterms;date"/>
        <rdfs:range rdf:resource="&rdfs;Literal"/>
    </owl:DatatypeProperty>
    


    <!-- http://purl.org/dc/terms/title -->

    <owl:DatatypeProperty rdf:about="&dcterms;title">
        <rdfs:label xml:lang="en">Title</rdfs:label>
        <dcterms:issued rdf:datatype="&xsd;date">2008-01-14</dcterms:issued>
        <dcterms:modified rdf:datatype="&xsd;date">2010-10-11</dcterms:modified>
        <rdfs:comment xml:lang="en">A name given to the resource.</rdfs:comment>
        <dcterms:hasVersion rdf:resource="http://dublincore.org/usage/terms/history/#titleT-002"/>
        <rdfs:subPropertyOf rdf:resource="&dc;title"/>
        <rdfs:isDefinedBy rdf:resource="http://purl.org/dc/terms/"/>
        <rdfs:range rdf:resource="&rdfs;Literal"/>
    </owl:DatatypeProperty>
    


    <!-- http://purl.org/dc/terms/valid -->

    <owl:DatatypeProperty rdf:about="&dcterms;valid">
        <rdfs:label xml:lang="en">Date Valid</rdfs:label>
        <dcterms:issued rdf:datatype="&xsd;date">2000-07-11</dcterms:issued>
        <dcterms:modified rdf:datatype="&xsd;date">2008-01-14</dcterms:modified>
        <rdfs:comment xml:lang="en">Date (often a range) of validity of a resource.</rdfs:comment>
        <dcterms:hasVersion rdf:resource="http://dublincore.org/usage/terms/history/#valid-003"/>
        <rdfs:subPropertyOf rdf:resource="&dc;date"/>
        <rdfs:isDefinedBy rdf:resource="http://purl.org/dc/terms/"/>
        <rdfs:subPropertyOf rdf:resource="&dcterms;date"/>
        <rdfs:range rdf:resource="&rdfs;Literal"/>
    </owl:DatatypeProperty>
    


    <!-- 
    ///////////////////////////////////////////////////////////////////////////////////////
    //
    // Classes
    //
    ///////////////////////////////////////////////////////////////////////////////////////
     -->

    


    <!-- http://bibframe.org/vocab/Archival -->

    <owl:Class rdf:about="http://bibframe.org/vocab/Archival">
        <rdfs:label>Archival controlled</rdfs:label>
        <rdfs:subClassOf rdf:resource="http://bibframe.org/vocab/Instance"/>
        <dcterms:modified>2014-10-28 (Updated)</dcterms:modified>
        <rdfs:comment>Resources organically created, accumulated, and/or used by a person, family, or organization in the course of conduct of affairs and preserved because of their continuing value.</rdfs:comment>
    </owl:Class>
    


    <!-- http://bibframe.org/vocab/Arrangement -->

    <owl:Class rdf:about="http://bibframe.org/vocab/Arrangement">
        <rdfs:label>Organization of materials information</rdfs:label>
        <rdfs:comment>Information about the organization and arrangement of a collection of items. For instance, for computer files, organization and arrangement information may be the file structure and sort sequence of a file; for visual materials, this information may be how a collection is arranged.</rdfs:comment>
    </owl:Class>
    


    <!-- http://bibframe.org/vocab/Audio -->

    <owl:Class rdf:about="http://bibframe.org/vocab/Audio">
        <rdfs:label>Audio</rdfs:label>
        <rdfs:subClassOf rdf:resource="http://bibframe.org/vocab/Work"/>
        <rdfs:comment>Resources expressed in an audible form, including music or other sounds.</rdfs:comment>
    </owl:Class>
    


    <!-- http://bibframe.org/vocab/Cartography -->

    <owl:Class rdf:about="http://bibframe.org/vocab/Cartography">
        <rdfs:label>Cartography</rdfs:label>
        <rdfs:subClassOf rdf:resource="http://bibframe.org/vocab/Work"/>
        <rdfs:comment>Resource that show spatial information, including maps, atlases, globes,digital maps, and other cartographic items.</rdfs:comment>
    </owl:Class>
    


    <!-- http://bibframe.org/vocab/Category -->

    <owl:Class rdf:about="http://bibframe.org/vocab/Category">
        <rdfs:label>Category</rdfs:label>
        <rdfs:comment>Generic list of values information.</rdfs:comment>
        <dcterms:modified>2014-03-21 (Definition Updated)</dcterms:modified>
    </owl:Class>
    


    <!-- http://bibframe.org/vocab/Classification -->

    <owl:Class rdf:about="http://bibframe.org/vocab/Classification">
        <rdfs:label>Classification Entity</rdfs:label>
        <rdfs:comment>System of coding, assorting and organizing materials according to their subject.</rdfs:comment>
    </owl:Class>
    


    <!-- http://bibframe.org/vocab/Collection -->

    <owl:Class rdf:about="http://bibframe.org/vocab/Collection">
        <rdfs:label>Collection</rdfs:label>
        <rdfs:subClassOf rdf:resource="http://bibframe.org/vocab/Instance"/>
        <rdfs:comment>Aggregation of resources, generally gathered together artificially.</rdfs:comment>
    </owl:Class>
    


    <!-- http://bibframe.org/vocab/Dataset -->

    <owl:Class rdf:about="http://bibframe.org/vocab/Dataset">
        <rdfs:label>Dataset</rdfs:label>
        <rdfs:subClassOf rdf:resource="http://bibframe.org/vocab/Work"/>
        <rdfs:comment>Data encoded in a defined structure. Includes numeric data, environmental data,etc., used by applications software to calculate averages, correlations, etc., or to produce models, etc., but not normally displayed in its raw form.</rdfs:comment>
    </owl:Class>
    


    <!-- http://bibframe.org/vocab/Electronic -->

    <owl:Class rdf:about="http://bibframe.org/vocab/Electronic">
        <rdfs:label>Electronic</rdfs:label>
        <rdfs:subClassOf rdf:resource="http://bibframe.org/vocab/Instance"/>
        <dcterms:modified>2014-10-28 (Updated)</dcterms:modified>
        <rdfs:comment>Resource that is intended for manipulation by a computer, residing in a carrier accessed either directly or remotely.</rdfs:comment>
    </owl:Class>
    


    <!-- http://bibframe.org/vocab/Identifier -->

    <owl:Class rdf:about="http://bibframe.org/vocab/Identifier">
        <rdfs:label>Identifier</rdfs:label>
        <rdfs:comment>Token or name that is associated with a resource, such as a URI, or an ISBN, etc..</rdfs:comment>
    </owl:Class>
    


    <!-- http://bibframe.org/vocab/Instance -->

    <owl:Class rdf:about="http://bibframe.org/vocab/Instance">
        <rdfs:label>Instance</rdfs:label>
        <owl:equivalentClass rdf:resource="http://www.rdaregistry.info/Elements/c/#C10007"/>
        <rdfs:comment>Resource reflecting an individual, material embodiment of the Work.</rdfs:comment>
    </owl:Class>
    


    <!-- http://bibframe.org/vocab/Integrating -->

    <owl:Class rdf:about="http://bibframe.org/vocab/Integrating">
        <rdfs:label>Integrating</rdfs:label>
        <rdfs:subClassOf rdf:resource="http://bibframe.org/vocab/Instance"/>
        <rdfs:comment>Cataloging resource that is added to or changed by means of updates that do not remain discrete but are integrated into the whole.</rdfs:comment>
    </owl:Class>
    


    <!-- http://bibframe.org/vocab/IntendedAudience -->

    <owl:Class rdf:about="http://bibframe.org/vocab/IntendedAudience">
        <rdfs:label>Intended Audience Information</rdfs:label>
        <rdfs:comment>Information that identifies the specific intended or target audience or intellectual level for which the content described item is considered appropriate. Used to record interest and motivation levels and special learner characteristics.</rdfs:comment>
    </owl:Class>
    


    <!-- http://bibframe.org/vocab/Item -->

    <owl:Class rdf:about="http://bibframe.org/vocab/Item">
        <rdfs:comment rdf:datatype="&rdfs;Literal">A physical item that can be held, checked out, etc. Barbara Tillet&apos;s door stop.</rdfs:comment>
    </owl:Class>
    


    <!-- http://bibframe.org/vocab/Language -->

    <owl:Class rdf:about="http://bibframe.org/vocab/Language">
        <rdfs:label>Language Entity</rdfs:label>
        <rdfs:comment>Language entity.</rdfs:comment>
    </owl:Class>
    


    <!-- http://bibframe.org/vocab/Manuscript -->

    <owl:Class rdf:about="http://bibframe.org/vocab/Manuscript">
        <rdfs:label>Manuscript</rdfs:label>
        <rdfs:subClassOf rdf:resource="http://bibframe.org/vocab/Instance"/>
        <rdfs:comment>Resource that is written in handwriting or typescript. These are generally unique resources.</rdfs:comment>
    </owl:Class>
    


    <!-- http://bibframe.org/vocab/MixedMaterial -->

    <owl:Class rdf:about="http://bibframe.org/vocab/MixedMaterial">
        <rdfs:label>Mixed Material</rdfs:label>
        <rdfs:subClassOf rdf:resource="http://bibframe.org/vocab/Work"/>
        <rdfs:comment>Resource comprised of multiple types which are not driven by software. This may include materials in two or more forms that are related by virtue of their having been accumulated by or about a person or body, e.g. archival forms.</rdfs:comment>
    </owl:Class>
    


    <!-- http://bibframe.org/vocab/Monograph -->

    <owl:Class rdf:about="http://bibframe.org/vocab/Monograph">
        <rdfs:label>Monograph</rdfs:label>
        <rdfs:subClassOf rdf:resource="http://bibframe.org/vocab/Instance"/>
        <rdfs:comment>Single unit cataloging resource.</rdfs:comment>
    </owl:Class>
    


    <!-- http://bibframe.org/vocab/MovingImage -->

    <owl:Class rdf:about="http://bibframe.org/vocab/MovingImage">
        <rdfs:label>Moving Image</rdfs:label>
        <rdfs:subClassOf rdf:resource="http://bibframe.org/vocab/Work"/>
        <rdfs:comment>Images intended to be perceived as moving, including motion pictures (using liveaction and/or animation), film and video recordings of performances, events,etc.</rdfs:comment>
    </owl:Class>
    


    <!-- http://bibframe.org/vocab/Multimedia -->

    <owl:Class rdf:about="http://bibframe.org/vocab/Multimedia">
        <rdfs:label>Software or Multimedia</rdfs:label>
        <rdfs:subClassOf rdf:resource="http://bibframe.org/vocab/Work"/>
        <rdfs:comment>Electronic resource that is a computer program (i.e. digitally encoded instructions intended to be processed and performed by a computer) or which consist of multiple media types that are software driven. Examples include videogames and websites.</rdfs:comment>
    </owl:Class>
    


    <!-- http://bibframe.org/vocab/MultipartMonograph -->

    <owl:Class rdf:about="http://bibframe.org/vocab/MultipartMonograph">
        <rdfs:label>Multipart Monograph</rdfs:label>
        <rdfs:subClassOf rdf:resource="http://bibframe.org/vocab/Instance"/>
        <rdfs:comment>Multiple unit cataloging resource that is complete or intended to be completed within a finite number of parts.</rdfs:comment>
    </owl:Class>
    


    <!-- http://bibframe.org/vocab/NotatedMovement -->

    <owl:Class rdf:about="http://bibframe.org/vocab/NotatedMovement">
        <rdfs:label>Notated Movement</rdfs:label>
        <rdfs:subClassOf rdf:resource="http://bibframe.org/vocab/Work"/>
        <rdfs:comment>Graphic, non-realized representations of movement intended to be perceived visually, e.g. dance.</rdfs:comment>
    </owl:Class>
    


    <!-- http://bibframe.org/vocab/NotatedMusic -->

    <owl:Class rdf:about="http://bibframe.org/vocab/NotatedMusic">
        <rdfs:label>Notated Music</rdfs:label>
        <rdfs:subClassOf rdf:resource="http://bibframe.org/vocab/Work"/>
        <rdfs:comment>Graphic, non-realized representations of musical works intended to be perceived visually.</rdfs:comment>
    </owl:Class>
    


    <!-- http://bibframe.org/vocab/Print -->

    <owl:Class rdf:about="http://bibframe.org/vocab/Print">
        <rdfs:label>Printed</rdfs:label>
        <rdfs:subClassOf rdf:resource="http://bibframe.org/vocab/Instance"/>
        <rdfs:comment>Resource that is printed.</rdfs:comment>
    </owl:Class>
    


    <!-- http://bibframe.org/vocab/Provider -->

    <owl:Class rdf:about="http://bibframe.org/vocab/Provider">
        <rdfs:label>Provider Entity</rdfs:label>
        <rdfs:comment>Name of agent relating to the publication, printing, distribution, issue,release, or production of a resource.</rdfs:comment>
    </owl:Class>
    


    <!-- http://bibframe.org/vocab/Relator -->

    <owl:Class rdf:about="http://bibframe.org/vocab/Relator">
        <rdfs:label>Relationship</rdfs:label>
        <rdfs:comment>How an agent is related to a resource.</rdfs:comment>
        <dcterms:modified>2014-04-30 (New)</dcterms:modified>
    </owl:Class>
    


    <!-- http://bibframe.org/vocab/Serial -->

    <owl:Class rdf:about="http://bibframe.org/vocab/Serial">
        <rdfs:label>Serial</rdfs:label>
        <rdfs:subClassOf rdf:resource="http://bibframe.org/vocab/Instance"/>
        <rdfs:comment>Multiple unit cataloging resource issued in successive parts that has no predetermined conclusion.</rdfs:comment>
    </owl:Class>
    


    <!-- http://bibframe.org/vocab/StillImage -->

    <owl:Class rdf:about="http://bibframe.org/vocab/StillImage">
        <rdfs:label>Still Image</rdfs:label>
        <rdfs:subClassOf rdf:resource="http://bibframe.org/vocab/Work"/>
        <rdfs:comment>Resource expressed through line, shape, shading, etc., intended to be perceived visually as a still image or images in two dimensions. Includes two-dimensional images and slides and transparencies.</rdfs:comment>
    </owl:Class>
    


    <!-- http://bibframe.org/vocab/Tactile -->

    <owl:Class rdf:about="http://bibframe.org/vocab/Tactile">
        <rdfs:label>Tactile Material</rdfs:label>
        <rdfs:subClassOf rdf:resource="http://bibframe.org/vocab/Instance"/>
        <rdfs:comment>Resource that is intended to be perceived by touch.</rdfs:comment>
    </owl:Class>
    


    <!-- http://bibframe.org/vocab/Text -->

    <owl:Class rdf:about="http://bibframe.org/vocab/Text">
        <rdfs:label>Text</rdfs:label>
        <rdfs:subClassOf rdf:resource="http://bibframe.org/vocab/Work"/>
        <rdfs:comment>Form of notation for language intended to be perceived visually and understood through the use of language in written or spoken form.</rdfs:comment>
    </owl:Class>
    


    <!-- http://bibframe.org/vocab/ThreeDimensionalObject -->

    <owl:Class rdf:about="http://bibframe.org/vocab/ThreeDimensionalObject">
        <rdfs:label>Three-dimensional Object</rdfs:label>
        <rdfs:subClassOf rdf:resource="http://bibframe.org/vocab/Work"/>
        <rdfs:comment>Resource in a form intended to be perceived visually in three-dimensions.Includes man-made objects such as models, sculptures, clothing, and toys, as well as naturally occurring objects such as specimens mounted for viewing.</rdfs:comment>
    </owl:Class>
    


    <!-- http://bibframe.org/vocab/Title -->

    <owl:Class rdf:about="http://bibframe.org/vocab/Title">
        <rdfs:label>Title Entity</rdfs:label>
        <rdfs:comment>Title information relating to a resource: title proper, translated title, or variant form of title.</rdfs:comment>
    </owl:Class>
    


    <!-- http://bibframe.org/vocab/Work -->

    <owl:Class rdf:about="http://bibframe.org/vocab/Work">
        <rdfs:label>Work</rdfs:label>
        <rdfs:comment>Resource reflecting a conceptual essence of the cataloging resource.</rdfs:comment>
    </owl:Class>
    


    <!-- http://id.loc.gov/ontologies/RecordInfo#RecordInfo -->

    <owl:Class rdf:about="&RecordInfo;RecordInfo"/>
    


    <!-- http://purl.org/dc/dcam/VocabularyEncodingScheme -->

    <owl:Class rdf:about="http://purl.org/dc/dcam/VocabularyEncodingScheme"/>
    


    <!-- http://purl.org/dc/terms/Agent -->

    <owl:Class rdf:about="&dcterms;Agent">
        <rdfs:label xml:lang="en">Agent</rdfs:label>
        <dcterms:issued rdf:datatype="&xsd;date">2008-01-14</dcterms:issued>
        <rdfs:comment xml:lang="en">A resource that acts or has the power to act.</rdfs:comment>
        <dcterms:description xml:lang="en">Examples of Agent include person, organization, and software agent.</dcterms:description>
        <dcterms:hasVersion rdf:resource="http://dublincore.org/usage/terms/history/#Agent-001"/>
        <rdfs:isDefinedBy rdf:resource="http://purl.org/dc/terms/"/>
    </owl:Class>
    


    <!-- http://purl.org/dc/terms/AgentClass -->

    <owl:Class rdf:about="&dcterms;AgentClass">
        <rdfs:label xml:lang="en">Agent Class</rdfs:label>
        <rdfs:subClassOf rdf:resource="&rdfs;Class"/>
        <dcterms:issued rdf:datatype="&xsd;date">2008-01-14</dcterms:issued>
        <dcterms:modified rdf:datatype="&xsd;date">2012-06-14</dcterms:modified>
        <rdfs:comment xml:lang="en">A group of agents.</rdfs:comment>
        <dcterms:description xml:lang="en">Examples of Agent Class include groups seen as classes, such as students, women, charities, lecturers.</dcterms:description>
        <dcterms:hasVersion rdf:resource="http://dublincore.org/usage/terms/history/#AgentClass-003"/>
        <rdfs:isDefinedBy rdf:resource="http://purl.org/dc/terms/"/>
    </owl:Class>
    


    <!-- http://purl.org/dc/terms/BibliographicResource -->

    <owl:Class rdf:about="&dcterms;BibliographicResource">
        <rdfs:label xml:lang="en">Bibliographic Resource</rdfs:label>
        <dcterms:issued rdf:datatype="&xsd;date">2008-01-14</dcterms:issued>
        <rdfs:comment xml:lang="en">A book, article, or other documentary resource.</rdfs:comment>
        <dcterms:hasVersion rdf:resource="http://dublincore.org/usage/terms/history/#BibliographicResource-001"/>
        <rdfs:isDefinedBy rdf:resource="http://purl.org/dc/terms/"/>
    </owl:Class>
    


    <!-- http://purl.org/dc/terms/FileFormat -->

    <owl:Class rdf:about="&dcterms;FileFormat">
        <rdfs:label xml:lang="en">File Format</rdfs:label>
        <rdfs:subClassOf rdf:resource="&dcterms;MediaType"/>
        <dcterms:issued rdf:datatype="&xsd;date">2008-01-14</dcterms:issued>
        <rdfs:comment xml:lang="en">A digital resource format.</rdfs:comment>
        <dcterms:description xml:lang="en">Examples include the formats defined by the list of Internet Media Types.</dcterms:description>
        <dcterms:hasVersion rdf:resource="http://dublincore.org/usage/terms/history/#FileFormat-001"/>
        <rdfs:isDefinedBy rdf:resource="http://purl.org/dc/terms/"/>
    </owl:Class>
    


    <!-- http://purl.org/dc/terms/Frequency -->

    <owl:Class rdf:about="&dcterms;Frequency">
        <rdfs:label xml:lang="en">Frequency</rdfs:label>
        <dcterms:issued rdf:datatype="&xsd;date">2008-01-14</dcterms:issued>
        <rdfs:comment xml:lang="en">A rate at which something recurs.</rdfs:comment>
        <dcterms:hasVersion rdf:resource="http://dublincore.org/usage/terms/history/#Frequency-001"/>
        <rdfs:isDefinedBy rdf:resource="http://purl.org/dc/terms/"/>
    </owl:Class>
    


    <!-- http://purl.org/dc/terms/Jurisdiction -->

    <owl:Class rdf:about="&dcterms;Jurisdiction">
        <rdfs:label xml:lang="en">Jurisdiction</rdfs:label>
        <rdfs:subClassOf rdf:resource="&dcterms;LocationPeriodOrJurisdiction"/>
        <dcterms:issued rdf:datatype="&xsd;date">2008-01-14</dcterms:issued>
        <rdfs:comment xml:lang="en">The extent or range of judicial, law enforcement, or other authority.</rdfs:comment>
        <dcterms:hasVersion rdf:resource="http://dublincore.org/usage/terms/history/#Jurisdiction-001"/>
        <rdfs:isDefinedBy rdf:resource="http://purl.org/dc/terms/"/>
    </owl:Class>
    


    <!-- http://purl.org/dc/terms/LicenseDocument -->

    <owl:Class rdf:about="&dcterms;LicenseDocument">
        <rdfs:label xml:lang="en">License Document</rdfs:label>
        <rdfs:subClassOf rdf:resource="&dcterms;RightsStatement"/>
        <dcterms:issued rdf:datatype="&xsd;date">2008-01-14</dcterms:issued>
        <rdfs:comment xml:lang="en">A legal document giving official permission to do something with a Resource.</rdfs:comment>
        <dcterms:hasVersion rdf:resource="http://dublincore.org/usage/terms/history/#LicenseDocument-001"/>
        <rdfs:isDefinedBy rdf:resource="http://purl.org/dc/terms/"/>
    </owl:Class>
    


    <!-- http://purl.org/dc/terms/LinguisticSystem -->

    <owl:Class rdf:about="&dcterms;LinguisticSystem">
        <rdfs:label xml:lang="en">Linguistic System</rdfs:label>
        <dcterms:issued rdf:datatype="&xsd;date">2008-01-14</dcterms:issued>
        <rdfs:comment xml:lang="en">A system of signs, symbols, sounds, gestures, or rules used in communication.</rdfs:comment>
        <dcterms:description xml:lang="en">Examples include written, spoken, sign, and computer languages.</dcterms:description>
        <dcterms:hasVersion rdf:resource="http://dublincore.org/usage/terms/history/#LinguisticSystem-001"/>
        <rdfs:isDefinedBy rdf:resource="http://purl.org/dc/terms/"/>
    </owl:Class>
    


    <!-- http://purl.org/dc/terms/Location -->

    <owl:Class rdf:about="&dcterms;Location">
        <rdfs:label xml:lang="en">Location</rdfs:label>
        <rdfs:subClassOf rdf:resource="&dcterms;LocationPeriodOrJurisdiction"/>
        <dcterms:issued rdf:datatype="&xsd;date">2008-01-14</dcterms:issued>
        <rdfs:comment xml:lang="en">A spatial region or named place.</rdfs:comment>
        <dcterms:hasVersion rdf:resource="http://dublincore.org/usage/terms/history/#Location-001"/>
        <rdfs:isDefinedBy rdf:resource="http://purl.org/dc/terms/"/>
    </owl:Class>
    


    <!-- http://purl.org/dc/terms/LocationPeriodOrJurisdiction -->

    <owl:Class rdf:about="&dcterms;LocationPeriodOrJurisdiction">
        <rdfs:label xml:lang="en">Location, Period, or Jurisdiction</rdfs:label>
        <dcterms:issued rdf:datatype="&xsd;date">2008-01-14</dcterms:issued>
        <rdfs:comment xml:lang="en">A location, period of time, or jurisdiction.</rdfs:comment>
        <dcterms:hasVersion rdf:resource="http://dublincore.org/usage/terms/history/#LocationPeriodOrJurisdiction-001"/>
        <rdfs:isDefinedBy rdf:resource="http://purl.org/dc/terms/"/>
    </owl:Class>
    


    <!-- http://purl.org/dc/terms/MediaType -->

    <owl:Class rdf:about="&dcterms;MediaType">
        <rdfs:label xml:lang="en">Media Type</rdfs:label>
        <rdfs:subClassOf rdf:resource="&dcterms;MediaTypeOrExtent"/>
        <dcterms:issued rdf:datatype="&xsd;date">2008-01-14</dcterms:issued>
        <rdfs:comment xml:lang="en">A file format or physical medium.</rdfs:comment>
        <dcterms:hasVersion rdf:resource="http://dublincore.org/usage/terms/history/#MediaType-001"/>
        <rdfs:isDefinedBy rdf:resource="http://purl.org/dc/terms/"/>
    </owl:Class>
    


    <!-- http://purl.org/dc/terms/MediaTypeOrExtent -->

    <owl:Class rdf:about="&dcterms;MediaTypeOrExtent">
        <rdfs:label xml:lang="en">Media Type or Extent</rdfs:label>
        <dcterms:issued rdf:datatype="&xsd;date">2008-01-14</dcterms:issued>
        <rdfs:comment xml:lang="en">A media type or extent.</rdfs:comment>
        <dcterms:hasVersion rdf:resource="http://dublincore.org/usage/terms/history/#MediaTypeOrExtent-001"/>
        <rdfs:isDefinedBy rdf:resource="http://purl.org/dc/terms/"/>
    </owl:Class>
    


    <!-- http://purl.org/dc/terms/MethodOfAccrual -->

    <owl:Class rdf:about="&dcterms;MethodOfAccrual">
        <rdfs:label xml:lang="en">Method of Accrual</rdfs:label>
        <dcterms:issued rdf:datatype="&xsd;date">2008-01-14</dcterms:issued>
        <rdfs:comment xml:lang="en">A method by which resources are added to a collection.</rdfs:comment>
        <dcterms:hasVersion rdf:resource="http://dublincore.org/usage/terms/history/#MethodOfAccrual-001"/>
        <rdfs:isDefinedBy rdf:resource="http://purl.org/dc/terms/"/>
    </owl:Class>
    


    <!-- http://purl.org/dc/terms/MethodOfInstruction -->

    <owl:Class rdf:about="&dcterms;MethodOfInstruction">
        <rdfs:label xml:lang="en">Method of Instruction</rdfs:label>
        <dcterms:issued rdf:datatype="&xsd;date">2008-01-14</dcterms:issued>
        <rdfs:comment xml:lang="en">A process that is used to engender knowledge, attitudes, and skills.</rdfs:comment>
        <dcterms:hasVersion rdf:resource="http://dublincore.org/usage/terms/history/#MethodOfInstruction-001"/>
        <rdfs:isDefinedBy rdf:resource="http://purl.org/dc/terms/"/>
    </owl:Class>
    


    <!-- http://purl.org/dc/terms/PeriodOfTime -->

    <owl:Class rdf:about="&dcterms;PeriodOfTime">
        <rdfs:label xml:lang="en">Period of Time</rdfs:label>
        <rdfs:subClassOf rdf:resource="&dcterms;LocationPeriodOrJurisdiction"/>
        <dcterms:issued rdf:datatype="&xsd;date">2008-01-14</dcterms:issued>
        <rdfs:comment xml:lang="en">An interval of time that is named or defined by its start and end dates.</rdfs:comment>
        <dcterms:hasVersion rdf:resource="http://dublincore.org/usage/terms/history/#PeriodOfTime-001"/>
        <rdfs:isDefinedBy rdf:resource="http://purl.org/dc/terms/"/>
    </owl:Class>
    


    <!-- http://purl.org/dc/terms/PhysicalMedium -->

    <owl:Class rdf:about="&dcterms;PhysicalMedium">
        <rdfs:label xml:lang="en">Physical Medium</rdfs:label>
        <rdfs:subClassOf rdf:resource="&dcterms;MediaType"/>
        <dcterms:issued rdf:datatype="&xsd;date">2008-01-14</dcterms:issued>
        <rdfs:comment xml:lang="en">A physical material or carrier.</rdfs:comment>
        <dcterms:description xml:lang="en">Examples include paper, canvas, or DVD.</dcterms:description>
        <dcterms:hasVersion rdf:resource="http://dublincore.org/usage/terms/history/#PhysicalMedium-001"/>
        <rdfs:isDefinedBy rdf:resource="http://purl.org/dc/terms/"/>
    </owl:Class>
    


    <!-- http://purl.org/dc/terms/PhysicalResource -->

    <owl:Class rdf:about="&dcterms;PhysicalResource">
        <rdfs:label xml:lang="en">Physical Resource</rdfs:label>
        <dcterms:issued rdf:datatype="&xsd;date">2008-01-14</dcterms:issued>
        <rdfs:comment xml:lang="en">A material thing.</rdfs:comment>
        <dcterms:hasVersion rdf:resource="http://dublincore.org/usage/terms/history/#PhysicalResource-001"/>
        <rdfs:isDefinedBy rdf:resource="http://purl.org/dc/terms/"/>
    </owl:Class>
    


    <!-- http://purl.org/dc/terms/Policy -->

    <owl:Class rdf:about="&dcterms;Policy">
        <rdfs:label xml:lang="en">Policy</rdfs:label>
        <dcterms:issued rdf:datatype="&xsd;date">2008-01-14</dcterms:issued>
        <rdfs:comment xml:lang="en">A plan or course of action by an authority, intended to influence and determine decisions, actions, and other matters.</rdfs:comment>
        <dcterms:hasVersion rdf:resource="http://dublincore.org/usage/terms/history/#Policy-001"/>
        <rdfs:isDefinedBy rdf:resource="http://purl.org/dc/terms/"/>
    </owl:Class>
    


    <!-- http://purl.org/dc/terms/ProvenanceStatement -->

    <owl:Class rdf:about="&dcterms;ProvenanceStatement">
        <rdfs:label xml:lang="en">Provenance Statement</rdfs:label>
        <dcterms:issued rdf:datatype="&xsd;date">2008-01-14</dcterms:issued>
        <rdfs:comment xml:lang="en">A statement of any changes in ownership and custody of a resource since its creation that are significant for its authenticity, integrity, and interpretation.</rdfs:comment>
        <dcterms:hasVersion rdf:resource="http://dublincore.org/usage/terms/history/#ProvenanceStatement-001"/>
        <rdfs:isDefinedBy rdf:resource="http://purl.org/dc/terms/"/>
    </owl:Class>
    


    <!-- http://purl.org/dc/terms/RightsStatement -->

    <owl:Class rdf:about="&dcterms;RightsStatement">
        <rdfs:label xml:lang="en">Rights Statement</rdfs:label>
        <dcterms:issued rdf:datatype="&xsd;date">2008-01-14</dcterms:issued>
        <rdfs:comment xml:lang="en">A statement about the intellectual property rights (IPR) held in or over a Resource, a legal document giving official permission to do something with a resource, or a statement about access rights.</rdfs:comment>
        <dcterms:hasVersion rdf:resource="http://dublincore.org/usage/terms/history/#RightsStatement-001"/>
        <rdfs:isDefinedBy rdf:resource="http://purl.org/dc/terms/"/>
    </owl:Class>
    


    <!-- http://purl.org/dc/terms/SizeOrDuration -->

    <owl:Class rdf:about="&dcterms;SizeOrDuration">
        <rdfs:label xml:lang="en">Size or Duration</rdfs:label>
        <rdfs:subClassOf rdf:resource="&dcterms;MediaTypeOrExtent"/>
        <dcterms:issued rdf:datatype="&xsd;date">2008-01-14</dcterms:issued>
        <rdfs:comment xml:lang="en">A dimension or extent, or a time taken to play or execute.</rdfs:comment>
        <dcterms:description xml:lang="en">Examples include a number of pages, a specification of length, width, and breadth, or a period in hours, minutes, and seconds.</dcterms:description>
        <dcterms:hasVersion rdf:resource="http://dublincore.org/usage/terms/history/#SizeOrDuration-001"/>
        <rdfs:isDefinedBy rdf:resource="http://purl.org/dc/terms/"/>
    </owl:Class>
    


    <!-- http://purl.org/dc/terms/Standard -->

    <owl:Class rdf:about="&dcterms;Standard">
        <rdfs:label xml:lang="en">Standard</rdfs:label>
        <dcterms:issued rdf:datatype="&xsd;date">2008-01-14</dcterms:issued>
        <rdfs:comment xml:lang="en">A basis for comparison; a reference point against which other things can be evaluated.</rdfs:comment>
        <dcterms:hasVersion rdf:resource="http://dublincore.org/usage/terms/history/#Standard-001"/>
        <rdfs:isDefinedBy rdf:resource="http://purl.org/dc/terms/"/>
    </owl:Class>
    


    <!-- http://www.loc.gov/mads/rdf/v1#Authority -->

    <owl:Class rdf:about="&v1;Authority"/>
    


    <!-- http://www.loc.gov/mads/rdf/v1#Topic -->

    <owl:Class rdf:about="&v1;Topic"/>
    


    <!-- http://www.rdaregistry.info/Elements/c/#C10007 -->

    <owl:Class rdf:about="http://www.rdaregistry.info/Elements/c/#C10007">
        <rdfs:label rdf:datatype="&rdfs;Literal">Manifestation</rdfs:label>
        <rdfs:comment rdf:datatype="&rdfs;Literal">The physical embodiment of an expression of a work.</rdfs:comment>
    </owl:Class>
    


    <!-- 
    ///////////////////////////////////////////////////////////////////////////////////////
    //
    // Individuals
    //
    ///////////////////////////////////////////////////////////////////////////////////////
     -->

    


    <!-- http://id.loc.gov/vocabulary/relators/cre -->

    <owl:NamedIndividual rdf:about="&marcrel;cre">
        <rdf:type rdf:resource="&v1;Authority"/>
        <rdf:type rdf:resource="&v1;Topic"/>
        <v1:code>cre</v1:code>
        <v1:definitionNote>A person or organization responsible for the intellectual or artistic content of a resource</v1:definitionNote>
        <v1:authoritativeLabel xml:lang="en">Creator</v1:authoritativeLabel>
        <v1:isMemberOfMADSScheme rdf:resource="http://id.loc.gov/vocabulary/relators"/>
        <v1:isMemberOfMADSCollection rdf:resource="&marcrel;collection_BIBFRAMEWork"/>
        <v1:isMemberOfMADSCollection rdf:resource="&marcrel;collection_RDA"/>
        <v1:isMemberOfMADSCollection rdf:resource="&marcrel;collection_RDACreator"/>
        <v1:isMemberOfMADSCollection rdf:resource="&marcrel;collection_RDAWork"/>
        <owl:sameAs rdf:resource="info:lc/vocabulary/relators/cre"/>
        <v1:adminMetadata>
            <rdf:Description>
                <rdf:type rdf:resource="&RecordInfo;RecordInfo"/>
                <RecordInfo:recordContentSource rdf:resource="http://id.loc.gov/vocabulary/organizations/dlcmrc"/>
            </rdf:Description>
        </v1:adminMetadata>
        <v1:adminMetadata>
            <rdf:Description>
                <rdf:type rdf:resource="&RecordInfo;RecordInfo"/>
                <RecordInfo:recordContentSource rdf:resource="http://id.loc.gov/vocabulary/organizations/dlcmrc"/>
            </rdf:Description>
        </v1:adminMetadata>
        <v1:adminMetadata>
            <rdf:Description>
                <rdf:type rdf:resource="&RecordInfo;RecordInfo"/>
                <RecordInfo:recordContentSource rdf:resource="http://id.loc.gov/vocabulary/organizations/dlcmrc"/>
            </rdf:Description>
        </v1:adminMetadata>
        <v1:adminMetadata>
            <rdf:Description>
                <rdf:type rdf:resource="&RecordInfo;RecordInfo"/>
                <RecordInfo:recordContentSource rdf:resource="http://id.loc.gov/vocabulary/organizations/dlcmrc"/>
            </rdf:Description>
        </v1:adminMetadata>
        <v1:adminMetadata>
            <rdf:Description>
                <rdf:type rdf:resource="&RecordInfo;RecordInfo"/>
                <RecordInfo:recordContentSource rdf:resource="http://id.loc.gov/vocabulary/organizations/dlcmrc"/>
            </rdf:Description>
        </v1:adminMetadata>
        <v1:adminMetadata>
            <rdf:Description>
                <rdf:type rdf:resource="&RecordInfo;RecordInfo"/>
                <RecordInfo:recordContentSource rdf:resource="http://id.loc.gov/vocabulary/organizations/dlcmrc"/>
            </rdf:Description>
        </v1:adminMetadata>
        <v1:adminMetadata>
            <rdf:Description>
                <rdf:type rdf:resource="&RecordInfo;RecordInfo"/>
                <RecordInfo:recordContentSource rdf:resource="http://id.loc.gov/vocabulary/organizations/dlcmrc"/>
            </rdf:Description>
        </v1:adminMetadata>
        <v1:adminMetadata>
            <rdf:Description>
                <rdf:type rdf:resource="&RecordInfo;RecordInfo"/>
                <RecordInfo:recordContentSource rdf:resource="http://id.loc.gov/vocabulary/organizations/dlcmrc"/>
            </rdf:Description>
        </v1:adminMetadata>
    </owl:NamedIndividual>
    


    <!-- http://id.loc.gov/vocabulary/relators/ctb -->

    <owl:NamedIndividual rdf:about="&marcrel;ctb">
        <rdf:type rdf:resource="&v1;Authority"/>
        <rdf:type rdf:resource="&v1;Topic"/>
        <v1:editorialNote>Changed MARC def; Collaborator deprecated in MARC list and reference made</v1:editorialNote>
        <v1:definitionNote>A person, family or organization responsible for making contributions to the resource. This includes those whose work has been contributed to a larger work, such as an anthology, serial publication, or other compilation of individual works. If a more specific role is available, prefer that, e.g. editor, compiler, illustrator</v1:definitionNote>
        <v1:code>ctb</v1:code>
        <v1:authoritativeLabel xml:lang="en">Contributor</v1:authoritativeLabel>
        <v1:isMemberOfMADSScheme rdf:resource="http://id.loc.gov/vocabulary/relators"/>
        <v1:isMemberOfMADSCollection rdf:resource="&marcrel;collection_BIBFRAMEWork"/>
        <v1:isMemberOfMADSCollection rdf:resource="&marcrel;collection_RDA"/>
        <v1:isMemberOfMADSCollection rdf:resource="&marcrel;collection_RDAContributor"/>
        <v1:isMemberOfMADSCollection rdf:resource="&marcrel;collection_RDAExpression"/>
        <owl:sameAs rdf:resource="info:lc/vocabulary/relators/ctb"/>
        <v1:hasVariant>
            <rdf:Description>
                <rdf:type rdf:resource="&v1;Topic"/>
            </rdf:Description>
        </v1:hasVariant>
        <v1:hasVariant>
            <rdf:Description>
                <rdf:type rdf:resource="&v1;Topic"/>
            </rdf:Description>
        </v1:hasVariant>
        <v1:adminMetadata>
            <rdf:Description>
                <rdf:type rdf:resource="&RecordInfo;RecordInfo"/>
                <RecordInfo:recordContentSource rdf:resource="http://id.loc.gov/vocabulary/organizations/dlcmrc"/>
            </rdf:Description>
        </v1:adminMetadata>
        <v1:adminMetadata>
            <rdf:Description>
                <rdf:type rdf:resource="&RecordInfo;RecordInfo"/>
                <RecordInfo:recordContentSource rdf:resource="http://id.loc.gov/vocabulary/organizations/dlcmrc"/>
            </rdf:Description>
        </v1:adminMetadata>
        <v1:adminMetadata>
            <rdf:Description>
                <rdf:type rdf:resource="&RecordInfo;RecordInfo"/>
                <RecordInfo:recordContentSource rdf:resource="http://id.loc.gov/vocabulary/organizations/dlcmrc"/>
            </rdf:Description>
        </v1:adminMetadata>
        <v1:adminMetadata>
            <rdf:Description>
                <rdf:type rdf:resource="&RecordInfo;RecordInfo"/>
                <RecordInfo:recordContentSource rdf:resource="http://id.loc.gov/vocabulary/organizations/dlcmrc"/>
            </rdf:Description>
        </v1:adminMetadata>
        <v1:hasVariant>
            <rdf:Description>
                <rdf:type rdf:resource="&v1;Topic"/>
            </rdf:Description>
        </v1:hasVariant>
        <v1:hasVariant>
            <rdf:Description>
                <rdf:type rdf:resource="&v1;Topic"/>
            </rdf:Description>
        </v1:hasVariant>
        <v1:adminMetadata>
            <rdf:Description>
                <rdf:type rdf:resource="&RecordInfo;RecordInfo"/>
                <RecordInfo:recordContentSource rdf:resource="http://id.loc.gov/vocabulary/organizations/dlcmrc"/>
            </rdf:Description>
        </v1:adminMetadata>
        <v1:adminMetadata>
            <rdf:Description>
                <rdf:type rdf:resource="&RecordInfo;RecordInfo"/>
                <RecordInfo:recordContentSource rdf:resource="http://id.loc.gov/vocabulary/organizations/dlcmrc"/>
            </rdf:Description>
        </v1:adminMetadata>
        <v1:adminMetadata>
            <rdf:Description>
                <rdf:type rdf:resource="&RecordInfo;RecordInfo"/>
                <RecordInfo:recordContentSource rdf:resource="http://id.loc.gov/vocabulary/organizations/dlcmrc"/>
            </rdf:Description>
        </v1:adminMetadata>
        <v1:adminMetadata>
            <rdf:Description>
                <rdf:type rdf:resource="&RecordInfo;RecordInfo"/>
                <RecordInfo:recordContentSource rdf:resource="http://id.loc.gov/vocabulary/organizations/dlcmrc"/>
            </rdf:Description>
        </v1:adminMetadata>
    </owl:NamedIndividual>
    


    <!-- http://purl.org/dc/terms/Agent -->

    <owl:NamedIndividual rdf:about="&dcterms;Agent">
        <rdf:type rdf:resource="&dcterms;AgentClass"/>
    </owl:NamedIndividual>
    


    <!-- http://purl.org/dc/terms/DCMIType -->

    <owl:NamedIndividual rdf:about="&dcterms;DCMIType">
        <rdf:type rdf:resource="http://purl.org/dc/dcam/VocabularyEncodingScheme"/>
        <rdfs:label xml:lang="en">DCMI Type Vocabulary</rdfs:label>
        <dcterms:issued rdf:datatype="&xsd;date">2000-07-11</dcterms:issued>
        <dcterms:modified rdf:datatype="&xsd;date">2012-06-14</dcterms:modified>
        <rdfs:comment xml:lang="en">The set of classes specified by the DCMI Type Vocabulary, used to categorize the nature or genre of the resource.</rdfs:comment>
        <dcterms:hasVersion rdf:resource="http://dublincore.org/usage/terms/history/#DCMIType-005"/>
        <rdfs:seeAlso rdf:resource="http://purl.org/dc/dcmitype/"/>
        <rdfs:isDefinedBy rdf:resource="http://purl.org/dc/terms/"/>
    </owl:NamedIndividual>
    


    <!-- http://purl.org/dc/terms/DDC -->

    <owl:NamedIndividual rdf:about="&dcterms;DDC">
        <rdf:type rdf:resource="http://purl.org/dc/dcam/VocabularyEncodingScheme"/>
        <rdfs:label xml:lang="en">DDC</rdfs:label>
        <dcterms:issued rdf:datatype="&xsd;date">2000-07-11</dcterms:issued>
        <dcterms:modified rdf:datatype="&xsd;date">2008-01-14</dcterms:modified>
        <rdfs:comment xml:lang="en">The set of conceptual resources specified by the Dewey Decimal Classification.</rdfs:comment>
        <dcterms:hasVersion rdf:resource="http://dublincore.org/usage/terms/history/#DDC-003"/>
        <rdfs:isDefinedBy rdf:resource="http://purl.org/dc/terms/"/>
        <rdfs:seeAlso rdf:resource="http://www.oclc.org/dewey/"/>
    </owl:NamedIndividual>
    


    <!-- http://purl.org/dc/terms/IMT -->

    <owl:NamedIndividual rdf:about="&dcterms;IMT">
        <rdf:type rdf:resource="http://purl.org/dc/dcam/VocabularyEncodingScheme"/>
        <rdfs:label xml:lang="en">IMT</rdfs:label>
        <dcterms:issued rdf:datatype="&xsd;date">2000-07-11</dcterms:issued>
        <dcterms:modified rdf:datatype="&xsd;date">2008-01-14</dcterms:modified>
        <rdfs:comment xml:lang="en">The set of media types specified by the Internet Assigned Numbers Authority.</rdfs:comment>
        <dcterms:hasVersion rdf:resource="http://dublincore.org/usage/terms/history/#IMT-004"/>
        <rdfs:isDefinedBy rdf:resource="http://purl.org/dc/terms/"/>
        <rdfs:seeAlso rdf:resource="http://www.iana.org/assignments/media-types/"/>
    </owl:NamedIndividual>
    


    <!-- http://purl.org/dc/terms/LCC -->

    <owl:NamedIndividual rdf:about="&dcterms;LCC">
        <rdf:type rdf:resource="http://purl.org/dc/dcam/VocabularyEncodingScheme"/>
        <rdfs:label xml:lang="en">LCC</rdfs:label>
        <dcterms:issued rdf:datatype="&xsd;date">2000-07-11</dcterms:issued>
        <dcterms:modified rdf:datatype="&xsd;date">2008-01-14</dcterms:modified>
        <rdfs:comment xml:lang="en">The set of conceptual resources specified by the Library of Congress Classification.</rdfs:comment>
        <dcterms:hasVersion rdf:resource="http://dublincore.org/usage/terms/history/#LCC-003"/>
        <rdfs:seeAlso rdf:resource="http://lcweb.loc.gov/catdir/cpso/lcco/lcco.html"/>
        <rdfs:isDefinedBy rdf:resource="http://purl.org/dc/terms/"/>
    </owl:NamedIndividual>
    


    <!-- http://purl.org/dc/terms/LCSH -->

    <owl:NamedIndividual rdf:about="&dcterms;LCSH">
        <rdf:type rdf:resource="http://purl.org/dc/dcam/VocabularyEncodingScheme"/>
        <rdfs:label xml:lang="en">LCSH</rdfs:label>
        <dcterms:issued rdf:datatype="&xsd;date">2000-07-11</dcterms:issued>
        <dcterms:modified rdf:datatype="&xsd;date">2008-01-14</dcterms:modified>
        <rdfs:comment xml:lang="en">The set of labeled concepts specified by the Library of Congress Subject Headings.</rdfs:comment>
        <dcterms:hasVersion rdf:resource="http://dublincore.org/usage/terms/history/#LCSH-003"/>
        <rdfs:isDefinedBy rdf:resource="http://purl.org/dc/terms/"/>
    </owl:NamedIndividual>
    


    <!-- http://purl.org/dc/terms/MESH -->

    <owl:NamedIndividual rdf:about="&dcterms;MESH">
        <rdf:type rdf:resource="http://purl.org/dc/dcam/VocabularyEncodingScheme"/>
        <rdfs:label xml:lang="en">MeSH</rdfs:label>
        <dcterms:issued rdf:datatype="&xsd;date">2000-07-11</dcterms:issued>
        <dcterms:modified rdf:datatype="&xsd;date">2008-01-14</dcterms:modified>
        <rdfs:comment xml:lang="en">The set of labeled concepts specified by the Medical Subject Headings.</rdfs:comment>
        <dcterms:hasVersion rdf:resource="http://dublincore.org/usage/terms/history/#MESH-003"/>
        <rdfs:isDefinedBy rdf:resource="http://purl.org/dc/terms/"/>
        <rdfs:seeAlso rdf:resource="http://www.nlm.nih.gov/mesh/meshhome.html"/>
    </owl:NamedIndividual>
    


    <!-- http://purl.org/dc/terms/NLM -->

    <owl:NamedIndividual rdf:about="&dcterms;NLM">
        <rdf:type rdf:resource="http://purl.org/dc/dcam/VocabularyEncodingScheme"/>
        <rdfs:label xml:lang="en">NLM</rdfs:label>
        <dcterms:issued rdf:datatype="&xsd;date">2005-06-13</dcterms:issued>
        <dcterms:modified rdf:datatype="&xsd;date">2008-01-14</dcterms:modified>
        <rdfs:comment xml:lang="en">The set of conceptual resources specified by the National Library of Medicine Classification.</rdfs:comment>
        <dcterms:hasVersion rdf:resource="http://dublincore.org/usage/terms/history/#NLM-002"/>
        <rdfs:isDefinedBy rdf:resource="http://purl.org/dc/terms/"/>
        <rdfs:seeAlso rdf:resource="http://wwwcf.nlm.nih.gov/class/"/>
    </owl:NamedIndividual>
    


    <!-- http://purl.org/dc/terms/TGN -->

    <owl:NamedIndividual rdf:about="&dcterms;TGN">
        <rdf:type rdf:resource="http://purl.org/dc/dcam/VocabularyEncodingScheme"/>
        <rdfs:label xml:lang="en">TGN</rdfs:label>
        <dcterms:issued rdf:datatype="&xsd;date">2000-07-11</dcterms:issued>
        <dcterms:modified rdf:datatype="&xsd;date">2008-01-14</dcterms:modified>
        <rdfs:comment xml:lang="en">The set of places specified by the Getty Thesaurus of Geographic Names.</rdfs:comment>
        <dcterms:hasVersion rdf:resource="http://dublincore.org/usage/terms/history/#TGN-003"/>
        <rdfs:isDefinedBy rdf:resource="http://purl.org/dc/terms/"/>
        <rdfs:seeAlso rdf:resource="http://www.getty.edu/research/tools/vocabulary/tgn/index.html"/>
    </owl:NamedIndividual>
    


    <!-- http://purl.org/dc/terms/UDC -->

    <owl:NamedIndividual rdf:about="&dcterms;UDC">
        <rdf:type rdf:resource="http://purl.org/dc/dcam/VocabularyEncodingScheme"/>
        <rdfs:label xml:lang="en">UDC</rdfs:label>
        <dcterms:issued rdf:datatype="&xsd;date">2000-07-11</dcterms:issued>
        <dcterms:modified rdf:datatype="&xsd;date">2008-01-14</dcterms:modified>
        <rdfs:comment xml:lang="en">The set of conceptual resources specified by the Universal Decimal Classification.</rdfs:comment>
        <dcterms:hasVersion rdf:resource="http://dublincore.org/usage/terms/history/#UDC-003"/>
        <rdfs:isDefinedBy rdf:resource="http://purl.org/dc/terms/"/>
        <rdfs:seeAlso rdf:resource="http://www.udcc.org/"/>
    </owl:NamedIndividual>
    


    <!-- info:lc/vocabulary/relators/cre -->

    <owl:NamedIndividual rdf:about="info:lc/vocabulary/relators/cre"/>
    


    <!-- info:lc/vocabulary/relators/ctb -->

    <owl:NamedIndividual rdf:about="info:lc/vocabulary/relators/ctb"/>
    


    <!-- 
    ///////////////////////////////////////////////////////////////////////////////////////
    //
    // Annotations
    //
    ///////////////////////////////////////////////////////////////////////////////////////
     -->

    <rdf:Description rdf:about="http://purl.org/dc/terms/">
        <dcterms:modified rdf:datatype="&xsd;date">2012-06-14</dcterms:modified>
        <dcterms:title xml:lang="en">DCMI Metadata Terms - other</dcterms:title>
        <dcterms:publisher rdf:resource="http://purl.org/dc/aboutdcmi#DCMI"/>
    </rdf:Description>
</rdf:RDF>



<!-- Generated by the OWL API (version 3.4.2) http://owlapi.sourceforge.net -->

