@prefix xsd: <http://www.w3.org/2001/XMLSchema#> .
@prefix owl: <http://www.w3.org/2002/07/owl#> .
@prefix : <http://www.lingvoj.org/ontology#> .
@prefix xml: <http://www.w3.org/XML/1998/namespace> .
@prefix rdf: <http://www.w3.org/1999/02/22-rdf-syntax-ns#> .
@prefix rdfs: <http://www.w3.org/2000/01/rdf-schema#> .
@prefix voaf: <http://purl.org/vocommons/voaf#> .
@prefix dcterms: <http://purl.org/dc/terms/> .
@prefix vann: <http://purl.org/vocab/vann/> .
@prefix foaf: <http://xmlns.com/foaf/0.1/> .
@prefix schema: <http://schema.org/> .
@prefix lode: <http://linkedevents.org/ontology/> .
@prefix olca: <http://www.lingvoj.org/olca#> .
@prefix lvont: <http://lexvo.org/ontology#> .
@prefix skos: <http://www.w3.org/2004/02/skos/core#> .
@base <http://www.lingvoj.org/ontology> .

### Vocabulary metadata ###

<http://www.lingvoj.org/ontology> 
	a owl:Ontology;
	a voaf:Vocabulary ;
	rdfs:label "The Lingvoj Ontology"@en ;
	dcterms:title "The Lingvoj Ontology"@en ;
	rdfs:label "Ontología de lenguajes"@es ;
	dcterms:title "Ontología de lenguajes"@es ;
	rdfs:label "Ontologie des langues"@fr ;
	dcterms:title "Ontologie des langues"@fr ;
	rdfs:label  "Taal Ontologie"@nl ;
	dcterms:title  "Taal Ontologie"@nl ;
	rdfs:label "言語オントロジー"@ja ;
	dcterms:title "言語オントロジー"@ja ;
	rdfs:label "Ontologia de idiomas"@pt ;
	dcterms:title "A Ontologia dos idiomas"@pt ;
	dcterms:language <http://lexvo.org/id/iso639-3/eng>, <http://lexvo.org/id/iso639-3/spa>, <http://lexvo.org/id/iso639-3/fra>,<http://lexvo.org/id/iso639-3/nld>, <http://lexvo.org/id/iso639-3/jap>, <http://www.lexvo.org/id/iso639-3/por> ;
	rdfs:comment "A vocabulary for describing the use of languages by people and organizations, their geographical scope and status as well as their usage in documents or during events"@en ;
	rdfs:comment "Un vocabulaire pour décrire l'utilisation des langues par les personnes et les organisations, leur répartition géographique et leur statut, ainsi que leur usage dans les documents ou lors des événements"@fr ;
	rdfs:comment "Un vocabulario para describir la utilización de lenguas por parte de personas y organizaciones, su ambito geográfico y su estatus, así como su utilización en documentos o durante eventos"@es ;
    rdfs:comment "Een vokabular voor de beschrijving en het gebruik van talen door personen en organisaties, de geografische extensie en status en het gebruik ervan in documenten en tijdens evenmenten"@nl ;
	rdfs:comment "人や組織による言語の使用、ドキュメント内やイベント期間中におけるその使用に加え、その地理的範囲と状況を記述するための語彙"@ja ;
	rdfs:comment "Um vocabulário para descrever a utilização de idiomas por parte de pessoas ou organizações, o seu âmbito geográfico e seu estatuto, assim como a sua utilização em documentos ou durante eventos"@pt ;
	vann:preferredNamespacePrefix "lingvo" ;
	vann:preferredNamespaceUri "http://www.lingvoj.org/ontology#" ;
	dcterms:creator <http://google.com/+BernardVatant> ;
	dcterms:contributor <http://google.com/+MaríaPovedaVillalón> ;
	dcterms:contributor <http://google.com/+RonaldPoell> ;
	dcterms:contributor [foaf:name "Shuji Kamitsuna"; foaf:homepage <http://www.asahi-net.or.jp/~ax2s-kmtn/>] ;
	dcterms:contributor <https://plus.google.com/113072078430654119300> ;
	dcterms:modified "2014-08-11";
	dcterms:issued "2007-09-17";
	skos:historyNote "v2.33 : Corrected minor typos, and added portuguese translations, provided by Mariana Curado Malta" ;	
	skos:historyNote "v2.32 : Added japanese translations, provided by Shuji Kamitsuna" ;
	skos:historyNote "v2.31 : Added more translations, language metadata, fixed typos plus cosmetic changes in the .ttl file" ;
	skos:historyNote "v2.3 : Added :LanguageResource class, subclasses and properties. Added properties :tag :officialIn :fromCountry" ;
	skos:historyNote "v2.21 : Added dutch translations plus 'interpreter' property suggested by Ronald Poell, along with minor corrections" ;
	skos:historyNote "v2.2 : Added spanish translations, provided by María Poveda Villalón" ;
	skos:historyNote "v2.1 : Relaxed domain constraints on several properties, replaced by Ontology Loose Coupling Annotations" ;
	rdfs:seeAlso  <http://www.lingvoj.org/> ;
	owl:versionIRI <http://www.lingvoj.org/ontology_v2.33.ttl> ;
	owl:priorVersion <http://www.lingvoj.org/ontology_v2.32.ttl> ;
	owl:incompatibleWith <http://www.lingvoj.org/ontology_v1.3.rdf> ;
	owl:versionInfo "v2.33" .
	
								  
###  Language Class ###

:Lingvo 
	a owl:Class ;    
	rdfs:label "Sprache"@de , "Language"@en ,"Lingvo"@eo , "Lenguaje"@es , "Kieli"@fi , "Langue"@fr , "Linguaggio"@it , "言語"@ja , "Taal"@nl , "Språk"@no , "Jezyk"@pl , "Idioma"@pt , "Язык"@ru , "Språk"@sv , "Dil"@tr , "语言"@zh ;    
	rdfs:subClassOf <http://purl.org/dc/terms/LinguisticSystem> , <http://www.loc.gov/mads/rdf/v1#Language> ;
	owl:equivalentClass <http://schema.org/Language>, <http://d-nb.info/standards/elementset/gnd#Language>, <http://purl.org/linguistics/gold/Language> , <http://www.ontotext.com/proton/protontop#Language> ;
	lvont:somewhatSameAs <http://lexvo.org/ontology#Language> ;
	vann:example  <http://lexvo.org/id/iso639-3/fra>, <http://id.loc.gov/vocabulary/iso639-1/ja> ;		
	rdfs:comment "A language used in spoken or written human communication, or in which a resource is written or recorded. It is recommended to use instances defined on the basis of ISO 639 codes, such as those in examples"@en ;
	rdfs:comment "Una lengua utilizada en la comunicación oral o escrita entre personas, o en la que se escribe o graba un recurso. Se recomienda el uso de las instancias definidas según los códigos ISO 639, como los que aparecen en los ejemplos"@es ;
	rdfs:comment "Une langue utilisée dans la communication orale ou écrite entre humains, ou dans laquelle une ressource est écrite ou enregistrée. Il est recommandé d'utiliser des instances définies sur la base d'un code ISO 639, comme dans les exemples"@fr ;
	rdfs:comment "Een taal gebruikt in geschreven of gesproken communicatie tussen mensen of in welke een bron is geschreven of opgenomen. Het is aan te raden instanties te gebruiken gedefinieerd op basis van de ISO 630 codes, zoals in deze voorbeelden"@nl ;
	rdfs:comment "会話または記述による人間のコミュニケーションで使用される言語、または資源が記述または記録される言語。例にあるような、ISO 639コードに基づいて定義されたインスタンスを使用することが推奨される"@ja ;
	rdfs:comment "Um idioma utilizado na comunicação oral ou escrita entre pessoas, ou na que se escreve ou grava um recurso. Recomenda-se a utilização das instâncias definidas segundo os códigos ISO 639, como os que aparecem nos excemplos"@pt .
	
:tag
	a owl:DatatypeProperty;
	rdfs:label "language tag"@en ;
	rdfs:label "tag de langue"@fr ;
	rdfs:label "etiqueta"@es ;
	rdfs:label "言語タグ"@ja ;
	rdfs:label "taal tag"@nl ;
	rdfs:label "tag de idioma"@pt ;
	rdfs:comment "The tag to use for the language, for example as value of xml:lang. See https://tools.ietf.org/html/bcp47"@en ;
	rdfs:comment "Le tag à utiliser pour la langue, par exemple comme valeur de xml:lang. Voir https://tools.ietf.org/html/bcp47"@fr ;
	rdfs:comment "La etiqueta a utilizar para el lenguaje, por ejemplo como valor de xml:lang. Ver https://tools.ietf.org/html/bcp47"@es ;
	rdfs:comment "例えばxml:langの値として、言語に用いるタグ。https://tools.ietf.org/html/bcp47を参照"@ja ;
	rdfs:comment "A tag para ser usada, por exemplo como valor de xml:lang. Ver https://tools.ietf.org/html/bcp47"@pt ;
	rdfs:subPropertyOf dcterms:identifier ;
	rdfs:domain :Lingvo.
	
### Properties used to describe the status of a language at a given date###

:livingLanguage 
	a owl:DatatypeProperty;
	rdfs:label "living language"@en ;
	rdfs:label "lengua viva"@es ;
	rdfs:label "langue vivante"@fr ;
	rdfs:label "levende taal"@nl ;
	rdfs:label "現用言語"@ja ;
	rdfs:label "Idioma vivo"@pt;
	rdfs:comment "The language has speakers at the given date"@en ;
	rdfs:comment "La lengua tiene hablantes en la fecha dada"@es ;
	rdfs:comment "La langue possède des locuteurs à la date indiquée"@fr ;
	rdfs:comment "De taal wordt door mensen gesproken op het aangegeven moment"@nl ;
	rdfs:comment "ある時点でその言語を話す人がいる"@ja ;
	rdfs:comment "O idioma possui pessoas que o falam na data indicada"@pt ;
	rdfs:domain :Lingvo ;
	rdfs:range  xsd:date .
			 
:endangeredLanguage 
	a owl:DatatypeProperty;
	rdfs:label "endangered language"@en ;
	rdfs:label "lengua en vías de extinción"@es ;
	rdfs:label "langue menacée"@fr ;
	rdfs:label "bedreigde taal"@nl ;
	rdfs:label "絶滅危惧言語"@ja ;
	rdfs:label "idioma em vias de extinção"@pt ;
	rdfs:comment "The language is endangered at the given date"@en ;
	rdfs:comment "La lengua está en vías de extinción en la fecha dada"@es ;
	rdfs:comment "La langue est menacée à la date indiquée"@fr ;
	rdfs:comment "De taal is bedreigd met uitsterven op de gegeven datum"@nl ;
	rdfs:comment "ある時点でその言語は絶滅寸前である"@ja ;
	rdfs:comment "O idioma está em vias de extinção na data indicada"@pt ;
	rdfs:subPropertyOf  :livingLanguage;
	rdfs:domain :Lingvo ;
	rdfs:range  xsd:date .
			 
:extinctLanguage 
	a owl:DatatypeProperty;
	rdfs:label "extinct language"@en ;
	rdfs:label "lengua muerta"@es ;
	rdfs:label "langue morte"@fr ;
	rdfs:label "uitgestorven taal"@nl ;
	rdfs:label "死語"@ja ;
	rdfs:label "Idioma morto"@pt ;
	rdfs:comment "The language has no longer any speaker at the given date"@en ;
	rdfs:comment "La lengua no tiene ningún hablante en la fecha dada"@es ;
	rdfs:comment "La langue n'a plus de locuteurs à la date indiquée"@fr ;
	rdfs:comment "Er zijn geen mensen meer die deze taal spreken"@nl ;
	rdfs:comment "ある時点でその言語を話す人はいなくなった"@ja ;
	rdfs:comment "O idioma já não possui pessoas que o falam na data indicada"@pt ;
	rdfs:domain :Lingvo ;
	rdfs:range  xsd:date .
		 
### Ability of a person to understand, speak, read or write a language ###

:notUnderstood 
	a owl:ObjectProperty ;           
	rdfs:label "not understood"@en ;
	rdfs:label "no comprendido"@es ;
	rdfs:label "non comprise"@fr ;
	rdfs:label "niet verstaan"@nl ;
	rdfs:label "理解されない"@ja ;
	rdfs:label "não compreendido"@pt;
	rdfs:comment "The person does not understand at all the spoken language"@en ;
	rdfs:comment "La persona no comprende la lengua hablada"@es ;
	rdfs:comment "La personne ne comprend pas du tout la langue parlée"@fr ;
	rdfs:comment "De persoon verstaat de taal in het geheel niet"@nl ;
	rdfs:comment "その人はその話し言葉をまったく理解しない"@ja ;
	rdfs:comment "A pessoa não compreende o idioma falado"@pt;	
	rdfs:range :Lingvo ;
	rdfs:domain  foaf:Person .
			 
:notSpoken 
	a owl:ObjectProperty ;           
	rdfs:label "not spoken"@en ;
	rdfs:label "no hablado"@es ;
	rdfs:label "non parlée"@fr ;
	rdfs:label "niet spreken"@nl ;
	rdfs:label "話されない"@ja ;
	rdfs:label "não falado"@pt ;
	rdfs:comment "The person does not speak at all the language"@en ;
	rdfs:comment "La persona no puede hablar la lengua"@es ;
	rdfs:comment "La personne ne parle pas du tout la langue"@fr ;
	rdfs:comment "De persoon spreekt de taal in het geheel niet"@nl ;
	rdfs:comment "その人はその言語をまったく話さない"@ja ;
	rdfs:comment "A pessoa não sabe falar o idioma"@pt ;
	rdfs:range :Lingvo ;
	rdfs:domain  foaf:Person .
			 
:notRead 
	a owl:ObjectProperty ;           
	rdfs:label "not read"@en ;
	rdfs:label "no leído"@es ;
	rdfs:label "non lue"@fr ;
	rdfs:label "niet lezen"@nl ;
	rdfs:label "読まれない"@ja ;
	rdfs:label "não lido"@pt ;
	rdfs:comment "The person does not read at all the language"@en ;
	rdfs:comment "La persona no puede leer la lengua"@es ;
	rdfs:comment "La personne ne lit pas du tout la langue"@fr ;
	rdfs:comment "De persoon leest de taal in het geheel niet"@nl ;
	rdfs:comment "その人はその言語をまったく読まない"@ja ;
	rdfs:comment "A pessoa não sabe ler o idioma"@pt ;
	rdfs:range :Lingvo ;
	rdfs:domain  foaf:Person .
			 
:notWritten 
	a owl:ObjectProperty ;           
	rdfs:label "not written"@en ;
	rdfs:label "no escrito"@es ;
	rdfs:label "non écrite"@fr ;
	rdfs:label "niet schrijven"@nl ;
	rdfs:label "書かれない"@ja ;
	rdfs:label "não escrito"@pt ;
	rdfs:comment "The person does not write at all the language"@en ;
	rdfs:comment "La persona no puede escribir la lengua"@es ;
	rdfs:comment "La personne n'écrit pas du tout la langue"@fr ;
    rdfs:comment "De persoon schrijft de taal in het geheel niet"@nl ;
	rdfs:comment "その人はその言語をまったく書かない"@ja ;
	rdfs:comment "A pessoa não sabe escrever no idioma"@pt ;
	rdfs:range :Lingvo ;
	rdfs:domain  foaf:Person .

:basicUnderstanding 
	a owl:ObjectProperty ;           
	rdfs:label "basic understanding"@en ;
	rdfs:label "comprensión básica"@es ;
	rdfs:label "compréhension élémentaire"@fr ;
	rdfs:label "basis luisterniveau"@nl ;
	rdfs:label "基礎的な理解"@ja ;
	rdfs:label "entendimento básico"@pt ;
	rdfs:comment "The person has a basic understanding of the spoken language"@en ;
	rdfs:comment "La persona tiene un nivel básico de comprensión de la lengua hablada"@es ;
	rdfs:comment "La personne a une compréhension élémentaire de la langue parlée"@fr ;
	rdfs:comment "De persoon kan eenvoudige gesproken taal begrijpen"@nl ;
	rdfs:comment "その人はその話し言語について基礎的な理解力を有している"@ja ;
	rdfs:comment "A pessoa tem um nível de compreensão básico do idioma falado"@pt ;
	dcterms:replaces  :hasAbility1 ;
	rdfs:range :Lingvo ;
	rdfs:domain  foaf:Person .
			 
:basicSpeaking 
	a owl:ObjectProperty ;           
	rdfs:label "basic speaking"@en ;
	rdfs:label "expresión oral básica"@es ;
	rdfs:label "expression élémentaire"@fr ;
	rdfs:label "basis spraakniveau"@nl ;
	rdfs:label "基礎的な会話"@ja ;
	rdfs:label "expressão oral básica"@pt ;
	rdfs:comment "The person can speak the language at a basic level"@en ;
	rdfs:comment "La persona puede hablar la lengua a un nivel básico"@es ;
	rdfs:comment "La personne parle la langue à un niveau élémentaire"@fr ;
	rdfs:comment "De persoon kan eenvoudige taal spreken"@nl ;	
	rdfs:comment "その人はその言語を基礎レベルで話すことができる"@ja ;
	rdfs:comment "A pessoa consegue falar o idioma a um nível básico"@pt ;
	dcterms:replaces  :hasAbility1 ;
	rdfs:range :Lingvo ;
	rdfs:domain  foaf:Person .
			 
:basicReading 
	a owl:ObjectProperty ;           
	rdfs:label "basic reading"@en ;
	rdfs:label "lectura básica"@es ;
	rdfs:label "lecture élémentaire"@fr ;
	rdfs:label "basis leesniveau"@nl ;
	rdfs:label "基礎的な読解"@ja ;
	rdfs:label "leitura básica"@pt ;
	rdfs:comment "The person can read the language at a basic level"@en ;
	rdfs:comment "La persona puede leer la lengua a un nivel básico"@es ;
	rdfs:comment "La personne lit la langue à un niveau élémentaire"@fr ;
	rdfs:comment "De persoon kan eenvoudige taal lezen"@nl ;
	rdfs:comment "その人はその言語を基礎レベルで読むことができる"@ja ;
	rdfs:comment "A pessoa consegue ler o idioma a um nível básico"@pt ;
	dcterms:replaces  :hasAbility1 ;
	rdfs:range :Lingvo ;
	rdfs:domain  foaf:Person .
			 
:basicWriting 
	a owl:ObjectProperty ;           
	rdfs:label "basic writing"@en ;
	rdfs:label "escritura básica"@es ;
	rdfs:label "écriture élémentaire"@fr ;
	rdfs:label "basis schrijfniveau"@nl ;
	rdfs:label "基礎的な記述"@ja ;
	rdfs:label "escrita básica"@pt ;
	rdfs:comment "The person can write the language at a basic level"@en ;
	rdfs:comment "La persona puede escribir la lengua a un nivel básico"@es ;
	rdfs:comment "La personne écrit la langue à un niveau élémentaire"@fr ;
	rdfs:comment "De persoon kan eenvoudige taal schrijven"@nl ;
	rdfs:comment "その人はその言語を基礎レベルで書くことができる"@ja ;
	rdfs:comment "A pessoa consegue escrever o idioma a um nível básico"@pt ;	
	dcterms:replaces  :hasAbility1 ;
	rdfs:range :Lingvo ;
	rdfs:domain  foaf:Person .
			 
:intermediateUnderstanding 
	a owl:ObjectProperty ;           
	rdfs:label "intermediate understanding"@en ;
	rdfs:label "comprensión intermedia"@es ;
	rdfs:label "compréhension moyenne"@fr ;
	rdfs:label "voertaal"@nl ;
	rdfs:label "中級の理解"@ja ;
	rdfs:label "compreensão intermédia"@pt ;
	rdfs:comment "The person has an intermediate understanding of the spoken language"@en ;
	rdfs:comment "La persona tiene un nivel intermedio de comprensión de la lengua hablada"@es ;
	rdfs:comment "La personne a une compréhension moyenne de la langue parlée"@fr ;
	rdfs:comment "De persoon begrijpt de gesproken taal op een gemiddeld niveau"@nl ;
	rdfs:comment "その人はその話し言葉について中級レベルの理解力を有している"@ja ;
	rdfs:comment "A pessoa possui um nível intermédio de compreensão do idioma falado"@pt ;
	dcterms:replaces  :hasAbility2 ;
	rdfs:range :Lingvo ;
	rdfs:domain  foaf:Person .
			 
:intermediateSpeaking 
	a owl:ObjectProperty ;           
	rdfs:label "intermediate speaking"@en ;
	rdfs:label "nivel oral intermedio"@es ;
	rdfs:label "expression moyenne"@fr ;
	rdfs:label "gemiddeld spraakniveau"@nl ;
	rdfs:label "中級の会話"@ja ;
	rdfs:label "nivel oral intermédio"@pt ;
	rdfs:comment "The person can speak the language at an intermediate level"@en ;
	rdfs:comment "La persona puede hablar la lengua a un nivel intermedio"@es ;	
	rdfs:comment "La personne parle la langue à un niveau moyen"@fr ;	
	rdfs:comment "De persoon spreekt de taal op een gemiddeld niveau"@nl ;
	rdfs:comment "その人はその言語を中級レベルで話すことができる"@ja ;
	rdfs:comment "A pessoa consegue falar o idioma a um nível intermédio"@pt ;
	dcterms:replaces  :hasAbility2 ;
	rdfs:range :Lingvo ;
	rdfs:domain  foaf:Person .
			 
:intermediateReading 
	a owl:ObjectProperty ;           
	rdfs:label "intermediate reading"@en ;
	rdfs:label "lecture moyenne"@fr ;
	rdfs:label "nivel de lectura intermedio"@es ;
	rdfs:label "gemiddeld leesniveau"@nl ;
	rdfs:label "中級の読解"@ja ;
	rdfs:label "leitura intermédia"@pt ;
	rdfs:comment "The person can read the language at a intermediate level"@en ;
	rdfs:comment "La persona puede leer la lengua a un nivel intermedio"@es ;	
	rdfs:comment "La personne lit la langue à un niveau moyen"@fr ;
	rdfs:comment "De persoon leest de taal op een gemiddeld niveau"@nl ;	
	rdfs:comment "その人はその言語を中級レベルで読むことができる"@ja ;
	rdfs:comment "A pessoa consegue ler o idioma a um nível intermédio"@pt ;
	dcterms:replaces  :hasAbility2 ;
	rdfs:range :Lingvo ;
	rdfs:domain  foaf:Person .
			 
:intermediateWriting 
	a owl:ObjectProperty ;           
	rdfs:label "intermediate writing"@en ;
	rdfs:label "nivel escrito intermedio"@es ;
	rdfs:label "écriture moyenne"@fr ;	
	rdfs:label "gemiddeld schrijfniveau"@nl ;
	rdfs:label "中級の記述"@ja ;
	rdfs:label "escrita intermédia"@pt ;
	rdfs:comment "The person can write the language at an intermediate level"@en ;
	rdfs:comment "La persona puede escribir la lengua a un nivel intermedio"@es ;	
	rdfs:comment "La personne écrit la langue à un niveau moyen"@fr ;
	rdfs:comment "De persoon schrijft de taal op een gemiddeld niveau"@nl ;
	rdfs:comment "その人はその言語を中級レベルで書くことができる"@ja ;
	rdfs:comment "A pessoa consegue escrever o idioma com um nível intermédio"@pt ;
	dcterms:replaces  :hasAbility2 ;
	rdfs:range :Lingvo ;
	rdfs:domain  foaf:Person .
			 		 
:advancedUnderstanding 
	a owl:ObjectProperty ;           
	rdfs:label "advanced understanding"@en ;
	rdfs:label "buena comprensión"@es ;
	rdfs:label "bonne compréhension"@fr ;
	rdfs:label "goed luisterniveau"@nl ;
	rdfs:label "高度な理解"@ja ;
	rdfs:label "compreensão avançada"@pt ;
	rdfs:comment "The person has an advanced understanding of the spoken language"@en ;
	rdfs:comment "La persona tiene un nivel avanzado de comprensión de la lengua hablada"@es ;	
	rdfs:comment "La personne a une bonne compréhension de la langue parlée"@fr ;
	rdfs:comment "De persoon kan de gesproken taal goed begrijpen"@nl ;
	rdfs:comment "その人はその話し言葉について高度な理解力を有している"@ja ;
	rdfs:comment "A pessoa possui uma compreensão avançada do idioma falado"@pt ;	
	dcterms:replaces  :hasAbility3 ;
	rdfs:range :Lingvo ;
	rdfs:domain  foaf:Person .
			 
:advancedSpeaking 
	a owl:ObjectProperty ;           
	rdfs:label "advanced speaking"@en ;
	rdfs:label "buena expresión oral"@es ;
	rdfs:label "bonne expression"@fr ;
	rdfs:label "goed spraakniveau"@nl ;
	rdfs:label "高度な会話"@ja ;
	rdfs:label "boa expressão oral"@pt ;
	rdfs:comment "The person can speak the language at an advanced level"@en ;
	rdfs:comment "La persona puede hablar la lengua a un nivel avanzado"@es ;
	rdfs:comment "La personne parle la langue à un bon niveau"@fr ;
	rdfs:comment "De persoon kan de taal goed spreken"@nl ;		
	rdfs:comment "その人はその言語を上級レベルで話すことができる"@ja ;
	rdfs:comment "A pessoa consegue falar o idioma a um nível avançado"@pt ;
	dcterms:replaces  :hasAbility3 ;
	rdfs:range :Lingvo ;
	rdfs:domain  foaf:Person .
			 
:advancedReading 
	a owl:ObjectProperty ;           
	rdfs:label "advanced reading"@en ;
	rdfs:label "buen nivel de lectura"@es ;
	rdfs:label "bon niveau de lecture"@fr ;
	rdfs:label "goed leesniveau"@nl ;
	rdfs:label "高度な読解"@ja ;
	rdfs:label "leitura avançada"@pt ;
	rdfs:comment "The person can read the language at an advanced level"@en ;
	rdfs:comment "La persona puede leer la lengua a un nivel avanzado"@es ;	
	rdfs:comment "La personne lit la langue à un bon niveau"@fr ;
	rdfs:comment "De persoon kan de taal goed lezen"@nl ;	
	rdfs:comment "その人はその言語を上級レベルで読むことができる"@ja ;
	rdfs:comment "A pessoa consegue ler o idioma a um nível avançado"@pt ;
	dcterms:replaces  :hasAbility3 ;
	rdfs:range :Lingvo ;
	rdfs:domain  foaf:Person .
			 
:advancedWriting 
	a owl:ObjectProperty ;           
	rdfs:label "advanced writing"@en ;
	rdfs:label "buen nivel de escritura"@es ;
	rdfs:label "bon niveau d'écriture"@fr ;
	rdfs:label "goed schrijfniveau"@nl ;
	rdfs:label "高度な記述"@ja ;
	rdfs:label "escrita avançada"@pt ;
	rdfs:comment "The person can write the language at an advanced level"@en ;
	rdfs:comment "La persona puede escribir la lengua a un nivel avanzado"@es ;	
	rdfs:comment "La personne écrit la langue à un bon niveau"@fr ;
	rdfs:comment "De persoon kan de taal goed schrijven"@nl ;	
	rdfs:comment "その人はその言語を上級レベルで書くことができる"@ja ;
	rdfs:comment "A pessoa consegue escrever o idioma a um nível avançado"@pt ;
	dcterms:replaces  :hasAbility3 ;
	rdfs:range :Lingvo ;
	rdfs:domain  foaf:Person .
			 
:expertUnderstanding 
	a owl:ObjectProperty ;           
	rdfs:label "expert understanding"@en ;
	rdfs:label "comprensión excelente"@es ;
	rdfs:label "excellente compréhension"@fr ;	
	rdfs:label "uitstekend luisterniveau"@nl ;
	rdfs:label "専門家レベルの理解"@ja ;
	rdfs:label "compreensão a um nível de especialista"@pt ;
	rdfs:comment "The person has an expert understanding of the spoken language"@en ;
	rdfs:comment "La persona tiene un nivel experto de comprensión de la lengua hablada"@es ;	
	rdfs:comment "La personne a une excellente compréhension de la langue parlée"@fr ;
	rdfs:comment "De persoon kan de gesproken taal uitstekend begrijpen"@nl ;	
	rdfs:comment "その人はその話し言葉について専門家レベルの理解力を有している"@ja ;
	rdfs:comment "A pessoa tem um nível de especialista do idioma falado"@pt ;
	dcterms:replaces  :hasAbility4 ;
	rdfs:range :Lingvo ;
	rdfs:domain  foaf:Person .
			 
:expertSpeaking 
	a owl:ObjectProperty ;           
	rdfs:label "expert speaking"@en ;
	rdfs:label "expresión oral excelente"@es ;
	rdfs:label "excellente expression"@fr ;
	rdfs:label "uitstekend spraakniveau"@nl ;
	rdfs:label "専門家レベルの会話"@ja ;
	rdfs:label "expressão oral a um nível de especialista"@pt ;
	rdfs:comment "The person can speak the language at an expert level"@en ;
	rdfs:comment "La persona puede hablar la lengua a un nivel experto"@es ;	
	rdfs:comment "La personne parle la langue à niveau excellent"@fr ;
	rdfs:comment "De persoon kan de taal uitstekend spreken"@nl ;	
	rdfs:comment "その人はその言語を専門家レベルで話すことができる"@ja ;
	rdfs:comment "A pessoa consegue falar o idioma a um nível de especialista"@pt ;
	dcterms:replaces  :hasAbility4 ;
	rdfs:range :Lingvo ;
	rdfs:domain  foaf:Person .
			 
:expertReading 
	a owl:ObjectProperty ;           
	rdfs:label "expert reading"@en ;
	rdfs:label "nivel de lectura excelente"@es ;
	rdfs:label "excellente lecture"@fr ;
	rdfs:label "uitstekend leesniveau"@nl ;
	rdfs:label "専門家レベルの読解"@ja ;
	rdfs:label "leitura a um nível de especialista"@pt ;
	rdfs:comment "The person can read the language at a expert level"@en ;
	rdfs:comment "La persona puede leer en la lengua a un nivel experto"@es ;	
	rdfs:comment "La personne lit la langue à un niveau excellent"@fr ;
	rdfs:comment "De persoon kan de taal uitstekend lezen"@nl ;
	rdfs:comment "その人はその言語を専門家レベルで読むことができる"@ja ;	
	dcterms:replaces  :hasAbility4;
	rdfs:range :Lingvo ;
	rdfs:domain  foaf:Person .
			 
:expertWriting 
	a owl:ObjectProperty ;           
	rdfs:label "expert writing"@en ;
	rdfs:label "nivel de escritura excelente"@es ;
	rdfs:label "excellente écriture"@fr ;
	rdfs:label "uitstekend schrijfniveau"@nl ;
	rdfs:label "専門家レベルの記述"@ja ;
	rdfs:label "escrita a um nível de especialista"@pt ;
	rdfs:comment "The person can write the language at an expert level"@en ;
	rdfs:comment "La persona puede escribir la lengua a un nivel experto"@es ;	
	rdfs:comment "La personne écrit la langue à un niveau excellent"@fr ;
	rdfs:comment "De persoon kan de taal uitstekend schrijven"@nl ;	
	rdfs:comment "その人はその言語を専門家レベルで書くことができる"@ja ;
	rdfs:comment "A pessoa consegue escrever o idioma a um nível de especialista"@pt ;
	dcterms:replaces  :hasAbility4 ;
	rdfs:range :Lingvo ;
	rdfs:domain  foaf:Person .		 

:nativeLanguage 
	a owl:ObjectProperty ;           
	rdfs:label "native language"@en ; 
	rdfs:label "母国語"@ja ;
    rdfs:label "lengua materna"@es ;	
	rdfs:label "langue maternelle"@fr ; 
	rdfs:label "moedertaal"@nl ;
	rdfs:label "idioma mãe"@pt ;
	rdfs:comment "This property is independent of the level of fluency, reading or writing ability"@en ;
	rdfs:comment "Esta propiedad es independiente de el nivel de fluidez o de las habilidades de lectura o escritura"@es ;
	rdfs:comment "Cette propriété est indépendante du niveau de langue parlée, lue ou écrite"@fr ;
	rdfs:comment "Deze eigenschap is onafhankelijk van het niveau van spreken, lezen of schrijven"@nl ;	
	rdfs:comment "このプロパティーは、流暢さ、読解力、記述能力のレベルに依存しない"@ja ;
	rdfs:comment "Esta propriedade é independente do nível de fluência, de leitura ou de escrita"@pt ; 
	dcterms:replaces  :hasNativeLanguage ;
	rdfs:range :Lingvo ;
	rdfs:domain  foaf:Person .

### Properties describing the use of languages by various entities ###		 

:communicationLanguage 
	a owl:ObjectProperty ;
	rdfs:label "communication language"@en ;
	rdfs:label "lenguaje de comunicación"@es ;
	rdfs:label "langue de communication"@fr ;
	rdfs:label "kommunikation taal"@nl ;
	rdfs:label "コミュニケーション言語"@ja ;
	rdfs:label "idioma de comunicação"@pt ;
	rdfs:comment "A language used for external communication"@en ;
	rdfs:comment "Una lengua utilizada para la comunicación externa"@es ;
	rdfs:comment "Une langue utilisée pour la communication externe"@fr ;
	rdfs:comment "Een taal gebruikt voor externe communicatie"@nl ;             
	rdfs:comment "外部とのコミュニケーションに用いる言語"@ja ;
	rdfs:comment "Um idioma utilizado para a comunicação externa"@pt ;
	dcterms:replaces  :hasCommunicationLanguage;
	rdfs:range :Lingvo ;
	olca:domainIncludes foaf:Organization;
	olca:domainIncludes foaf:Project.
                           
:workingLanguage 
	a owl:ObjectProperty ;                
	rdfs:label "working language"@en ;   
	rdfs:label "lenguaje de trabajo"@es ;
	rdfs:label "langue de travail"@fr ;		
    rdfs:label  "werktaal"@nl ;
	rdfs:label "実用言語"@ja ;
	rdfs:label "idioma de trabalho"@pt ;
	rdfs:comment "A language the project or organization uses for internal communication"@en ;
	rdfs:comment "Una lengua que el proyecto o la organización utiliza para comunicación interna"@es ;	
	rdfs:comment "Une langue utilisée par l'organisation ou le projet pour sa communication interne"@fr ;
	rdfs:comment "De taal gebruikt voor interne communicatie door een organisatie of binnen een project"@nl ;
	rdfs:comment "プロジェクトや組織が内部コミュニケーションに用いる言語"@ja ;
	rdfs:comment "O idioma que o projecto ou organização usa para a comunicação interna"@pt ;	
	dcterms:replaces  :hasWorkingLanguage ;
	rdfs:range :Lingvo ;
	olca:domainIncludes foaf:Organization ;
	olca:domainIncludes foaf:Project.

:officialLanguage 
	a owl:ObjectProperty ;                
	rdfs:label "official language"@en ;   
	rdfs:label "lengua oficial"@es ;
	rdfs:label "langue officielle"@fr ;		
    rdfs:label "officiële taal"@nl ;	
	rdfs:label "公用語"@ja ;
	rdfs:label "idioma oficial"@pt ;
	rdfs:comment "An official language of a country, project, organization or event"@en ;
	rdfs:comment "Una lengua oficial en un país, proyecto, organización o evento"@es ;
	rdfs:comment "Une langue officielle d'un pays, d'une organisation, d'un projet ou d'un événement"@fr ;
	rdfs:comment "De officiële taal van een land, organisatie, prject of evenement"@nl ;
	rdfs:comment "国、プロジェクト、組織やイベントの公用語"@ja ;
	rdfs:comment "Um idioma oficial de um país, projecto, organização ou evento"@pt ;
	rdfs:range :Lingvo ;
	owl:inverseOf :officialIn ;
	olca:similarProperty <http://www.telegraphis.net/ontology/geography/geography#officialLanguage>;
	olca:domainIncludes foaf:Organization;
	olca:domainIncludes foaf:Project;
	olca:domainIncludes lode:Event;
	olca:domainIncludes schema:Place.
	
:officialIn 
	a owl:ObjectProperty ;                
	rdfs:label "official language of"@en ;   
	rdfs:label "lengua oficial de"@es ;
	rdfs:label "langue officielle de"@fr ;
	rdfs:label "officiële taal"@nl;			
	rdfs:label "～の公用語"@ja ;
	rdfs:label "idioma oficial de"@pt ;
	rdfs:domain :Lingvo ;
	owl:inverseOf :officialLanguage ;
	olca:rangeIncludes foaf:Organization;
	olca:rangeIncludes foaf:Project;
	olca:rangeIncludes lode:Event;
	olca:rangeIncludes schema:Place.

:spokenLanguage 
	a owl:ObjectProperty ;                
	rdfs:label "spoken language"@en ;   
	rdfs:label "lengua hablada"@es ;
	rdfs:label "langue parlée"@fr ;		
    rdfs:label "gesproken taal"@nl ;	
	rdfs:label "話し言葉"@ja ;
	rdfs:label "idioma falado"@pt ;
	rdfs:comment "A language which is spoken in some place or event"@en ;
	rdfs:comment "Una lengua que se habla en algún lugar o evento"@es ;	
	rdfs:comment "Une langue parlée dans un lieu ou lors d'un événement"@fr ;
	rdfs:comment "Een taal gesproken op een bepaalde plek of tijdens een evenement"@nl ;	
	rdfs:comment "ある場所やイベントで話される言語"@ja ;
	rdfs:comment "O idioma que é falado num determinado lugar ou evento"@pt ;
	rdfs:range :Lingvo ;
	olca:domainIncludes foaf:Organization;
	olca:domainIncludes foaf:Project;
	olca:domainIncludes lode:Event;
	olca:domainIncludes schema:Place.
	
:fromCountry 
	a owl:ObjectProperty ;                
	rdfs:label "from country"@en ;   
	rdfs:label "país de origen"@es ;	
	rdfs:label "pays d'origine"@fr ;
	rdfs:label "land van herkomst"@nl ;	
	rdfs:label "起源の国"@ja ;
	rdfs:label "do país"@pt ;
    rdfs:comment "Country of origin of the language"@en ;
	rdfs:comment "País de origen de la lengua"@es ;	
	rdfs:comment "Pays d'origine de la langue"@fr ;	
	rdfs:comment "Land van herkomst van de taal"@nl ;
    rdfs:comment "言語の起源の国"@ja ;
    rdfs:comment "País de origem do idioma"@pt ;
	rdfs:domain :Lingvo ;
	rdfs:range schema:Country.
						  
:mainLanguage 
	a owl:ObjectProperty ;                
	rdfs:label "main language"@en ;   
	rdfs:label "lengua principal"@es ;
	rdfs:label "langue principale"@fr ;	
    rdfs:label "hoofdtaal"@nl ;	
	rdfs:label "主要言語"@ja ;
	rdfs:label "Idioma principal"@pt ;
	rdfs:comment "The main language used in the place or language resource "@en ;
	rdfs:comment "Una lengua ampliamente hablada en un lugar (país, región, ciudad...)"@es ;	
	rdfs:comment "La langue principale utilisée dans le lieu ou la ressource linguistique"@fr ;
	rdfs:comment "De meest gebruikte taal op deze plek (land, regio, stad ...)"@nl ;	
	rdfs:comment "その場所または言語資源で用いられる主要言語"@ja ;
	rdfs:comment "O idioma principal utilizado num local ou recurso linguístico"@pt ;
	rdfs:range :Lingvo ;
	olca:domainIncludes  schema:Place;
	olca:domainIncludes  :LanguageResource.
			
:regionalLanguage 
	a owl:ObjectProperty ;                
	rdfs:label "regional language"@en ; 
    rdfs:label "lengua regional"@es ;	
	rdfs:label "langue régionale"@fr ;		
	rdfs:label "streektaal"@nl ;
	rdfs:label "地方言語"@ja ;
	rdfs:label "idioma regional"@pt ;
	rdfs:comment "A language spoken in a region of a country"@en ;
	rdfs:comment "Una lengua hablada en una región o un país"@es ;	
	rdfs:comment "Une langue parlée dans une région d'un pays"@fr ;
	rdfs:comment "Een taal gesproken in bepaalde streek van een land"@nl ;
	rdfs:comment "ある国のある地域で話される言語"@ja ;
	rdfs:comment "Um idioma falado num região de um país"@pt ;
	rdfs:range :Lingvo ;
	olca:domainIncludes   schema:Country.
			
:minorityLanguage 
	a owl:ObjectProperty ;                
	rdfs:label "minority language"@en ;   
	rdfs:label "lengua minoritaria"@es ;
	rdfs:label "langue minoritaire"@fr ;
    rdfs:label "minderheidstaal"@nl ;	
	rdfs:label "少数言語"@ja ;
	rdfs:label "idioma minoritário"@pt ;
	rdfs:comment "A language spoken by a minority in some country, but not necessarily in a specific region"@en ;
	rdfs:comment "Un lengua hablada por una minoría en algún país, pero no necesariamente en una región específica"@es ;
	rdfs:comment "Une langue parlée par une minorité dans un pays, mais pas nécessairement dans une région spécifique"@fr ;
	rdfs:comment "Een taal die door een minderheid van de bevolking van een land gesproken wordt, maar niet noodzakelijkerwijs in een specifieke regio"@nl ;
	rdfs:comment "ある国の少数の人々（必ずしも特定地域ではない）が話す言語"@ja ;
    rdfs:comment "O idioma falado por uma minoria num país, mas não necessariamente numa região específica"@pt ;	
	rdfs:range :Lingvo ;
	olca:domainIncludes   schema:Country.
			
:historicalLanguage 
	a owl:ObjectProperty ;                
	rdfs:label "historical language"@en ;   
	rdfs:label "lengua histórica"@es ;
	rdfs:label "langue historique"@fr ;
    rdfs:label "historische taal"@nl ;	
	rdfs:label "歴史的言語"@ja ;
	rdfs:label "idioma histórico"@pt ;
	rdfs:comment "A language spoken in the past in this place, but not used anymore"@en ;
	rdfs:comment "Una lengua hablada en el pasado en este lugar, pero ya no se utiliza"@es ;
	rdfs:comment "Une langue parlée dans le passé dans ce lieu, mais plus utilisée aujourd'hui"@fr ;
	rdfs:comment "Een taal die vroeger in dit gebied gesproken werd, maar wordt nu niet meer gebruikt"@nl ;		
	rdfs:comment "この場所で過去に話されていたが、もはや用いられていない言語"@ja ;
	rdfs:comment "Um idioma falado no passado num determinado lugar, não sendo já utilizado no presente"@pt ;
	rdfs:range :Lingvo ;
	olca:domainIncludes   schema:Place.

### Class and properties used to document the translation of a resource ###

:Translation 
	a owl:Class ;
	rdfs:label "Translation"@en ;   
	rdfs:label "Traducción"@es ;
	rdfs:label "Traduction"@fr ;
	rdfs:label "Vertaling"@nl ;
	rdfs:label "翻訳"@ja ;
	rdfs:label "Tradução"@pt ;
	rdfs:comment "Description of a Translation should include original resource, translated resource, original language and target language. It might also include translator(s) and translation date, and relevant other information using properties inherited from the generic Event class"@en ;
    rdfs:comment "La descripción de una Traducción debe incluir la fuente original, la fuente traducida, la lengua  original y la lengua de  destino. También puede incluir  el o los traductor(es) , la fecha de traducción y otra información relevante utilizando propiedades heredadas de la clase generica Event"@es ;	
	rdfs:comment "La description d'une Traduction inclut au minimum la ressource originale, la ressource traduite, la langue d'origine et la langue cible. Elle peut aussi inclure le(s) traducteur(s), la date de traduction, et toute autre information pertinente utilisant les propriétés de la classe générique Evénement"@fr ;
	rdfs:comment "De beschrijving of een vertaling zou de oorspronkelijke bron, de vertaalde bron, de brontaal en de doeltaal moeten bevatten. Het kan ook de vertaler(s), de vertaaldatum en andere relevante informatie, gebruik makend van de eigenschappen geërfd van de generieke Event klasse, bevatten"@nl ;
	rdfs:comment "Translation（翻訳）の記述には、元の資源、翻訳後の資源、元の言語および翻訳先の言語が含まれているべきである。さらに、それには、翻訳者と翻訳日、そして、汎用的なEventクラスから継承されたプロパティーを用いた、関連するその他の情報が含まれるかもしれない"@ja ;
	rdfs:comment "Descrição de uma tradução deverá inclrui o recurso original, o recurso traduzido, o idioma original e o idioma de destino. Também pode incluir o(s)/a(s) tradutore(s)/tradutora(s), a data de tradução e outra informação relevante utilizando propriedades herdadas da classe genérica Event"@pt ;
	rdfs:subClassOf lode:Event;
	olca:expectedProperty  dcterms:date;
	vann:example <http://www.lingvoj.org/translations/w3c-recs.rdf#translation-css1-en-to-bg>.

:originalLanguage 
	a owl:ObjectProperty ;
	rdfs:label "original language"@en ; 
	rdfs:label "lengua original"@es ;
	rdfs:label "langue d'origine"@fr ;	
	rdfs:label "oorspronkelijke taal"@nl ;
	rdfs:label "元の言語"@ja ;
	rdfs:label "idioma original"@pt ;	
	rdfs:comment "The language of the original ressource"@en ;
	rdfs:comment "La langue de la ressource originale"@fr ;		
	rdfs:comment "De taal van de de bron"@nl ;
	rdfs:comment "La lengua de la fuente original"@es ;	
	rdfs:comment "元の資源の言語"@ja ;
	rdfs:comment "O idioma do recurso original"@pt ;
	rdfs:range :Lingvo ;
	rdfs:domain :Translation .
		  
:targetLanguage 
	a owl:ObjectProperty ;
	rdfs:label "target language"@en ; 
	rdfs:label "lengua destino"@es ;
	rdfs:label "langue cible"@fr ;	
	rdfs:label "doeltaal"@nl ;
	rdfs:label "翻訳先の言語"@ja ;
	rdfs:label "idioma destino"@pt ;
	rdfs:comment "The language of the translated ressource"@en ;
	rdfs:comment "La lengua de la fuente traducida"@es ;
	rdfs:comment "La langue de la ressource traduite"@fr ;	
	rdfs:comment "De taal waarin de bron vertaald is"@nl ;
	rdfs:comment "翻訳後の資源の言語"@ja ;
	rdfs:comment "O idioma do recurso traduzido"@pt ;
	rdfs:range :Lingvo ;
	rdfs:domain :Translation .
		  
:originalResource 
	a owl:ObjectProperty ;
	rdfs:label "original resource"@en ;
	rdfs:label "recurso original"@es ;
	rdfs:label "ressource originale"@fr ;	
	rdfs:label "oorspronkelijke bron"@nl ;
	rdfs:label "元の資源"@ja ;	
	rdfs:label "recurso original"@pt ;
	rdfs:comment "The resource which is translated"@en ;
	rdfs:comment "La fuente que se traduce"@es ;	
	rdfs:comment "La ressource qui est traduite"@fr ;	
	rdfs:comment "De vertaalde bron"@nl ;
	rdfs:comment "翻訳元の資源"@ja ;
	rdfs:comment "o recurso que se traduz"@pt ;
	rdfs:domain :Translation .

:translatedResource 
	a owl:ObjectProperty ;  
	rdfs:label "translated resource"@en ;
	rdfs:label "recurso traducido"@es ;
	rdfs:label "ressource traduite"@fr ;
    rdfs:label "vertaalde bron"@nl ;	
	rdfs:label "翻訳後の資源"@ja ;
	rdfs:label "recurso traduzido"@pt ;
	rdfs:comment "The resource which is the result of the translation"@en ;
	rdfs:comment "La fuente que resulta de la traducción"@es ;	
	rdfs:comment "La ressource qui est le résultat de la traduction"@fr ;
	rdfs:comment "Het resultaat van de vertaling"@nl ;		
	rdfs:comment "翻訳の結果である資源"@ja ;
	rdfs:comment "O recurso que é o resultado da tradução"@pt ;
	rdfs:domain :Translation .

:translator 
	a owl:ObjectProperty ;
	rdfs:label "translator"@en ;
	rdfs:label "traductor"@es ;
	rdfs:label "traducteur"@fr ;
    rdfs:label "vertaler"@nl ;	
	rdfs:label "翻訳者"@ja ;
	rdfs:label "tradutor"@pt ;
	rdfs:comment "An agent (person, organization or sofware) responsible of the translation"@en ;
	rdfs:comment "Un agente (persona, organización o software) responsable de la traducción"@es ;
	rdfs:comment "Un agent (personne, organisation ou logiciel) responsable de la traduction"@fr ;	
	rdfs:comment "De agent (persoon, organisatie of applicatie) verantwoordelijk voor de vertaling"@nl ;
	rdfs:comment "翻訳に責任を持つエージェント（人、組織またはソフトウェア）"@ja ;
	rdfs:comment "um agente (pessoa, organização ou programa) responsável pela tradução"@pt ;
	rdfs:domain :Translation ;
	rdfs:range foaf:Agent.
	
:interpreter
	a owl:ObjectProperty ;
    rdfs:label "interpreter"@en ;
    rdfs:label "intérprete"@es ;
    rdfs:label "interprète"@fr ;
    rdfs:label "tolk"@nl ;
    rdfs:label "通訳者"@ja ;
    rdfs:label "interprete"@pt ;
    rdfs:comment "An agent (person or software) responsible of a real-time oral translation"@en ;
    rdfs:comment "Un agente (persona, organización o software) responsable de la interpretación oral"@es ;
    rdfs:comment "Un agent (personne ou logiciel) responsable de la traduction orale en temps réel"@fr ;
    rdfs:comment "De agent (persoon of applicatie) verantwoordelijk voor het tolken"@nl ;
    rdfs:comment "即時の通訳に責任を持つエージェント（人またはソフトウェア）"@ja ;
    rdfs:comment "Um agente (pessoa ou programa) responsável por uma tradução oral em tempo real"@pt ;
	rdfs:subPropertyOf :translator ;
	rdfs:domain :Translation ;
	rdfs:range foaf:Agent.
	
### Language resources ###

:LanguageResource
	a owl:Class ;
	rdfs:label "Language resource"@en ;
	rdfs:label "Recurso lingüístico"@es ;	   
	rdfs:label "Ressource linguistique"@fr ;
	rdfs:label "Taal bron"@nl ;
	rdfs:label "言語資源"@ja ;
	rdfs:label "Recurso linguístico"@pt ;
	rdfs:comment "Dictionaries, thesauri, language courses, translation services, etc."@en ;
	rdfs:comment "Dictionnaires, thesaurus, cours de langue, services de traduction, etc."@fr ;
	rdfs:comment "Woordenboeken, thesauri, taalcursussen, vertaaldiensten, etc."@nl ;
	rdfs:comment "Diccionarios, tesauros, cursos de idiomas, servicios de traducción, etc."@es ;
	rdfs:comment "辞書、シソーラス、言語コース、翻訳サービスなど"@ja ;
	rdfs:comment "Dicionários, tesauros, cursos de idiomas, serviços de tradução, etc."@pt ;
	rdfs:seeAlso <http://www.language-archives.org/documents/faq.html#2>.
	
:resourceType
 	a owl:ObjectProperty ;
    rdfs:label "resource type"@en ;
	rdfs:label "tipo de recurso"@es ;
    rdfs:label "type de ressource"@fr ;
    rdfs:label "bron type"@nl ;
    rdfs:label "資源の種類"@ja ;
    rdfs:label "tipo de recurso"@pt ;   
    rdfs:comment "A concept defining the type of the language resource"@en ;
	rdfs:comment "Un concepto que define el tipo de recurso lingüístico"@es ;
    rdfs:comment "Un concept définissant le type de la ressource linguistique"@fr ;
	rdfs:comment "Een concept van het definiëren van de aard van de taal bron"@nl ;	
	rdfs:comment "言語資源の種類を定義する概念"@ja ;
	rdfs:comment "Um conceito que define o tipo de recuso linguístico"@pt ;
	rdfs:domain :LanguageResource ;
	rdfs:range skos:Concept.
	
:supportedLanguage
 	a owl:ObjectProperty ;
    rdfs:label "supported language"@en ;
    rdfs:label "idioma soportado"@es ;
    rdfs:label "langue supportée"@fr ;
	rdfs:label "ondersteunde taal"@nl ;
    rdfs:label "サポートされている言語 "@ja ;
	rdfs:label "idioma suportado"@pt ;
    rdfs:comment "A language supported by the language resource"@en ;
	rdfs:comment "Un idioma soportado por el recurso lingüístico"@es ;   
    rdfs:comment "Une langue supportée par la ressource linguistique"@fr ;
	rdfs:comment "Een taal die wordt ondersteund door de taal bron"@nl ;
    rdfs:comment "言語資源でサポートされている言語"@ja ;
	rdfs:comment "Um idioma suportado pelo recurso linguístico"@pt ;	
	rdfs:domain :LanguageResource ;
	rdfs:range :Lingvo.
	
:supportingResource
 	a owl:ObjectProperty ;
    rdfs:label "support resource"@en ;
	rdfs:label "recurso soportado"@es ;
	rdfs:label "ressource support"@fr ;
	rdfs:label "ondersteunende bron"@nl ;
    rdfs:label "サポート資源"@ja ;
	rdfs:label "recurso suportado"@pt ;
    rdfs:comment "A language resource for this language"@en ;
    rdfs:comment "Un recurso lingüístico para este idioma"@es ;
    rdfs:comment "Une ressource linguistique pour cette langue"@fr ;
	rdfs:comment "Een taal bron voor deze taal"@nl ;	
    rdfs:comment "この言語の言語資源"@ja ;
	rdfs:comment "Um recurso linguístico para este idioma"@pt ;	
	owl:inverseOf :supportedLanguage ;
	rdfs:domain :Lingvo ;
	rdfs:range :LanguageResource.
	
### Deprecated properties ###

### Properties defining ISO codes defined in versions prior to 2.0 are deprecated. Use those defined by lexvo.org instead ###

:iso1 
	rdfs:isDefinedBy <http://www.lingvoj.org/ontology_v1.3.rdf> ;
	owl:deprecated  "true"^^xsd:boolean;
	dcterms:isReplacedBy <http://lexvo.org/ontology#iso639P1Code>.
		
:iso2b 
	rdfs:isDefinedBy <http://www.lingvoj.org/ontology_v1.3.rdf> ;
	owl:deprecated  "true"^^xsd:boolean;
	dcterms:isReplacedBy <http://lexvo.org/ontology#iso639P2BCode>.

:iso2t 
	rdfs:isDefinedBy <http://www.lingvoj.org/ontology_v1.3.rdf> ;
	owl:deprecated  "true"^^xsd:boolean;
	dcterms:isReplacedBy <http://lexvo.org/ontology#iso639P2TCode>.

:iso3 
	rdfs:isDefinedBy <http://www.lingvoj.org/ontology_v1.3.rdf> ;
	owl:deprecated  "true"^^xsd:boolean;
	dcterms:isReplacedBy <http://lexvo.org/ontology#iso639P3Code>.
	  
### Properties describing language level of a person, replaced by more specific ones ###

:hasAbility1 
	rdfs:isDefinedBy <http://www.lingvoj.org/ontology_v1.3.rdf> ;
	owl:deprecated  "true"^^xsd:boolean;
	dcterms:isReplacedBy :basicUnderstanding, :basicSpeaking, :basicReading, :basicWriting.
			 
:hasAbility2 
	rdfs:isDefinedBy <http://www.lingvoj.org/ontology_v1.3.rdf> ;
	owl:deprecated  "true"^^xsd:boolean;
	dcterms:isReplacedBy :intermediateUnderstanding, :intermediateSpeaking, :intermediateReading, :intermediateWriting.
			 
:hasAbility3 
	rdfs:isDefinedBy <http://www.lingvoj.org/ontology_v1.3.rdf> ;
	owl:deprecated  "true"^^xsd:boolean;
	dcterms:isReplacedBy :advancedUnderstanding, :advancedSpeaking, :advancedReading, :advancedWriting.
			 
:hasAbility4 
	rdfs:isDefinedBy <http://www.lingvoj.org/ontology_v1.3.rdf> ;
	owl:deprecated  "true"^^xsd:boolean;
	dcterms:isReplacedBy :expertUnderstanding, :expertSpeaking, :expertReading, :expertWriting.
			 
:hasAbility5 
	rdfs:isDefinedBy <http://www.lingvoj.org/ontology_v1.3.rdf> ;
	owl:deprecated  "true"^^xsd:boolean.
			 
### Change of URIs to meet best practice - trimming the initial "has" ###
			 
:hasNativeLanguage 
	rdfs:isDefinedBy <http://www.lingvoj.org/ontology_v1.3.rdf> ;
	owl:deprecated  "true"^^xsd:boolean;
	dcterms:isReplacedBy :nativeLanguage.
			 
:hasCommunicationLanguage 
	rdfs:isDefinedBy <http://www.lingvoj.org/ontology_v1.3.rdf> ;
	owl:deprecated  "true"^^xsd:boolean;
	dcterms:isReplacedBy :communicationLanguage.
			 							
:hasWorkingLanguage 
	rdfs:isDefinedBy <http://www.lingvoj.org/ontology_v1.3.rdf> ;
	owl:deprecated  "true"^^xsd:boolean;
	dcterms:isReplacedBy :workingLanguage.

### Deprecated properties for the Translation class ###
		   
:original_resource 
	rdfs:isDefinedBy <http://www.lingvoj.org/ontology_v1.3.rdf> ;
	owl:deprecated  "true"^^xsd:boolean;
	dcterms:isReplacedBy :originalResource.

:originalTitle 
	rdfs:isDefinedBy <http://www.lingvoj.org/ontology_v1.3.rdf> ;
	owl:deprecated  "true"^^xsd:boolean;
	rdfs:comment "The original title is a property of the original resource (use dcterms:title) and not a property of the Translation itself"@en;
	rdfs:comment "Le titre original est une propriété de la ressource originale (utiliser dcterms:title) et non une propriété de la Traduction elle-même"@fr;
	rdfs:comment "原タイトルは、Translation（翻訳）自体のプロパティーではなく、元の資源のプロパティー（dcterms:titleを使用）"@ja.
			 
:translatedTitle 
	rdfs:isDefinedBy <http://www.lingvoj.org/ontology_v1.3.rdf> ;
	owl:deprecated  "true"^^xsd:boolean;
	rdfs:comment "The translated title is a property of the translated resource (use dcterms:title) and not a property of the Translation itself"@en;
	rdfs:comment "Le titre traduit est une propriété de la ressource traduite (utiliser dcterms:title) et non une propriété de la Traduction elle-même"@fr;
	rdfs:comment "翻訳タイトルは、Translation（翻訳）自体のプロパティーではなく、翻訳された資源のプロパティー（dcterms:titleを使用）"@ja.
			 